@prefix : <http://iec.ch/TC57/CIM-generic#> .
@prefix dc: <http://purl.org/dc/elements/1.1/> .
@prefix msg: <http://langdale.com.au/2005/Message#> .
@prefix owl: <http://www.w3.org/2002/07/owl#> .
@prefix rdf: <http://www.w3.org/1999/02/22-rdf-syntax-ns#> .
@prefix uml: <http://langdale.com.au/2005/UML#> .
@prefix xml: <http://www.w3.org/XML/1998/namespace> .
@prefix xsd: <http://www.w3.org/2001/XMLSchema#> .
@prefix rdfs: <http://www.w3.org/2000/01/rdf-schema#> .
@base <http://iec.ch/TC57/CIM-generic#> .

<http://iec.ch/TC57/CIM-generic> rdf:type owl:Ontology .

#################################################################
#    Annotation properties
#################################################################

###  http://iec.ch/TC57/CIM-generic#OldTransformerEndInfo.solidInsulationWeight
:OldTransformerEndInfo.solidInsulationWeight rdf:type owl:AnnotationProperty ;
                                             
                                             rdfs:comment "Weight of solid insultation in transformer." ;
                                             rdfs:label "solidInsulationWeight" ;
                                             rdfs:domain :OldTransformerEndInfo .


###  http://iec.ch/TC57/CIM-generic#OldTransformerTankInfo.coreCoilsWeight
:OldTransformerTankInfo.coreCoilsWeight rdf:type owl:AnnotationProperty ;
                                        
                                        rdfs:comment "Weight of core and coils in transformer." ;
                                        rdfs:label "coreCoilsWeight" ;
                                        rdfs:domain :OldTransformerTankInfo .


###  http://iec.ch/TC57/CIM-generic#ProductAssetModel.weightTotal
:ProductAssetModel.weightTotal rdf:type owl:AnnotationProperty ;
                               
                               rdfs:comment "Total manufactured weight of asset." ;
                               rdfs:label "weightTotal" ;
                               rdfs:domain :ProductAssetModel .


###  http://iec.ch/TC57/CIM-generic#SwitchInfo.gasWeightPerTank
:SwitchInfo.gasWeightPerTank rdf:type owl:AnnotationProperty ;
                             
                             rdfs:comment "Weight of gas in each tank of SF6 dead tank breaker." ;
                             rdfs:label "gasWeightPerTank" ;
                             rdfs:domain :SwitchInfo .


###  http://langdale.com.au/2005/UML#baseprefix
uml:baseprefix rdf:type owl:AnnotationProperty .


###  http://langdale.com.au/2005/UML#baseuri
uml:baseuri rdf:type owl:AnnotationProperty .


###  http://langdale.com.au/2005/UML#hasInitialValue
uml:hasInitialValue rdf:type owl:AnnotationProperty .


###  http://langdale.com.au/2005/UML#hasMaxCardinality
uml:hasMaxCardinality rdf:type owl:AnnotationProperty .


###  http://langdale.com.au/2005/UML#hasMinCardinality
uml:hasMinCardinality rdf:type owl:AnnotationProperty .


###  http://langdale.com.au/2005/UML#hasMultiplier
uml:hasMultiplier rdf:type owl:AnnotationProperty .


###  http://langdale.com.au/2005/UML#hasStereotype
uml:hasStereotype rdf:type owl:AnnotationProperty .


###  http://langdale.com.au/2005/UML#hasUnits
uml:hasUnits rdf:type owl:AnnotationProperty .


###  http://langdale.com.au/2005/UML#id
uml:id rdf:type owl:AnnotationProperty .


###  http://langdale.com.au/2005/UML#roleALabel
uml:roleALabel rdf:type owl:AnnotationProperty .


###  http://langdale.com.au/2005/UML#roleAOf
uml:roleAOf rdf:type owl:AnnotationProperty .


###  http://langdale.com.au/2005/UML#roleBLabel
uml:roleBLabel rdf:type owl:AnnotationProperty .


###  http://langdale.com.au/2005/UML#roleBOf
uml:roleBOf rdf:type owl:AnnotationProperty .


###  http://langdale.com.au/2005/UML#uriHasPrefix
uml:uriHasPrefix rdf:type owl:AnnotationProperty .


#################################################################
#    Datatypes
#################################################################

###  http://iec.ch/TC57/CIM-generic#ActivePower
:ActivePower rdf:type rdfs:Datatype ;
             uml:hasUnits "W" ;
             rdfs:comment "Product of RMS value of the voltage and the RMS value of the in-phase component of the current." ;
             rdfs:label "ActivePower" ;
             owl:equivalentClass xsd:float .


###  http://iec.ch/TC57/CIM-generic#ActivePowerChangeRate
:ActivePowerChangeRate rdf:type rdfs:Datatype ;
                       uml:hasUnits "WPers" ;
                       rdfs:comment "Rate of change of active power per time." ;
                       rdfs:label "ActivePowerChangeRate" ;
                       owl:equivalentClass xsd:float .


###  http://iec.ch/TC57/CIM-generic#ActivePowerPerCurrentFlow
:ActivePowerPerCurrentFlow rdf:type rdfs:Datatype ;
                           uml:hasUnits "WPerA" ;
                           rdfs:comment "Active power variation with current flow." ;
                           rdfs:label "ActivePowerPerCurrentFlow" ;
                           owl:equivalentClass xsd:float .


###  http://iec.ch/TC57/CIM-generic#ActivePowerPerFrequency
:ActivePowerPerFrequency rdf:type rdfs:Datatype ;
                         uml:hasUnits "WPers" ;
                         rdfs:comment "Active power variation with frequency." ;
                         rdfs:label "ActivePowerPerFrequency" ;
                         owl:equivalentClass xsd:float .


###  http://iec.ch/TC57/CIM-generic#Admittance
:Admittance rdf:type rdfs:Datatype ;
            uml:hasUnits "S" ;
            rdfs:comment "Ratio of current to voltage." ;
            rdfs:label "Admittance" ;
            owl:equivalentClass xsd:float .


###  http://iec.ch/TC57/CIM-generic#AngleDegrees
:AngleDegrees rdf:type rdfs:Datatype ;
              uml:hasMultiplier "none" ;
              uml:hasUnits "deg" ;
              rdfs:comment "Measurement of angle in degrees." ;
              rdfs:label "AngleDegrees" ;
              owl:equivalentClass xsd:float .


###  http://iec.ch/TC57/CIM-generic#AngleRadians
:AngleRadians rdf:type rdfs:Datatype ;
              uml:hasMultiplier "none" ;
              uml:hasUnits "rad" ;
              rdfs:comment "Phase angle in radians." ;
              rdfs:label "AngleRadians" ;
              owl:equivalentClass xsd:float .


###  http://iec.ch/TC57/CIM-generic#ApparentPower
:ApparentPower rdf:type rdfs:Datatype ;
               uml:hasUnits "VA" ;
               rdfs:comment "Product of the RMS value of the voltage and the RMS value of the current." ;
               rdfs:label "ApparentPower" ;
               owl:equivalentClass xsd:float .


###  http://iec.ch/TC57/CIM-generic#Area
:Area rdf:type rdfs:Datatype ;
      uml:hasUnits "m2" ;
      rdfs:comment "Area." ;
      rdfs:label "Area" ;
      owl:equivalentClass xsd:float .


###  http://iec.ch/TC57/CIM-generic#Bearing
:Bearing rdf:type rdfs:Datatype ;
         uml:hasMultiplier "none" ;
         uml:hasUnits "deg" ;
         rdfs:comment "The bearing in degrees (with 360 degrees being True North).  Measured in degrees clockwise from True North.  0 degrees indicates no direction being given." ;
         rdfs:label "Bearing" ;
         owl:equivalentClass xsd:float .


###  http://iec.ch/TC57/CIM-generic#Capacitance
:Capacitance rdf:type rdfs:Datatype ;
             uml:hasUnits "F" ;
             rdfs:comment "Capacitive part of reactance (imaginary part of impedance), at rated frequency." ;
             rdfs:label "Capacitance" ;
             owl:equivalentClass xsd:float .


###  http://iec.ch/TC57/CIM-generic#CapacitancePerLength
:CapacitancePerLength rdf:type rdfs:Datatype ;
                      uml:hasMultiplier "none" ;
                      uml:hasUnits "FPerm" ;
                      rdfs:comment "Capacitance per unit of length." ;
                      rdfs:label "CapacitancePerLength" ;
                      owl:equivalentClass xsd:float .


###  http://iec.ch/TC57/CIM-generic#Classification
:Classification rdf:type rdfs:Datatype ;
                uml:hasMultiplier "none" ;
                uml:hasUnits "none" ;
                rdfs:comment "Classification of level.  Specify as 1..n, with 1 being the most detailed, highest priority, etc as described on the attribute using this data type." ;
                rdfs:label "Classification" ;
                owl:equivalentClass xsd:integer .

###  http://iec.ch/TC57/CIM-generic#Conductance
:Conductance rdf:type rdfs:Datatype ;
             uml:hasUnits "S" ;
             rdfs:comment "Factor by which voltage must be multiplied to give corresponding power lost from a circuit. Real part of admittance." ;
             rdfs:label "Conductance" ;
             owl:equivalentClass xsd:float .


###  http://iec.ch/TC57/CIM-generic#ConductancePerLength
:ConductancePerLength rdf:type rdfs:Datatype ;
                      uml:hasMultiplier "none" ;
                      uml:hasUnits "SPerm" ;
                      rdfs:comment "Real part of admittance per unit of length." ;
                      rdfs:label "ConductancePerLength" ;
                      owl:equivalentClass xsd:float .


###  http://iec.ch/TC57/CIM-generic#CostPerEnergyUnit
:CostPerEnergyUnit rdf:type rdfs:Datatype ;
                   rdfs:comment "Cost, in units of currency, per quantity of electrical energy generated." ;
                   rdfs:label "CostPerEnergyUnit" ;
                   owl:equivalentClass xsd:float .


###  http://iec.ch/TC57/CIM-generic#CostPerHeatUnit
:CostPerHeatUnit rdf:type rdfs:Datatype ;
                 rdfs:comment "Cost, in units of currency, per quantity of heat generated." ;
                 rdfs:label "CostPerHeatUnit" ;
                 owl:equivalentClass xsd:float .


###  http://iec.ch/TC57/CIM-generic#CostPerVolume
:CostPerVolume rdf:type rdfs:Datatype ;
               rdfs:comment "Cost per unit volume." ;
               rdfs:label "CostPerVolume" ;
               owl:equivalentClass xsd:float .


###  http://iec.ch/TC57/CIM-generic#CostRate
:CostRate rdf:type rdfs:Datatype ;
          rdfs:comment "Cost, in units of currency, per elapsed time." ;
          rdfs:label "CostRate" ;
          owl:equivalentClass xsd:float .


###  http://iec.ch/TC57/CIM-generic#CurrentFlow
:CurrentFlow rdf:type rdfs:Datatype ;
             uml:hasUnits "A" ;
             rdfs:comment "Electrical current with sign convention: positive flow is out of the conducting equipment into the connectivity node. Can be both AC and DC." ;
             rdfs:label "CurrentFlow" ;
             owl:equivalentClass xsd:float .


###  http://iec.ch/TC57/CIM-generic#Damping
:Damping rdf:type rdfs:Datatype ;
         uml:hasUnits "onePerHz" ;
         rdfs:comment "Per-unit active power variation with frequency referenced on the system apparent power base. Typical values are in the range 1,0 - 2,0." ;
         rdfs:label "Damping" ;
         owl:equivalentClass xsd:float .


###  http://iec.ch/TC57/CIM-generic#Displacement
:Displacement rdf:type rdfs:Datatype ;
              uml:hasMultiplier "none" ;
              uml:hasUnits "m" ;
              rdfs:comment "Unit of displacement relative to a reference position, hence can be negative." ;
              rdfs:label "Displacement" ;
              owl:equivalentClass xsd:float .


###  http://iec.ch/TC57/CIM-generic#Emission
:Emission rdf:type rdfs:Datatype ;
          uml:hasMultiplier "none" ;
          uml:hasUnits "kgPerJ" ;
          rdfs:comment "Quantity of emission per fuel heat content." ;
          rdfs:label "Emission" ;
          owl:equivalentClass xsd:float .


###  http://iec.ch/TC57/CIM-generic#Frequency
:Frequency rdf:type rdfs:Datatype ;
           uml:hasUnits "Hz" ;
           rdfs:comment "Cycles per second." ;
           rdfs:label "Frequency" ;
           owl:equivalentClass xsd:float .


###  http://iec.ch/TC57/CIM-generic#HeatRate
:HeatRate rdf:type rdfs:Datatype ;
          uml:hasUnits "J" ;
          rdfs:comment "Heat generated, in energy per time unit of elapsed time." ;
          rdfs:label "HeatRate" ;
          owl:equivalentClass xsd:float .


###  http://iec.ch/TC57/CIM-generic#Hours
:Hours rdf:type rdfs:Datatype ;
       uml:hasMultiplier "none" ;
       uml:hasUnits "h" ;
       rdfs:comment "Time specified in hours." ;
       rdfs:label "Hours" ;
       owl:equivalentClass xsd:float .


###  http://iec.ch/TC57/CIM-generic#Impedance
:Impedance rdf:type rdfs:Datatype ;
           uml:hasUnits "ohm" ;
           rdfs:comment "Ratio of voltage to current." ;
           rdfs:label "Impedance" ;
           owl:equivalentClass xsd:float .


###  http://iec.ch/TC57/CIM-generic#Inductance
:Inductance rdf:type rdfs:Datatype ;
            uml:hasUnits "H" ;
            rdfs:comment "Inductive part of reactance (imaginary part of impedance), at rated frequency." ;
            rdfs:label "Inductance" ;
            owl:equivalentClass xsd:float .


###  http://iec.ch/TC57/CIM-generic#InductancePerLength
:InductancePerLength rdf:type rdfs:Datatype ;
                     uml:hasMultiplier "none" ;
                     uml:hasUnits "HPerm" ;
                     rdfs:comment "Inductance per unit of length." ;
                     rdfs:label "InductancePerLength" ;
                     owl:equivalentClass xsd:float .


###  http://iec.ch/TC57/CIM-generic#KiloActivePower
:KiloActivePower rdf:type rdfs:Datatype ;
                 uml:hasMultiplier "k" ;
                 uml:hasUnits "W" ;
                 rdfs:comment "Active power in kilowatts." ;
                 rdfs:label "KiloActivePower" ;
                 owl:equivalentClass xsd:float .


###  http://iec.ch/TC57/CIM-generic#Length
:Length rdf:type rdfs:Datatype ;
        uml:hasUnits "m" ;
        rdfs:comment "Unit of length. It shall be a positive value or zero." ;
        rdfs:label "Length" ;
        owl:equivalentClass xsd:float .


###  http://iec.ch/TC57/CIM-generic#MagneticField
:MagneticField rdf:type rdfs:Datatype ;
               uml:hasMultiplier "n" ;
               uml:hasUnits "T" ;
               rdfs:comment "Magnetic field in nanotesla." ;
               rdfs:label "MagneticField" ;
               owl:equivalentClass xsd:float .


###  http://iec.ch/TC57/CIM-generic#Mass
:Mass rdf:type rdfs:Datatype ;
      uml:hasMultiplier "k" ;
      uml:hasUnits "g" ;
      rdfs:comment "Mass." ;
      rdfs:label "Mass" ;
      owl:equivalentClass xsd:float .


###  http://iec.ch/TC57/CIM-generic#Minutes
:Minutes rdf:type rdfs:Datatype ;
         uml:hasMultiplier "none" ;
         uml:hasUnits "min" ;
         rdfs:comment "Time in minutes." ;
         rdfs:label "Minutes" ;
         owl:equivalentClass xsd:float .


###  http://iec.ch/TC57/CIM-generic#Money
:Money rdf:type rdfs:Datatype ;
       rdfs:comment "Amount of money." ;
       rdfs:label "Money" ;
       owl:equivalentClass xsd:decimal .


###  http://iec.ch/TC57/CIM-generic#MonthDay
:MonthDay rdf:type rdfs:Datatype ;
          rdfs:comment "MonthDay format as \"--mm-dd\", which conforms with XSD data type gMonthDay." ;
          rdfs:label "MonthDay" .


###  http://iec.ch/TC57/CIM-generic#PU
:PU rdf:type rdfs:Datatype ;
    uml:hasMultiplier "none" ;
    uml:hasUnits "none" ;
    rdfs:comment "Per Unit - a positive or negative value referred to a defined base. Values typically range from -10 to +10." ;
    rdfs:label "PU" ;
    owl:equivalentClass xsd:float .


###  http://iec.ch/TC57/CIM-generic#ParticulateDensity
:ParticulateDensity rdf:type rdfs:Datatype ;
                    uml:hasMultiplier "none" ;
                    uml:hasUnits "kgPerm3" ;
                    rdfs:comment "Particulate density as kg/m<sup>3</sup>." ;
                    rdfs:label "ParticulateDensity" ;
                    owl:equivalentClass xsd:float .


###  http://iec.ch/TC57/CIM-generic#PerCent
:PerCent rdf:type rdfs:Datatype ;
         uml:hasMultiplier "none" ;
         uml:hasUnits "none" ;
         rdfs:comment "Percentage on a defined base.   For example, specify as 100 to indicate at the defined base." ;
         rdfs:label "PerCent" ;
         owl:equivalentClass xsd:float .


###  http://iec.ch/TC57/CIM-generic#Pressure
:Pressure rdf:type rdfs:Datatype ;
          uml:hasUnits "Pa" ;
          rdfs:comment "Pressure in pascals." ;
          rdfs:label "Pressure" ;
          owl:equivalentClass xsd:float .


###  http://iec.ch/TC57/CIM-generic#Reactance
:Reactance rdf:type rdfs:Datatype ;
           uml:hasUnits "ohm" ;
           rdfs:comment "Reactance (imaginary part of impedance), at rated frequency." ;
           rdfs:label "Reactance" ;
           owl:equivalentClass xsd:float .


###  http://iec.ch/TC57/CIM-generic#ReactancePerLength
:ReactancePerLength rdf:type rdfs:Datatype ;
                    uml:hasMultiplier "none" ;
                    uml:hasUnits "ohmPerm" ;
                    rdfs:comment "Reactance (imaginary part of impedance) per unit of length, at rated frequency." ;
                    rdfs:label "ReactancePerLength" ;
                    owl:equivalentClass xsd:float .


###  http://iec.ch/TC57/CIM-generic#ReactivePower
:ReactivePower rdf:type rdfs:Datatype ;
               uml:hasUnits "VAr" ;
               rdfs:comment "Product of RMS value of the voltage and the RMS value of the quadrature component of the current." ;
               rdfs:label "ReactivePower" ;
               owl:equivalentClass xsd:float .


###  http://iec.ch/TC57/CIM-generic#RealEnergy
:RealEnergy rdf:type rdfs:Datatype ;
            uml:hasUnits "Wh" ;
            rdfs:comment "Real electrical energy." ;
            rdfs:label "RealEnergy" ;
            owl:equivalentClass xsd:float .


###  http://iec.ch/TC57/CIM-generic#Resistance
:Resistance rdf:type rdfs:Datatype ;
            uml:hasUnits "ohm" ;
            rdfs:comment "Resistance (real part of impedance)." ;
            rdfs:label "Resistance" ;
            owl:equivalentClass xsd:float .


###  http://iec.ch/TC57/CIM-generic#ResistancePerLength
:ResistancePerLength rdf:type rdfs:Datatype ;
                     uml:hasMultiplier "none" ;
                     uml:hasUnits "ohmPerm" ;
                     rdfs:comment "Resistance (real part of impedance) per unit of length." ;
                     rdfs:label "ResistancePerLength" ;
                     owl:equivalentClass xsd:float .


###  http://iec.ch/TC57/CIM-generic#RotationSpeed
:RotationSpeed rdf:type rdfs:Datatype ;
               uml:hasMultiplier "none" ;
               uml:hasUnits "Hz" ;
               rdfs:comment "Number of revolutions per second." ;
               rdfs:label "RotationSpeed" ;
               owl:equivalentClass xsd:float .


###  http://iec.ch/TC57/CIM-generic#Seconds
:Seconds rdf:type rdfs:Datatype ;
         uml:hasMultiplier "none" ;
         uml:hasUnits "s" ;
         
         rdfs:comment "Time, in seconds." ;
         rdfs:label "Seconds" ;
         owl:equivalentClass xsd:float .


###  http://iec.ch/TC57/CIM-generic#Speed
:Speed rdf:type rdfs:Datatype ;
       uml:hasMultiplier "none" ;
       uml:hasUnits "mPers" ;
       
       rdfs:comment "Distance per unit of time." ;
       rdfs:label "Speed" ;
       owl:equivalentClass xsd:float .


###  http://iec.ch/TC57/CIM-generic#Susceptance
:Susceptance rdf:type rdfs:Datatype ;
             uml:hasUnits "S" ;
             
             rdfs:comment "Imaginary part of admittance." ;
             rdfs:label "Susceptance" ;
             owl:equivalentClass xsd:float .


###  http://iec.ch/TC57/CIM-generic#SusceptancePerLength
:SusceptancePerLength rdf:type rdfs:Datatype ;
                      uml:hasMultiplier "none" ;
                      uml:hasUnits "SPerm" ;
                      
                      rdfs:comment "Imaginary part of admittance per unit of length." ;
                      rdfs:label "SusceptancePerLength" ;
                      owl:equivalentClass xsd:float .


###  http://iec.ch/TC57/CIM-generic#Temperature
:Temperature rdf:type rdfs:Datatype ;
             uml:hasMultiplier "none" ;
             uml:hasUnits "degC" ;
             
             rdfs:comment "Value of temperature in degrees Celsius." ;
             rdfs:label "Temperature" ;
             owl:equivalentClass xsd:float .


###  http://iec.ch/TC57/CIM-generic#Voltage
:Voltage rdf:type rdfs:Datatype ;
         uml:hasUnits "V" ;
         
         rdfs:comment "Electrical voltage, can be both AC and DC." ;
         rdfs:label "Voltage" ;
         owl:equivalentClass xsd:float .


###  http://iec.ch/TC57/CIM-generic#VoltagePerReactivePower
:VoltagePerReactivePower rdf:type rdfs:Datatype ;
                         uml:hasUnits "VPerVAr" ;
                         
                         rdfs:comment "Voltage variation with reactive power." ;
                         rdfs:label "VoltagePerReactivePower" ;
                         owl:equivalentClass xsd:float .


###  http://iec.ch/TC57/CIM-generic#Volume
:Volume rdf:type rdfs:Datatype ;
        uml:hasUnits "m3" ;
        
        rdfs:comment "Volume." ;
        rdfs:label "Volume" ;
        owl:equivalentClass xsd:float .


###  http://iec.ch/TC57/CIM-generic#VolumeFlowRate
:VolumeFlowRate rdf:type rdfs:Datatype ;
                uml:hasMultiplier "none" ;
                uml:hasUnits "m3Pers" ;
                
                rdfs:comment "Volume per time." ;
                rdfs:label "VolumeFlowRate" ;
                owl:equivalentClass xsd:float .


###  http://iec.ch/TC57/CIM-generic#WaterLevel
:WaterLevel rdf:type rdfs:Datatype ;
            uml:hasUnits "m" ;
            
            rdfs:comment "Reservoir water level referred to a given datum such as mean sea level." ;
            rdfs:label "WaterLevel" ;
            owl:equivalentClass xsd:float .


###  http://www.w3.org/2001/XMLSchema#date
xsd:date rdf:type rdfs:Datatype .


###  http://www.w3.org/2001/XMLSchema#duration
xsd:duration rdf:type rdfs:Datatype .


###  http://www.w3.org/2001/XMLSchema#time
xsd:time rdf:type rdfs:Datatype .


#################################################################
#    Object Properties
#################################################################Object Propert


###  http://iec.ch/TC57/CIM-generic#BaseVoltage.ConductingEquipment
:BaseVoltage.ConductingEquipment rdf:type owl:ObjectProperty ;
                                 owl:inverseOf :ConductingEquipment.BaseVoltage ;
                                 rdf:type owl:InverseFunctionalProperty ;
                                 rdfs:domain :BaseVoltage ;
                                 rdfs:range :ConductingEquipment ;
                                 
                                 rdfs:comment "All conducting equipment with this base voltage.  Use only when there is no voltage level container used and only one base voltage applies.  For example, not used for transformers." ;
                                 rdfs:label "ConductingEquipment" .


###  http://iec.ch/TC57/CIM-generic#BaseVoltage.VoltageLevel
:BaseVoltage.VoltageLevel rdf:type owl:ObjectProperty ;
                          owl:inverseOf :VoltageLevel.BaseVoltage ;
                          rdf:type owl:InverseFunctionalProperty ;
                          rdfs:domain :BaseVoltage ;
                          rdfs:range :VoltageLevel ;
                          
                          rdfs:comment "The voltage levels having this base voltage." ;
                          rdfs:label "VoltageLevel" .


###  http://iec.ch/TC57/CIM-generic#Bay.Substation
:Bay.Substation rdf:type owl:ObjectProperty ;
                owl:inverseOf :Substation.Bays ;
                rdf:type owl:FunctionalProperty ;
                rdfs:domain :Bay ;
                rdfs:range :Substation ;
                
                rdfs:comment "Substation containing the bay." ;
                rdfs:label "Substation" .


###  http://iec.ch/TC57/CIM-generic#Bay.VoltageLevel
:Bay.VoltageLevel rdf:type owl:ObjectProperty ;
                  owl:inverseOf :VoltageLevel.Bays ;
                  rdf:type owl:FunctionalProperty ;
                  rdfs:domain :Bay ;
                  rdfs:range :VoltageLevel ;
                  
                  rdfs:comment "The voltage level containing this bay." ;
                  rdfs:label "VoltageLevel" .


###  http://iec.ch/TC57/CIM-generic#ConductingEquipment.BaseVoltage
:ConductingEquipment.BaseVoltage rdf:type owl:ObjectProperty ,
                                          owl:FunctionalProperty ;
                                 rdfs:domain :ConductingEquipment ;
                                 rdfs:range :BaseVoltage ;
                                 
                                 rdfs:comment "Base voltage of this conducting equipment.  Use only when there is no voltage level container used and only one base voltage applies.  For example, not used for transformers." ;
                                 rdfs:label "BaseVoltage" .


###  http://iec.ch/TC57/CIM-generic#ConductingEquipment.Terminals
:ConductingEquipment.Terminals rdf:type owl:ObjectProperty ;
                               owl:inverseOf :Terminal.ConductingEquipment ;
                               rdf:type owl:InverseFunctionalProperty ;
                               rdfs:domain :ConductingEquipment ;
                               rdfs:range :Terminal ;
                               
                               rdfs:comment "Conducting equipment have terminals that may be connected to other conducting equipment terminals via connectivity nodes or topological nodes." ;
                               rdfs:label "Terminals" .


###  http://iec.ch/TC57/CIM-generic#ConnectivityNode.ConnectivityNodeContainer
:ConnectivityNode.ConnectivityNodeContainer rdf:type owl:ObjectProperty ;
                                            owl:inverseOf :ConnectivityNodeContainer.ConnectivityNodes ;
                                            rdf:type owl:FunctionalProperty ;
                                            rdfs:domain :ConnectivityNode ;
                                            rdfs:range :ConnectivityNodeContainer ;
                                            
                                            rdfs:comment "Container of this connectivity node." ;
                                            rdfs:label "ConnectivityNodeContainer" .


###  http://iec.ch/TC57/CIM-generic#ConnectivityNode.Terminals
:ConnectivityNode.Terminals rdf:type owl:ObjectProperty ;
                            owl:inverseOf :Terminal.ConnectivityNode ;
                            rdf:type owl:InverseFunctionalProperty ;
                            rdfs:domain :ConnectivityNode ;
                            rdfs:range :Terminal ;
                            
                            rdfs:comment "Terminals interconnected with zero impedance at a this connectivity node." ;
                            rdfs:label "Terminals" .


###  http://iec.ch/TC57/CIM-generic#ConnectivityNodeContainer.ConnectivityNodes
:ConnectivityNodeContainer.ConnectivityNodes rdf:type owl:ObjectProperty ,
                                                      owl:InverseFunctionalProperty ;
                                             rdfs:domain :ConnectivityNodeContainer ;
                                             rdfs:range :ConnectivityNode ;
                                             
                                             rdfs:comment "Connectivity nodes which belong to this connectivity node container." ;
                                             rdfs:label "ConnectivityNodes" .


###  http://iec.ch/TC57/CIM-generic#Equipment.AdditionalEquipmentContainer
:Equipment.AdditionalEquipmentContainer rdf:type owl:ObjectProperty ;
                                        owl:inverseOf :EquipmentContainer.AdditionalGroupedEquipment ;
                                        rdfs:domain :Equipment ;
                                        rdfs:range :EquipmentContainer ;
                                        
                                        rdfs:comment "Additional equipment container beyond the primary equipment container.  The equipment is contained in another equipment container, but also grouped with this equipment container." ;
                                        rdfs:label "AdditionalEquipmentContainer" .


###  http://iec.ch/TC57/CIM-generic#Equipment.EquipmentContainer
:Equipment.EquipmentContainer rdf:type owl:ObjectProperty ;
                              owl:inverseOf :EquipmentContainer.Equipments ;
                              rdf:type owl:FunctionalProperty ;
                              rdfs:domain :Equipment ;
                              rdfs:range :EquipmentContainer ;
                              
                              rdfs:comment "Container of this equipment." ;
                              rdfs:label "EquipmentContainer" .


###  http://iec.ch/TC57/CIM-generic#EquipmentContainer.AdditionalGroupedEquipment
:EquipmentContainer.AdditionalGroupedEquipment rdf:type owl:ObjectProperty ;
                                               rdfs:domain :EquipmentContainer ;
                                               rdfs:range :Equipment ;
                                               
                                               rdfs:comment "The additonal contained equipment.  The equipment belong to the equipment container. The equipment is contained in another equipment container, but also grouped with this equipment container.  Examples include when a switch contained in a substation is also desired to be grouped with a line contianer or when a switch is included in a secondary substation and also grouped in a feeder." ;
                                               rdfs:label "AdditionalGroupedEquipment" .


###  http://iec.ch/TC57/CIM-generic#EquipmentContainer.Equipments
:EquipmentContainer.Equipments rdf:type owl:ObjectProperty ,
                                        owl:InverseFunctionalProperty ;
                               rdfs:domain :EquipmentContainer ;
                               rdfs:range :Equipment ;
                               
                               rdfs:comment "Contained equipment." ;
                               rdfs:label "Equipments" .


###  http://iec.ch/TC57/CIM-generic#GeographicalRegion.Regions
:GeographicalRegion.Regions rdf:type owl:ObjectProperty ;
                            owl:inverseOf :SubGeographicalRegion.Region ;
                            rdf:type owl:InverseFunctionalProperty ;
                            rdfs:domain :GeographicalRegion ;
                            rdfs:range :SubGeographicalRegion ;
                            
                            rdfs:comment "All sub-geographical regions within this geographical region." ;
                            rdfs:label "Regions" .


###  http://iec.ch/TC57/CIM-generic#IdentifiedObject.Names
:IdentifiedObject.Names rdf:type owl:ObjectProperty ;
                        owl:inverseOf :Name.IdentifiedObject ;
                        rdf:type owl:InverseFunctionalProperty ;
                        rdfs:domain :IdentifiedObject ;
                        rdfs:range :Name ;
                        
                        rdfs:comment "All names of this identified object." ;
                        rdfs:label "Names" .


###  http://iec.ch/TC57/CIM-generic#Line.Region
:Line.Region rdf:type owl:ObjectProperty ;
             owl:inverseOf :SubGeographicalRegion.Lines ;
             rdf:type owl:FunctionalProperty ;
             rdfs:domain :Line ;
             rdfs:range :SubGeographicalRegion ;
             
             rdfs:comment "The sub-geographical region of the line." ;
             rdfs:label "Region" .


### http://iec.ch/TC57/CIM-generic#Measurement.PowerSystemResource
:Measurement.PowerSystemResource rdf:type owl:ObjectProperty ;
                                 owl:inverseOf :PowerSystemResource.Measurements ;
                                 rdf:type owl:InverseFunctionalProperty ;
                                 rdfs:domain :Measurement ;
                                 rdfs:range :PowerSystemResource ;
                                 
                                 rdfs:comment "Power system resource to which this measurement belongs." ;
                                 rdfs:label "PowerSystemResource" .


### http://iec.ch/TC57/CIM-generic#Measurement.Measurements
:Measurement.Measurements rdf:type owl:ObjectProperty ;
                          owl:inverseOf :Measurement.Terminal ;
                          rdfs:domain :Measurement ;
                          rdfs:range :ACDCTerminal ;
                          rdfs:comment "Power system resources to which this measurement belongs." ;
                          rdfs:label "Measurements" .


### http://iec.ch/TC57/CIM-generic#Measurement.Locations
:Measurement.Locations rdf:type owl:ObjectProperty ;
                       owl:inverseOf :Location.Measurements ;
                       rdfs:domain :Measurement ;
                       rdfs:range :Location ;
                       rdfs:comment "The location of this measurement." ;
                       rdfs:label "Locations" .


# ### http://iec.ch/TC57/CIM-generic#Measurement.Asset
# :Measurement.Asset rdf:type owl:ObjectProperty ;
#                    owl:inverseOf :Asset.Measurements ;
#                    rdfs:domain :Measurement ;
#                    rdfs:range :Asset ;
#                    rdfs:comment "The asset to which this measurement is associated." ;
#                    rdfs:label "Asset" .




###  http://iec.ch/TC57/CIM-generic#Name.IdentifiedObject
:Name.IdentifiedObject rdf:type owl:ObjectProperty ,
                                owl:FunctionalProperty ;
                       rdfs:domain :Name ;
                       rdfs:range :IdentifiedObject ;
                       
                       rdfs:comment "Identified object that this name designates." ;
                       rdfs:label "IdentifiedObject" .


###  http://iec.ch/TC57/CIM-generic#Name.NameType
:Name.NameType rdf:type owl:ObjectProperty ;
               owl:inverseOf :NameType.Names ;
               rdf:type owl:FunctionalProperty ;
               rdfs:domain :Name ;
               rdfs:range :NameType ;
               
               rdfs:comment "Type of this name." ;
               rdfs:label "NameType" .


###  http://iec.ch/TC57/CIM-generic#NameType.Names
:NameType.Names rdf:type owl:ObjectProperty ,
                         owl:InverseFunctionalProperty ;
                rdfs:domain :NameType ;
                rdfs:range :Name ;
                
                rdfs:comment "All names of this type." ;
                rdfs:label "Names" .


###  http://iec.ch/TC57/CIM-generic#PSRType.PowerSystemResources
:PSRType.PowerSystemResources rdf:type owl:ObjectProperty ;
                              owl:inverseOf :PowerSystemResource.PSRType ;
                              rdf:type owl:InverseFunctionalProperty ;
                              rdfs:domain :PSRType ;
                              rdfs:range :PowerSystemResource ;
                              
                              rdfs:comment "Power system resources classified with this power system resource type." ;
                              rdfs:label "PowerSystemResources" .


###  http://iec.ch/TC57/CIM-generic#PowerSystemResource.PSRType
:PowerSystemResource.PSRType rdf:type owl:ObjectProperty ,
                                      owl:FunctionalProperty ;
                             rdfs:domain :PowerSystemResource ;
                             rdfs:range :PSRType ;
                             
                             rdfs:comment "Custom classification for this power system resource." ;
                             rdfs:label "PSRType" .


### http://iec.ch/TC57/CIM-generic#PowerSystemResource.Measurements
:PowerSystemResource.Measurements rdf:type owl:ObjectProperty ;
                                 owl:inverseOf :Measurement.PowerSystemResource ;
                                 rdfs:domain :PowerSystemResource ;
                                 rdfs:range :Measurement ;
                                 rdfs:comment "Measurements for this power system resource." ;
                                 rdfs:label "Measurements" .


###  http://iec.ch/TC57/CIM-generic#SubGeographicalRegion.Lines
:SubGeographicalRegion.Lines rdf:type owl:ObjectProperty ,
                                      owl:InverseFunctionalProperty ;
                             rdfs:domain :SubGeographicalRegion ;
                             rdfs:range :Line ;
                             
                             rdfs:comment "The lines within the sub-geographical region." ;
                             rdfs:label "Lines" .



###  http://iec.ch/TC57/CIM-generic#SubGeographicalRegion.Region
:SubGeographicalRegion.Region rdf:type owl:ObjectProperty ,
                                       owl:FunctionalProperty ;
                              rdfs:domain :SubGeographicalRegion ;
                              rdfs:range :GeographicalRegion ;
                              
                              rdfs:comment "The geographical region which this sub-geographical region is within." ;
                              rdfs:label "Region" .


###  http://iec.ch/TC57/CIM-generic#SubGeographicalRegion.Substations
:SubGeographicalRegion.Substations rdf:type owl:ObjectProperty ;
                                   owl:inverseOf :Substation.Region ;
                                   rdf:type owl:InverseFunctionalProperty ;
                                   rdfs:domain :SubGeographicalRegion ;
                                   rdfs:range :Substation ;
                                   
                                   rdfs:comment "The substations in this sub-geographical region." ;
                                   rdfs:label "Substations" .


###  http://iec.ch/TC57/CIM-generic#Substation.Bays
:Substation.Bays rdf:type owl:ObjectProperty ,
                          owl:InverseFunctionalProperty ;
                 rdfs:domain :Substation ;
                 rdfs:range :Bay ;
                 
                 rdfs:comment "Bays contained in the substation." ;
                 rdfs:label "Bays" .


###  http://iec.ch/TC57/CIM-generic#Substation.Region
:Substation.Region rdf:type owl:ObjectProperty ,
                            owl:FunctionalProperty ;
                   rdfs:domain :Substation ;
                   rdfs:range :SubGeographicalRegion ;
                   
                   rdfs:comment "The SubGeographicalRegion containing the substation." ;
                   rdfs:label "Region" .


###  http://iec.ch/TC57/CIM-generic#Substation.VoltageLevels
:Substation.VoltageLevels rdf:type owl:ObjectProperty ;
                          owl:inverseOf :VoltageLevel.Substation ;
                          rdf:type owl:InverseFunctionalProperty ;
                          rdfs:domain :Substation ;
                          rdfs:range :VoltageLevel ;
                          
                          rdfs:comment "The voltage levels within this substation." ;
                          rdfs:label "VoltageLevels" .


###  http://iec.ch/TC57/CIM-generic#Terminal.ConductingEquipment
:Terminal.ConductingEquipment rdf:type owl:ObjectProperty ,
                                       owl:FunctionalProperty ;
                              rdfs:domain :Terminal ;
                              rdfs:range :ConductingEquipment ;
                              
                              rdfs:comment "The conducting equipment of the terminal.  Conducting equipment have  terminals that may be connected to other conducting equipment terminals via connectivity nodes or topological nodes." ;
                              rdfs:label "ConductingEquipment" .


###  http://iec.ch/TC57/CIM-generic#Terminal.ConnectivityNode
:Terminal.ConnectivityNode rdf:type owl:ObjectProperty ,
                                    owl:FunctionalProperty ;
                           rdfs:domain :Terminal ;
                           rdfs:range :ConnectivityNode ;
                           
                           rdfs:comment "The connectivity node to which this terminal connects with zero impedance." ;
                           rdfs:label "ConnectivityNode" .


###  http://iec.ch/TC57/CIM-generic#Terminal.phases
:Terminal.phases rdf:type owl:ObjectProperty ,
                          owl:FunctionalProperty ;
                 rdfs:domain :Terminal ;
                 rdfs:range :PhaseCode ;
                 
                 rdfs:comment """Represents the normal network phasing condition. If the attribute is missing, three phases (ABC) shall be assumed, except for terminals of grounding classes (specializations of EarthFaultCompensator, GroundDisconnector, and Ground) which will be assumed to be N. Therefore, phase code ABCN is explicitly declared when needed, e.g. for star point grounding equipment.
The phase code on terminals connecting same ConnectivityNode or same TopologicalNode as well as for equipment between two terminals shall be consistent.""" ;
                 rdfs:label "phases" .


###  http://iec.ch/TC57/CIM-generic#VoltageLevel.BaseVoltage
:VoltageLevel.BaseVoltage rdf:type owl:ObjectProperty ,
                                   owl:FunctionalProperty ;
                          rdfs:domain :VoltageLevel ;
                          rdfs:range :BaseVoltage ;
                          
                          rdfs:comment "The base voltage used for all equipment within the voltage level." ;
                          rdfs:label "BaseVoltage" .


###  http://iec.ch/TC57/CIM-generic#VoltageLevel.Bays
:VoltageLevel.Bays rdf:type owl:ObjectProperty ,
                            owl:InverseFunctionalProperty ;
                   rdfs:domain :VoltageLevel ;
                   rdfs:range :Bay ;
                   
                   rdfs:comment "The bays within this voltage level." ;
                   rdfs:label "Bays" .


###  http://iec.ch/TC57/CIM-generic#VoltageLevel.Substation
:VoltageLevel.Substation rdf:type owl:ObjectProperty ,
                                  owl:FunctionalProperty ;
                         rdfs:domain :VoltageLevel ;
                         rdfs:range :Substation ;
                         
                         rdfs:comment "The substation of the voltage level." ;
                         rdfs:label "Substation" .


#################################################################
#    Data properties
#################################################################

###  http://iec.ch/TC57/CIM-generic#ACDCTerminal.connected
:ACDCTerminal.connected rdf:type owl:DatatypeProperty ,
                                 owl:FunctionalProperty ;
                        rdfs:domain :ACDCTerminal ;
                        rdfs:range xsd:boolean ;
                        
                        rdfs:comment """The connected status is related to a bus-branch model and the topological node to terminal relation.  True implies the terminal is connected to the related topological node and false implies it is not. 
In a bus-branch model, the connected status is used to tell if equipment is disconnected without having to change the connectivity described by the topological node to terminal relation. A valid case is that conducting equipment can be connected in one end and open in the other. In particular for an AC line segment, where the reactive line charging can be significant, this is a relevant case.""" ;
                        rdfs:label "connected" .


###  http://iec.ch/TC57/CIM-generic#ACDCTerminal.sequenceNumber
:ACDCTerminal.sequenceNumber rdf:type owl:DatatypeProperty ,
                                      owl:FunctionalProperty ;
                             rdfs:domain :ACDCTerminal ;
                             rdfs:range xsd:integer ;
                             
                             rdfs:comment "The orientation of the terminal connections for a multiple terminal conducting equipment.  The sequence numbering starts with 1 and additional terminals should follow in increasing order.   The first terminal is the \"starting point\" for a two terminal branch." ;
                             rdfs:label "sequenceNumber" .


### http://iec.ch/TC57/CIM-generic#Analog.maxValue
:Analog.maxValue rdf:type owl:DatatypeProperty ,
                        owl:FunctionalProperty ;
               rdfs:domain :Analog ;
               rdfs:range xsd:float ;
               rdfs:comment "The maximum value that can be measured by the analog." ;
               rdfs:label "maxValue" .


### http://iec.ch/TC57/CIM-generic#Analog.minValue
:Analog.minValue rdf:type owl:DatatypeProperty ,
                        owl:FunctionalProperty ;
               rdfs:domain :Analog ;
               rdfs:range xsd:float ;
               rdfs:comment "The minimum value that can be measured by the analog." ;
               rdfs:label "minValue" .


### http://iec.ch/TC57/CIM-generic#Analog.normalValue
:Analog.normalValue rdf:type owl:DatatypeProperty ,
                           owl:FunctionalProperty ;
                  rdfs:domain :Analog ;
                  rdfs:range xsd:float ;
                  rdfs:comment "The normal value for the analog." ;
                  rdfs:label "normalValue" .


### http://iec.ch/TC57/CIM-generic#Analog.positiveFlowIn
:Analog.positiveFlowIn rdf:type owl:DatatypeProperty ,
                            owl:FunctionalProperty ;
                   rdfs:domain :Analog ;
                   rdfs:range xsd:boolean ;
                   rdfs:comment "The positive flow direction into the conducting equipment when current is positive." ;
                   rdfs:label "positiveFlowIn" .



###  http://iec.ch/TC57/CIM-generic#BaseFrequency.frequency
:BaseFrequency.frequency rdf:type owl:DatatypeProperty ,
                                  owl:FunctionalProperty ;
                         rdfs:domain :BaseFrequency ;
                         rdfs:range :Frequency ;
                         
                         rdfs:comment "The base frequency." ;
                         rdfs:label "frequency" .


###  http://iec.ch/TC57/CIM-generic#BasePower.basePower
:BasePower.basePower rdf:type owl:DatatypeProperty ,
                              owl:FunctionalProperty ;
                     rdfs:domain :BasePower ;
                     rdfs:range :ApparentPower ;
                     
                     rdfs:comment "Value used as base power." ;
                     rdfs:label "basePower" .


###  http://iec.ch/TC57/CIM-generic#BaseVoltage.nominalVoltage
:BaseVoltage.nominalVoltage rdf:type owl:DatatypeProperty ,
                                     owl:FunctionalProperty ;
                            rdfs:domain :BaseVoltage ;
                            rdfs:range :Voltage ;
                            
                            rdfs:comment "The power system resource's base voltage.  Shall be a positive value and not zero." ;
                            rdfs:label "nominalVoltage" .


###  http://iec.ch/TC57/CIM-generic#Bay.bayEnergyMeasFlag
:Bay.bayEnergyMeasFlag rdf:type owl:DatatypeProperty ,
                                owl:FunctionalProperty ;
                       rdfs:domain :Bay ;
                       rdfs:range xsd:boolean ;
                       
                       rdfs:comment "Indicates the presence/absence of energy measurements." ;
                       rdfs:label "bayEnergyMeasFlag" .


###  http://iec.ch/TC57/CIM-generic#Bay.bayPowerMeasFlag
:Bay.bayPowerMeasFlag rdf:type owl:DatatypeProperty ,
                               owl:FunctionalProperty ;
                      rdfs:domain :Bay ;
                      rdfs:range xsd:boolean ;
                      
                      rdfs:comment "Indicates the presence/absence of active/reactive power measurements." ;
                      rdfs:label "bayPowerMeasFlag" .


###  http://iec.ch/TC57/CIM-generic#Breaker.inTransitTime
:Breaker.inTransitTime rdf:type owl:DatatypeProperty ,
                                owl:FunctionalProperty ;
                       rdfs:domain :Breaker ;
                       rdfs:range :Seconds ;
                       
                       rdfs:comment "The transition time from open to close." ;
                       rdfs:label "inTransitTime" .


###  http://iec.ch/TC57/CIM-generic#Equipment.aggregate
:Equipment.aggregate rdf:type owl:DatatypeProperty ,
                              owl:FunctionalProperty ;
                     rdfs:domain :Equipment ;
                     rdfs:range xsd:boolean ;
                     
                     rdfs:comment """The aggregate flag provides an alternative way of representing an aggregated (equivalent) element. It is applicable in cases when the dedicated classes for equivalent equipment do not have all of the attributes necessary to represent the required level of detail.  In case the flag is set to “true” the single instance of equipment represents multiple pieces of equipment that have been modelled together as an aggregate equivalent obtained by a network reduction procedure. Examples would be power transformers or synchronous machines operating in parallel modelled as a single aggregate power transformer or aggregate synchronous machine.  
The attribute is not used for EquivalentBranch, EquivalentShunt and EquivalentInjection.""" ;
                     rdfs:label "aggregate" .


###  http://iec.ch/TC57/CIM-generic#Equipment.inService
:Equipment.inService rdf:type owl:DatatypeProperty ,
                              owl:FunctionalProperty ;
                     rdfs:domain :Equipment ;
                     rdfs:range xsd:boolean ;
                     
                     rdfs:comment "Specifies the availability of the equipment. True means the equipment is available for topology processing, which determines if the equipment is energized or not. False means that the equipment is treated by network applications as if it is not in the model." ;
                     rdfs:label "inService" .


###  http://iec.ch/TC57/CIM-generic#Equipment.networkAnalysisEnabled
:Equipment.networkAnalysisEnabled rdf:type owl:DatatypeProperty ,
                                           owl:FunctionalProperty ;
                                  rdfs:domain :Equipment ;
                                  rdfs:range xsd:boolean ;
                                  
                                  rdfs:comment "The equipment is enabled to participate in network analysis.  If unspecified, the value is assumed to be true." ;
                                  rdfs:label "networkAnalysisEnabled" .


###  http://iec.ch/TC57/CIM-generic#Equipment.normallyInService
:Equipment.normallyInService rdf:type owl:DatatypeProperty ,
                                      owl:FunctionalProperty ;
                             rdfs:domain :Equipment ;
                             rdfs:range xsd:boolean ;
                             
                             rdfs:comment "Specifies the availability of the equipment under normal operating conditions. True means the equipment is available for topology processing, which determines if the equipment is energized or not. False means that the equipment is treated by network applications as if it is not in the model." ;
                             rdfs:label "normallyInService" .


###  http://iec.ch/TC57/CIM-generic#IEC61970CIMVersion.date
:IEC61970CIMVersion.date rdf:type owl:DatatypeProperty ,
                                  owl:FunctionalProperty ;
                         rdfs:range xsd:date ;
                         uml:hasInitialValue "2020-08-24" ;
                         
                         rdfs:comment "Form is YYYY-MM-DD for example for January 5, 2009 it is 2009-01-05." ;
                         rdfs:label "date" .


###  http://iec.ch/TC57/CIM-generic#IdentifiedObject.aliasName
:IdentifiedObject.aliasName rdf:type owl:DatatypeProperty ,
                                     owl:FunctionalProperty ;
                            rdfs:domain :IdentifiedObject ;
                            rdfs:range xsd:string ;
                            
                            rdfs:comment """The aliasName is free text human readable name of the object alternative to IdentifiedObject.name. It may be non unique and may not correlate to a naming hierarchy.
The attribute aliasName is retained because of backwards compatibility between CIM relases. It is however recommended to replace aliasName with the Name class as aliasName is planned for retirement at a future time.""" ;
                            rdfs:label "aliasName" .


###  http://iec.ch/TC57/CIM-generic#IdentifiedObject.description
:IdentifiedObject.description rdf:type owl:DatatypeProperty ,
                                       owl:FunctionalProperty ;
                              rdfs:domain :IdentifiedObject ;
                              rdfs:range xsd:string ;
                              
                              rdfs:comment "The description is a free human readable text describing or naming the object. It may be non unique and may not correlate to a naming hierarchy." ;
                              rdfs:label "description" .


###  http://iec.ch/TC57/CIM-generic#IdentifiedObject.mRID
:IdentifiedObject.mRID rdf:type owl:DatatypeProperty ,
                                owl:FunctionalProperty ;
                       rdfs:domain :IdentifiedObject ;
                       rdfs:range xsd:string ;
                       
                       rdfs:comment """Master resource identifier issued by a model authority. The mRID is unique within an exchange context. Global uniqueness is easily achieved by using a UUID, as specified in RFC 4122, for the mRID. The use of UUID is strongly recommended.
For CIMXML data files in RDF syntax conforming to IEC 61970-552, the mRID is mapped to rdf:ID or rdf:about attributes that identify CIM object elements.""" ;
                       rdfs:label "mRID" .


###  http://iec.ch/TC57/CIM-generic#IdentifiedObject.name
:IdentifiedObject.name rdf:type owl:DatatypeProperty ,
                                owl:FunctionalProperty ;
                       rdfs:domain :IdentifiedObject ;
                       rdfs:range xsd:string ;
                       
                       rdfs:comment "The name is any free human readable and possibly non unique text naming the object." ;
                       rdfs:label "name" .


### http://iec.ch/TC57/CIM-generic#Location.address
:Location.address rdf:type owl:DatatypeProperty ,
                          owl:FunctionalProperty ;
                 rdfs:domain :Location ;
                 rdfs:range xsd:string ;
                 #
                 rdfs:comment "The address of the location." ;
                 rdfs:label "address" . 


### http://iec.ch/TC57/CIM-generic#Location.xPosition
:Location.xPosition rdf:type owl:DatatypeProperty ,
                           owl:FunctionalProperty ;
                  rdfs:domain :Location ;
                  rdfs:range xsd:string ;
                  #
                  rdfs:comment "The x-coordinate of the point in the coordinate system specified by the associated PositionPoint." ;
                  rdfs:label "xPosition" .


### http://iec.ch/TC57/CIM-generic#Location.yPosition
:Location.yPosition rdf:type owl:DatatypeProperty ,
                           owl:FunctionalProperty ;
                  rdfs:domain :Location ;
                  rdfs:range xsd:string ;
                  #
                  rdfs:comment "The y-coordinate of the point in the coordinate system specified by the associated PositionPoint." ;
                  rdfs:label "yPosition" .


### http://iec.ch/TC57/CIM-generic#Measurement.measurementType
:Measurement.measurementType rdf:type owl:DatatypeProperty ,
                                      owl:FunctionalProperty ;
                        rdfs:domain :Measurement ;
                        rdfs:range xsd:string ;
                        #
                        rdfs:comment "Type of measurement." ;
                        rdfs:label "measurementType" .


### http://iec.ch/TC57/CIM-generic#Measurement.phases
:Measurement.phases rdf:type owl:DatatypeProperty ,
                             owl:FunctionalProperty ;
                    rdfs:domain :Measurement ;
                    rdfs:range :PhaseCode ;
                    #
                    rdfs:comment "Represents the normal network phasing condition. If the attribute is missing, three phases (ABC) shall be assumed, except for terminals of grounding classes (specializations of EarthFaultCompensator, GroundDisconnector, and Ground) which will be assumed to be N. Therefore, phase code ABCN is explicitly declared when needed, e.g. for star point grounding equipment." ;
                    rdfs:label "phases" .


### http://iec.ch/TC57/CIM-generic#Measurement.unitMultiplier
:Measurement.unitMultiplier rdf:type owl:DatatypeProperty ,
                             owl:FunctionalProperty ;
                    rdfs:domain :Measurement ;
                    rdfs:range :UnitMultiplier ;
                    rdfs:comment "Unit multiplier for the measurement value." ;
                    rdfs:label "unitMultiplier" .


### http://iec.ch/TC57/CIM-generic#Measurement.unitSymbol
:Measurement.unitSymbol rdf:type owl:DatatypeProperty ,
                             owl:FunctionalProperty ;
                    rdfs:domain :Measurement ;
                    rdfs:range xsd:string ;
                    rdfs:comment "Unit symbol for the measurement value." ;
                    rdfs:label "unitSymbol" .


###  http://iec.ch/TC57/CIM-generic#Name.name
:Name.name rdf:type owl:DatatypeProperty ,
                    owl:FunctionalProperty ;
           rdfs:domain :Name ;
           rdfs:range xsd:string ;
           
           rdfs:comment "Any free text that name the object." ;
           rdfs:label "name" .


###  http://iec.ch/TC57/CIM-generic#NameType.description
:NameType.description rdf:type owl:DatatypeProperty ,
                               owl:FunctionalProperty ;
                      rdfs:domain :NameType ;
                      rdfs:range xsd:string ;
                      
                      rdfs:comment "Description of the name type." ;
                      rdfs:label "description" .


###  http://iec.ch/TC57/CIM-generic#NameType.name
:NameType.name rdf:type owl:DatatypeProperty ,
                        owl:FunctionalProperty ;
               rdfs:domain :NameType ;
               rdfs:range xsd:string ;
               
               rdfs:comment "Name of the name type." ;
               rdfs:label "name" .


###  http://iec.ch/TC57/CIM-generic#ProtectedSwitch.breakingCapacity
:ProtectedSwitch.breakingCapacity rdf:type owl:DatatypeProperty ,
                                           owl:FunctionalProperty ;
                                  rdfs:domain :ProtectedSwitch ;
                                  rdfs:range :CurrentFlow ;
                                  
                                  rdfs:comment "The maximum fault current a breaking device can break safely under prescribed conditions of use." ;
                                  rdfs:label "breakingCapacity" .


###  http://iec.ch/TC57/CIM-generic#Switch.locked
:Switch.locked rdf:type owl:DatatypeProperty ,
                        owl:FunctionalProperty ;
               rdfs:domain :Switch ;
               rdfs:range xsd:boolean ;
               
               rdfs:comment """If true, the switch is locked. The resulting switch state is a combination of locked and Switch.open attributes as follows:
<ul>
	<li>locked=true and Switch.open=true. The resulting state is open and locked;</li>
	<li>locked=false and Switch.open=true. The resulting state is open;</li>
	<li>locked=false and Switch.open=false. The resulting state is closed.</li>
</ul>""" ;
               rdfs:label "locked" .


###  http://iec.ch/TC57/CIM-generic#Switch.normalOpen
:Switch.normalOpen rdf:type owl:DatatypeProperty ,
                            owl:FunctionalProperty ;
                   rdfs:domain :Switch ;
                   rdfs:range xsd:boolean ;
                   
                   rdfs:comment "The attribute is used in cases when no Measurement for the status value is present. If the Switch has a status measurement the Discrete.normalValue is expected to match with the Switch.normalOpen." ;
                   rdfs:label "normalOpen" .


###  http://iec.ch/TC57/CIM-generic#Switch.open
:Switch.open rdf:type owl:DatatypeProperty ,
                      owl:FunctionalProperty ;
             rdfs:domain :Switch ;
             rdfs:range xsd:boolean ;
             
             rdfs:comment "The attribute tells if the switch is considered open when used as input to topology processing." ;
             rdfs:label "open" .


###  http://iec.ch/TC57/CIM-generic#Switch.ratedCurrent
:Switch.ratedCurrent rdf:type owl:DatatypeProperty ,
                              owl:FunctionalProperty ;
                     rdfs:domain :Switch ;
                     rdfs:range :CurrentFlow ;
                     
                     rdfs:comment """The maximum continuous current carrying capacity in amps governed by the device material and construction.
The attribute shall be a positive value.""" ;
                     rdfs:label "ratedCurrent" .


###  http://iec.ch/TC57/CIM-generic#Switch.retained
:Switch.retained rdf:type owl:DatatypeProperty ,
                          owl:FunctionalProperty ;
                 rdfs:domain :Switch ;
                 rdfs:range xsd:boolean ;
                 
                 rdfs:comment "Branch is retained in the topological solution.  The flow through retained switches will normally be calculated in power flow." ;
                 rdfs:label "retained" .


###  http://iec.ch/TC57/CIM-generic#Switch.switchOnCount
:Switch.switchOnCount rdf:type owl:DatatypeProperty ,
                               owl:FunctionalProperty ;
                      rdfs:domain :Switch ;
                      rdfs:range xsd:integer ;
                      
                      rdfs:comment "The switch on count since the switch was last reset or initialized." ;
                      rdfs:label "switchOnCount" .


###  http://iec.ch/TC57/CIM-generic#Switch.switchOnDate
:Switch.switchOnDate rdf:type owl:DatatypeProperty ,
                              owl:FunctionalProperty ;
                     rdfs:domain :Switch ;
                     rdfs:range xsd:dateTime ;
                     
                     rdfs:comment "The date and time when the switch was last switched on." ;
                     rdfs:label "switchOnDate" .


###  http://iec.ch/TC57/CIM-generic#TapChanger.controlEnabled
:TapChanger.controlEnabled rdf:type owl:DatatypeProperty ,
                                    owl:FunctionalProperty ;
                           rdfs:domain :TapChanger ;
                           rdfs:range xsd:boolean ;
                           
                           rdfs:comment "Specifies the regulation status of the equipment.  True is regulating, false is not regulating." ;
                           rdfs:label "controlEnabled" .


###  http://iec.ch/TC57/CIM-generic#TapChanger.highStep
:TapChanger.highStep rdf:type owl:DatatypeProperty ,
                              owl:FunctionalProperty ;
                     rdfs:domain :TapChanger ;
                     rdfs:range xsd:integer ;
                     
                     rdfs:comment """Highest possible tap step position, advance from neutral.
The attribute shall be greater than lowStep.""" ;
                     rdfs:label "highStep" .


###  http://iec.ch/TC57/CIM-generic#TapChanger.initialDelay
:TapChanger.initialDelay rdf:type owl:DatatypeProperty ,
                                  owl:FunctionalProperty ;
                         rdfs:domain :TapChanger ;
                         rdfs:range :Seconds ;
                         
                         rdfs:comment "For an LTC, the delay for initial tap changer operation (first step change)." ;
                         rdfs:label "initialDelay" .


###  http://iec.ch/TC57/CIM-generic#TapChanger.lowStep
:TapChanger.lowStep rdf:type owl:DatatypeProperty ,
                             owl:FunctionalProperty ;
                    rdfs:domain :TapChanger ;
                    rdfs:range xsd:integer ;
                    
                    rdfs:comment "Lowest possible tap step position, retard from neutral." ;
                    rdfs:label "lowStep" .


###  http://iec.ch/TC57/CIM-generic#TapChanger.ltcFlag
:TapChanger.ltcFlag rdf:type owl:DatatypeProperty ,
                             owl:FunctionalProperty ;
                    rdfs:domain :TapChanger ;
                    rdfs:range xsd:boolean ;
                    
                    rdfs:comment "Specifies whether or not a TapChanger has load tap changing capabilities." ;
                    rdfs:label "ltcFlag" .


###  http://iec.ch/TC57/CIM-generic#TapChanger.neutralStep
:TapChanger.neutralStep rdf:type owl:DatatypeProperty ,
                                 owl:FunctionalProperty ;
                        rdfs:domain :TapChanger ;
                        rdfs:range xsd:integer ;
                        
                        rdfs:comment """The neutral tap step position for this winding.
The attribute shall be equal to or greater than lowStep and equal or less than highStep.
It is the step position where the voltage is neutralU when the other terminals of the transformer are at the ratedU.  If there are other tap changers on the transformer those taps are kept constant at their neutralStep.""" ;
                        rdfs:label "neutralStep" .


###  http://iec.ch/TC57/CIM-generic#TapChanger.neutralU
:TapChanger.neutralU rdf:type owl:DatatypeProperty ,
                              owl:FunctionalProperty ;
                     rdfs:domain :TapChanger ;
                     rdfs:range :Voltage ;
                     
                     rdfs:comment """Voltage at which the winding operates at the neutral tap setting. It is the voltage at the terminal of the PowerTransformerEnd associated with the tap changer when all tap changers on the transformer are at their neutralStep position.  Normally neutralU of the tap changer is the same as ratedU of the PowerTransformerEnd, but it can differ in special cases such as when the tapping mechanism is separate from the winding more common on lower voltage transformers.
This attribute is not relevant for PhaseTapChangerAsymmetrical, PhaseTapChangerSymmetrical and PhaseTapChangerLinear.""" ;
                     rdfs:label "neutralU" .


###  http://iec.ch/TC57/CIM-generic#TapChanger.normalStep
:TapChanger.normalStep rdf:type owl:DatatypeProperty ,
                                owl:FunctionalProperty ;
                       rdfs:domain :TapChanger ;
                       rdfs:range xsd:integer ;
                       
                       rdfs:comment """The tap step position used in \"normal\" network operation for this winding. For a \"Fixed\" tap changer indicates the current physical tap setting.
The attribute shall be equal to or greater than lowStep and equal to or less than highStep.""" ;
                       rdfs:label "normalStep" .


###  http://iec.ch/TC57/CIM-generic#TapChanger.step
:TapChanger.step rdf:type owl:DatatypeProperty ,
                          owl:FunctionalProperty ;
                 rdfs:domain :TapChanger ;
                 rdfs:range xsd:float ;
                 
                 rdfs:comment """Tap changer position.
Starting step for a steady state solution. Non integer values are allowed to support continuous tap variables. The reasons for continuous value are to support study cases where no discrete tap changer has yet been designed, a solution where a narrow voltage band forces the tap step to oscillate or to accommodate for a continuous solution as input.
The attribute shall be equal to or greater than lowStep and equal to or less than highStep.""" ;
                 rdfs:label "step" .


###  http://iec.ch/TC57/CIM-generic#TapChanger.subsequentDelay
:TapChanger.subsequentDelay rdf:type owl:DatatypeProperty ,
                                     owl:FunctionalProperty ;
                            rdfs:domain :TapChanger ;
                            rdfs:range :Seconds ;
                            
                            rdfs:comment "For an LTC, the delay for subsequent tap changer operation (second and later step changes)." ;
                            rdfs:label "subsequentDelay" .


###  http://iec.ch/TC57/CIM-generic#VoltageLevel.highVoltageLimit
:VoltageLevel.highVoltageLimit rdf:type owl:DatatypeProperty ,
                                        owl:FunctionalProperty ;
                               rdfs:domain :VoltageLevel ;
                               rdfs:range :Voltage ;
                               
                               rdfs:comment """The bus bar's high voltage limit.
The limit applies to all equipment and nodes contained in a given VoltageLevel. It is not required that it is exchanged in pair with lowVoltageLimit. It is preferable to use operational VoltageLimit, which prevails, if present.""" ;
                               rdfs:label "highVoltageLimit" .


###  http://iec.ch/TC57/CIM-generic#VoltageLevel.lowVoltageLimit
:VoltageLevel.lowVoltageLimit rdf:type owl:DatatypeProperty ,
                                       owl:FunctionalProperty ;
                              rdfs:domain :VoltageLevel ;
                              rdfs:range :Voltage ;
                              
                              rdfs:comment """The bus bar's low voltage limit.
The limit applies to all equipment and nodes contained in a given VoltageLevel. It is not required that it is exchanged in pair with highVoltageLimit. It is preferable to use operational VoltageLimit, which prevails, if present.""" ;
                              rdfs:label "lowVoltageLimit" .


#################################################################
#    Classes
#################################################################

###  http://iec.ch/TC57/CIM-generic#ACDCTerminal
:ACDCTerminal rdf:type owl:Class ;
              rdfs:subClassOf :IdentifiedObject ;
              
              rdfs:comment "An electrical connection point (AC or DC) to a piece of conducting equipment. Terminals are connected at physical connection points called connectivity nodes." ;
              rdfs:label "ACDCTerminal" .


### http://iec.ch/TC57/CIM-generic#ACLineSegment
:ACLineSegment rdf:type owl:Class ;
               rdfs:subClassOf :Conductor ;
               
               rdfs:comment "A wire or combination of wires, with consistent electrical characteristics, building a single electrical system, used to carry alternating current between points in the power system." ;
               rdfs:label "ACLineSegment" .


### http://iec.ch/TC57/CIM-generic#Analog
:Analog rdf:type owl:Class ;
        rdfs:subClassOf :Measurement ;
        ##
        rdfs:comment "Analog represents an analog Measurement." ;
        rdfs:label "Analog" .



###  http://iec.ch/TC57/CIM-generic#BaseFrequency
:BaseFrequency rdf:type owl:Class ;
               rdfs:subClassOf :IdentifiedObject ;
               
               rdfs:comment "The BaseFrequency class describes a base frequency for a power system network. In case of multiple power networks with different frequencies, e.g. 50 Hz or 60 Hz each network will have its own base frequency class. Hence it is assumed that power system objects having different base frequencies appear in separate documents where each document has a single base frequency instance." ;
               rdfs:label "BaseFrequency" .


###  http://iec.ch/TC57/CIM-generic#BasePower
:BasePower rdf:type owl:Class ;
           rdfs:subClassOf :IdentifiedObject ;
           
           rdfs:comment "The BasePower class defines the base power used in the per unit calculations." ;
           rdfs:label "BasePower" .


###  http://iec.ch/TC57/CIM-generic#BaseVoltage
:BaseVoltage rdf:type owl:Class ;
             rdfs:subClassOf :IdentifiedObject ;
             
             rdfs:comment "Defines a system base voltage which is referenced." ;
             rdfs:label "BaseVoltage" .


###  http://iec.ch/TC57/CIM-generic#Bay
:Bay rdf:type owl:Class ;
     rdfs:subClassOf :EquipmentContainer ;
     
     rdfs:comment "A collection of power system resources (within a given substation) including conducting equipment, protection relays, measurements, and telemetry.  A bay typically represents a physical grouping related to modularization of equipment." ;
     rdfs:label "Bay" .


###  http://iec.ch/TC57/CIM-generic#Breaker
:Breaker rdf:type owl:Class ;
         rdfs:subClassOf :ProtectedSwitch ;
         
         rdfs:comment "A mechanical switching device capable of making, carrying, and breaking currents under normal circuit conditions and also making, carrying for a specified time, and breaking currents under specified abnormal circuit conditions e.g.  those of short circuit." ;
         rdfs:label "Breaker" .

### http://iec.ch/TC57/CIM-generic#Conductor
:Conductor rdf:type owl:Class ;
        rdfs:subClassOf :ConductingEquipment ;
           
           rdfs:comment "A conductor is a material which permits the flow of electricity." ;
           rdfs:label "Conductor" . 


###  http://iec.ch/TC57/CIM-generic#ConductingEquipment
:ConductingEquipment rdf:type owl:Class ;
                     rdfs:subClassOf :Equipment ;
                     
                     rdfs:comment "The parts of the AC power system that are designed to carry current or that are conductively connected through terminals." ;
                     rdfs:label "ConductingEquipment" .


###  http://iec.ch/TC57/CIM-generic#ConnectivityNode
:ConnectivityNode rdf:type owl:Class ;
                  rdfs:subClassOf :IdentifiedObject ;
                  
                  rdfs:comment "Connectivity nodes are points where terminals of AC conducting equipment are connected together with zero impedance." ;
                  rdfs:label "ConnectivityNode" .


###  http://iec.ch/TC57/CIM-generic#ConnectivityNodeContainer
:ConnectivityNodeContainer rdf:type owl:Class ;
                           rdfs:subClassOf :PowerSystemResource ;
                           
                           rdfs:comment "A base class for all objects that may contain connectivity nodes or topological nodes." ;
                           rdfs:label "ConnectivityNodeContainer" .


###  http://iec.ch/TC57/CIM-generic#Equipment
:Equipment rdf:type owl:Class ;
           rdfs:subClassOf :PowerSystemResource ;
           
           rdfs:comment "The parts of a power system that are physical devices, electronic or mechanical." ;
           rdfs:label "Equipment" .


###  http://iec.ch/TC57/CIM-generic#EquipmentContainer
:EquipmentContainer rdf:type owl:Class ;
                    rdfs:subClassOf :ConnectivityNodeContainer ;
                    
                    rdfs:comment "A modelling construct to provide a root class for containing equipment." ;
                    rdfs:label "EquipmentContainer" .


###  http://iec.ch/TC57/CIM-generic#EquivalentNetwork
:EquivalentNetwork rdf:type owl:Class ;
                   rdfs:subClassOf :ConnectivityNodeContainer ;
                   
                   rdfs:comment "A class that groups electrical equivalents, including internal nodes, of a network that has been reduced. The ConnectivityNodes contained in the equivalent are intended to reflect internal nodes of the equivalent. The boundary Connectivity nodes where the equivalent connects outside itself are not contained by the equivalent." ;
                   rdfs:label "EquivalentNetwork" .


###  http://iec.ch/TC57/CIM-generic#GeographicalRegion
:GeographicalRegion rdf:type owl:Class ;
                    rdfs:subClassOf :IdentifiedObject ;
                    
                    rdfs:comment "A geographical region of a power system network model." ;
                    rdfs:label "GeographicalRegion" .


###  http://iec.ch/TC57/CIM-generic#IdentifiedObject
:IdentifiedObject rdf:type owl:Class ;
                  
                  rdfs:comment "This is a root class to provide common identification for all classes needing identification and naming attributes." ;
                  rdfs:label "IdentifiedObject" .


###  http://iec.ch/TC57/CIM-generic#Line
:Line rdf:type owl:Class ;
      rdfs:subClassOf :EquipmentContainer ;
      
      rdfs:comment "Contains equipment beyond a substation belonging to a power transmission line." ;
      rdfs:label "Line" .


### http://iec.ch/TC57/CIM-generic#Location
:Location rdf:type owl:Class ;
         rdfs:subClassOf :IdentifiedObject;
         
         rdfs:comment "The physical space at a particular point in a network." ;
         rdfs:label "Location" .


### http://iec.ch/TC57/CIM-generic#Measurement
:Measurement rdf:type owl:Class ;
      rdfs:subClassOf :IdentifiedObject ;
      
      rdfs:comment "Any measuerd, calculated or non-measured non-calculated quantity of interest in a power system operation." ;
      rdfs:label "Measurement" .


###  http://iec.ch/TC57/CIM-generic#Name
:Name rdf:type owl:Class ;
      
      rdfs:comment "The Name class provides the means to define any number of human readable  names for an object. A name is <b>not</b> to be used for defining inter-object relationships. For inter-object relationships instead use the object identification 'mRID'." ;
      rdfs:label "Name" .


###  http://iec.ch/TC57/CIM-generic#NameType
:NameType rdf:type owl:Class ;
          
          rdfs:comment """Type of name. Possible values for attribute 'name' are implementation dependent but standard profiles may specify types. An enterprise may have multiple IT systems each having its own local name for the same object, e.g. a planning system may have different names from an EMS. An object may also have different names within the same IT system, e.g. localName as defined in CIM version 14. The definition from CIM14 is:
The localName is a human readable name of the object. It is a free text name local to a node in a naming hierarchy similar to a file directory structure. A power system related naming hierarchy may be: Substation, VoltageLevel, Equipment etc. Children of the same parent in such a hierarchy have names that typically are unique among them.""" ;
          rdfs:label "NameType" .


###  http://iec.ch/TC57/CIM-generic#PSRType
:PSRType rdf:type owl:Class ;
         rdfs:subClassOf :IdentifiedObject ;
         
         rdfs:comment "Classifying instances of the same class, e.g. overhead and underground ACLineSegments. This classification mechanism is intended to provide flexibility outside the scope of this document, i.e. provide customisation that is non standard." ;
         rdfs:label "PSRType" .


###  http://iec.ch/TC57/CIM-generic#PhaseCode
:PhaseCode rdf:type owl:Class ;
           
           rdfs:comment """An unordered enumeration of phase identifiers.  Allows designation of phases for both transmission and distribution equipment, circuits and loads.   The enumeration, by itself, does not describe how the phases are connected together or connected to ground.  Ground is not explicitly denoted as a phase.
Residential and small commercial loads are often served from single-phase, or split-phase, secondary circuits. For the example of s12N, phases 1 and 2 refer to hot wires that are 180 degrees out of phase, while N refers to the neutral wire. Through single-phase transformer connections, these secondary circuits may be served from one or two of the primary phases A, B, and C. For three-phase loads, use the A, B, C phase codes instead of s12N.
The integer values are from IEC 61968-9 to support revenue metering applications.""" ;
           rdfs:label "PhaseCode" .


###  http://iec.ch/TC57/CIM-generic#PowerSystemResource
:PowerSystemResource rdf:type owl:Class ;
                     rdfs:subClassOf :IdentifiedObject ;
                     
                     rdfs:comment "A power system resource (PSR) can be an item of equipment such as a switch, an equipment container containing many individual items of equipment such as a substation, or an organisational entity such as sub-control area. Power system resources can have measurements associated." ;
                     rdfs:label "PowerSystemResource" .


###  http://iec.ch/TC57/CIM-generic#ProtectedSwitch
:ProtectedSwitch rdf:type owl:Class ;
                 rdfs:subClassOf :Switch ;
                 
                 rdfs:comment "A ProtectedSwitch is a switching device that can be operated by ProtectionEquipment." ;
                 rdfs:label "ProtectedSwitch" .


### http://iec.ch/TC57/CIM-generic#PositionPoint
:PositionPoint rdf:type owl:Class ;
              rdfs:subClassOf :IdentifiedObject ;
              
              rdfs:comment "A point in space defined by the position coordinates." ;
              rdfs:label "PositionPoint" .


###  http://iec.ch/TC57/CIM-generic#SubGeographicalRegion
:SubGeographicalRegion rdf:type owl:Class ;
                       rdfs:subClassOf :IdentifiedObject ;
                       
                       rdfs:comment "A subset of a geographical region of a power system network model." ;
                       rdfs:label "SubGeographicalRegion" .


###  http://iec.ch/TC57/CIM-generic#Substation
:Substation rdf:type owl:Class ;
            rdfs:subClassOf :EquipmentContainer ;
            
            rdfs:comment "A collection of equipment for purposes other than generation or utilization, through which electric energy in bulk is passed for the purposes of switching or modifying its characteristics." ;
            rdfs:label "Substation" .


###  http://iec.ch/TC57/CIM-generic#Switch
:Switch rdf:type owl:Class ;
        rdfs:subClassOf :ConductingEquipment ;
        
        rdfs:comment "A generic device designed to close, or open, or both, one or more electric circuits.  All switches are two terminal devices including grounding switches. The ACDCTerminal.connected at the two sides of the switch shall not be considered for assessing switch connectivity, i.e. only Switch.open, .normalOpen and .locked are relevant." ;
        rdfs:label "Switch" .


###  http://iec.ch/TC57/CIM-generic#TapChanger
:TapChanger rdf:type owl:Class ;
            rdfs:subClassOf :PowerSystemResource ;
            
            rdfs:comment "Mechanism for changing transformer winding tap positions." ;
            rdfs:label "TapChanger" .


###  http://iec.ch/TC57/CIM-generic#Terminal
:Terminal rdf:type owl:Class ;
          rdfs:subClassOf :ACDCTerminal ;
          
          rdfs:comment "An AC electrical connection point to a piece of conducting equipment. Terminals are connected at physical connection points called connectivity nodes." ;
          rdfs:label "Terminal" .


###  http://iec.ch/TC57/CIM-generic#VoltageLevel
:VoltageLevel rdf:type owl:Class ;
              rdfs:subClassOf :EquipmentContainer ;
              
              rdfs:comment "A collection of equipment at one common system voltage forming a switchgear. The equipment typically consists of breakers, busbars, instrumentation, control, regulation and protection devices as well as assemblies of all these." ;
              rdfs:label "VoltageLevel" .


#################################################################
#    Individuals
#################################################################


#################################################################
#    Annotations
#################################################################

:ADSInstructionTypeCommitment.SHUT_DOWN 
                                        rdfs:label "SHUT_DOWN" .


:ADSInstructionTypeCommitment.START_UP 
                                       rdfs:label "START_UP" .


:ADSInstructionTypeOOS.FIXED_CONSTRAINT 
                                        rdfs:label "FIXED_CONSTRAINT" .


:ADSInstructionTypeOOS.MAX_CONSTRAINT 
                                      rdfs:label "MAX_CONSTRAINT" .


:ADSInstructionTypeOOS.MIN_CONSTRAINT 
                                      rdfs:label "MIN_CONSTRAINT" .


:ASTMStandardEditionKind._00_2005_ 
                                   rdfs:comment "00(2005) standard edition." ;
                                   rdfs:label "00(2005)" .


:ASTMStandardEditionKind._00_2005_e1 
                                     rdfs:comment "00(2005)e1 standard edition." ;
                                     rdfs:label "00(2005)e1" .


:ASTMStandardEditionKind._00_2010_ 
                                   rdfs:comment "00(2010) standard edition." ;
                                   rdfs:label "00(2010)" .


:ASTMStandardEditionKind._01 
                             rdfs:comment "01 standard edition." ;
                             rdfs:label "01" .


:ASTMStandardEditionKind._01a_2007_ 
                                    rdfs:comment "01a(2007) standard edition." ;
                                    rdfs:label "01a(2007)" .


:ASTMStandardEditionKind._01e1 
                               rdfs:comment "01e1 standard edition." ;
                               rdfs:label "01e1" .


:ASTMStandardEditionKind._02 
                             rdfs:comment "02 standard edition." ;
                             rdfs:label "02" .


:ASTMStandardEditionKind._02_2007_ 
                                   rdfs:comment "02(2007) standard edition." ;
                                   rdfs:label "02(2007)" .


:ASTMStandardEditionKind._02_2008_ 
                                   rdfs:comment "02(2008) standard edition." ;
                                   rdfs:label "02(2008)" .


:ASTMStandardEditionKind._02_2009_ 
                                   rdfs:comment "02(2009) standard edition." ;
                                   rdfs:label "02(2009)" .


:ASTMStandardEditionKind._02_2012_ 
                                   rdfs:comment "02(2012) standard edition." ;
                                   rdfs:label "02(2012)" .


:ASTMStandardEditionKind._02_2014_ 
                                   rdfs:comment "02(2014) standard edition." ;
                                   rdfs:label "02(2014)" .


:ASTMStandardEditionKind._02a 
                              rdfs:comment "02a standard edition." ;
                              rdfs:label "02a" .


:ASTMStandardEditionKind._02b 
                              rdfs:comment "02b standard edition." ;
                              rdfs:label "02b" .


:ASTMStandardEditionKind._02e1 
                               rdfs:comment "02e1 standard edition." ;
                               rdfs:label "02e1" .


:ASTMStandardEditionKind._03 
                             rdfs:comment "03 standard edition." ;
                             rdfs:label "03" .


:ASTMStandardEditionKind._03_2008_ 
                                   rdfs:comment "03(2008) standard edition." ;
                                   rdfs:label "03(2008)" .


:ASTMStandardEditionKind._03_2014_ 
                                   rdfs:comment "03(2014) standard edition." ;
                                   rdfs:label "03(2014)" .


:ASTMStandardEditionKind._03a 
                              rdfs:comment "03a standard edition." ;
                              rdfs:label "03a" .


:ASTMStandardEditionKind._04 
                             rdfs:comment "04 standard edition." ;
                             rdfs:label "04" .


:ASTMStandardEditionKind._04a 
                              rdfs:comment "04a standard edition." ;
                              rdfs:label "04a" .


:ASTMStandardEditionKind._04ae1 
                                rdfs:comment "04ae1 standard edition." ;
                                rdfs:label "04ae1" .


:ASTMStandardEditionKind._04e1 
                               rdfs:comment "04e1 standard edition." ;
                               rdfs:label "04e1" .


:ASTMStandardEditionKind._04e2 
                               rdfs:comment "04e2 standard edition." ;
                               rdfs:label "04e2" .


:ASTMStandardEditionKind._05 
                             rdfs:comment "05 standard edition." ;
                             rdfs:label "05" .


:ASTMStandardEditionKind._05_2010_ 
                                   rdfs:comment "05(2010) standard edition." ;
                                   rdfs:label "05(2010)" .


:ASTMStandardEditionKind._05a 
                              rdfs:comment "05a standard edition." ;
                              rdfs:label "05a" .


:ASTMStandardEditionKind._05a_2010_ 
                                    rdfs:comment "05a(2010) standard edition." ;
                                    rdfs:label "05a(2010)" .


:ASTMStandardEditionKind._06 
                             rdfs:comment "06 standard edition." ;
                             rdfs:label "06" .


:ASTMStandardEditionKind._07 
                             rdfs:comment "07 standard edition." ;
                             rdfs:label "07" .


:ASTMStandardEditionKind._07_2013_ 
                                   rdfs:comment "07(2013) standard edition." ;
                                   rdfs:label "07(2013)" .


:ASTMStandardEditionKind._08 
                             rdfs:comment "08 standard edition." ;
                             rdfs:label "08" .


:ASTMStandardEditionKind._08e1 
                               rdfs:comment "08e1 standard edition." ;
                               rdfs:label "08e1" .


:ASTMStandardEditionKind._09 
                             rdfs:comment "09 standard edition." ;
                             rdfs:label "09" .


:ASTMStandardEditionKind._09_2013_ 
                                   rdfs:comment "09(2013) standard edition." ;
                                   rdfs:label "09(2013)" .


:ASTMStandardEditionKind._10 
                             rdfs:comment "10 standard edition." ;
                             rdfs:label "10" .


:ASTMStandardEditionKind._10a 
                              rdfs:comment "10a standard edition." ;
                              rdfs:label "10a" .


:ASTMStandardEditionKind._11 
                             rdfs:comment "11 standard edition." ;
                             rdfs:label "11" .


:ASTMStandardEditionKind._11a 
                              rdfs:comment "11a standard edition." ;
                              rdfs:label "11a" .


:ASTMStandardEditionKind._12 
                             rdfs:comment "12 standard edition." ;
                             rdfs:label "12" .


:ASTMStandardEditionKind._12a 
                              rdfs:comment "12a standard edition." ;
                              rdfs:label "12a" .


:ASTMStandardEditionKind._12b 
                              rdfs:comment "12b standard edition." ;
                              rdfs:label "12b" .


:ASTMStandardEditionKind._13 
                             rdfs:comment "13 standard edition." ;
                             rdfs:label "13" .


:ASTMStandardEditionKind._13e1 
                               rdfs:comment "13e1 standard edition." ;
                               rdfs:label "13e1" .


:ASTMStandardEditionKind._14 
                             rdfs:comment "14 standard edition." ;
                             rdfs:label "14" .


:ASTMStandardEditionKind._14a 
                              rdfs:comment "14a standard edition." ;
                              rdfs:label "14a" .


:ASTMStandardEditionKind._14e1 
                               rdfs:comment "14e1 standard edition." ;
                               rdfs:label "14e1" .


:ASTMStandardEditionKind._14e2 
                               rdfs:comment "14e2 standard edition." ;
                               rdfs:label "14e2" .


:ASTMStandardEditionKind._15 
                             rdfs:comment "15 standard edition." ;
                             rdfs:label "15" .


:ASTMStandardEditionKind._15a 
                              rdfs:comment "15a standard edition." ;
                              rdfs:label "15a" .


:ASTMStandardEditionKind._65 
                             rdfs:comment "65 standard edition." ;
                             rdfs:label "65" .


:ASTMStandardEditionKind._71 
                             rdfs:comment "71 standard edition." ;
                             rdfs:label "71" .


:ASTMStandardEditionKind._74 
                             rdfs:comment "74 standard edition." ;
                             rdfs:label "74" .


:ASTMStandardEditionKind._80e1 
                               rdfs:comment "80e1 standard edition." ;
                               rdfs:label "80e1" .


:ASTMStandardEditionKind._82 
                             rdfs:comment "82 standard edition." ;
                             rdfs:label "82" .


:ASTMStandardEditionKind._83_1996_e1 
                                     rdfs:comment "83(1996)e1 standard edition." ;
                                     rdfs:label "83(1996)e1" .


:ASTMStandardEditionKind._85 
                             rdfs:comment "85 standard edition." ;
                             rdfs:label "85" .


:ASTMStandardEditionKind._85_1990_e1 
                                     rdfs:comment "85(1990)e1 standard edition." ;
                                     rdfs:label "85(1990)e1" .


:ASTMStandardEditionKind._87_1995_ 
                                   rdfs:comment "87(1995) standard edition." ;
                                   rdfs:label "87(1995)" .


:ASTMStandardEditionKind._87e1 
                               rdfs:comment "87e1 standard edition." ;
                               rdfs:label "87e1" .


:ASTMStandardEditionKind._88 
                             rdfs:comment "88 standard edition." ;
                             rdfs:label "88" .


:ASTMStandardEditionKind._90e1 
                               rdfs:comment "90e1 standard edition." ;
                               rdfs:label "90e1" .


:ASTMStandardEditionKind._91 
                             rdfs:comment "91 standard edition." ;
                             rdfs:label "91" .


:ASTMStandardEditionKind._92 
                             rdfs:comment "92 standard edition." ;
                             rdfs:label "92" .


:ASTMStandardEditionKind._94 
                             rdfs:comment "94 standard edition." ;
                             rdfs:label "94" .


:ASTMStandardEditionKind._94_1999_ 
                                   rdfs:comment "94(1999) standard edition." ;
                                   rdfs:label "94(1999)" .


:ASTMStandardEditionKind._94_2004_ 
                                   rdfs:comment "94(2004) standard edition." ;
                                   rdfs:label "94(2004)" .


:ASTMStandardEditionKind._94_2010_ 
                                   rdfs:comment "94(2010) standard edition." ;
                                   rdfs:label "94(2010)" .


:ASTMStandardEditionKind._94e1 
                               rdfs:comment "94e1 standard edition." ;
                               rdfs:label "94e1" .


:ASTMStandardEditionKind._95 
                             rdfs:comment "95 standard edition." ;
                             rdfs:label "95" .


:ASTMStandardEditionKind._95_2000_e1 
                                     rdfs:comment "95(2000)e1 standard edition." ;
                                     rdfs:label "95(2000)e1" .


:ASTMStandardEditionKind._96 
                             rdfs:comment "96 standard edition." ;
                             rdfs:label "96" .


:ASTMStandardEditionKind._96_2002_e1 
                                     rdfs:comment "96(2002)e1 standard edition." ;
                                     rdfs:label "96(2002)e1" .


:ASTMStandardEditionKind._96a 
                              rdfs:comment "96a standard edition." ;
                              rdfs:label "96a" .


:ASTMStandardEditionKind._96e1 
                               rdfs:comment "96e1 standard edition." ;
                               rdfs:label "96e1" .


:ASTMStandardEditionKind._97 
                             rdfs:comment "97 standard edition." ;
                             rdfs:label "97" .


:ASTMStandardEditionKind._97_2002_ 
                                   rdfs:comment "97(2002) standard edition." ;
                                   rdfs:label "97(2002)" .


:ASTMStandardEditionKind._97_2003_ 
                                   rdfs:comment "97(2003) standard edition." ;
                                   rdfs:label "97(2003)" .


:ASTMStandardEditionKind._97_2008_ 
                                   rdfs:comment "97(2008) standard edition." ;
                                   rdfs:label "97(2008)" .


:ASTMStandardEditionKind._97a 
                              rdfs:comment "97a standard edition." ;
                              rdfs:label "97a" .


:ASTMStandardEditionKind._97a_2004_ 
                                    rdfs:comment "97a(2004) standard edition." ;
                                    rdfs:label "97a(2004)" .


:ASTMStandardEditionKind._98 
                             rdfs:comment "98 standard edition." ;
                             rdfs:label "98" .


:ASTMStandardEditionKind._98a 
                              rdfs:comment "98a standard edition." ;
                              rdfs:label "98a" .


:ASTMStandardEditionKind._99 
                             rdfs:comment "99 standard edition." ;
                             rdfs:label "99" .


:ASTMStandardEditionKind._99_2004_e1 
                                     rdfs:comment "99(2004)e1 standard edition." ;
                                     rdfs:label "99(2004)e1" .


:ASTMStandardEditionKind._99_2005_ 
                                   rdfs:comment "99(2005) standard edition." ;
                                   rdfs:label "99(2005)" .


:ASTMStandardEditionKind._99_2009_ 
                                   rdfs:comment "99(2009) standard edition." ;
                                   rdfs:label "99(2009)" .


:ASTMStandardEditionKind._99a 
                              rdfs:comment "99a standard edition." ;
                              rdfs:label "99a" .


:ASTMStandardEditionKind._99a_2004_ 
                                    rdfs:comment "99a(2004) standard edition." ;
                                    rdfs:label "99a(2004)" .


:ASTMStandardEditionKind._99e1 
                               rdfs:comment "99e1 standard edition." ;
                               rdfs:label "99e1" .


:ASTMStandardEditionKind._99e2 
                               rdfs:comment "99e2 standard edition." ;
                               rdfs:label "99e2" .


:ASTMStandardEditionKind.none 
                              rdfs:comment "No kind of standard." ;
                              rdfs:label "none" .


:ASTMStandardEditionKind.unknown 
                                 rdfs:comment "Unknown kind of standard." ;
                                 rdfs:label "unknown" .


:ASTMStandardKind.D1169 
                        rdfs:comment "Standard Test Method for Specific Resistance (Resistivity) of Electrical Insulating Liquids." ;
                        rdfs:label "D1169" .


:ASTMStandardKind.D1275 
                        rdfs:comment "Standard Test Method for Corrosive Sulfur in Electrical Insulating Oils." ;
                        rdfs:label "D1275" .


:ASTMStandardKind.D1298 
                        rdfs:comment """Standard Test Method for Density, Relative Density, or API Gravity of Crude Petroleum and Liquid Petroleum Products by Hydrometer Method  -or-
Standard Test Method for Density, Relative Density (Specific Gravity), or API Gravity of Crude Petroleum and Liquid Petroleum Products by Hydrometer Method.""" ;
                        rdfs:label "D1298" .


:ASTMStandardKind.D149 
                       rdfs:comment "Standard Test Method for Dielectric Breakdown Voltage and Dielectric Strength of Solid Electrical Insulating Materials at Commercial Power Frequencies." ;
                       rdfs:label "D149" .


:ASTMStandardKind.D1500 
                        rdfs:comment "Standard Test Method for ASTM Color of Petroleum Products (ASTM Color Scale)." ;
                        rdfs:label "D1500" .


:ASTMStandardKind.D1524 
                        rdfs:comment "Standard Test Method for Visual Examination of Used Electrical Insulating Oils of Petroleum Origin in the Field." ;
                        rdfs:label "D1524" .


:ASTMStandardKind.D1533 
                        rdfs:comment "Standard Test Method for Water in Insulating Liquids by Coulometric Karl Fischer Titration." ;
                        rdfs:label "D1533" .


:ASTMStandardKind.D1816 
                        rdfs:comment "Standard Test Method for Dielectric Breakdown Voltage of Insulating Liquids Using VDE Electrodes." ;
                        rdfs:label "D1816" .


:ASTMStandardKind.D2029 
                        rdfs:comment "Standard Test Methods for Water Vapor Content of Electrical Insulating Gases by Measurement of Dew Point." ;
                        rdfs:label "D2029" .


:ASTMStandardKind.D2112 
                        rdfs:comment "Standard Test Method for Oxidation Stability of Inhibited Mineral Insulating Oil by Pressure Vessel." ;
                        rdfs:label "D2112" .


:ASTMStandardKind.D2129 
                        rdfs:comment "Standard Test Method for Color of Clear Electrical Insulating Liquids (Platinum-Cobalt Scale)." ;
                        rdfs:label "D2129" .


:ASTMStandardKind.D2140 
                        rdfs:comment """Standard Practice for Calculating Carbon-Type Composition of Insulating Oils of Petroleum Origin  -or-
Standard Test Method for Carbon-Type Composition of Insulating Oils of Petroleum Origin.""" ;
                        rdfs:label "D2140" .


:ASTMStandardKind.D2144 
                        rdfs:comment """Standard Practices for Examination of Electrical Insulating Oils by Infrared Absorption  -or-
Standard Test Methods for Examination of Electrical Insulating Oils by Infrared Absorption.""" ;
                        rdfs:label "D2144" .


:ASTMStandardKind.D2668 
                        rdfs:comment """Standard Test Method for 2,6-di-tert-Butyl- p-Cresol and 2,6-di-tert-Butyl Phenol in Electrical Insulating Oil by Infrared Absorption  -or-
Standard Test Method for 2,6-Ditertiary-Butyl Para Cresol and 2,6-Ditertiary-Butyl Phenol in Electrical Insulating Oil by Infrared Absorption.""" ;
                        rdfs:label "D2668" .


:ASTMStandardKind.D3612 
                        rdfs:comment "Standard Test Method for Analysis of Gases Dissolved in Electrical Insulating Oil by Gas Chromatography." ;
                        rdfs:label "D3612" .


:ASTMStandardKind.D4052 
                        rdfs:comment """Standard Test Method for Density, Relative Density, and API Gravity of Liquids by Digital Density Meter  -or-
Standard Test Method for Density and Relative Density of Liquids by Digital Density Meter.""" ;
                        rdfs:label "D4052" .


:ASTMStandardKind.D4059 
                        rdfs:comment "Standard Test Method for Analysis of Polychlorinated Biphenyls in Insulating Liquids by Gas Chromatography." ;
                        rdfs:label "D4059" .


:ASTMStandardKind.D4230 
                        rdfs:comment "Standard Test Method of Measuring Humidity with Cooled-Surface Condensation (Dew-Point) Hygrometer." ;
                        rdfs:label "D4230" .


:ASTMStandardKind.D4243 
                        rdfs:comment "Standard Test Method for Measurement of Average Viscometric Degree of Polymerization of New and Aged Electrical Papers and Boards." ;
                        rdfs:label "D4243" .


:ASTMStandardKind.D445 
                       rdfs:comment """Standard Test Method for Kinematic Viscosity of Transparent and Opaque Liquids (and Calculation of Dynamic Viscosity)  -or-
Standard Method Of Test For Viscosity Of Transparent And Opaque Liquids (Kinematic And Dynamic Viscosities).""" ;
                       rdfs:label "D445" .


:ASTMStandardKind.D4768 
                        rdfs:comment "Standard Test Method for Analysis of 2,6-Ditertiary-Butyl Para-Cresol and 2,6-Ditertiary-Butyl Phenol in Insulating Liquids by Gas Chromatography." ;
                        rdfs:label "D4768" .


:ASTMStandardKind.D5837 
                        rdfs:comment "Standard Test Method for Furanic Compounds in Electrical Insulating Liquids by High-Performance Liquid Chromatography (HPLC)." ;
                        rdfs:label "D5837" .


:ASTMStandardKind.D5853 
                        rdfs:comment "Standard Test Method for Pour Point of Crude Oils." ;
                        rdfs:label "D5853" .


:ASTMStandardKind.D5949 
                        rdfs:comment "Standard Test Method for Pour Point of Petroleum Products (Automatic Pressure Pulsing Method)." ;
                        rdfs:label "D5949" .


:ASTMStandardKind.D5950 
                        rdfs:comment "Standard Test Method for Pour Point of Petroleum Products (Automatic Tilt Method)." ;
                        rdfs:label "D5950" .


:ASTMStandardKind.D5985 
                        rdfs:comment "Standard Test Method for Pour Point of Petroleum Products (Rotational Method)." ;
                        rdfs:label "D5985" .


:ASTMStandardKind.D6304 
                        rdfs:comment "Standard Test Method for Determination of Water in Petroleum Products, Lubricating Oils, and Additives by Coulometric Karl Fischer Titration." ;
                        rdfs:label "D6304" .


:ASTMStandardKind.D6749 
                        rdfs:comment "Standard Test Method for Pour Point of Petroleum Products (Automatic Air Pressure Method)." ;
                        rdfs:label "D6749" .


:ASTMStandardKind.D6786 
                        rdfs:comment "Standard Test Method for Particle Count in Mineral Insulating Oil Using Automatic Optical Particle Counters." ;
                        rdfs:label "D6786" .


:ASTMStandardKind.D6892 
                        rdfs:comment "Standard Test Method for Pour Point of Petroleum Products (Robotic Tilt Method)." ;
                        rdfs:label "D6892" .


:ASTMStandardKind.D7151 
                        rdfs:comment "Standard Test Method for Determination of Elements in Insulating Oils by Inductively Coupled Plasma Atomic Emission Spectrometry (ICP-AES)." ;
                        rdfs:label "D7151" .


:ASTMStandardKind.D7346 
                        rdfs:comment """Standard Test Method for No Flow Point and Pour Point of Petroleum Products and Liquid Fuels  -or-
Standard Test Method for No Flow Point and Pour Point of Petroleum Products  -or-
Standard Test Method for No Flow Point of Petroleum Products.""" ;
                        rdfs:label "D7346" .


:ASTMStandardKind.D828 
                       rdfs:comment "Standard Test Method for Tensile Properties of Paper and Paperboard Using Constant-Rate-of-Elongation Apparatus (Withdrawn 2009)." ;
                       rdfs:label "D828" .


:ASTMStandardKind.D877 
                       rdfs:comment "Standard Test Method for Dielectric Breakdown Voltage of Insulating Liquids Using Disk Electrodes." ;
                       rdfs:label "D877" .


:ASTMStandardKind.D877_D877M 
                             rdfs:comment "Standard Test Method for Dielectric Breakdown Voltage of Insulating Liquids Using Disk Electrodes." ;
                             rdfs:label "D877/D877M" .


:ASTMStandardKind.D92 
                      rdfs:comment """Standard Test Method for Flash and Fire Points by Cleveland Open Cup Tester  -or-
Standard Test Method for Flash and Fire Points by Cleveland Open Cup.""" ;
                      rdfs:label "D92" .


:ASTMStandardKind.D924 
                       rdfs:comment "Standard Test Method for Dissipation Factor (or Power Factor) and Relative Permittivity (Dielectric Constant) of Electrical Insulating Liquids." ;
                       rdfs:label "D924" .


:ASTMStandardKind.D93 
                      rdfs:comment """Standard Test Methods for Flash Point by Pensky-Martens Closed Cup Tester  -or-
Standard Test Method for Flash Point by Pensky-Martens Closed Tester  -or-
Standard Method Of Test For Flash Point by Pensky-Martens Closed Tester.""" ;
                      rdfs:label "D93" .


:ASTMStandardKind.D97 
                      rdfs:comment """Standard Test Method for Pour Point of Petroleum Products  -or-
Standard Test Method for Pour Point of Petroleum Oils.""" ;
                      rdfs:label "D97" .


:ASTMStandardKind.D974 
                       rdfs:comment "Standard Test Method for Acid and Base Number by Color-Indicator Titration." ;
                       rdfs:label "D974" .


:AccumulationKind.boundedQuantity uml:hasInitialValue "14" ;
                                  
                                  rdfs:comment "A time-independent cumulative quantity much like a 'bulkQuantity' or a 'latchingQuantity', except that the accumulation stops at the maximum or minimum values. When the maximum is reached, any additional positive accumulation is discarded, but negative accumulation may be accepted (thus lowering the counter.) Likewise, when the negative bound is reached, any additional negative accumulation is discarded, but positive accumulation is accepted (thus increasing the counter.)" ;
                                  rdfs:label "boundedQuantity" .


:AccumulationKind.bulkQuantity uml:hasInitialValue "1" ;
                               
                               rdfs:comment """A value from a register which represents the bulk quantity of a commodity. This quantity is computed as the integral of the commodity usage rate. This value is typically used as the basis for the dial reading at the meter, and as a result, will roll over upon reaching a maximum dial value. 
Note 1: With the metering system, the roll-over behaviour typically implies a roll-under behavior so that the value presented is always a positive value (e.g. unsigned integer or positive decimal.) However, when communicating data between enterprise applications a negative value might occur in a case such as net metering.
Note 2: A 'bulkQuantity' refers primarily to the dial reading and not the consumption over a specific period of time.""" ;
                               rdfs:label "bulkQuantity" .


:AccumulationKind.continuousCumulative uml:hasInitialValue "2" ;
                                       
                                       rdfs:comment """The sum of the previous billing period values and the present period value.
Note: 'continuousCumulative' is commonly used in conjunction with 'demand', and it  would represent the cumulative sum of the previous billing period maximum demand values (as occurring with each demand reset) summed with the present period maximum demand value (which has yet to be reset.)""" ;
                                       rdfs:label "continuousCumulative" .


:AccumulationKind.cumulative uml:hasInitialValue "3" ;
                             
                             rdfs:comment """The sum of the previous billing period values.
Note: 'cumulative' is commonly used in conjunction with “demand.” Each demand reset causes the maximum demand value for the present billing period (since the last demand reset) to accumulate as an accumulative total of all maximum demands. So instead of 'zeroing' the demand register, a demand reset has the effect of adding the present maximum demand to this accumulating total.""" ;
                             rdfs:label "cumulative" .


:AccumulationKind.deltaData uml:hasInitialValue "4" ;
                            
                            rdfs:comment """The difference between the value at the end of the prescribed interval and the beginning of the interval. This is used for incremental interval data. 
Note: One common application would be for load profile data, another use might be to report the number of events within an interval (such as the number of equipment energisations within the specified period of time.)""" ;
                            rdfs:label "deltaData" .


:AccumulationKind.indicating uml:hasInitialValue "6" ;
                             
                             rdfs:comment """As if a needle is swung out on the meter face to a value to indicate the current value.
Note: An 'indicating' value is typically measured over hundreds of milliseconds or greater, or may imply a “pusher” mechanism to capture a value. Compare this to 'instantaneous' which is measured over a shorter period of time.""" ;
                             rdfs:label "indicating" .


:AccumulationKind.instantaneous uml:hasInitialValue "12" ;
                                
                                rdfs:comment """Typically measured over the fastest period of time allowed by the definition of the metric (usually milliseconds or tens of milliseconds.)
Note: 'instantaneous' was moved to attribute #3 in Ed.2 of IEC 61968-9, from attribute #1 in Ed.1 of IEC 61968-9.""" ;
                                rdfs:label "instantaneous" .


:AccumulationKind.latchingQuantity uml:hasInitialValue "13" ;
                                   
                                   rdfs:comment """When this description is applied to a metered value, it implies that the value is a time-independent cumulative quantity much like a 'bulkQuantity', except that it latches upon the maximum value upon reaching that value. Any additional accumulation (positive or negative) is discarded until a reset occurs. 
Note: A 'latchingQuantity' may also occur in the downward direction – upon reaching a minimum value. The terms 'maximum' or 'minimum' (for 'aggregate') will usually be included when this type of accumulation behaviour is present. 
When this description is applied to an encoded value (UOM= 'Code'), it implies that the value has one or more bits which are latching. The condition that caused the bit to be set may have long since evaporated.
In either case, the timestamp that accompanies the value may not coincide with the moment the value was initially set.
In both cases a system will need to perform an operation to clear the latched value.""" ;
                                   rdfs:label "latchingQuantity" .


:AccumulationKind.none uml:hasInitialValue "0" ;
                       
                       rdfs:comment "Not applicable, or implied by the unit of measure." ;
                       rdfs:label "none" .


:AccumulationKind.summation uml:hasInitialValue "9" ;
                            
                            rdfs:comment """A form of accumulation which is selective with respect to time. 
Note : 'summation' could be considered a specialisation of 'bulkQuantity' as it selectively accumulates pulses over a timing pattern (while 'bulkQuantity' accumulates pulses all of the time).""" ;
                            rdfs:label "summation" .


:AccumulationKind.timeDelay uml:hasInitialValue "10" ;
                            
                            rdfs:comment "A form of computation which introduces a time delay characteristic to the data value." ;
                            rdfs:label "timeDelay" .


:ActionType.CANCEL 
                   rdfs:comment "Cancel a trade." ;
                   rdfs:label "CANCEL" .


:AdderType.BASELINE 
                    rdfs:label "BASELINE" .


:AdderType.NEGOTIATED 
                      rdfs:label "NEGOTIATED" .


:AggregateKind.average uml:hasInitialValue "2" ;
                       
                       rdfs:comment "The value represents average." ;
                       rdfs:label "average" .


:AggregateKind.excess uml:hasInitialValue "4" ;
                      
                      rdfs:comment "The value represents an amount over which a threshold was exceeded." ;
                      rdfs:label "excess" .


:AggregateKind.fifthMaximum uml:hasInitialValue "25" ;
                            
                            rdfs:comment "The fifth highest value observed." ;
                            rdfs:label "fifthMaximum" .


:AggregateKind.fourthMaximum uml:hasInitialValue "24" ;
                             
                             rdfs:comment "The fourth highest value observed." ;
                             rdfs:label "fourthMaximum" .


:AggregateKind.highThreshold uml:hasInitialValue "5" ;
                             
                             rdfs:comment "The value represents a programmed high threshold." ;
                             rdfs:label "highThreshold" .


:AggregateKind.lowThreshold uml:hasInitialValue "7" ;
                            
                            rdfs:comment "The value represents a programmed low threshold." ;
                            rdfs:label "lowThreshold" .


:AggregateKind.maximum uml:hasInitialValue "8" ;
                       
                       rdfs:comment "The highest value observed." ;
                       rdfs:label "maximum" .


:AggregateKind.minimum uml:hasInitialValue "9" ;
                       
                       rdfs:comment "The smallest value observed." ;
                       rdfs:label "minimum" .


:AggregateKind.nominal uml:hasInitialValue "11" ;
                       
                       rdfs:comment "The nominal value." ;
                       rdfs:label "nominal" .


:AggregateKind.none uml:hasInitialValue "0" ;
                    
                    rdfs:comment "Not applicable." ;
                    rdfs:label "none" .


:AggregateKind.normal uml:hasInitialValue "12" ;
                      
                      rdfs:comment "The normal value." ;
                      rdfs:label "normal" .


:AggregateKind.secondMaximum uml:hasInitialValue "16" ;
                             
                             rdfs:comment "The second highest value observed." ;
                             rdfs:label "secondMaximum" .


:AggregateKind.secondMinimum uml:hasInitialValue "17" ;
                             
                             rdfs:comment "The second smallest value observed." ;
                             rdfs:label "secondMinimum" .


:AggregateKind.sum uml:hasInitialValue "26" ;
                   
                   rdfs:comment "The accumulated sum." ;
                   rdfs:label "sum" .


:AggregateKind.thirdMaximum uml:hasInitialValue "23" ;
                            
                            rdfs:comment "The third highest value observed." ;
                            rdfs:label "thirdMaximum" .


:AlarmDisplayType.Appear 
                         rdfs:label "Appear" .


:AlarmDisplayType.Disappear 
                            rdfs:label "Disappear" .


:AlarmDisplayType.Fleeting 
                           rdfs:label "Fleeting" .


:AllocationEnergyTypeCode.ACNG 
                               rdfs:label "ACNG" .


:AllocationEnergyTypeCode.BS 
                             rdfs:label "BS" .


:AllocationEnergyTypeCode.DAPE 
                               rdfs:label "DAPE" .


:AllocationEnergyTypeCode.DASE 
                               rdfs:label "DASE" .


:AllocationEnergyTypeCode.ESRT 
                               rdfs:label "ESRT" .


:AllocationEnergyTypeCode.ESYS 
                               rdfs:label "ESYS" .


:AllocationEnergyTypeCode.ETC 
                              rdfs:label "ETC" .


:AllocationEnergyTypeCode.HASE 
                               rdfs:label "HASE" .


:AllocationEnergyTypeCode.LMPM 
                               rdfs:label "LMPM" .


:AllocationEnergyTypeCode.MINL 
                               rdfs:label "MINL" .


:AllocationEnergyTypeCode.MLE 
                              rdfs:label "MLE" .


:AllocationEnergyTypeCode.MSSLFE 
                                 rdfs:label "MSSLFE" .


:AllocationEnergyTypeCode.OE 
                             rdfs:label "OE" .


:AllocationEnergyTypeCode.OTHER 
                                rdfs:label "OTHER" .


:AllocationEnergyTypeCode.OVGN 
                               rdfs:label "OVGN" .


:AllocationEnergyTypeCode.PE 
                             rdfs:label "PE" .


:AllocationEnergyTypeCode.RCNG 
                               rdfs:label "RCNG" .


:AllocationEnergyTypeCode.RE 
                             rdfs:label "RE" .


:AllocationEnergyTypeCode.RED 
                              rdfs:label "RED" .


:AllocationEnergyTypeCode.RMRD 
                               rdfs:label "RMRD" .


:AllocationEnergyTypeCode.RMRH 
                               rdfs:label "RMRH" .


:AllocationEnergyTypeCode.RMRR 
                               rdfs:label "RMRR" .


:AllocationEnergyTypeCode.RMRS 
                               rdfs:label "RMRS" .


:AllocationEnergyTypeCode.RMRT 
                               rdfs:label "RMRT" .


:AllocationEnergyTypeCode.RSYS 
                               rdfs:label "RSYS" .


:AllocationEnergyTypeCode.RTSSE 
                                rdfs:label "RTSSE" .


:AllocationEnergyTypeCode.SDWN 
                               rdfs:label "SDWN" .


:AllocationEnergyTypeCode.SE 
                             rdfs:label "SE" .


:AllocationEnergyTypeCode.SLIC 
                               rdfs:label "SLIC" .


:AllocationEnergyTypeCode.SRE 
                              rdfs:label "SRE" .


:AllocationEnergyTypeCode.STRT 
                               rdfs:label "STRT" .


:AllocationEnergyTypeCode.SUMR 
                               rdfs:label "SUMR" .


:AllocationEnergyTypeCode.TCNG 
                               rdfs:label "TCNG" .


:AllocationEnergyTypeCode.TEST 
                               rdfs:label "TEST" .


:AllocationEnergyTypeCode.TOR 
                              rdfs:label "TOR" .


:AllocationEnergyTypeCode.VS 
                             rdfs:label "VS" .


:AmiBillingReadyKind.amiCapable 
                                rdfs:comment "Usage point is equipped with an AMI capable meter that is not yet currently equipped with a communications module." ;
                                rdfs:label "amiCapable" .


:AmiBillingReadyKind.amiDisabled 
                                 rdfs:comment "Usage point is equipped with an AMI capable meter; however, the AMI functionality has been disabled or is not being used." ;
                                 rdfs:label "amiDisabled" .


:AmiBillingReadyKind.billingApproved 
                                     rdfs:comment "Usage point is equipped with an operating AMI capable meter and accuracy has been certified for billing purposes." ;
                                     rdfs:label "billingApproved" .


:AmiBillingReadyKind.enabled 
                             rdfs:comment "Usage point is equipped with an AMI capable meter having communications capability." ;
                             rdfs:label "enabled" .


:AmiBillingReadyKind.nonAmi 
                            rdfs:comment "Usage point is equipped with a non AMI capable meter." ;
                            rdfs:label "nonAmi" .


:AmiBillingReadyKind.nonMetered 
                                rdfs:comment "Usage point is not currently equipped with a meter." ;
                                rdfs:label "nonMetered" .


:AmiBillingReadyKind.operable 
                              rdfs:comment "Usage point is equipped with an AMI capable meter that is functioning and communicating with the AMI network." ;
                              rdfs:label "operable" .


:AnalogLimitType.BranchLongTerm 
                                rdfs:comment "Branch Long Term Limit" ;
                                rdfs:label "BranchLongTerm" .


:AnalogLimitType.BranchMediumTerm 
                                  rdfs:comment "Branch Medium Term Limit" ;
                                  rdfs:label "BranchMediumTerm" .


:AnalogLimitType.BranchShortTerm 
                                 rdfs:comment "Branch Short Term Limit" ;
                                 rdfs:label "BranchShortTerm" .


:AnalogLimitType.VoltageHigh 
                             rdfs:comment "Voltage High Limit" ;
                             rdfs:label "VoltageHigh" .


:AnalogLimitType.VoltageLow 
                            rdfs:comment "Voltage Low Limit" ;
                            rdfs:label "VoltageLow" .


:AnalogToDigitalLogicKind.eq 
                             rdfs:comment "Equal (like) comparison operation." ;
                             rdfs:label "eq" .


:AnalogToDigitalLogicKind.ge 
                             rdfs:comment "Greater or equal comparison operation." ;
                             rdfs:label "ge" .


:AnalogToDigitalLogicKind.gt 
                             rdfs:comment "Greater than comparison operation." ;
                             rdfs:label "gt" .


:AnalogToDigitalLogicKind.le 
                             rdfs:comment "Less or equal comparison operation." ;
                             rdfs:label "le" .


:AnalogToDigitalLogicKind.lt 
                             rdfs:comment "Less than comparison operation." ;
                             rdfs:label "lt" .


:AnalogToDigitalLogicKind.ne 
                             rdfs:comment "Not equal (unlike) comparison operation." ;
                             rdfs:label "ne" .


:AnalyticKind.agingAnalytic 
                            rdfs:comment "Analytic evaluates aging." ;
                            rdfs:label "agingAnalytic" .


:AnalyticKind.faultAnalytic 
                            rdfs:comment "Analytic evaluates fault." ;
                            rdfs:label "faultAnalytic" .


:AnalyticKind.healthAnalytic 
                             rdfs:comment "Analytic evaluates asset health." ;
                             rdfs:label "healthAnalytic" .


:AnalyticKind.other 
                    rdfs:comment "Analytic evaluates other factor." ;
                    rdfs:label "other" .


:AnalyticKind.replacementAnalytic 
                                  rdfs:comment "Analytic evaluates need for replacement." ;
                                  rdfs:label "replacementAnalytic" .


:AnalyticKind.riskAnalytic 
                           rdfs:comment "Analytic evaluates risk." ;
                           rdfs:label "riskAnalytic" .


:AnchorKind.concrete 
                     rdfs:label "concrete" .


:AnchorKind.helix 
                  rdfs:label "helix" .


:AnchorKind.multiHelix 
                       rdfs:label "multiHelix" .


:AnchorKind.other 
                  rdfs:label "other" .


:AnchorKind.rod 
                rdfs:label "rod" .


:AnchorKind.screw 
                  rdfs:label "screw" .


:AnchorKind.unknown 
                    rdfs:label "unknown" .


:AncillaryCommodityType.NONSPIN 
                                rdfs:comment "non spinning reserve" ;
                                rdfs:label "NONSPIN" .


:AncillaryCommodityType.REGDN 
                              rdfs:comment "regulation down" ;
                              rdfs:label "REGDN" .


:AncillaryCommodityType.REGUP 
                              rdfs:comment "regulation up" ;
                              rdfs:label "REGUP" .


:AncillaryCommodityType.SPIN 
                             rdfs:comment "spinning reserve" ;
                             rdfs:label "SPIN" .


:AnodeType.ACA 
               rdfs:comment "Adjacent Control Area" ;
               rdfs:label "ACA" .


:AnodeType.AGR 
               rdfs:comment "Aggregate Generation Resource;" ;
               rdfs:label "AGR" .


:AnodeType.ALR 
               rdfs:comment "Aggregate Load Resource;" ;
               rdfs:label "ALR" .


:AnodeType.ASR 
               rdfs:comment "Aggregated System Resource" ;
               rdfs:label "ASR" .


:AnodeType.DER 
               rdfs:comment "Distributed Energy Resource." ;
               rdfs:label "DER" .


:AnodeType.ECA 
               rdfs:comment "Embedded Control Area" ;
               rdfs:label "ECA" .


:AnodeType.LFZ 
               rdfs:comment "Load Forecast Zone" ;
               rdfs:label "LFZ" .


:AnodeType.LTAC 
                rdfs:comment "Load TransmissionAccessCharge (TAC) Group;" ;
                rdfs:label "LTAC" .


:AnodeType.POD 
               rdfs:comment "Point of Delivery;" ;
               rdfs:label "POD" .


:AnodeType.REG 
               rdfs:comment "Market Energy/Ancillary Service Region;" ;
               rdfs:label "REG" .


:AnodeType.RUC 
               rdfs:comment "RUC Zone" ;
               rdfs:label "RUC" .


:AnodeType.SYS 
               rdfs:comment "System Zone/Region;" ;
               rdfs:label "SYS" .


:ApnodeType.AG 
               rdfs:comment "Aggregated Generation" ;
               rdfs:label "AG" .


:ApnodeType.BUS 
                rdfs:comment "Bus" ;
                rdfs:label "BUS" .


:ApnodeType.CA 
               rdfs:comment "Control Area" ;
               rdfs:label "CA" .


:ApnodeType.CPZ 
                rdfs:comment "Custom Price Zone" ;
                rdfs:label "CPZ" .


:ApnodeType.DCA 
                rdfs:comment "Designated Congestion Area" ;
                rdfs:label "DCA" .


:ApnodeType.DPZ 
                rdfs:comment "Default Price Zone" ;
                rdfs:label "DPZ" .


:ApnodeType.EHV 
                rdfs:comment "500 kV - Extra High Voltage aggregate price nodes" ;
                rdfs:label "EHV" .


:ApnodeType.GA 
               rdfs:comment "generic aggregation" ;
               rdfs:label "GA" .


:ApnodeType.GH 
               rdfs:comment "generic hub" ;
               rdfs:label "GH" .


:ApnodeType.INT 
                rdfs:comment "Interface" ;
                rdfs:label "INT" .


:ApnodeType.SYS 
                rdfs:comment "System Zone" ;
                rdfs:label "SYS" .


:ApnodeType.TH 
               rdfs:comment "Trading  Hub" ;
               rdfs:label "TH" .


:ApnodeType.ZN 
               rdfs:comment "Zone" ;
               rdfs:label "ZN" .


:ApplicationSecurityKind.endToEndSecure 
                                        rdfs:comment "Indicates that E2E-security shall be used in order to allow establishment of an MMS association." ;
                                        rdfs:label "endToEndSecure" .


:ApplicationSecurityKind.nonSecure 
                                   rdfs:comment "Indicates that an application security shall not be used in order to allow establishment of an MSS association." ;
                                   rdfs:label "nonSecure" .


:ApplicationSecurityKind.secure 
                                rdfs:comment "Indicates that the A-security-profile as specified in Clause 11 (or IEC TS 62351-4:2007) shall be used in order to allow establishment of an MMS association." ;
                                rdfs:label "secure" .


:AreaControlMode.CF 
                    rdfs:comment "CF = Constant Frequency" ;
                    rdfs:label "CF" .


:AreaControlMode.CTL 
                     rdfs:comment "Constant Tie-Line" ;
                     rdfs:label "CTL" .


:AreaControlMode.OFF 
                     rdfs:comment "Off control" ;
                     rdfs:label "OFF" .


:AreaControlMode.TLB 
                     rdfs:comment "Tie-Line Bias" ;
                     rdfs:label "TLB" .


:AreaKind.borough 
                  rdfs:comment "Enumeration for the type of area defined for the borough" ;
                  rdfs:label "borough" .


:AreaKind.county 
                 rdfs:comment "Enumeration for the type of area defined for the county" ;
                 rdfs:label "county" .


:AreaKind.parish 
                 rdfs:comment "Enumeration for the type of area defined for the parish" ;
                 rdfs:label "parish" .


:AreaKind.serviceArea 
                      rdfs:comment "Enumeration for the type of area defined for the service area" ;
                      rdfs:label "serviceArea" .


:AreaKind.state 
                rdfs:comment "Enumeration for the type of area defined for the state" ;
                rdfs:label "state" .


:AreaKind.township 
                   rdfs:comment "Enumeration for the type of area defined for the township" ;
                   rdfs:label "township" .


:AreaKind.ward 
               rdfs:comment "Enumeration for the type of area defined for the ward" ;
               rdfs:label "ward" .


:AreaKind.zipcode 
                  rdfs:comment "Enumeration for the type of area defined for the zipcode" ;
                  rdfs:label "zipcode" .


:AssetFailureClassification.defect 
                                   rdfs:comment "Failure due to defect." ;
                                   rdfs:label "defect" .


:AssetFailureClassification.major 
                                  rdfs:comment "Major failure." ;
                                  rdfs:label "major" .


:AssetFailureClassification.majorNeedsReplacement 
                                                  rdfs:comment "Major failure – asset needs to be replaced." ;
                                                  rdfs:label "majorNeedsReplacement" .


:AssetFailureClassification.minor 
                                  rdfs:comment "Minor failure." ;
                                  rdfs:label "minor" .


:AssetFailureMode.failToCarryLoad 
                                  rdfs:comment "Failure to carry load." ;
                                  rdfs:label "failToCarryLoad" .


:AssetFailureMode.failToClose 
                              rdfs:comment "Failure to close." ;
                              rdfs:label "failToClose" .


:AssetFailureMode.failToInterrupt 
                                  rdfs:comment "Failure to interrupt." ;
                                  rdfs:label "failToInterrupt" .


:AssetFailureMode.failToOpen 
                             rdfs:comment "Failure to open." ;
                             rdfs:label "failToOpen" .


:AssetFailureMode.failToProvideInsulationLevel 
                                               rdfs:comment "Failure to provide insulation." ;
                                               rdfs:label "failToProvideInsulationLevel" .


:AssetGroupKind.analysisGroup 
                              rdfs:comment "Group is used for analysis purposes." ;
                              rdfs:label "analysisGroup" .


:AssetGroupKind.complianceGroup 
                                rdfs:comment "Group is used for compliance purposes." ;
                                rdfs:label "complianceGroup" .


:AssetGroupKind.functionalGroup 
                                rdfs:comment "Group is used for functional purposes, for example assets which are grouped together because they are part of a for a particular function - such as a group of feeders." ;
                                rdfs:label "functionalGroup" .


:AssetGroupKind.inventoryGroup 
                               rdfs:comment "Group is used for inventory purposes." ;
                               rdfs:label "inventoryGroup" .


:AssetGroupKind.other 
                      rdfs:label "other" .


:AssetHazardKind.ambientTempAbove38 
                                    rdfs:comment "Subject to ambient temperature above 38 °C." ;
                                    rdfs:label "ambientTempAbove38" .


:AssetHazardKind.ambientTempBelowMinus12 
                                         rdfs:comment "Subject to ambient temperature of below -12 °C." ;
                                         rdfs:label "ambientTempBelowMinus12" .


:AssetHazardKind.childrenAtPlay 
                                rdfs:comment "Children play in area (stray kite/ball hazard)." ;
                                rdfs:label "childrenAtPlay" .


:AssetHazardKind.fishingArea 
                             rdfs:comment "Fishing in area (fishing pole/line hazard)." ;
                             rdfs:label "fishingArea" .


:AssetHazardKind.other 
                       rdfs:comment "If other, look at type field for more information." ;
                       rdfs:label "other" .


:AssetHazardKind.vegetation 
                            rdfs:comment "Vegetation growing below asset that may cause problem." ;
                            rdfs:label "vegetation" .


:AssetKind.breakerAirBlastBreaker 
                                  rdfs:comment "Air blast circuit breaker." ;
                                  rdfs:label "breakerAirBlastBreaker" .


:AssetKind.breakerBulkOilBreaker 
                                 rdfs:comment "Bulk oil circuit breaker." ;
                                 rdfs:label "breakerBulkOilBreaker" .


:AssetKind.breakerInsulatingStackAssembly 
                                          rdfs:comment "Breaker insulating stack assembly (for live tank breaker)." ;
                                          rdfs:label "breakerInsulatingStackAssembly" .


:AssetKind.breakerMinimumOilBreaker 
                                    rdfs:comment "Minimum oil circuit breaker." ;
                                    rdfs:label "breakerMinimumOilBreaker" .


:AssetKind.breakerSF6DeadTankBreaker 
                                     rdfs:comment "SF6 dead tank breaker." ;
                                     rdfs:label "breakerSF6DeadTankBreaker" .


:AssetKind.breakerSF6LiveTankBreaker 
                                     rdfs:comment "SF6 live tank breaker." ;
                                     rdfs:label "breakerSF6LiveTankBreaker" .


:AssetKind.breakerTankAssembly 
                               rdfs:comment "Breaker tank assembly." ;
                               rdfs:label "breakerTankAssembly" .


:AssetKind.other 
                 rdfs:comment "Other type of Asset. The type attribute may provide more details in this case." ;
                 rdfs:label "other" .


:AssetKind.transformer 
                       rdfs:comment "Transformer." ;
                       rdfs:label "transformer" .


:AssetKind.transformerTank 
                           rdfs:comment "Transformer tank." ;
                           rdfs:label "transformerTank" .


:AssetLifecycleStateKind.disposedOf 
                                    rdfs:comment "Asset disposed of." ;
                                    rdfs:label "disposedOf" .


:AssetLifecycleStateKind.manufactured 
                                      rdfs:comment "Asset manufactured." ;
                                      rdfs:label "manufactured" .


:AssetLifecycleStateKind.purchased 
                                   rdfs:comment "Asset purchased." ;
                                   rdfs:label "purchased" .


:AssetLifecycleStateKind.received 
                                  rdfs:comment "Asset received." ;
                                  rdfs:label "received" .


:AssetLifecycleStateKind.retired 
                                 rdfs:comment "Asset retired." ;
                                 rdfs:label "retired" .


:AssetModelUsageKind.customerSubstation 
                                        rdfs:comment "Asset model is intended for use in customer substation." ;
                                        rdfs:label "customerSubstation" .


:AssetModelUsageKind.distributionOverhead 
                                          rdfs:comment "Asset model is intended for use in distribution overhead network." ;
                                          rdfs:label "distributionOverhead" .


:AssetModelUsageKind.distributionUnderground 
                                             rdfs:comment "Asset model is intended for use in underground distribution network." ;
                                             rdfs:label "distributionUnderground" .


:AssetModelUsageKind.other 
                           rdfs:comment "Other kind of asset model usage." ;
                           rdfs:label "other" .


:AssetModelUsageKind.streetlight 
                                 rdfs:comment "Asset model is intended for use as streetlight." ;
                                 rdfs:label "streetlight" .


:AssetModelUsageKind.substation 
                                rdfs:comment "Asset model is intended for use in substation." ;
                                rdfs:label "substation" .


:AssetModelUsageKind.transmission 
                                  rdfs:comment "Asset model is intended for use in transmission network." ;
                                  rdfs:label "transmission" .


:AssetModelUsageKind.unknown 
                             rdfs:comment "Usage of the asset model is unknown." ;
                             rdfs:label "unknown" .


:AssetStringKind.visualExamRemarks 
                                   rdfs:comment """Remarks related to a visual exam.
Could be used for remarks on oil appearance resulting from visual examination, including sediment, appearance, free water.""" ;
                                   rdfs:label "visualExamRemarks" .


:AssetTemperaturePressureAnalogKind.oilPressureAtValve 
                                                       rdfs:comment "Oil pressure at valve (in KPa)." ;
                                                       rdfs:label "oilPressureAtValve" .


:AssetTemperaturePressureAnalogKind.oilTemperatureAtValve 
                                                          rdfs:comment "Oil temperature at valve (in °C)." ;
                                                          rdfs:label "oilTemperatureAtValve" .


:AsynchronousMachineKind.generator 
                                   rdfs:comment "The Asynchronous Machine is a generator." ;
                                   rdfs:label "generator" .


:AsynchronousMachineKind.motor 
                               rdfs:comment "The Asynchronous Machine is a motor." ;
                               rdfs:label "motor" .


:AtmosphericAnalogKind.albedo 
                              rdfs:label "albedo" .


:AtmosphericAnalogKind.ambientTemperature 
                                          rdfs:comment "The temperature measured b<font color=\"#0f0f0f\">y a thermometer exposed to the air in a place sheltered from direct solar radiation. </font>Also known as \"dry bulb\" because<font color=\"#0f0f0f\"> the air temperature is indicated by a thermometer not affecte</font>d by the moisture of the air." ;
                                          rdfs:label "ambientTemperature" .


:AtmosphericAnalogKind.atmosphericPressure 
                                           rdfs:label "atmosphericPressure" .


:AtmosphericAnalogKind.ceiling 
                               rdfs:label "ceiling" .


:AtmosphericAnalogKind.dewPoint 
                                rdfs:comment "The temperature to which air must be cooled at constant pressure and constant water-vapor content in order for saturation to occur. In other words, it is the temperature at which water vapor starts to condense out of the air." ;
                                rdfs:label "dewPoint" .


:AtmosphericAnalogKind.heatIndex 
                                 rdfs:comment "The temperature of how hot it \"feels like\" for a given combination of warm air temperature and relative humidity." ;
                                 rdfs:label "heatIndex" .


:AtmosphericAnalogKind.horizontalVisibility 
                                            rdfs:label "horizontalVisibility" .


:AtmosphericAnalogKind.humidity 
                                rdfs:label "humidity" .


:AtmosphericAnalogKind.ice 
                           rdfs:label "ice" .


:AtmosphericAnalogKind.illuminanceDiffuseHorizontal 
                                                    rdfs:label "illuminanceDiffuseHorizontal" .


:AtmosphericAnalogKind.illuminanceDirectNormal 
                                               rdfs:label "illuminanceDirectNormal" .


:AtmosphericAnalogKind.illuminanceGlobalHorizontal 
                                                   rdfs:label "illuminanceGlobalHorizontal" .


:AtmosphericAnalogKind.irradianceDiffuseHorizonal 
                                                  rdfs:label "irradianceDiffuseHorizonal" .


:AtmosphericAnalogKind.irradianceDirectNormal 
                                              rdfs:label "irradianceDirectNormal" .


:AtmosphericAnalogKind.irradianceExtraTerrestrialHorizontal 
                                                            rdfs:label "irradianceExtraTerrestrialHorizontal" .


:AtmosphericAnalogKind.irradianceExtraTerrestrialVertical 
                                                          rdfs:label "irradianceExtraTerrestrialVertical" .


:AtmosphericAnalogKind.irradianceGlobalHorizontal 
                                                  rdfs:label "irradianceGlobalHorizontal" .


:AtmosphericAnalogKind.luminanceZenith 
                                       rdfs:label "luminanceZenith" .


:AtmosphericAnalogKind.precipitation 
                                     rdfs:label "precipitation" .


:AtmosphericAnalogKind.rain 
                            rdfs:label "rain" .


:AtmosphericAnalogKind.skyCoverageOpaque 
                                         rdfs:label "skyCoverageOpaque" .


:AtmosphericAnalogKind.skyCoverageTotal 
                                        rdfs:label "skyCoverageTotal" .


:AtmosphericAnalogKind.snow 
                            rdfs:comment "Snow amount over a specified period of time." ;
                            rdfs:label "snow" .


:AtmosphericAnalogKind.verticalVisibility 
                                          rdfs:label "verticalVisibility" .


:AtmosphericAnalogKind.windChill 
                                 rdfs:comment "The temperature of how cold it \"feels like\" based on the rate of heat loss from exposed skin caused by the effects of wind and cold temperatures." ;
                                 rdfs:label "windChill" .


:AtmosphericAnalogKind.windSpeedGust 
                                     rdfs:comment """Maximum instantaneous wind speed in the 10 minute period preceding a moment in time so long as more than 10 knots of difference has been exhibited between peaks and lulls during that 10 minute time period. 
0 value means no gusts during preceding 10 minute period.""" ;
                                     rdfs:label "windSpeedGust" .


:AtmosphericAnalogKind.windSpeedInstantaneous 
                                              rdfs:comment "Wind speed at a moment in time." ;
                                              rdfs:label "windSpeedInstantaneous" .


:AtmosphericAnalogKind.windSpeedPeak 
                                     rdfs:comment """Peak instantaneous wind speed in the 60 minutes preceding a moment in time as long as peak speed greater than 25 knots.  
0 value means speed did not exceed 25 knots during preceding 60 minutes.""" ;
                                     rdfs:label "windSpeedPeak" .


:AtmosphericAnalogKind.windSpeedSustained 
                                          rdfs:comment "Average instantaneous wind speed over the 2-minute time period preceding a moment in time." ;
                                          rdfs:label "windSpeedSustained" .


:AutomaticDispInstTypeCommitment.DR_ADJUSTMENT 
                                               rdfs:comment "Distributed Resource adjustment for a distributed resource that is already deployed (committed)." ;
                                               rdfs:label "DR_ADJUSTMENT" .


:AutomaticDispInstTypeCommitment.DR_DEPLOY 
                                           rdfs:comment "Distributed Resource Deployment" ;
                                           rdfs:label "DR_DEPLOY" .


:AutomaticDispInstTypeCommitment.DR_RELEASE 
                                            rdfs:comment "Distributed Resource Release" ;
                                            rdfs:label "DR_RELEASE" .


:AutomaticDispInstTypeCommitment.SHUT_DOWN 
                                           rdfs:comment "Shut down instruction type" ;
                                           rdfs:label "SHUT_DOWN" .


:AutomaticDispInstTypeCommitment.START_UP 
                                          rdfs:comment "Start up instruction type" ;
                                          rdfs:label "START_UP" .


:AutomaticDispatchMode.CONTINGENCY 
                                   rdfs:comment "Contingnency occurance, redispatch of contingency reserves" ;
                                   rdfs:label "CONTINGENCY" .


:AutomaticDispatchMode.INTERVAL 
                                rdfs:label "INTERVAL" .


:AutomaticDispatchMode.MANUAL 
                              rdfs:comment "Operator override" ;
                              rdfs:label "MANUAL" .


:BatteryStateKind.charging 
                           rdfs:comment "Stored energy is increasing." ;
                           rdfs:label "charging" .


:BatteryStateKind.discharging 
                              rdfs:comment "Stored energy is decreasing." ;
                              rdfs:label "discharging" .


:BatteryStateKind.empty 
                        rdfs:comment "Unable to discharge, and not charging." ;
                        rdfs:label "empty" .


:BatteryStateKind.full 
                       rdfs:comment "Unable to charge, and not discharging." ;
                       rdfs:label "full" .


:BatteryStateKind.waiting 
                          rdfs:comment "Neither charging nor discharging, but able to do so." ;
                          rdfs:label "waiting" .


:BidCalculationBasis.COST_BASED 
                                rdfs:comment "Based on unit generation characteristics and a cost of fuel." ;
                                rdfs:label "COST_BASED" .


:BidCalculationBasis.LMP_BASED 
                               rdfs:comment "Based on prices paid at particular pricing location." ;
                               rdfs:label "LMP_BASED" .


:BidCalculationBasis.NEGOTIATED 
                                rdfs:comment "An amount negotiated with the designated Independent Entity." ;
                                rdfs:label "NEGOTIATED" .


:BidMitigationStatus.B 
                       rdfs:label "B" .


:BidMitigationStatus.L 
                       rdfs:label "L" .


:BidMitigationStatus.M 
                       rdfs:label "M" .


:BidMitigationStatus.O 
                       rdfs:label "O" .


:BidMitigationStatus.R 
                       rdfs:label "R" .


:BidMitigationStatus.S 
                       rdfs:label "S" .


:BidMitigationType.F 
                     rdfs:label "F" .


:BidMitigationType.I 
                     rdfs:label "I" .


:BidPriceCapType.AS 
                    rdfs:label "AS" .


:BidPriceCapType.ENERGY 
                        rdfs:label "ENERGY" .


:BidPriceCapType.RUC 
                     rdfs:label "RUC" .


:BidStatusType.CL 
                  rdfs:comment "Clean" ;
                  rdfs:label "CL" .


:BidStatusType.CM 
                  rdfs:label "CM" .


:BidStatusType.CV 
                  rdfs:label "CV" .


:BidStatusType.CX 
                  rdfs:label "CX" .


:BidStatusType.I 
                 rdfs:label "I" .


:BidStatusType.M 
                 rdfs:label "M" .


:BidStatusType.O 
                 rdfs:label "O" .


:BidStatusType.RJ 
                  rdfs:label "RJ" .


:BidStatusType.RP 
                  rdfs:comment "Replicated" ;
                  rdfs:label "RP" .


:BidStatusType.V 
                 rdfs:label "V" .


:BidType.DEFAULT_ENERGY_BID 
                            rdfs:label "DEFAULT_ENERGY_BID" .


:BidType.DEFAULT_MINIMUM_LOAD_BID 
                                  rdfs:label "DEFAULT_MINIMUM_LOAD_BID" .


:BidType.DEFAULT_STARTUP_BID 
                             rdfs:label "DEFAULT_STARTUP_BID" .


:BidTypeRMR.QUALIFIED_PREDISPATCH 
                                  rdfs:comment "Output of requirements bid self schedule type." ;
                                  rdfs:label "QUALIFIED_PREDISPATCH" .


:BidTypeRMR.REQUIREMENTS 
                         rdfs:comment "Qualified pre-dispatch bid self schedule type." ;
                         rdfs:label "REQUIREMENTS" .


:BillMediaKind.electronic 
                          rdfs:label "electronic" .


:BillMediaKind.other 
                     rdfs:label "other" .


:BillMediaKind.paper 
                     rdfs:label "paper" .


:BoilerControlMode.coordinated 
                               rdfs:comment "Coordinated." ;
                               rdfs:label "coordinated" .


:BoilerControlMode.following 
                             rdfs:comment "Following." ;
                             rdfs:label "following" .


:BreakerApplicationKind.busBreaker 
                                   rdfs:comment "Bus breaker." ;
                                   rdfs:label "busBreaker" .


:BreakerApplicationKind.busTieBreaker 
                                      rdfs:comment "Bus tie breaker." ;
                                      rdfs:label "busTieBreaker" .


:BreakerApplicationKind.capacitorOrReactorBankBreaker 
                                                      rdfs:comment "Capacitor or reactor breaker." ;
                                                      rdfs:label "capacitorOrReactorBankBreaker" .


:BreakerApplicationKind.feederBreaker 
                                      rdfs:comment "Feeder breaker." ;
                                      rdfs:label "feederBreaker" .


:BreakerApplicationKind.other 
                              rdfs:comment "Other type of breaker application." ;
                              rdfs:label "other" .


:BreakerApplicationKind.spare 
                              rdfs:comment "Spare breaker." ;
                              rdfs:label "spare" .


:BreakerApplicationKind.stepUpTransformerBreakerFossil 
                                                       rdfs:comment "Step-up transformer breaker for fossil generator." ;
                                                       rdfs:label "stepUpTransformerBreakerFossil" .


:BreakerApplicationKind.stepUpTransformerBreakerHydro 
                                                      rdfs:comment "Step-up transformer breaker for hydro generator." ;
                                                      rdfs:label "stepUpTransformerBreakerHydro" .


:BreakerApplicationKind.stepUpTransformerBreakerNuclear 
                                                        rdfs:comment "Step-up transformer breaker for nuclear generator." ;
                                                        rdfs:label "stepUpTransformerBreakerNuclear" .


:BreakerApplicationKind.stepUpTransformerBreakerPumpedStorage 
                                                              rdfs:comment "Step-up transformer breaker for pumped storage." ;
                                                              rdfs:label "stepUpTransformerBreakerPumpedStorage" .


:BreakerApplicationKind.substationTransformerBreaker 
                                                     rdfs:comment "Substation transformer breaker." ;
                                                     rdfs:label "substationTransformerBreaker" .


:BreakerApplicationKind.transmissionFlowGateLineBreaker 
                                                        rdfs:comment "Transmission flow gate line breaker." ;
                                                        rdfs:label "transmissionFlowGateLineBreaker" .


:BreakerApplicationKind.transmissionLineBreaker 
                                                rdfs:comment "Transmission line breaker." ;
                                                rdfs:label "transmissionLineBreaker" .


:BreakerApplicationKind.transmissionTieLineBreaker 
                                                   rdfs:comment "Transmission tie line breaker." ;
                                                   rdfs:label "transmissionTieLineBreaker" .


:BreakerConfiguration.breakerAndAHalf 
                                      rdfs:comment "Breaker and a half." ;
                                      rdfs:label "breakerAndAHalf" .


:BreakerConfiguration.doubleBreaker 
                                    rdfs:comment "Double breaker." ;
                                    rdfs:label "doubleBreaker" .


:BreakerConfiguration.noBreaker 
                                rdfs:comment "No breaker." ;
                                rdfs:label "noBreaker" .


:BreakerConfiguration.singleBreaker 
                                    rdfs:comment "Single breaker." ;
                                    rdfs:label "singleBreaker" .


:BreakerFailureReasonKind.SF6BlastValveFailure 
                                               rdfs:comment "SF6 blast valve failure." ;
                                               rdfs:label "SF6BlastValveFailure" .


:BreakerFailureReasonKind.SF6PufferFailure 
                                           rdfs:comment "SF6 puffer valve failure." ;
                                           rdfs:label "SF6PufferFailure" .


:BreakerFailureReasonKind.blastValveFailure 
                                            rdfs:comment "Blast valve failure." ;
                                            rdfs:label "blastValveFailure" .


:BreakerFailureReasonKind.bushingFailure 
                                         rdfs:comment "Bushing failure." ;
                                         rdfs:label "bushingFailure" .


:BreakerFailureReasonKind.closeCoilOpenShortedFailed 
                                                     rdfs:comment "Close coil open shorted failure." ;
                                                     rdfs:label "closeCoilOpenShortedFailed" .


:BreakerFailureReasonKind.contaminatedAir 
                                          rdfs:comment "Contaminated air." ;
                                          rdfs:label "contaminatedAir" .


:BreakerFailureReasonKind.contaminatedArcChutes 
                                                rdfs:comment "Contaminated arc chutes." ;
                                                rdfs:label "contaminatedArcChutes" .


:BreakerFailureReasonKind.contaminatedGas 
                                          rdfs:comment "Contaminated gas." ;
                                          rdfs:label "contaminatedGas" .


:BreakerFailureReasonKind.contaminatedGasAir 
                                             rdfs:comment "Contaminated gas or air." ;
                                             rdfs:label "contaminatedGasAir" .


:BreakerFailureReasonKind.controlCircuitFailure 
                                                rdfs:comment "Control circuit failure." ;
                                                rdfs:label "controlCircuitFailure" .


:BreakerFailureReasonKind.degradedLubrication 
                                              rdfs:comment "Degraded lubrication." ;
                                              rdfs:label "degradedLubrication" .


:BreakerFailureReasonKind.externalOrInternalContamination 
                                                          rdfs:comment "External or internal contamination." ;
                                                          rdfs:label "externalOrInternalContamination" .


:BreakerFailureReasonKind.highPressureAirPlant 
                                               rdfs:comment "High pressure air plant." ;
                                               rdfs:label "highPressureAirPlant" .


:BreakerFailureReasonKind.highResistanceLoadPath 
                                                 rdfs:comment "High resistance load path." ;
                                                 rdfs:label "highResistanceLoadPath" .


:BreakerFailureReasonKind.highResistancePath 
                                             rdfs:comment "High resistance path." ;
                                             rdfs:label "highResistancePath" .


:BreakerFailureReasonKind.interrupterContactFailure 
                                                    rdfs:comment "Interrupter contact failure." ;
                                                    rdfs:label "interrupterContactFailure" .


:BreakerFailureReasonKind.interrupterFailure 
                                             rdfs:comment "Interrupter failure." ;
                                             rdfs:label "interrupterFailure" .


:BreakerFailureReasonKind.linkageFailure 
                                         rdfs:comment "Linkage failure." ;
                                         rdfs:label "linkageFailure" .


:BreakerFailureReasonKind.lossOfOil 
                                    rdfs:comment "Loss of oil." ;
                                    rdfs:label "lossOfOil" .


:BreakerFailureReasonKind.lossOfVacuum 
                                       rdfs:comment "Loss of vacuum." ;
                                       rdfs:label "lossOfVacuum" .


:BreakerFailureReasonKind.lowGasPressure 
                                         rdfs:comment "Low gas pressure." ;
                                         rdfs:label "lowGasPressure" .


:BreakerFailureReasonKind.mechanismFailure 
                                           rdfs:comment "Blast valve failure." ;
                                           rdfs:label "mechanismFailure" .


:BreakerFailureReasonKind.mechanismOrLinkageFailure 
                                                    rdfs:comment "Mechanism or linkage failure." ;
                                                    rdfs:label "mechanismOrLinkageFailure" .


:BreakerFailureReasonKind.oilRelatedFailure 
                                            rdfs:comment "Oil-related failure." ;
                                            rdfs:label "oilRelatedFailure" .


:BreakerFailureReasonKind.poorOilQuality 
                                         rdfs:comment "Poor oil quality." ;
                                         rdfs:label "poorOilQuality" .


:BreakerFailureReasonKind.rackingMechanismFailure 
                                                  rdfs:comment "Racking mechanism failure." ;
                                                  rdfs:label "rackingMechanismFailure" .


:BreakerFailureReasonKind.resistorFailure 
                                          rdfs:comment "Resistor failure." ;
                                          rdfs:label "resistorFailure" .


:BreakerFailureReasonKind.resistorGradingCapacitorFailure 
                                                          rdfs:comment "Resistor grading capacitor failure." ;
                                                          rdfs:label "resistorGradingCapacitorFailure" .


:BreakerFailureReasonKind.solidDielectricFailure 
                                                 rdfs:comment "Solid dielectric failure." ;
                                                 rdfs:label "solidDielectricFailure" .


:BreakerFailureReasonKind.storedEnergyFailure 
                                              rdfs:comment "Stored energy failure." ;
                                              rdfs:label "storedEnergyFailure" .


:BreakerFailureReasonKind.tripCoilOpenShortedFailed 
                                                    rdfs:comment "Trip coil open shorted failure." ;
                                                    rdfs:label "tripCoilOpenShortedFailed" .


:BreakerMaintenanceKind.externalOutOfService 
                                             rdfs:comment "External out-of-service inspection and maintenance." ;
                                             rdfs:label "externalOutOfService" .


:BreakerMaintenanceKind.internalOutOfService 
                                             rdfs:comment "Internal (interrupter) inspection and maintenance (breaker out of service)." ;
                                             rdfs:label "internalOutOfService" .


:BreakerMaintenanceKind.interrupterOverhaul 
                                            rdfs:comment "Overhaul of breaker interrupter unit." ;
                                            rdfs:label "interrupterOverhaul" .


:BreakerRepairItemKind.SF6GasLeak 
                                  rdfs:comment "SF6 gas leak repair." ;
                                  rdfs:label "SF6GasLeak" .


:BreakerRepairItemKind.airCompressor 
                                     rdfs:comment "Air compressor repair." ;
                                     rdfs:label "airCompressor" .


:BreakerRepairItemKind.auxiliarySwitchAndLinkage 
                                                 rdfs:comment "Auxiliary switch and linkage repair." ;
                                                 rdfs:label "auxiliarySwitchAndLinkage" .


:BreakerRepairItemKind.busConnection 
                                     rdfs:comment "Bus connection repair." ;
                                     rdfs:label "busConnection" .


:BreakerRepairItemKind.checkValve 
                                  rdfs:comment "Check valve repair." ;
                                  rdfs:label "checkValve" .


:BreakerRepairItemKind.closeCoil 
                                 rdfs:comment "Close coil repair." ;
                                 rdfs:label "closeCoil" .


:BreakerRepairItemKind.contactor 
                                 rdfs:comment "Contactor repair." ;
                                 rdfs:label "contactor" .


:BreakerRepairItemKind.controlCircuit 
                                      rdfs:comment "Control circuit repair." ;
                                      rdfs:label "controlCircuit" .


:BreakerRepairItemKind.corrosion 
                                 rdfs:comment "Corrosion repair." ;
                                 rdfs:label "corrosion" .


:BreakerRepairItemKind.gasDensitySupervision 
                                             rdfs:comment "Gas density supervision repair." ;
                                             rdfs:label "gasDensitySupervision" .


:BreakerRepairItemKind.heaterOrThermostat 
                                          rdfs:comment "Heater or thermostat repair." ;
                                          rdfs:label "heaterOrThermostat" .


:BreakerRepairItemKind.hydraulicFluidLeak 
                                          rdfs:comment "Hydraulic fluid leak repair." ;
                                          rdfs:label "hydraulicFluidLeak" .


:BreakerRepairItemKind.interrupterAssembly 
                                           rdfs:comment "Interrupter assembly repair." ;
                                           rdfs:label "interrupterAssembly" .


:BreakerRepairItemKind.other 
                             rdfs:comment "Other type of repair." ;
                             rdfs:label "other" .


:BreakerRepairItemKind.positionIndicator 
                                         rdfs:comment "Position indicator repair." ;
                                         rdfs:label "positionIndicator" .


:BreakerRepairItemKind.pressureSwitch 
                                      rdfs:comment "Pressure switch repair." ;
                                      rdfs:label "pressureSwitch" .


:BreakerRepairItemKind.pumpOrMotor 
                                   rdfs:comment "Pump or motor repair." ;
                                   rdfs:label "pumpOrMotor" .


:BreakerRepairItemKind.relay 
                             rdfs:comment "Relay repair." ;
                             rdfs:label "relay" .


:BreakerRepairItemKind.storedEnergySystem 
                                          rdfs:comment "Stored energy system repair." ;
                                          rdfs:label "storedEnergySystem" .


:BreakerRepairItemKind.tripCoil 
                                rdfs:comment "Trip coil repair." ;
                                rdfs:label "tripCoil" .


:BreakerRepairItemKind.tripControlValve 
                                        rdfs:comment "Trip control valve repair." ;
                                        rdfs:label "tripControlValve" .


:BreakerRepairItemKind.wiring 
                              rdfs:comment "Wiring repair." ;
                              rdfs:label "wiring" .


:BusbarConfiguration.doubleBus 
                               rdfs:comment "Double bus." ;
                               rdfs:label "doubleBus" .


:BusbarConfiguration.mainWithTransfer 
                                      rdfs:comment "Main bus with transfer bus." ;
                                      rdfs:label "mainWithTransfer" .


:BusbarConfiguration.ringBus 
                             rdfs:comment "Ring bus." ;
                             rdfs:label "ringBus" .


:BusbarConfiguration.singleBus 
                               rdfs:comment "Single bus." ;
                               rdfs:label "singleBus" .


:BushingInsulationKind.compound 
                                rdfs:comment "Compound." ;
                                rdfs:label "compound" .


:BushingInsulationKind.oilImpregnatedPaper 
                                           rdfs:comment "Oil impregnated paper." ;
                                           rdfs:label "oilImpregnatedPaper" .


:BushingInsulationKind.other 
                             rdfs:comment "Other." ;
                             rdfs:label "other" .


:BushingInsulationKind.resinBondedPaper 
                                        rdfs:comment "Resin bonded paper." ;
                                        rdfs:label "resinBondedPaper" .


:BushingInsulationKind.resinImpregnatedPaper 
                                             rdfs:comment "Resin impregnated paper." ;
                                             rdfs:label "resinImpregnatedPaper" .


:BushingInsulationKind.solidPorcelain 
                                      rdfs:comment "Solid porcelain." ;
                                      rdfs:label "solidPorcelain" .


:BushingInsulationPfTestKind.c1 
                                rdfs:comment "Power factor tap-to-ground." ;
                                rdfs:label "c1" .


:BushingInsulationPfTestKind.c2 
                                rdfs:comment "Power factor tap-to-conductor." ;
                                rdfs:label "c2" .


:CIGREStandardEditionKind._2000 
                                rdfs:comment "2000 standard edition." ;
                                rdfs:label "2000" .


:CIGREStandardEditionKind.none 
                               rdfs:comment "No standard edition." ;
                               rdfs:label "none" .


:CIGREStandardEditionKind.unknown 
                                  rdfs:comment "Unknown standard edition." ;
                                  rdfs:label "unknown" .


:CIGREStandardKind.TB_170 
                          rdfs:comment "CIGRE Technical Brochure 170 Static Electrification in Power Transformers." ;
                          rdfs:label "TB 170" .


:CRRCategoryType.NSR 
                     rdfs:comment "Network Service" ;
                     rdfs:label "NSR" .


:CRRCategoryType.PTP 
                     rdfs:comment "Point to Point" ;
                     rdfs:label "PTP" .


:CRRHedgeType.OBLIGATION 
                         rdfs:label "OBLIGATION" .


:CRRHedgeType.OPTION 
                     rdfs:label "OPTION" .


:CRRRoleType.BUYER 
                   rdfs:label "BUYER" .


:CRRRoleType.OWNER 
                   rdfs:label "OWNER" .


:CRRRoleType.SELLER 
                    rdfs:label "SELLER" .


:CRRSegmentType.AUC 
                    rdfs:label "AUC" .


:CRRSegmentType.CAP 
                    rdfs:label "CAP" .


:CRRSegmentType.CF 
                   rdfs:label "CF" .


:CRRSegmentType.CVR 
                    rdfs:comment "Converted rights." ;
                    rdfs:label "CVR" .


:CRRSegmentType.ETC 
                    rdfs:comment "Existing Transmission Contract." ;
                    rdfs:label "ETC" .


:CRRSegmentType.LSE 
                    rdfs:comment "Load Serving Entity." ;
                    rdfs:label "LSE" .


:CRRSegmentType.MT 
                   rdfs:comment "Merchant transmission." ;
                   rdfs:label "MT" .


:CRRSegmentType.TOR 
                    rdfs:comment "Transmission Ownership Rights." ;
                    rdfs:label "TOR" .


:CableConstructionKind.compacted 
                                 rdfs:comment "Compacted cable." ;
                                 rdfs:label "compacted" .


:CableConstructionKind.compressed 
                                  rdfs:comment "Compressed cable." ;
                                  rdfs:label "compressed" .


:CableConstructionKind.other 
                             rdfs:comment "Other kind of cable construction." ;
                             rdfs:label "other" .


:CableConstructionKind.sector 
                              rdfs:comment "Sector cable." ;
                              rdfs:label "sector" .


:CableConstructionKind.segmental 
                                 rdfs:comment "Segmental cable." ;
                                 rdfs:label "segmental" .


:CableConstructionKind.solid 
                             rdfs:comment "Solid cable." ;
                             rdfs:label "solid" .


:CableConstructionKind.stranded 
                                rdfs:comment "Stranded cable." ;
                                rdfs:label "stranded" .


:CableOuterJacketKind.insulating 
                                 rdfs:comment "Insulating cable outer jacket." ;
                                 rdfs:label "insulating" .


:CableOuterJacketKind.linearLowDensityPolyethylene 
                                                   rdfs:comment "Linear low density polyethylene cable outer jacket." ;
                                                   rdfs:label "linearLowDensityPolyethylene" .


:CableOuterJacketKind.none 
                           rdfs:comment "Cable has no outer jacket." ;
                           rdfs:label "none" .


:CableOuterJacketKind.other 
                            rdfs:comment "Pther kind of cable outer jacket." ;
                            rdfs:label "other" .


:CableOuterJacketKind.polyethylene 
                                   rdfs:comment "Polyethylene cable outer jacket." ;
                                   rdfs:label "polyethylene" .


:CableOuterJacketKind.pvc 
                          rdfs:comment "PVC cable outer jacket." ;
                          rdfs:label "pvc" .


:CableOuterJacketKind.semiconducting 
                                     rdfs:comment "Semiconducting cable outer jacket." ;
                                     rdfs:label "semiconducting" .


:CableShieldMaterialKind.aluminum 
                                  rdfs:comment "Aluminum cable shield." ;
                                  rdfs:label "aluminum" .


:CableShieldMaterialKind.copper 
                                rdfs:comment "Copper cable shield." ;
                                rdfs:label "copper" .


:CableShieldMaterialKind.lead 
                              rdfs:comment "Lead cable shield." ;
                              rdfs:label "lead" .


:CableShieldMaterialKind.other 
                               rdfs:comment "Other kind of cable shield material." ;
                               rdfs:label "other" .


:CableShieldMaterialKind.steel 
                               rdfs:comment "Steel cable shield." ;
                               rdfs:label "steel" .


:CalculationIntervalUnitKind.cycle 
                                   rdfs:comment "Period expressed in cycles." ;
                                   rdfs:label "cycle" .


:CalculationIntervalUnitKind.day 
                                 rdfs:comment "Period expressed in days." ;
                                 rdfs:label "day" .


:CalculationIntervalUnitKind.hour 
                                  rdfs:comment "Period expressed in hours." ;
                                  rdfs:label "hour" .


:CalculationIntervalUnitKind.milliSecond 
                                         rdfs:comment "Period expressed in milli-seconds." ;
                                         rdfs:label "milliSecond" .


:CalculationIntervalUnitKind.minute 
                                    rdfs:comment "Period expressed in minutes." ;
                                    rdfs:label "minute" .


:CalculationIntervalUnitKind.month 
                                   rdfs:comment "Period expressed in months." ;
                                   rdfs:label "month" .


:CalculationIntervalUnitKind.perCycle 
                                      rdfs:comment "Period expressed in per-cycle." ;
                                      rdfs:label "perCycle" .


:CalculationIntervalUnitKind.season 
                                    rdfs:comment "Period expressed in seasons." ;
                                    rdfs:label "season" .


:CalculationIntervalUnitKind.second 
                                    rdfs:comment "Period expressed in seconds." ;
                                    rdfs:label "second" .


:CalculationIntervalUnitKind.week 
                                  rdfs:comment "Period expressed in weeks." ;
                                  rdfs:label "week" .


:CalculationIntervalUnitKind.year 
                                  rdfs:comment "Period expressed in years." ;
                                  rdfs:label "year" .


:CalculationKind.div 
                     rdfs:comment "Division operation the input values (operands)." ;
                     rdfs:label "div" .


:CalculationKind.mul 
                     rdfs:comment "Multiplication operation the input values (operands)." ;
                     rdfs:label "mul" .


:CalculationKind.sqrt 
                      rdfs:comment "Square root operator - only one input value (operands)." ;
                      rdfs:label "sqrt" .


:CalculationKind.sum 
                     rdfs:comment "Summation operation over the input values (operands)." ;
                     rdfs:label "sum" .


:CalculationModeKind.period 
                            rdfs:comment "Calcuation is for fixed period." ;
                            rdfs:label "period" .


:CalculationModeKind.sliding 
                             rdfs:comment "Calculation is for sliding period." ;
                             rdfs:label "sliding" .


:CalculationModeKind.total 
                           rdfs:comment "Calculation is for total period." ;
                           rdfs:label "total" .


:CalculationTechniqueKind.average 
                                  rdfs:comment "Result is average value for period." ;
                                  rdfs:label "average" .


:CalculationTechniqueKind.maximum 
                                  rdfs:comment "Result is maximum value for period." ;
                                  rdfs:label "maximum" .


:CalculationTechniqueKind.minimum 
                                  rdfs:comment "Result is minimum value for period." ;
                                  rdfs:label "minimum" .


:CalculationTechniqueKind.trueRMS 
                                  rdfs:comment "Result is RMS value for period." ;
                                  rdfs:label "trueRMS" .


:ChargeKind.auxiliaryCharge 
                            rdfs:comment "Any other charge which is not a consumptionCharge or demandCharge. For example: debt recovery, arrears, standing charge or charge for another service such as street lighting." ;
                            rdfs:label "auxiliaryCharge" .


:ChargeKind.consumptionCharge 
                              rdfs:comment "The charge levied for the actual usage of the service, normally expressed in terms of a tariff. For example: usage x price per kWh = total charge for consumption." ;
                              rdfs:label "consumptionCharge" .


:ChargeKind.demandCharge 
                         rdfs:comment "The charge related to the usage within a defined time interval, normally expressed in terms of a tariff. For example: a maximum-demand tariff will levy an additional charge on top of the consumption charge if the usage exceeds a defined limit per hour." ;
                         rdfs:label "demandCharge" .


:ChargeKind.other 
                  rdfs:comment "Other kind of charge." ;
                  rdfs:label "other" .


:ChargeKind.taxCharge 
                      rdfs:comment "Any charge that is classified as a tax of a kind. For example: VAT, GST, TV tax, etc." ;
                      rdfs:label "taxCharge" .


:CheckOutType.AFTER_THE_FACT 
                             rdfs:label "AFTER_THE_FACT" .


:CheckOutType.PRE_HOUR 
                       rdfs:label "PRE_HOUR" .


:CheckOutType.PRE_SCHEDULE 
                           rdfs:label "PRE_SCHEDULE" .


:ChequeKind.bankOrder 
                      rdfs:comment "Payment order used by a bank." ;
                      rdfs:label "bankOrder" .


:ChequeKind.other 
                  rdfs:comment "Other kind of cheque." ;
                  rdfs:label "other" .


:ChequeKind.postalOrder 
                        rdfs:comment "Payment order used by institutions other than banks." ;
                        rdfs:label "postalOrder" .


:CleanTradeProductType.APN 
                           rdfs:comment "Energy Trades at Aggregated Pricing Nodes" ;
                           rdfs:label "APN" .


:CleanTradeProductType.CPT 
                           rdfs:comment "Converted Physical Energy Trade" ;
                           rdfs:label "CPT" .


:CleanTradeProductType.NRT 
                           rdfs:comment "Non-Spinning Reserve Trade" ;
                           rdfs:label "NRT" .


:CleanTradeProductType.PHY 
                           rdfs:comment "Physical Energy Tra" ;
                           rdfs:label "PHY" .


:CleanTradeProductType.RDT 
                           rdfs:comment "Regulation Down Trade" ;
                           rdfs:label "RDT" .


:CleanTradeProductType.RUT 
                           rdfs:comment "Regulation Up Trade" ;
                           rdfs:label "RUT" .


:CleanTradeProductType.SRT 
                           rdfs:comment "Spinning Reserve Trade" ;
                           rdfs:label "SRT" .


:ClearanceActionKind.issue 
                           rdfs:comment "Issue clearance." ;
                           rdfs:label "issue" .


:ClearanceActionKind.release 
                             rdfs:comment "Release clearance." ;
                             rdfs:label "release" .


:ClearanceActionKind.update 
                            rdfs:comment "Update clearance." ;
                            rdfs:label "update" .


:CloudKind.altoCumulus 
                       rdfs:label "altoCumulus" .


:CloudKind.altoStratus 
                       rdfs:label "altoStratus" .


:CloudKind.cirroCumulus 
                        rdfs:label "cirroCumulus" .


:CloudKind.cirroStratus 
                        rdfs:label "cirroStratus" .


:CloudKind.cirrus 
                  rdfs:label "cirrus" .


:CloudKind.cumuloNimbus 
                        rdfs:label "cumuloNimbus" .


:CloudKind.cumulus 
                   rdfs:label "cumulus" .


:CloudKind.nimboStratus 
                        rdfs:label "nimboStratus" .


:CloudKind.other 
                 rdfs:label "other" .


:CloudKind.stratoCumulus 
                         rdfs:label "stratoCumulus" .


:CloudKind.stratus 
                   rdfs:label "stratus" .


:CloudKind.toweringCumulus 
                           rdfs:label "toweringCumulus" .


:ComDirectionKind.biDirectional 
                                rdfs:comment "Communication with the device is bi-directional." ;
                                rdfs:label "biDirectional" .


:ComDirectionKind.fromDevice 
                             rdfs:comment "Communication is from device." ;
                             rdfs:label "fromDevice" .


:ComDirectionKind.toDevice 
                           rdfs:comment "Communication is to device." ;
                           rdfs:label "toDevice" .


:ComTechnologyKind.cellular 
                            rdfs:comment "Communicates using a public cellular radio network. A specific variant of 'rf'." ;
                            rdfs:label "cellular" .


:ComTechnologyKind.ethernet 
                            rdfs:comment "Communicates using one or more of a family of frame-based computer networking technologies conforming to the IEEE 802.3 standard." ;
                            rdfs:label "ethernet" .


:ComTechnologyKind.homePlug 
                            rdfs:comment "Communicates using power line communication technologies conforming to the standards established by the HomePlug Powerline Alliance. A specific variant of 'plc'." ;
                            rdfs:label "homePlug" .


:ComTechnologyKind.pager 
                         rdfs:comment "Communicates using a public one-way or two-way radio-based paging network. A specific variant of 'rf'." ;
                         rdfs:label "pager" .


:ComTechnologyKind.phone 
                         rdfs:comment "Communicates using a basic, wireline telephone system." ;
                         rdfs:label "phone" .


:ComTechnologyKind.plc 
                       rdfs:comment "Communicates using power line communication technologies." ;
                       rdfs:label "plc" .


:ComTechnologyKind.rf 
                      rdfs:comment "Communicates using private or public radio-based technology." ;
                      rdfs:label "rf" .


:ComTechnologyKind.rfMesh 
                          rdfs:comment "Communicates using a mesh radio technology. A specific variant of 'rf'." ;
                          rdfs:label "rfMesh" .


:ComTechnologyKind.zigbee 
                          rdfs:comment "Communicates using radio communication technologies conforming to the standards established by the ZigBee. A specific variant of 'rf'." ;
                          rdfs:label "zigbee" .


:CommitmentType.ISO 
                    rdfs:label "ISO" .


:CommitmentType.SELF 
                     rdfs:label "SELF" .


:CommitmentType.UC 
                   rdfs:label "UC" .


:CommodityKind.air uml:hasInitialValue "4" ;
                   
                   rdfs:comment "Atmospheric air" ;
                   rdfs:label "air" .


:CommodityKind.carbon uml:hasInitialValue "19" ;
                      
                      rdfs:comment "The element has an atomic number of 6." ;
                      rdfs:label "carbon" .


:CommodityKind.ch4 uml:hasInitialValue "17" ;
                   
                   rdfs:comment "Methane CH4" ;
                   rdfs:label "ch4" .


:CommodityKind.co2 uml:hasInitialValue "18" ;
                   
                   rdfs:comment "Carbon Dioxide CO2" ;
                   rdfs:label "co2" .


:CommodityKind.communication uml:hasInitialValue "3" ;
                             
                             rdfs:comment "A measurement of the communication infrastructure itself." ;
                             rdfs:label "communication" .


:CommodityKind.coolingFluid uml:hasInitialValue "13" ;
                            
                            rdfs:comment "The cool fluid returns warmer than when it was sent. The heat conveyed may be metered." ;
                            rdfs:label "coolingFluid" .


:CommodityKind.electricityPrimaryMetered uml:hasInitialValue "2" ;
                                         
                                         rdfs:comment "It is possible for a meter to be outfitted with an external VT and/or CT. The meter might not be aware of these devices, and the display not compensate for their presence. Ultimately, when these scalars are applied, the value that represents the service value is called the “primary metered” value. The “index” in sub-category 3 mirrors those of sub-category 0." ;
                                         rdfs:label "electricityPrimaryMetered" .


:CommodityKind.electricitySecondaryMetered uml:hasInitialValue "1" ;
                                           
                                           rdfs:comment "All types of metered quantities. This type of reading comes from the meter and represents a “secondary” metered value." ;
                                           rdfs:label "electricitySecondaryMetered" .


:CommodityKind.hch uml:hasInitialValue "20" ;
                   
                   rdfs:comment "Hexachlorocyclohexane HCH" ;
                   rdfs:label "hch" .


:CommodityKind.heatingFluid uml:hasInitialValue "12" ;
                            
                            rdfs:comment "This fluid is likely in liquid form. It is not necessarily water or water based. The warm fluid returns cooler than when it was sent. The heat conveyed may be metered." ;
                            rdfs:label "heatingFluid" .


:CommodityKind.insulativeGas uml:hasInitialValue "5" ;
                             
                             rdfs:comment "(SF6 is found separately below.)" ;
                             rdfs:label "insulativeGas" .


:CommodityKind.insulativeOil uml:hasInitialValue "6" ;
                             
                             rdfs:comment "Oil that is used in transformers to provide insulation and heat conduction." ;
                             rdfs:label "insulativeOil" .


:CommodityKind.internet uml:hasInitialValue "24" ;
                        
                        rdfs:comment "Internet service" ;
                        rdfs:label "internet" .


:CommodityKind.naturalGas uml:hasInitialValue "7" ;
                          
                          rdfs:comment "A naturally occurring hydrocarbon  gas mixture." ;
                          rdfs:label "naturalGas" .


:CommodityKind.none uml:hasInitialValue "0" ;
                    
                    rdfs:comment "Not Applicable" ;
                    rdfs:label "none" .


:CommodityKind.nonpotableWater uml:hasInitialValue "14" ;
                               
                               rdfs:comment "Reclaimed water – possibly used for irrigation but not sufficiently treated to be considered safe for drinking." ;
                               rdfs:label "nonpotableWater" .


:CommodityKind.nox uml:hasInitialValue "15" ;
                   
                   rdfs:comment "Nitrous Oxides NOX" ;
                   rdfs:label "nox" .


:CommodityKind.pfc uml:hasInitialValue "21" ;
                   
                   rdfs:comment "Perfluorocarbons PFC" ;
                   rdfs:label "pfc" .


:CommodityKind.potableWater uml:hasInitialValue "9" ;
                            
                            rdfs:comment "Drinkable water" ;
                            rdfs:label "potableWater" .


:CommodityKind.propane uml:hasInitialValue "8" ;
                       
                       rdfs:comment "The formula is C3H8" ;
                       rdfs:label "propane" .


:CommodityKind.refuse uml:hasInitialValue "25" ;
                      
                      rdfs:comment "trash" ;
                      rdfs:label "refuse" .


:CommodityKind.sf6 uml:hasInitialValue "22" ;
                   
                   rdfs:comment "Sulfurhexafluoride SF6" ;
                   rdfs:label "sf6" .


:CommodityKind.so2 uml:hasInitialValue "16" ;
                   
                   rdfs:comment "Sulfur Dioxide SO2" ;
                   rdfs:label "so2" .


:CommodityKind.steam uml:hasInitialValue "10" ;
                     
                     rdfs:comment "Water in steam form, usually used for heating." ;
                     rdfs:label "steam" .


:CommodityKind.tvLicence uml:hasInitialValue "23" ;
                         
                         rdfs:comment "Television" ;
                         rdfs:label "tvLicence" .


:CommodityKind.wasteWater uml:hasInitialValue "11" ;
                          
                          rdfs:comment "(Sewerage)" ;
                          rdfs:label "wasteWater" .


:CompositeSwitchKind.escoThrowOver 
                                   rdfs:label "escoThrowOver" .


:CompositeSwitchKind.gral 
                          rdfs:label "gral" .


:CompositeSwitchKind.other 
                           rdfs:label "other" .


:CompositeSwitchKind.ral 
                         rdfs:label "ral" .


:CompositeSwitchKind.regulatorBypass 
                                     rdfs:label "regulatorBypass" .


:CompositeSwitchKind.throwOver 
                               rdfs:label "throwOver" .


:CompositeSwitchKind.ugMultiSwitch 
                                   rdfs:label "ugMultiSwitch" .


:ConditionFactorKind.accountAllocation 
                                       rdfs:label "accountAllocation" .


:ConditionFactorKind.labor 
                           rdfs:label "labor" .


:ConditionFactorKind.material 
                              rdfs:label "material" .


:ConditionFactorKind.other 
                           rdfs:label "other" .


:ConditionFactorKind.travel 
                            rdfs:label "travel" .


:ConstraintLimitType.MAXIMUM 
                             rdfs:label "MAXIMUM" .


:ConstraintLimitType.MINIMUM 
                             rdfs:label "MINIMUM" .


:ConstraintRampType.FAST 
                         rdfs:label "FAST" .


:ConstraintRampType.SLOW 
                         rdfs:label "SLOW" .


:ContingencyEquipmentStatusKind.inService 
                                          rdfs:comment "The equipment is to be put into service." ;
                                          rdfs:label "inService" .


:ContingencyEquipmentStatusKind.outOfService 
                                             rdfs:comment "The equipment is to be taken out of service." ;
                                             rdfs:label "outOfService" .


:ContractType.CVR 
                  rdfs:comment "CVR - Converted contract." ;
                  rdfs:label "CVR" .


:ContractType.ETC 
                  rdfs:comment "ETC - Existing Transmission Contract" ;
                  rdfs:label "ETC" .


:ContractType.O 
                rdfs:comment "O - Other" ;
                rdfs:label "O" .


:ContractType.RMR 
                  rdfs:comment "RMR - Reliability Must Run Contract" ;
                  rdfs:label "RMR" .


:ContractType.RMT 
                  rdfs:comment "RMT - RMT Contract" ;
                  rdfs:label "RMT" .


:ContractType.TE 
                 rdfs:comment "TE - Transmission Export" ;
                 rdfs:label "TE" .


:ContractType.TI 
                 rdfs:comment "TI - Transmission Import" ;
                 rdfs:label "TI" .


:ContractType.TOR 
                  rdfs:comment "TOR - Transmission Ownership Right" ;
                  rdfs:label "TOR" .


:ControlAreaTypeKind.AGC 
                         rdfs:comment "Used for automatic generation control." ;
                         rdfs:label "AGC" .


:ControlAreaTypeKind.Forecast 
                              rdfs:comment "Used for load forecast." ;
                              rdfs:label "Forecast" .


:ControlAreaTypeKind.Interchange 
                                 rdfs:comment "Used for interchange specification or control." ;
                                 rdfs:label "Interchange" .


:CoolantType.air 
                 rdfs:comment "Air." ;
                 rdfs:label "air" .


:CoolantType.hydrogenGas 
                         rdfs:comment "Hydrogen gas." ;
                         rdfs:label "hydrogenGas" .


:CoolantType.water 
                   rdfs:comment "Water." ;
                   rdfs:label "water" .


:CoolingKind.forcedAir 
                       rdfs:label "forcedAir" .


:CoolingKind.forcedOilAndAir 
                             rdfs:label "forcedOilAndAir" .


:CoolingKind.other 
                   rdfs:label "other" .


:CoolingKind.selfCooling 
                         rdfs:label "selfCooling" .


:CorporateStandardKind.experimental 
                                    rdfs:comment "Asset model is used experimentally." ;
                                    rdfs:label "experimental" .


:CorporateStandardKind.other 
                             rdfs:comment "Other kind of corporate standard for the asset model." ;
                             rdfs:label "other" .


:CorporateStandardKind.standard 
                                rdfs:comment "Asset model is used as corporate standard." ;
                                rdfs:label "standard" .


:CorporateStandardKind.underEvaluation 
                                       rdfs:comment "Asset model usage is under evaluation." ;
                                       rdfs:label "underEvaluation" .


:CostBasis.BIDC 
                rdfs:label "BIDC" .


:CostBasis.PRXC 
                rdfs:label "PRXC" .


:CostBasis.REGC 
                rdfs:label "REGC" .


:CoverageCodeKind.brief 
                        rdfs:label "brief" .


:CoverageCodeKind.frequent 
                           rdfs:label "frequent" .


:CoverageCodeKind.intermittant 
                               rdfs:label "intermittant" .


:CoverageCodeKind.isolated 
                           rdfs:label "isolated" .


:CoverageCodeKind.numerous 
                           rdfs:label "numerous" .


:CoverageCodeKind.occasional 
                             rdfs:label "occasional" .


:CoverageCodeKind.partly 
                         rdfs:label "partly" .


:CoverageCodeKind.patchy 
                         rdfs:label "patchy" .


:CoverageCodeKind.periodsOf 
                            rdfs:label "periodsOf" .


:CoverageCodeKind.scattered 
                            rdfs:label "scattered" .


:CoverageCodeKind.widespread 
                             rdfs:label "widespread" .


:CrewStatusKind.arrived 
                        rdfs:comment "the crew is on site at the outage location" ;
                        rdfs:label "arrived" .


:CrewStatusKind.assigned 
                         rdfs:comment "the crew has been assigned to work on a task" ;
                         rdfs:label "assigned" .


:CrewStatusKind.awaitingCrewAssignment 
                                       rdfs:comment "Indicates that the work is awaiting one or more crews to be assigned" ;
                                       rdfs:label "awaitingCrewAssignment" .


:CrewStatusKind.enroute 
                        rdfs:comment "the crew has been dispatched to work on an outage" ;
                        rdfs:label "enroute" .


:CrewStatusKind.fieldComplete 
                              rdfs:comment "the crew has corrected the outage in the field.  The equipment or other devices may not be energized at this time." ;
                              rdfs:label "fieldComplete" .


:CsOperatingModeKind.inverter 
                              rdfs:comment "Operating as inverter, which is the power receiving end." ;
                              rdfs:label "inverter" .


:CsOperatingModeKind.rectifier 
                               rdfs:comment "Operating as rectifier, which is the power sending end." ;
                               rdfs:label "rectifier" .


:CsPpccControlKind.activePower 
                               rdfs:comment "Control is active power control at AC side, at point of common coupling. Target is provided by ACDCConverter.targetPpcc." ;
                               rdfs:label "activePower" .


:CsPpccControlKind.dcCurrent 
                             rdfs:comment "Control is DC current  with target value provided by CsConverter.targetIdc." ;
                             rdfs:label "dcCurrent" .


:CsPpccControlKind.dcVoltage 
                             rdfs:comment "Control is DC voltage  with target value provided by ACDCConverter.targetUdc." ;
                             rdfs:label "dcVoltage" .


:Currency.AED uml:hasInitialValue "784" ;
              
              rdfs:comment "United Arab Emirates dirham." ;
              rdfs:label "AED" .


:Currency.AFN uml:hasInitialValue "971" ;
              
              rdfs:comment "Afghan afghani." ;
              rdfs:label "AFN" .


:Currency.ALL uml:hasInitialValue "008" ;
              
              rdfs:comment "Albanian lek." ;
              rdfs:label "ALL" .


:Currency.AMD uml:hasInitialValue "051" ;
              
              rdfs:comment "Armenian dram." ;
              rdfs:label "AMD" .


:Currency.ANG uml:hasInitialValue "532" ;
              
              rdfs:comment "Netherlands Antillean guilder." ;
              rdfs:label "ANG" .


:Currency.AOA uml:hasInitialValue "973" ;
              
              rdfs:comment "Angolan kwanza." ;
              rdfs:label "AOA" .


:Currency.ARS uml:hasInitialValue "032" ;
              
              rdfs:comment "Argentine peso." ;
              rdfs:label "ARS" .


:Currency.AUD uml:hasInitialValue "036" ;
              
              rdfs:comment "Australian dollar." ;
              rdfs:label "AUD" .


:Currency.AWG uml:hasInitialValue "533" ;
              
              rdfs:comment "Aruban florin." ;
              rdfs:label "AWG" .


:Currency.AZN uml:hasInitialValue "944" ;
              
              rdfs:comment "Azerbaijani manat." ;
              rdfs:label "AZN" .


:Currency.BAM uml:hasInitialValue "977" ;
              
              rdfs:comment "Bosnia and Herzegovina convertible mark." ;
              rdfs:label "BAM" .


:Currency.BBD uml:hasInitialValue "052" ;
              
              rdfs:comment "Barbados dollar." ;
              rdfs:label "BBD" .


:Currency.BDT uml:hasInitialValue "050" ;
              
              rdfs:comment "Bangladeshi taka." ;
              rdfs:label "BDT" .


:Currency.BGN uml:hasInitialValue "975" ;
              
              rdfs:comment "Bulgarian lev." ;
              rdfs:label "BGN" .


:Currency.BHD uml:hasInitialValue "048" ;
              
              rdfs:comment "Bahraini dinar." ;
              rdfs:label "BHD" .


:Currency.BIF uml:hasInitialValue "108" ;
              
              rdfs:comment "Burundian franc." ;
              rdfs:label "BIF" .


:Currency.BMD uml:hasInitialValue "060" ;
              
              rdfs:comment "Bermudian dollar (customarily known as Bermuda dollar)." ;
              rdfs:label "BMD" .


:Currency.BND uml:hasInitialValue "096" ;
              
              rdfs:comment "Brunei dollar." ;
              rdfs:label "BND" .


:Currency.BOB uml:hasInitialValue "068" ;
              
              rdfs:comment "Boliviano." ;
              rdfs:label "BOB" .


:Currency.BOV uml:hasInitialValue "984" ;
              
              rdfs:comment "Bolivian Mvdol (funds code)." ;
              rdfs:label "BOV" .


:Currency.BRL uml:hasInitialValue "986" ;
              
              rdfs:comment "Brazilian real." ;
              rdfs:label "BRL" .


:Currency.BSD uml:hasInitialValue "044" ;
              
              rdfs:comment "Bahamian dollar." ;
              rdfs:label "BSD" .


:Currency.BTN uml:hasInitialValue "064" ;
              
              rdfs:comment "Bhutanese ngultrum." ;
              rdfs:label "BTN" .


:Currency.BWP uml:hasInitialValue "072" ;
              
              rdfs:comment "Botswana pula." ;
              rdfs:label "BWP" .


:Currency.BYR uml:hasInitialValue "974" ;
              
              rdfs:comment "Belarusian ruble." ;
              rdfs:label "BYR" .


:Currency.BZD uml:hasInitialValue "084" ;
              
              rdfs:comment "Belize dollar." ;
              rdfs:label "BZD" .


:Currency.CAD uml:hasInitialValue "124" ;
              
              rdfs:comment "Canadian dollar." ;
              rdfs:label "CAD" .


:Currency.CDF uml:hasInitialValue "976" ;
              
              rdfs:comment "Congolese franc." ;
              rdfs:label "CDF" .


:Currency.CHF uml:hasInitialValue "756" ;
              
              rdfs:comment "Swiss franc." ;
              rdfs:label "CHF" .


:Currency.CLF uml:hasInitialValue "990" ;
              
              rdfs:comment "Unidad de Fomento (funds code), Chile." ;
              rdfs:label "CLF" .


:Currency.CLP uml:hasInitialValue "152" ;
              
              rdfs:comment "Chilean peso." ;
              rdfs:label "CLP" .


:Currency.CNY uml:hasInitialValue "156" ;
              
              rdfs:comment "Chinese yuan." ;
              rdfs:label "CNY" .


:Currency.COP uml:hasInitialValue "170" ;
              
              rdfs:comment "Colombian peso." ;
              rdfs:label "COP" .


:Currency.COU uml:hasInitialValue "970" ;
              
              rdfs:comment "Unidad de Valor Real." ;
              rdfs:label "COU" .


:Currency.CRC uml:hasInitialValue "188" ;
              
              rdfs:comment "Costa Rican colon." ;
              rdfs:label "CRC" .


:Currency.CUC uml:hasInitialValue "931" ;
              
              rdfs:comment "Cuban convertible peso." ;
              rdfs:label "CUC" .


:Currency.CUP uml:hasInitialValue "192" ;
              
              rdfs:comment "Cuban peso." ;
              rdfs:label "CUP" .


:Currency.CVE uml:hasInitialValue "132" ;
              
              rdfs:comment "Cape Verde escudo." ;
              rdfs:label "CVE" .


:Currency.CZK uml:hasInitialValue "203" ;
              
              rdfs:comment "Czech koruna." ;
              rdfs:label "CZK" .


:Currency.DJF uml:hasInitialValue "262" ;
              
              rdfs:comment "Djiboutian franc." ;
              rdfs:label "DJF" .


:Currency.DKK uml:hasInitialValue "208" ;
              
              rdfs:comment "Danish krone." ;
              rdfs:label "DKK" .


:Currency.DOP uml:hasInitialValue "214" ;
              
              rdfs:comment "Dominican peso." ;
              rdfs:label "DOP" .


:Currency.DZD uml:hasInitialValue "012" ;
              
              rdfs:comment "Algerian dinar." ;
              rdfs:label "DZD" .


:Currency.EEK uml:hasInitialValue "233" ;
              
              rdfs:comment "Estonian kroon." ;
              rdfs:label "EEK" .


:Currency.EGP uml:hasInitialValue "818" ;
              
              rdfs:comment "Egyptian pound." ;
              rdfs:label "EGP" .


:Currency.ERN uml:hasInitialValue "232" ;
              
              rdfs:comment "Eritrean nakfa." ;
              rdfs:label "ERN" .


:Currency.ETB uml:hasInitialValue "230" ;
              
              rdfs:comment "Ethiopian birr." ;
              rdfs:label "ETB" .


:Currency.EUR uml:hasInitialValue "978" ;
              
              rdfs:comment "Euro." ;
              rdfs:label "EUR" .


:Currency.FJD uml:hasInitialValue "242" ;
              
              rdfs:comment "Fiji dollar." ;
              rdfs:label "FJD" .


:Currency.FKP uml:hasInitialValue "238" ;
              
              rdfs:comment "Falkland Islands pound." ;
              rdfs:label "FKP" .


:Currency.GBP uml:hasInitialValue "826" ;
              
              rdfs:comment "Pound sterling." ;
              rdfs:label "GBP" .


:Currency.GEL uml:hasInitialValue "981" ;
              
              rdfs:comment "Georgian lari." ;
              rdfs:label "GEL" .


:Currency.GHS uml:hasInitialValue "936" ;
              
              rdfs:comment "Ghanaian cedi." ;
              rdfs:label "GHS" .


:Currency.GIP uml:hasInitialValue "929" ;
              
              rdfs:comment "Gibraltar pound." ;
              rdfs:label "GIP" .


:Currency.GMD uml:hasInitialValue "270" ;
              
              rdfs:comment "Gambian dalasi." ;
              rdfs:label "GMD" .


:Currency.GNF uml:hasInitialValue "324" ;
              
              rdfs:comment "Guinean franc." ;
              rdfs:label "GNF" .


:Currency.GTQ uml:hasInitialValue "320" ;
              
              rdfs:comment "Guatemalan quetzal." ;
              rdfs:label "GTQ" .


:Currency.GYD uml:hasInitialValue "328" ;
              
              rdfs:comment "Guyanese dollar." ;
              rdfs:label "GYD" .


:Currency.HKD uml:hasInitialValue "344" ;
              
              rdfs:comment "Hong Kong dollar." ;
              rdfs:label "HKD" .


:Currency.HNL uml:hasInitialValue "340" ;
              
              rdfs:comment "Honduran lempira." ;
              rdfs:label "HNL" .


:Currency.HRK uml:hasInitialValue "191" ;
              
              rdfs:comment "Croatian kuna." ;
              rdfs:label "HRK" .


:Currency.HTG uml:hasInitialValue "332" ;
              
              rdfs:comment "Haitian gourde." ;
              rdfs:label "HTG" .


:Currency.HUF uml:hasInitialValue "348" ;
              
              rdfs:comment "Hungarian forint." ;
              rdfs:label "HUF" .


:Currency.IDR uml:hasInitialValue "360" ;
              
              rdfs:comment "Indonesian rupiah." ;
              rdfs:label "IDR" .


:Currency.ILS uml:hasInitialValue "376" ;
              
              rdfs:comment "Israeli new sheqel." ;
              rdfs:label "ILS" .


:Currency.INR uml:hasInitialValue "356" ;
              
              rdfs:comment "Indian rupee." ;
              rdfs:label "INR" .


:Currency.IQD uml:hasInitialValue "368" ;
              
              rdfs:comment "Iraqi dinar." ;
              rdfs:label "IQD" .


:Currency.IRR uml:hasInitialValue "364" ;
              
              rdfs:comment "Iranian rial." ;
              rdfs:label "IRR" .


:Currency.ISK uml:hasInitialValue "352" ;
              
              rdfs:comment "Icelandic króna." ;
              rdfs:label "ISK" .


:Currency.JMD uml:hasInitialValue "388" ;
              
              rdfs:comment "Jamaican dollar." ;
              rdfs:label "JMD" .


:Currency.JOD uml:hasInitialValue "400" ;
              
              rdfs:comment "Jordanian dinar." ;
              rdfs:label "JOD" .


:Currency.JPY uml:hasInitialValue "392" ;
              
              rdfs:comment "Japanese yen." ;
              rdfs:label "JPY" .


:Currency.KES uml:hasInitialValue "404" ;
              
              rdfs:comment "Kenyan shilling." ;
              rdfs:label "KES" .


:Currency.KGS uml:hasInitialValue "417" ;
              
              rdfs:comment "Kyrgyzstani som." ;
              rdfs:label "KGS" .


:Currency.KHR uml:hasInitialValue "116" ;
              
              rdfs:comment "Cambodian riel." ;
              rdfs:label "KHR" .


:Currency.KMF uml:hasInitialValue "174" ;
              
              rdfs:comment "Comoro franc." ;
              rdfs:label "KMF" .


:Currency.KPW uml:hasInitialValue "408" ;
              
              rdfs:comment "North Korean won." ;
              rdfs:label "KPW" .


:Currency.KRW uml:hasInitialValue "410" ;
              
              rdfs:comment "South Korean won." ;
              rdfs:label "KRW" .


:Currency.KWD uml:hasInitialValue "414" ;
              
              rdfs:comment "Kuwaiti dinar." ;
              rdfs:label "KWD" .


:Currency.KYD uml:hasInitialValue "136" ;
              
              rdfs:comment "Cayman Islands dollar." ;
              rdfs:label "KYD" .


:Currency.KZT uml:hasInitialValue "398" ;
              
              rdfs:comment "Kazakhstani tenge." ;
              rdfs:label "KZT" .


:Currency.LAK uml:hasInitialValue "418" ;
              
              rdfs:comment "Lao kip." ;
              rdfs:label "LAK" .


:Currency.LBP uml:hasInitialValue "422" ;
              
              rdfs:comment "Lebanese pound." ;
              rdfs:label "LBP" .


:Currency.LKR uml:hasInitialValue "144" ;
              
              rdfs:comment "Sri Lanka rupee." ;
              rdfs:label "LKR" .


:Currency.LRD uml:hasInitialValue "430" ;
              
              rdfs:comment "Liberian dollar." ;
              rdfs:label "LRD" .


:Currency.LSL uml:hasInitialValue "426" ;
              
              rdfs:comment "Lesotho loti." ;
              rdfs:label "LSL" .


:Currency.LTL uml:hasInitialValue "440" ;
              
              rdfs:comment "Lithuanian litas." ;
              rdfs:label "LTL" .


:Currency.LVL uml:hasInitialValue "428" ;
              
              rdfs:comment "Latvian lats." ;
              rdfs:label "LVL" .


:Currency.LYD uml:hasInitialValue "434" ;
              
              rdfs:comment "Libyan dinar." ;
              rdfs:label "LYD" .


:Currency.MAD uml:hasInitialValue "504" ;
              
              rdfs:comment "Moroccan dirham." ;
              rdfs:label "MAD" .


:Currency.MDL uml:hasInitialValue "498" ;
              
              rdfs:comment "Moldovan leu." ;
              rdfs:label "MDL" .


:Currency.MGA uml:hasInitialValue "969" ;
              
              rdfs:comment "Malagasy ariary." ;
              rdfs:label "MGA" .


:Currency.MKD uml:hasInitialValue "807" ;
              
              rdfs:comment "Macedonian denar." ;
              rdfs:label "MKD" .


:Currency.MMK uml:hasInitialValue "104" ;
              
              rdfs:comment "Myanma kyat." ;
              rdfs:label "MMK" .


:Currency.MNT uml:hasInitialValue "496" ;
              
              rdfs:comment "Mongolian tugrik." ;
              rdfs:label "MNT" .


:Currency.MOP uml:hasInitialValue "446" ;
              
              rdfs:comment "Macanese pataca." ;
              rdfs:label "MOP" .


:Currency.MRO uml:hasInitialValue "478" ;
              
              rdfs:comment "Mauritanian ouguiya." ;
              rdfs:label "MRO" .


:Currency.MUR uml:hasInitialValue "480" ;
              
              rdfs:comment "Mauritian rupee." ;
              rdfs:label "MUR" .


:Currency.MVR uml:hasInitialValue "462" ;
              
              rdfs:comment "Maldivian rufiyaa." ;
              rdfs:label "MVR" .


:Currency.MWK uml:hasInitialValue "454" ;
              
              rdfs:comment "Malawian kwacha." ;
              rdfs:label "MWK" .


:Currency.MXN uml:hasInitialValue "484" ;
              
              rdfs:comment "Mexican peso." ;
              rdfs:label "MXN" .


:Currency.MYR uml:hasInitialValue "458" ;
              
              rdfs:comment "Malaysian ringgit." ;
              rdfs:label "MYR" .


:Currency.MZN uml:hasInitialValue "943" ;
              
              rdfs:comment "Mozambican metical." ;
              rdfs:label "MZN" .


:Currency.NAD uml:hasInitialValue "516" ;
              
              rdfs:comment "Namibian dollar." ;
              rdfs:label "NAD" .


:Currency.NGN uml:hasInitialValue "566" ;
              
              rdfs:comment "Nigerian naira." ;
              rdfs:label "NGN" .


:Currency.NIO uml:hasInitialValue "558" ;
              
              rdfs:comment "Cordoba oro." ;
              rdfs:label "NIO" .


:Currency.NOK uml:hasInitialValue "578" ;
              
              rdfs:comment "Norwegian krone." ;
              rdfs:label "NOK" .


:Currency.NPR uml:hasInitialValue "524" ;
              
              rdfs:comment "Nepalese rupee." ;
              rdfs:label "NPR" .


:Currency.NZD uml:hasInitialValue "554" ;
              
              rdfs:comment "New Zealand dollar." ;
              rdfs:label "NZD" .


:Currency.OMR uml:hasInitialValue "512" ;
              
              rdfs:comment "Omani rial." ;
              rdfs:label "OMR" .


:Currency.PAB uml:hasInitialValue "590" ;
              
              rdfs:comment "Panamanian balboa." ;
              rdfs:label "PAB" .


:Currency.PEN uml:hasInitialValue "604" ;
              
              rdfs:comment "Peruvian nuevo sol." ;
              rdfs:label "PEN" .


:Currency.PGK uml:hasInitialValue "598" ;
              
              rdfs:comment "Papua New Guinean kina." ;
              rdfs:label "PGK" .


:Currency.PHP uml:hasInitialValue "608" ;
              
              rdfs:comment "Philippine peso." ;
              rdfs:label "PHP" .


:Currency.PKR uml:hasInitialValue "586" ;
              
              rdfs:comment "Pakistani rupee." ;
              rdfs:label "PKR" .


:Currency.PLN uml:hasInitialValue "985" ;
              
              rdfs:comment "Polish zloty." ;
              rdfs:label "PLN" .


:Currency.PYG uml:hasInitialValue "600" ;
              
              rdfs:comment "Paraguayan guaraní." ;
              rdfs:label "PYG" .


:Currency.QAR uml:hasInitialValue "634" ;
              
              rdfs:comment "Qatari rial." ;
              rdfs:label "QAR" .


:Currency.RON uml:hasInitialValue "946" ;
              
              rdfs:comment "Romanian new leu." ;
              rdfs:label "RON" .


:Currency.RSD uml:hasInitialValue "941" ;
              
              rdfs:comment "Serbian dinar." ;
              rdfs:label "RSD" .


:Currency.RUB uml:hasInitialValue "643" ;
              
              rdfs:comment "Russian rouble." ;
              rdfs:label "RUB" .


:Currency.RWF uml:hasInitialValue "646" ;
              
              rdfs:comment "Rwandan franc." ;
              rdfs:label "RWF" .


:Currency.SAR uml:hasInitialValue "682" ;
              
              rdfs:comment "Saudi riyal." ;
              rdfs:label "SAR" .


:Currency.SBD uml:hasInitialValue "090" ;
              
              rdfs:comment "Solomon Islands dollar." ;
              rdfs:label "SBD" .


:Currency.SCR uml:hasInitialValue "690" ;
              
              rdfs:comment "Seychelles rupee." ;
              rdfs:label "SCR" .


:Currency.SDG uml:hasInitialValue "938" ;
              
              rdfs:comment "Sudanese pound." ;
              rdfs:label "SDG" .


:Currency.SEK uml:hasInitialValue "752" ;
              
              rdfs:comment "Swedish krona/kronor." ;
              rdfs:label "SEK" .


:Currency.SGD uml:hasInitialValue "702" ;
              
              rdfs:comment "Singapore dollar." ;
              rdfs:label "SGD" .


:Currency.SHP uml:hasInitialValue "654" ;
              
              rdfs:comment "Saint Helena pound." ;
              rdfs:label "SHP" .


:Currency.SLL uml:hasInitialValue "694" ;
              
              rdfs:comment "Sierra Leonean leone." ;
              rdfs:label "SLL" .


:Currency.SOS uml:hasInitialValue "706" ;
              
              rdfs:comment "Somali shilling." ;
              rdfs:label "SOS" .


:Currency.SRD uml:hasInitialValue "968" ;
              
              rdfs:comment "Surinamese dollar." ;
              rdfs:label "SRD" .


:Currency.STD uml:hasInitialValue "678" ;
              
              rdfs:comment "São Tomé and Príncipe dobra." ;
              rdfs:label "STD" .


:Currency.SYP uml:hasInitialValue "760" ;
              
              rdfs:comment "Syrian pound." ;
              rdfs:label "SYP" .


:Currency.SZL uml:hasInitialValue "748" ;
              
              rdfs:comment "Lilangeni." ;
              rdfs:label "SZL" .


:Currency.THB uml:hasInitialValue "764" ;
              
              rdfs:comment "Thai baht." ;
              rdfs:label "THB" .


:Currency.TJS uml:hasInitialValue "972" ;
              
              rdfs:comment "Tajikistani somoni." ;
              rdfs:label "TJS" .


:Currency.TMT uml:hasInitialValue "934" ;
              
              rdfs:comment "Turkmenistani manat." ;
              rdfs:label "TMT" .


:Currency.TND uml:hasInitialValue "788" ;
              
              rdfs:comment "Tunisian dinar." ;
              rdfs:label "TND" .


:Currency.TOP uml:hasInitialValue "776" ;
              
              rdfs:comment "Tongan pa'anga." ;
              rdfs:label "TOP" .


:Currency.TRY uml:hasInitialValue "949" ;
              
              rdfs:comment "Turkish lira." ;
              rdfs:label "TRY" .


:Currency.TTD uml:hasInitialValue "780" ;
              
              rdfs:comment "Trinidad and Tobago dollar." ;
              rdfs:label "TTD" .


:Currency.TWD uml:hasInitialValue "901" ;
              
              rdfs:comment "New Taiwan dollar." ;
              rdfs:label "TWD" .


:Currency.TZS uml:hasInitialValue "834" ;
              
              rdfs:comment "Tanzanian shilling." ;
              rdfs:label "TZS" .


:Currency.UAH uml:hasInitialValue "980" ;
              
              rdfs:comment "Ukrainian hryvnia." ;
              rdfs:label "UAH" .


:Currency.UGX uml:hasInitialValue "800" ;
              
              rdfs:comment "Ugandan shilling." ;
              rdfs:label "UGX" .


:Currency.USD uml:hasInitialValue "840" ;
              
              rdfs:comment "United States dollar." ;
              rdfs:label "USD" .


:Currency.UYU uml:hasInitialValue "858" ;
              
              rdfs:comment "Uruguayan peso." ;
              rdfs:label "UYU" .


:Currency.UZS uml:hasInitialValue "860" ;
              
              rdfs:comment "Uzbekistan som." ;
              rdfs:label "UZS" .


:Currency.VEF uml:hasInitialValue "937" ;
              
              rdfs:comment "Venezuelan bolívar fuerte." ;
              rdfs:label "VEF" .


:Currency.VND uml:hasInitialValue "704" ;
              
              rdfs:comment "Vietnamese Dong." ;
              rdfs:label "VND" .


:Currency.VUV uml:hasInitialValue "548" ;
              
              rdfs:comment "Vanuatu vatu." ;
              rdfs:label "VUV" .


:Currency.WST uml:hasInitialValue "882" ;
              
              rdfs:comment "Samoan tala." ;
              rdfs:label "WST" .


:Currency.XAF uml:hasInitialValue "950" ;
              
              rdfs:comment "CFA franc BEAC." ;
              rdfs:label "XAF" .


:Currency.XCD uml:hasInitialValue "951" ;
              
              rdfs:comment "East Caribbean dollar." ;
              rdfs:label "XCD" .


:Currency.XOF uml:hasInitialValue "952" ;
              
              rdfs:comment "CFA Franc BCEAO." ;
              rdfs:label "XOF" .


:Currency.XPF uml:hasInitialValue "953" ;
              
              rdfs:comment "CFP franc." ;
              rdfs:label "XPF" .


:Currency.YER uml:hasInitialValue "886" ;
              
              rdfs:comment "Yemeni rial." ;
              rdfs:label "YER" .


:Currency.ZAR uml:hasInitialValue "710" ;
              
              rdfs:comment "South African rand." ;
              rdfs:label "ZAR" .


:Currency.ZMK uml:hasInitialValue "894" ;
              
              rdfs:comment "Zambian kwacha." ;
              rdfs:label "ZMK" .


:Currency.ZWL uml:hasInitialValue "932" ;
              
              rdfs:comment "Zimbabwe dollar." ;
              rdfs:label "ZWL" .


:CurrentStatusSC.ACTIVE 
                        rdfs:label "ACTIVE" .


:CurrentStatusSC.INACTIVE 
                          rdfs:label "INACTIVE" .


:CurveStyle.constantYValue 
                           rdfs:comment "The Y-axis values are assumed constant until the next curve point and prior to the first curve point." ;
                           rdfs:label "constantYValue" .


:CurveStyle.straightLineYValues 
                                rdfs:comment "The Y-axis values are assumed to be a straight line between values.  Also known as linear interpolation." ;
                                rdfs:label "straightLineYValues" .


:CustomerBillingKind.consolidatedEss 
                                     rdfs:comment "Consolidated bill from energy service supplier (ESS)." ;
                                     rdfs:label "consolidatedEss" .


:CustomerBillingKind.consolidatedUdc 
                                     rdfs:comment "Consolidated bill from utility distribution company (UDC)." ;
                                     rdfs:label "consolidatedUdc" .


:CustomerBillingKind.other 
                           rdfs:label "other" .


:CustomerBillingKind.separateEssUdc 
                                    rdfs:comment "Separate bills from ESS and UDC." ;
                                    rdfs:label "separateEssUdc" .


:CustomerKind.commercialIndustrial 
                                   rdfs:comment "Commercial industrial customer." ;
                                   rdfs:label "commercialIndustrial" .


:CustomerKind.energyServiceScheduler 
                                     rdfs:comment "Customer as energy service scheduler." ;
                                     rdfs:label "energyServiceScheduler" .


:CustomerKind.energyServiceSupplier 
                                    rdfs:comment "Customer as energy service supplier." ;
                                    rdfs:label "energyServiceSupplier" .


:CustomerKind.enterprise 
                         rdfs:comment "Enterprise customer" ;
                         rdfs:label "enterprise" .


:CustomerKind.internalUse 
                          rdfs:comment "Internal use customer." ;
                          rdfs:label "internalUse" .


:CustomerKind.other 
                    rdfs:comment "Other kind of customer." ;
                    rdfs:label "other" .


:CustomerKind.pumpingLoad 
                          rdfs:comment "Pumping load customer." ;
                          rdfs:label "pumpingLoad" .


:CustomerKind.regionalOperator 
                               rdfs:comment "Regional Operator customer" ;
                               rdfs:label "regionalOperator" .


:CustomerKind.residential 
                          rdfs:comment "Residential customer." ;
                          rdfs:label "residential" .


:CustomerKind.residentialAndCommercial 
                                       rdfs:comment "Residential and commercial customer." ;
                                       rdfs:label "residentialAndCommercial" .


:CustomerKind.residentialAndStreetlight 
                                        rdfs:comment "Residential and streetlight customer." ;
                                        rdfs:label "residentialAndStreetlight" .


:CustomerKind.residentialFarmService 
                                     rdfs:comment "Residential farm service customer." ;
                                     rdfs:label "residentialFarmService" .


:CustomerKind.residentialStreetlightOthers 
                                           rdfs:comment "Residential streetlight or other related customer." ;
                                           rdfs:label "residentialStreetlightOthers" .


:CustomerKind.subsidiary 
                         rdfs:comment "Subsidiary customer" ;
                         rdfs:label "subsidiary" .


:CustomerKind.windMachine 
                          rdfs:comment "Wind machine customer." ;
                          rdfs:label "windMachine" .


:DAMMarketType.DAM 
                   rdfs:label "DAM" .


:DCConverterOperatingModeKind.bipolar 
                                      rdfs:comment "Bipolar operation." ;
                                      rdfs:label "bipolar" .


:DCConverterOperatingModeKind.monopolarGroundReturn 
                                                    rdfs:comment "Monopolar operation with ground return." ;
                                                    rdfs:label "monopolarGroundReturn" .


:DCConverterOperatingModeKind.monopolarMetallicReturn 
                                                      rdfs:comment "Monopolar operation with metallic return." ;
                                                      rdfs:label "monopolarMetallicReturn" .


:DCPolarityKind.middle 
                       rdfs:comment "Middle pole. The converter terminal is the midpoint in a bipolar or symmetric monopole configuration. The midpoint can be grounded and/or have a metallic return." ;
                       rdfs:label "middle" .


:DCPolarityKind.negative 
                         rdfs:comment "Negative pole. The converter terminal is intended to operate at a negative voltage relative the midpoint or positive terminal." ;
                         rdfs:label "negative" .


:DCPolarityKind.positive 
                         rdfs:comment "Positive pole. The converter terminal is intended to operate at a positive voltage relative the midpoint or negative terminal." ;
                         rdfs:label "positive" .


:DERParameterKind.activePower uml:hasInitialValue "2" ;
                              
                              rdfs:comment "The amount of power being used, measured in Watts." ;
                              rdfs:label "activePower" .


:DERParameterKind.apparentPower uml:hasInitialValue "1" ;
                                
                                rdfs:comment "The combination of reactive power and active power, and is the product of voltage and current without reference to the phase angle." ;
                                rdfs:label "apparentPower" .


:DERParameterKind.decreasingRampRate uml:hasInitialValue "11" ;
                                     
                                     rdfs:comment "An indication of whether the ramp rate associated with a curve is negative." ;
                                     rdfs:label "decreasingRampRate" .


:DERParameterKind.highFilterBiDirectionalRegulation uml:hasInitialValue "4" ;
                                                    
                                                    rdfs:comment "AC voltage regulation of high frequency" ;
                                                    rdfs:label "highFilterBiDirectionalRegulation" .


:DERParameterKind.highFilterDownRegulation uml:hasInitialValue "8" ;
                                           
                                           rdfs:comment "High Pass Frequency Regulation downwards." ;
                                           rdfs:label "highFilterDownRegulation" .


:DERParameterKind.highFilterUpRegulation uml:hasInitialValue "6" ;
                                         
                                         rdfs:comment "High Pass Frequency Regulation upwards." ;
                                         rdfs:label "highFilterUpRegulation" .


:DERParameterKind.increasingRampRate uml:hasInitialValue "10" ;
                                     
                                     rdfs:comment "An indication of whether the ramp rate associated with a curve is positive." ;
                                     rdfs:label "increasingRampRate" .


:DERParameterKind.lowFilterBiDirectionalRegulation uml:hasInitialValue "5" ;
                                                   
                                                   rdfs:comment "Used to filter out the sinosuidal disturbances to the grid." ;
                                                   rdfs:label "lowFilterBiDirectionalRegulation" .


:DERParameterKind.lowFilterDownRegulation uml:hasInitialValue "9" ;
                                          
                                          rdfs:comment "Low Pass Frequency Regulation downwards." ;
                                          rdfs:label "lowFilterDownRegulation" .


:DERParameterKind.lowFilterUpRegulation uml:hasInitialValue "7" ;
                                        
                                        rdfs:comment "Low Pass Frequency Regulation upwards." ;
                                        rdfs:label "lowFilterUpRegulation" .


:DERParameterKind.reactivePower uml:hasInitialValue "3" ;
                                
                                rdfs:comment "The measure of reactance, measured in Vars." ;
                                rdfs:label "reactivePower" .


:DERParameterKind.voltage uml:hasInitialValue "12" ;
                          
                          rdfs:comment "The measure of difference in potential between two points, measured in Volts." ;
                          rdfs:label "voltage" .


:DERUnitSymbol.A uml:hasInitialValue "5" ;
                 
                 rdfs:comment "Current in Ampere." ;
                 rdfs:label "A" .


:DERUnitSymbol.Ah uml:hasInitialValue "106" ;
                  
                  rdfs:comment "Ampere-hours, Ampere-hours." ;
                  rdfs:label "Ah" .


:DERUnitSymbol.As uml:hasInitialValue "68" ;
                  
                  rdfs:comment "Ampere seconds (A·s)." ;
                  rdfs:label "As" .


:DERUnitSymbol.Btu uml:hasInitialValue "132" ;
                   
                   rdfs:comment "Energy, British Thermal Unit." ;
                   rdfs:label "Btu" .


:DERUnitSymbol.Hz uml:hasInitialValue "33" ;
                  
                  rdfs:comment "Frequency in Hertz (1/s)." ;
                  rdfs:label "Hz" .


:DERUnitSymbol.Q uml:hasInitialValue "100" ;
                 
                 rdfs:comment "Quantity power, Q." ;
                 rdfs:label "Q" .


:DERUnitSymbol.Qh uml:hasInitialValue "101" ;
                  
                  rdfs:comment "Quantity energy, Qh." ;
                  rdfs:label "Qh" .


:DERUnitSymbol.V uml:hasInitialValue "29" ;
                 
                 rdfs:comment "Electric potential in Volt (W/A)." ;
                 rdfs:label "V" .


:DERUnitSymbol.VA uml:hasInitialValue "61" ;
                  
                  rdfs:comment "Apparent power in Volt Ampere (See also real power and reactive power.)" ;
                  rdfs:label "VA" .


:DERUnitSymbol.VAh uml:hasInitialValue "71" ;
                   
                   rdfs:comment "Apparent energy in Volt Ampere hours." ;
                   rdfs:label "VAh" .


:DERUnitSymbol.VAr uml:hasInitialValue "63" ;
                   
                   rdfs:comment """Reactive power in Volt Ampere reactive. The “reactive” or “imaginary” component of electrical power (VIsin(phi)). (See also real power and apparent power).
Note: Different meter designs use different methods to arrive at their results. Some meters may compute reactive power as an arithmetic value, while others compute the value vectorially. The data consumer should determine the method in use and the suitability of the measurement for the intended purpose.""" ;
                   rdfs:label "VAr" .


:DERUnitSymbol.VArh uml:hasInitialValue "73" ;
                    
                    rdfs:comment "Reactive energy in Volt Ampere reactive hours." ;
                    rdfs:label "VArh" .


:DERUnitSymbol.VPerVA uml:hasInitialValue "153" ;
                      
                      rdfs:comment "Power factor, PF, the ratio of the active power to the apparent power. Note: The sign convention used for power factor will differ between IEC meters and EEI (ANSI) meters. It is assumed that the data consumers understand the type of meter being used and agree on the sign convention in use at any given utility." ;
                      rdfs:label "VPerVA" .


:DERUnitSymbol.VPerVAr 
                       rdfs:comment "Power factor, PF, the ratio of the active power to the apparent power. Note: The sign convention used for power factor will differ between IEC meters and EEI (ANSI) meters. It is assumed that the data consumers understand the type of meter being used and agree on the sign convention in use at any given utility." ;
                       rdfs:label "VPerVAr" .


:DERUnitSymbol.Vh uml:hasInitialValue "280" ;
                  
                  rdfs:comment "Volt-hour, Volt hours." ;
                  rdfs:label "Vh" .


:DERUnitSymbol.Vs uml:hasInitialValue "66" ;
                  
                  rdfs:comment "Volt second (Ws/A)." ;
                  rdfs:label "Vs" .


:DERUnitSymbol.W uml:hasInitialValue "38" ;
                 
                 rdfs:comment "Real power in Watt (J/s). Electrical power may have real and reactive components. The real portion of electrical power (I²R or VIcos(phi)), is expressed in Watts. (See also apparent power and reactive power.)" ;
                 rdfs:label "W" .


:DERUnitSymbol.WPerA 
                     rdfs:comment "Active power per current flow, watt per Ampere." ;
                     rdfs:label "WPerA" .


:DERUnitSymbol.WPers uml:hasInitialValue "81" ;
                     
                     rdfs:comment "Ramp rate in Watt per second." ;
                     rdfs:label "WPers" .


:DERUnitSymbol.Wh uml:hasInitialValue "72" ;
                  
                  rdfs:comment "Real energy in Watt hours." ;
                  rdfs:label "Wh" .


:DERUnitSymbol.deg uml:hasInitialValue "9" ;
                   
                   rdfs:comment "Plane angle in degrees." ;
                   rdfs:label "deg" .


:DERUnitSymbol.degC uml:hasInitialValue "23" ;
                    
                    rdfs:comment """Relative temperature in degrees Celsius.
In the SI unit system the symbol is ºC. Electric charge is measured in coulomb that has the unit symbol C. To distinguish degree Celsius form coulomb the symbol used in the UML is degC. Reason for not using ºC is the special character º is difficult to manage in software.""" ;
                    rdfs:label "degC" .


:DERUnitSymbol.h uml:hasInitialValue "84" ;
                 
                 rdfs:comment "Time, hour = 60 min = 3600 s." ;
                 rdfs:label "h" .


:DERUnitSymbol.min uml:hasInitialValue "85" ;
                   
                   rdfs:comment "Time, minute  = 60 s." ;
                   rdfs:label "min" .


:DERUnitSymbol.ohm uml:hasInitialValue "30" ;
                   
                   rdfs:comment "Electric resistance in ohm (V/A)." ;
                   rdfs:label "ohm" .


:DERUnitSymbol.ohmPerm 
                       rdfs:comment "Electric resistance per length in ohm per metre ((V/A)/m)." ;
                       rdfs:label "ohmPerm" .


:DERUnitSymbol.ohmm uml:hasInitialValue "102" ;
                    
                    rdfs:comment "resistivity, Ohm metre, (rho)." ;
                    rdfs:label "ohmm" .


:DERUnitSymbol.onePerHz 
                        rdfs:comment "Reciprocal of frequency (1/Hz)." ;
                        rdfs:label "onePerHz" .


:DERUnitSymbol.s uml:hasInitialValue "4" ;
                 
                 rdfs:comment "Time in seconds." ;
                 rdfs:label "s" .


:DERUnitSymbol.therm uml:hasInitialValue "169" ;
                     
                     rdfs:comment "Energy, Therm." ;
                     rdfs:label "therm" .


:DINStandardEditionKind._1985 
                              rdfs:comment "1985 standard edition." ;
                              rdfs:label "1985" .


:DINStandardEditionKind.none 
                             rdfs:comment "No standard edition." ;
                             rdfs:label "none" .


:DINStandardEditionKind.unknown 
                                rdfs:comment "Unknown standard edition." ;
                                rdfs:label "unknown" .


:DINStandardKind._51353 
                        rdfs:comment "Testing of insulating oils; detection of corrosive sulfur; silver strip test." ;
                        rdfs:label "51353" .


:DemographicKind.other 
                       rdfs:label "other" .


:DemographicKind.rural 
                       rdfs:label "rural" .


:DemographicKind.urban 
                       rdfs:label "urban" .


:DependencyKind.mutuallyExclusive 
                                  rdfs:label "mutuallyExclusive" .


:DependencyKind.required 
                         rdfs:label "required" .


:DeploymentStateKind.inService 
                               rdfs:comment "Asset in service in deployment location." ;
                               rdfs:label "inService" .


:DeploymentStateKind.installed 
                               rdfs:comment "Asset installed in deployment location." ;
                               rdfs:label "installed" .


:DeploymentStateKind.notYetInstalled 
                                     rdfs:comment "Asset not yet installed in deployment location." ;
                                     rdfs:label "notYetInstalled" .


:DeploymentStateKind.outOfService 
                                  rdfs:comment "Asset out of service, but in deployment location." ;
                                  rdfs:label "outOfService" .


:DeploymentStateKind.removed 
                             rdfs:comment "Asset removed from deployment location." ;
                             rdfs:label "removed" .


:DesignKind.asBuilt 
                    rdfs:label "asBuilt" .


:DesignKind.estimated 
                      rdfs:label "estimated" .


:DesignKind.other 
                  rdfs:label "other" .


:DispatchAcceptStatus.ACCEPT 
                             rdfs:label "ACCEPT" .


:DispatchAcceptStatus.CANNOT 
                             rdfs:label "CANNOT" .


:DispatchAcceptStatus.DECLINE 
                              rdfs:label "DECLINE" .


:DispatchAcceptStatus.NON_RESPONSE 
                                   rdfs:label "NON_RESPONSE" .


:DispatchAcceptStatus.OK 
                         rdfs:label "OK" .


:DispatchAcceptStatus.PARTIAL 
                              rdfs:label "PARTIAL" .


:DispatchResponseType.ACCEPT 
                             rdfs:label "ACCEPT" .


:DispatchResponseType.DECLINE 
                              rdfs:label "DECLINE" .


:DispatchResponseType.NON_RESPONSE 
                                   rdfs:label "NON_RESPONSE" .


:DispatchResponseType.PARTIAL 
                              rdfs:label "PARTIAL" .


:DispatchTransactionType.Purchase 
                                  rdfs:label "Purchase" .


:DispatchTransactionType.Sale 
                              rdfs:label "Sale" .


:DobleStandardEditionKind.none 
                               rdfs:comment "No edition." ;
                               rdfs:label "none" .


:DobleStandardEditionKind.unknown 
                                  rdfs:comment "Unknown edition." ;
                                  rdfs:label "unknown" .


:DobleStandardKind.methanol 
                            rdfs:comment "Doble test for methanol." ;
                            rdfs:label "methanol" .


:DroopSignalFeedbackKind.electricalPower 
                                         rdfs:comment "Electrical power feedback (connection indicated as 1 in the block diagrams of models, e.g. GovCT1, GovCT2)." ;
                                         rdfs:label "electricalPower" .


:DroopSignalFeedbackKind.fuelValveStroke 
                                         rdfs:comment "Fuel valve stroke feedback (true stroke) (connection indicated as 2 in the block diagrams of model, e.g. GovCT1, GovCT2)." ;
                                         rdfs:label "fuelValveStroke" .


:DroopSignalFeedbackKind.governorOutput 
                                        rdfs:comment "Governor output feedback (requested stroke) (connection indicated as 3 in the block diagrams of models, e.g. GovCT1, GovCT2)." ;
                                        rdfs:label "governorOutput" .


:DroopSignalFeedbackKind.none 
                              rdfs:comment "No droop signal feedback, is isochronous governor." ;
                              rdfs:label "none" .


:EPAStandardEditionKind.A 
                          rdfs:comment "Standard edition A." ;
                          rdfs:label "A" .


:EPAStandardEditionKind.none 
                             rdfs:comment "No standard edition." ;
                             rdfs:label "none" .


:EPAStandardEditionKind.unknown 
                                rdfs:comment "Unknown standard edition." ;
                                rdfs:label "unknown" .


:EPAStandardKind._8082 
                       rdfs:comment "Polychlorinated Biphenyls (PCBs) by Gas Chromatography." ;
                       rdfs:label "8082" .


:ERTConfidenceKind.high 
                        rdfs:comment "there is a high confidence that the ERT will be accomplished" ;
                        rdfs:label "high" .


:ERTConfidenceKind.low 
                       rdfs:comment "there is a low confidence that the ERT will be accomplished." ;
                       rdfs:label "low" .


:EmissionType.carbonDioxide 
                            rdfs:comment "Carbon dioxide." ;
                            rdfs:label "carbonDioxide" .


:EmissionType.carbonDisulfide 
                              rdfs:comment "Carbon disulfide." ;
                              rdfs:label "carbonDisulfide" .


:EmissionType.chlorine 
                       rdfs:comment "Chlorine." ;
                       rdfs:label "chlorine" .


:EmissionType.hydrogenSulfide 
                              rdfs:comment "Hydrogen sulfide." ;
                              rdfs:label "hydrogenSulfide" .


:EmissionType.nitrogenOxide 
                            rdfs:comment "Nitrogen oxide." ;
                            rdfs:label "nitrogenOxide" .


:EmissionType.sulfurDioxide 
                            rdfs:comment "Sulfur dioxide." ;
                            rdfs:label "sulfurDioxide" .


:EmissionValueSource.calculated 
                                rdfs:comment "Calculated." ;
                                rdfs:label "calculated" .


:EmissionValueSource.measured 
                              rdfs:comment "Measured." ;
                              rdfs:label "measured" .


:EndDeviceFunctionKind.autonomousDst 
                                     rdfs:comment "Autonomous application of daylight saving time (DST)." ;
                                     rdfs:label "autonomousDst" .


:EndDeviceFunctionKind.demandResponse 
                                      rdfs:comment "Demand response functions." ;
                                      rdfs:label "demandResponse" .


:EndDeviceFunctionKind.electricMetering 
                                        rdfs:comment "Electricity metering." ;
                                        rdfs:label "electricMetering" .


:EndDeviceFunctionKind.gasMetering 
                                   rdfs:comment "Gas metering." ;
                                   rdfs:label "gasMetering" .


:EndDeviceFunctionKind.metrology 
                                 rdfs:comment "Presentation of metered values to a user or another system (always a function of a meter, but might not be supported by a load control unit)." ;
                                 rdfs:label "metrology" .


:EndDeviceFunctionKind.onRequestRead 
                                     rdfs:comment "On-request reads." ;
                                     rdfs:label "onRequestRead" .


:EndDeviceFunctionKind.outageHistory 
                                     rdfs:comment "Reporting historical power interruption data." ;
                                     rdfs:label "outageHistory" .


:EndDeviceFunctionKind.relaysProgramming 
                                         rdfs:comment "Support for one or more relays that may be programmable in the meter (and tied to TOU, time pulse, load control or other functions)." ;
                                         rdfs:label "relaysProgramming" .


:EndDeviceFunctionKind.reverseFlow 
                                   rdfs:comment "Detection and monitoring of reverse flow." ;
                                   rdfs:label "reverseFlow" .


:EndDeviceFunctionKind.waterMetering 
                                     rdfs:comment "Water metering." ;
                                     rdfs:label "waterMetering" .


:EnergyPriceIndexType.BOTH 
                           rdfs:label "BOTH" .


:EnergyPriceIndexType.RETAIL 
                             rdfs:label "RETAIL" .


:EnergyPriceIndexType.WHOLESALE 
                                rdfs:label "WHOLESALE" .


:EnergyProductType.DYN 
                       rdfs:comment "Dynamic" ;
                       rdfs:label "DYN" .


:EnergyProductType.FIRM 
                        rdfs:comment "Firm" ;
                        rdfs:label "FIRM" .


:EnergyProductType.NFRM 
                        rdfs:comment "Non Firm" ;
                        rdfs:label "NFRM" .


:EnergyProductType.WHL 
                       rdfs:comment "Wheeling" ;
                       rdfs:label "WHL" .


:EnergyTransactionType.approve 
                               rdfs:comment "Approve" ;
                               rdfs:label "approve" .


:EnergyTransactionType.deny 
                            rdfs:comment "Deny" ;
                            rdfs:label "deny" .


:EnergyTransactionType.study 
                             rdfs:comment "Study" ;
                             rdfs:label "study" .


:EnergyTypeCode.DABE 
                     rdfs:label "DABE" .


:EnergyTypeCode.DAPE 
                     rdfs:label "DAPE" .


:EnergyTypeCode.DASE 
                     rdfs:label "DASE" .


:EnergyTypeCode.DMLE 
                     rdfs:label "DMLE" .


:EnergyTypeCode.DSSE 
                     rdfs:label "DSSE" .


:EnergyTypeCode.EDE 
                    rdfs:label "EDE" .


:EnergyTypeCode.HASE 
                     rdfs:label "HASE" .


:EnergyTypeCode.MLE 
                    rdfs:label "MLE" .


:EnergyTypeCode.MSSLFE 
                       rdfs:label "MSSLFE" .


:EnergyTypeCode.OE 
                   rdfs:label "OE" .


:EnergyTypeCode.PE 
                   rdfs:label "PE" .


:EnergyTypeCode.RE 
                   rdfs:label "RE" .


:EnergyTypeCode.RED 
                    rdfs:label "RED" .


:EnergyTypeCode.RMRE 
                     rdfs:label "RMRE" .


:EnergyTypeCode.RTSSE 
                      rdfs:label "RTSSE" .


:EnergyTypeCode.SE 
                   rdfs:label "SE" .


:EnergyTypeCode.SRE 
                    rdfs:label "SRE" .


:EnergyTypeCode.TEE 
                    rdfs:label "TEE" .


:EnergyTypeKind.ConsumerLoad 
                             rdfs:label "ConsumerLoad" .


:EnergyTypeKind.IndustrialLoad 
                               rdfs:label "IndustrialLoad" .


:EnergyTypeKind.Other 
                      rdfs:label "Other" .


:EnergyTypeKind.PVpark 
                       rdfs:label "PVpark" .


:EnergyTypeKind.WindPark 
                         rdfs:label "WindPark" .


:EnvironmentalDiscreteKind.cloudCover 
                                      rdfs:comment "Cloud cover in octa." ;
                                      rdfs:label "cloudCover" .


:EquipmentStatusType.In 
                        rdfs:comment "Equipment is in." ;
                        rdfs:label "In" .


:EquipmentStatusType.Out 
                         rdfs:comment "Equipment is out." ;
                         rdfs:label "Out" .


:ErpAccountKind.estimate 
                         rdfs:label "estimate" .


:ErpAccountKind.normal 
                       rdfs:label "normal" .


:ErpAccountKind.reversal 
                         rdfs:label "reversal" .


:ErpAccountKind.statistical 
                            rdfs:label "statistical" .


:ErpInvoiceKind.purchase 
                         rdfs:label "purchase" .


:ErpInvoiceKind.sale 
                     rdfs:label "sale" .


:ErpInvoiceLineItemKind.initial 
                                rdfs:label "initial" .


:ErpInvoiceLineItemKind.other 
                              rdfs:label "other" .


:ErpInvoiceLineItemKind.recalculation 
                                      rdfs:label "recalculation" .


:ExcIEEEST1AUELselectorKind.ignoreUELsignal 
                                            rdfs:comment "Ignore UEL signal." ;
                                            rdfs:label "ignoreUELsignal" .


:ExcIEEEST1AUELselectorKind.inputAddedToErrorSignal 
                                                    rdfs:comment "UEL input added to error signal." ;
                                                    rdfs:label "inputAddedToErrorSignal" .


:ExcIEEEST1AUELselectorKind.inputHVgateErrorSignal 
                                                   rdfs:comment "UEL input HV gate with error signal." ;
                                                   rdfs:label "inputHVgateErrorSignal" .


:ExcIEEEST1AUELselectorKind.inputHVgateVoltageOutput 
                                                     rdfs:comment "UEL input HV gate with voltage regulator output." ;
                                                     rdfs:label "inputHVgateVoltageOutput" .


:ExcREXSFeedbackSignalKind.fieldCurrent 
                                        rdfs:comment "The exciter field current is used." ;
                                        rdfs:label "fieldCurrent" .


:ExcREXSFeedbackSignalKind.fieldVoltage 
                                        rdfs:comment "The voltage regulator output voltage is used. It is the same as exciter field voltage." ;
                                        rdfs:label "fieldVoltage" .


:ExcREXSFeedbackSignalKind.outputVoltage 
                                         rdfs:comment "The output voltage of the exciter is used." ;
                                         rdfs:label "outputVoltage" .


:ExcST6BOELselectorKind.afterUEL 
                                 rdfs:comment "The connection is after UEL. Corresponds to <i>OELin</i> = 2 on the ExcST6B diagram." ;
                                 rdfs:label "afterUEL" .


:ExcST6BOELselectorKind.beforeUEL 
                                  rdfs:comment "The connection is before UEL. Corresponds to <i>OELin</i> = 1 on the ExcST6B diagram." ;
                                  rdfs:label "beforeUEL" .


:ExcST6BOELselectorKind.noOELinput 
                                   rdfs:comment "No OEL input is used. Corresponds to <i>OELin</i> not = 1 and not = 2 on the ExcST6B diagram. Original ExcST6B model would have called this <i>OELin</i> = 0." ;
                                   rdfs:label "noOELinput" .


:ExcST7BOELselectorKind.addVref 
                                rdfs:comment "The signal is added to <i>Vref</i>.  Corresponds to <i>OELin</i> = 1 on the ExcST7B diagram." ;
                                rdfs:label "addVref" .


:ExcST7BOELselectorKind.inputLVgate 
                                    rdfs:comment "The signal is connected into the input <i>LVGate</i>. Corresponds to <i>OELin</i> = 2 on the ExcST7B diagram." ;
                                    rdfs:label "inputLVgate" .


:ExcST7BOELselectorKind.noOELinput 
                                   rdfs:comment "No OEL input is used. Corresponds to <i>OELin</i> not = 1 and not = 2 and not = 3 on the ExcST7B diagram. Original ExcST7B model would have called this <i>OELin</i> = 0." ;
                                   rdfs:label "noOELinput" .


:ExcST7BOELselectorKind.outputLVgate 
                                     rdfs:comment "The signal is connected into the output <i>LVGate</i>.  Corresponds to <i>OELin</i> = 3 on the ExcST7B diagram." ;
                                     rdfs:label "outputLVgate" .


:ExcST7BUELselectorKind.addVref 
                                rdfs:comment "The signal is added to <i>Vref</i>. Corresponds to <i>UELin</i> = 1 on the ExcST7B diagram." ;
                                rdfs:label "addVref" .


:ExcST7BUELselectorKind.inputHVgate 
                                    rdfs:comment "The signal is connected into the input <i>HVGate</i>.  Corresponds to <i>UELin</i> = 2 on the ExcST7B diagram." ;
                                    rdfs:label "inputHVgate" .


:ExcST7BUELselectorKind.noUELinput 
                                   rdfs:comment "No UEL input is used.  Corresponds to <i>UELin</i> not = 1 and not = 2 and not = 3 on the ExcST7B diagram. Original ExcST7B model would have called this <i>UELin</i> = 0." ;
                                   rdfs:label "noUELinput" .


:ExcST7BUELselectorKind.outputHVgate 
                                     rdfs:comment "The signal is connected into the output <i>HVGate</i>.  Corresponds to <i>UELin</i> = 3 on the ExcST7B diagram." ;
                                     rdfs:label "outputHVgate" .


:ExecutionType.DA 
                  rdfs:comment "Day Ahead" ;
                  rdfs:label "DA" .


:ExecutionType.HASP 
                    rdfs:comment "Real TIme Hour Ahead Execution" ;
                    rdfs:label "HASP" .


:ExecutionType.RTD 
                   rdfs:comment "Real Time Dispatch" ;
                   rdfs:label "RTD" .


:ExecutionType.RTPD 
                    rdfs:comment "Real Time Pre-dispatch" ;
                    rdfs:label "RTPD" .


:FACTSDeviceKind.statcom 
                         rdfs:comment "Static synchronous compensator." ;
                         rdfs:label "statcom" .


:FACTSDeviceKind.svc 
                     rdfs:comment "Static VAr compensator." ;
                     rdfs:label "svc" .


:FACTSDeviceKind.tcpar 
                       rdfs:comment "Thyristor-controlled phase-angle regulator." ;
                       rdfs:label "tcpar" .


:FACTSDeviceKind.tcsc 
                      rdfs:comment "Thyristor-controlled series capacitor." ;
                      rdfs:label "tcsc" .


:FACTSDeviceKind.tcvl 
                      rdfs:comment "Thyristor-controlled voltage limiter." ;
                      rdfs:label "tcvl" .


:FACTSDeviceKind.tsbr 
                      rdfs:comment "Thyristor-switched braking resistor." ;
                      rdfs:label "tsbr" .


:FACTSDeviceKind.tssc 
                      rdfs:comment "Thyristor-switched series capacitor." ;
                      rdfs:label "tssc" .


:FACTSDeviceKind.upfc 
                      rdfs:comment "Unified power flow controller." ;
                      rdfs:label "upfc" .


:FScale.five 
             rdfs:comment "Over 200 mph 3-second gust." ;
             rdfs:label "five" .


:FScale.four 
             rdfs:comment "166-200 mph 3-second gust." ;
             rdfs:label "four" .


:FScale.minusNine 
                  rdfs:comment "Unknown." ;
                  rdfs:label "minusNine" .


:FScale.one 
            rdfs:comment "86-110 mph 3-second gust." ;
            rdfs:label "one" .


:FScale.three 
              rdfs:comment "136-165 mph 3-second gust." ;
              rdfs:label "three" .


:FScale.two 
            rdfs:comment "111-135 mph 3-second gust." ;
            rdfs:label "two" .


:FScale.zero 
             rdfs:comment "65-85 mph 3-second gust." ;
             rdfs:label "zero" .


:FacilityKind.distributionPoleTop 
                                  rdfs:comment "Distribution pole top." ;
                                  rdfs:label "distributionPoleTop" .


:FacilityKind.substationDistribution 
                                     rdfs:comment "Distribution substation." ;
                                     rdfs:label "substationDistribution" .


:FacilityKind.substationFossilPlant 
                                    rdfs:comment "Fossil plant substation." ;
                                    rdfs:label "substationFossilPlant" .


:FacilityKind.substationHydroPlant 
                                   rdfs:comment "Hydro plant substation." ;
                                   rdfs:label "substationHydroPlant" .


:FacilityKind.substationNuclearPlant 
                                     rdfs:comment "Nuclear plant substation." ;
                                     rdfs:label "substationNuclearPlant" .


:FacilityKind.substationSubTransmission 
                                        rdfs:comment "Subtransmission substation." ;
                                        rdfs:label "substationSubTransmission" .


:FacilityKind.substationTransmission 
                                     rdfs:comment "Transmission substation." ;
                                     rdfs:label "substationTransmission" .


:FailureIsolationMethodKind.breakerOperation 
                                             rdfs:comment "Isolated via breaker operation." ;
                                             rdfs:label "breakerOperation" .


:FailureIsolationMethodKind.burnedInTheClear 
                                             rdfs:comment "Isolated by equipment burning in the clear." ;
                                             rdfs:label "burnedInTheClear" .


:FailureIsolationMethodKind.fuse 
                                 rdfs:comment "Isolated by fuse." ;
                                 rdfs:label "fuse" .


:FailureIsolationMethodKind.manuallyIsolated 
                                             rdfs:comment "Isolated by manual operation." ;
                                             rdfs:label "manuallyIsolated" .


:FailureIsolationMethodKind.other 
                                  rdfs:comment "Isolated by other action." ;
                                  rdfs:label "other" .


:FaultIndicatorResetKind.automatic 
                                   rdfs:label "automatic" .


:FaultIndicatorResetKind.manual 
                                rdfs:label "manual" .


:FaultIndicatorResetKind.other 
                               rdfs:label "other" .


:FaultIndicatorResetKind.remote 
                                rdfs:label "remote" .


:FlagTypeRMR.N 
               rdfs:comment "'N' - not an RMR unit" ;
               rdfs:label "N" .


:FlagTypeRMR._1 
                rdfs:comment "'1' - RMR Condition 1 unit" ;
                rdfs:label "1" .


:FlagTypeRMR._2 
                rdfs:comment "'2' - RMR Condition 2 unit" ;
                rdfs:label "2" .


:FlowDirectionKind.forward uml:hasInitialValue "1" ;
                           
                           rdfs:comment """\"Delivered,\" or \"Imported\" as defined 61968-2.
Forward Active Energy is a positive kWh value as one would naturally expect to find as energy is supplied by the utility and consumed at the service.
Forward Reactive Energy is a positive VArh value as one would naturally expect to find in the presence of inductive loading.
In polyphase metering, the forward energy register is incremented when the sum of the phase energies is greater than zero:
<img src=\"HTS_1.PNG\" width=\"209\" height=\"16\" border=\"0\" alt=\"graphic\"/>""" ;
                           rdfs:label "forward" .


:FlowDirectionKind.lagging uml:hasInitialValue "2" ;
                           
                           rdfs:comment """Typically used to describe that a power factor is lagging the reference value. 
Note 1: When used to describe VA, “lagging” describes a form of measurement where reactive power is considered in all four quadrants, but real power is considered only in quadrants I and IV.
Note 2: When used to describe power factor, the term “Lagging” implies that the PF is negative. The term “lagging” in this case takes the place of the negative sign. If a signed PF value is to be passed by the data producer, then the direction of flow enumeration zero (none) should be used in order to avoid the possibility of creating an expression that employs a double negative. The data consumer should be able to tell from the sign of the data if the PF is leading or lagging. This principle is analogous to the concept that “Reverse” energy is an implied negative value, and to publish a negative reverse value would be ambiguous.
Note 3: Lagging power factors typically indicate inductive loading.""" ;
                           rdfs:label "lagging" .


:FlowDirectionKind.leading uml:hasInitialValue "3" ;
                           
                           rdfs:comment """Typically used to describe that a power factor is leading the reference value.
Note: Leading power factors typically indicate capacitive loading.""" ;
                           rdfs:label "leading" .


:FlowDirectionKind.net uml:hasInitialValue "4" ;
                       
                       rdfs:comment """|Forward| - |Reverse|, See 61968-2.

Note: In some systems, the value passed as a “net” value could become negative. In other systems the value passed as a “net” value is always a positive number, and rolls-over and rolls-under as needed.""" ;
                       rdfs:label "net" .


:FlowDirectionKind.none uml:hasInitialValue "0" ;
                        
                        rdfs:comment "Not Applicable (N/A)" ;
                        rdfs:label "none" .


:FlowDirectionKind.q1minusQ4 uml:hasInitialValue "9" ;
                             
                             rdfs:comment "Q1 minus Q4" ;
                             rdfs:label "q1minusQ4" .


:FlowDirectionKind.q1plusQ2 uml:hasInitialValue "5" ;
                            
                            rdfs:comment "Reactive positive quadrants. (The term “lagging” is preferred.)" ;
                            rdfs:label "q1plusQ2" .


:FlowDirectionKind.q1plusQ3 uml:hasInitialValue "7" ;
                            
                            rdfs:comment "Quadrants 1 and 3" ;
                            rdfs:label "q1plusQ3" .


:FlowDirectionKind.q1plusQ4 uml:hasInitialValue "8" ;
                            
                            rdfs:comment "Quadrants 1 and 4 usually represent forward active energy" ;
                            rdfs:label "q1plusQ4" .


:FlowDirectionKind.q2minusQ3 uml:hasInitialValue "12" ;
                             
                             rdfs:comment "Q2 minus Q3" ;
                             rdfs:label "q2minusQ3" .


:FlowDirectionKind.q2plusQ3 uml:hasInitialValue "10" ;
                            
                            rdfs:comment "Quadrants 2 and 3 usually represent reverse active energy" ;
                            rdfs:label "q2plusQ3" .


:FlowDirectionKind.q2plusQ4 uml:hasInitialValue "11" ;
                            
                            rdfs:comment "Quadrants 2 and 4" ;
                            rdfs:label "q2plusQ4" .


:FlowDirectionKind.q3minusQ2 uml:hasInitialValue "14" ;
                             
                             rdfs:comment "Q3 minus Q2" ;
                             rdfs:label "q3minusQ2" .


:FlowDirectionKind.q3plusQ4 uml:hasInitialValue "13" ;
                            
                            rdfs:comment "Reactive negative quadrants. (The term “leading” is preferred.)" ;
                            rdfs:label "q3plusQ4" .


:FlowDirectionKind.quadrant1 uml:hasInitialValue "15" ;
                             
                             rdfs:comment "Q1 only" ;
                             rdfs:label "quadrant1" .


:FlowDirectionKind.quadrant2 uml:hasInitialValue "16" ;
                             
                             rdfs:comment "Q2 only" ;
                             rdfs:label "quadrant2" .


:FlowDirectionKind.quadrant3 uml:hasInitialValue "17" ;
                             
                             rdfs:comment "Q3 only" ;
                             rdfs:label "quadrant3" .


:FlowDirectionKind.quadrant4 uml:hasInitialValue "18" ;
                             
                             rdfs:comment "Q4 only" ;
                             rdfs:label "quadrant4" .


:FlowDirectionKind.reverse uml:hasInitialValue "19" ;
                           
                           rdfs:comment """Reverse Active Energy is equivalent to \"Received,\" or \"Exported\" as defined in 61968-2.
Reverse Active Energy is a positive kWh value as one would expect to find when energy is backfed by the service onto the utility network.
Reverse Reactive Energy is a positive VArh value as one would expect to find in the presence of capacitive loading and a leading Power Factor.
In polyphase metering, the reverse energy register is incremented when the sum of the phase energies is less than zero:
<img src=\"HTS_1.PNG\" width=\"209\" height=\"16\" border=\"0\" alt=\"graphic\"/>
Note: The value passed as a reverse value is always a positive value. It is understood by the label “reverse” that it represents negative flow.""" ;
                           rdfs:label "reverse" .


:FlowDirectionKind.total uml:hasInitialValue "20" ;
                         
                         rdfs:comment """|Forward| + |Reverse|, See 61968-2.
The sum of the commodity in all quadrants Q1+Q2+Q3+Q4.
In polyphase metering, the total energy register is incremented when the absolute value of the sum of the phase energies is greater than zero:
<img src=\"HTS_1.PNG\" width=\"217\" height=\"16\" border=\"0\" alt=\"graphic\"/>""" ;
                         rdfs:label "total" .


:FlowDirectionKind.totalByPhase uml:hasInitialValue "21" ;
                                
                                rdfs:comment """In polyphase metering, the total by phase energy register is incremented when the sum of the absolute values of the phase energies is greater than zero:
<img src=\"HTS_1.PNG\" width=\"234\" height=\"16\" border=\"0\" alt=\"graphic\"/>
In single phase metering, the formulas for “Total” and “Total by phase” collapse to the same expression. For communication purposes however, the “Total” enumeration should be used with single phase meter data.""" ;
                                rdfs:label "totalByPhase" .


:FlowDirectionType.Forward 
                           rdfs:comment "Forward direction." ;
                           rdfs:label "Forward" .


:FlowDirectionType.Reverse 
                           rdfs:comment "Reverse direction." ;
                           rdfs:label "Reverse" .


:FrancisGovernorControlKind.electromechanicalElectrohydraulic 
                                                              rdfs:comment "Electromechanical and electrohydraulic regulator (Cflag=3)." ;
                                                              rdfs:label "electromechanicalElectrohydraulic" .


:FrancisGovernorControlKind.mechanicHydraulicTransientFeedback 
                                                               rdfs:comment "Mechanic-hydraulic regulator with transient feedback (Cflag=2)." ;
                                                               rdfs:label "mechanicHydraulicTransientFeedback" .


:FrancisGovernorControlKind.mechanicHydrolicTachoAccelerator 
                                                             rdfs:comment "Mechanic-hydraulic regulator with tacho-accelerometer (Cflag = 1)." ;
                                                             rdfs:label "mechanicHydrolicTachoAccelerator" .


:FuelSource.BGAS 
                 rdfs:comment "Bio Gas (Landfill, Sewage, Digester, etc.)" ;
                 rdfs:label "BGAS" .


:FuelSource.BIOM 
                 rdfs:comment "Biomass" ;
                 rdfs:label "BIOM" .


:FuelSource.COAL 
                 rdfs:comment "Coal" ;
                 rdfs:label "COAL" .


:FuelSource.DIST 
                 rdfs:label "DIST" .


:FuelSource.GAS 
                rdfs:label "GAS" .


:FuelSource.GEOT 
                 rdfs:comment "GeoThermal" ;
                 rdfs:label "GEOT" .


:FuelSource.HRCV 
                 rdfs:label "HRCV" .


:FuelSource.NG 
               rdfs:comment "Natural Gas" ;
               rdfs:label "NG" .


:FuelSource.NNG 
                rdfs:comment "Non-Natural Gas" ;
                rdfs:label "NNG" .


:FuelSource.NONE 
                 rdfs:label "NONE" .


:FuelSource.NUCL 
                 rdfs:comment "Nuclear" ;
                 rdfs:label "NUCL" .


:FuelSource.OIL 
                rdfs:label "OIL" .


:FuelSource.OTHR 
                 rdfs:comment "Other" ;
                 rdfs:label "OTHR" .


:FuelSource.SOLR 
                 rdfs:comment "Solar" ;
                 rdfs:label "SOLR" .


:FuelSource.WAST 
                 rdfs:comment "Waste to Energy" ;
                 rdfs:label "WAST" .


:FuelSource.WATR 
                 rdfs:comment "Water" ;
                 rdfs:label "WATR" .


:FuelSource.WIND 
                 rdfs:comment "Wind" ;
                 rdfs:label "WIND" .


:FuelType.brownCoalLignite 
                           rdfs:comment "Brown coal lignite." ;
                           rdfs:label "brownCoalLignite" .


:FuelType.coal 
               rdfs:comment "Generic coal, not including lignite type." ;
               rdfs:label "coal" .


:FuelType.coalDerivedGas 
                         rdfs:comment "Coal derived gas." ;
                         rdfs:label "coalDerivedGas" .


:FuelType.gas 
              rdfs:comment "Natural gas." ;
              rdfs:label "gas" .


:FuelType.hardCoal 
                   rdfs:comment "Hard coal." ;
                   rdfs:label "hardCoal" .


:FuelType.lignite 
                  rdfs:comment "The fuel is lignite coal.  Note that this is a special type of coal, so the other enum of coal is reserved for hard coal types or if the exact type of coal is not known." ;
                  rdfs:label "lignite" .


:FuelType.oil 
              rdfs:comment "Oil." ;
              rdfs:label "oil" .


:FuelType.oilShale 
                   rdfs:comment "Oil Shale." ;
                   rdfs:label "oilShale" .


:FuelType.other 
                rdfs:comment "Any fuel type not included in the rest of the enumerated value." ;
                rdfs:label "other" .


:FuelType.peat 
               rdfs:comment "Peat." ;
               rdfs:label "peat" .


:GateLogicKind.and 
                   rdfs:comment "A logical AND operation. True when all input are true." ;
                   rdfs:label "and" .


:GateLogicKind.nand 
                    rdfs:comment "A logical NAND operation. False when all input are true." ;
                    rdfs:label "nand" .


:GateLogicKind.nor 
                   rdfs:comment "A logical NOR operation. False when one or more input are true." ;
                   rdfs:label "nor" .


:GateLogicKind.not 
                   rdfs:comment "A logical NOT operation. Only one input and true input will give false out and false in will give true out. An inverter." ;
                   rdfs:label "not" .


:GateLogicKind.or 
                  rdfs:comment "A logical OR operation. True when one or more input are true." ;
                  rdfs:label "or" .


:GateLogicKind.xnor 
                    rdfs:comment "A logical XNOR operation. The function is the inverse of the exclusive OR (XOR) gate. All input false or true will give true. Otherwise false." ;
                    rdfs:label "xnor" .


:GateLogicKind.xor 
                   rdfs:comment "A logical XOR operation.  All input false or true will give false. Otherwise true." ;
                   rdfs:label "xor" .


:GeneratorControlMode.pulse 
                            rdfs:comment "Pulse control mode." ;
                            rdfs:label "pulse" .


:GeneratorControlMode.setpoint 
                               rdfs:comment "Setpoint control mode." ;
                               rdfs:label "setpoint" .


:GeneratorControlSource.offAGC 
                               rdfs:comment "Off of automatic generation control (AGC)." ;
                               rdfs:label "offAGC" .


:GeneratorControlSource.onAGC 
                              rdfs:comment "On automatic generation control (AGC)." ;
                              rdfs:label "onAGC" .


:GeneratorControlSource.plantControl 
                                     rdfs:comment "Plant is controlling." ;
                                     rdfs:label "plantControl" .


:GeneratorControlSource.unavailable 
                                    rdfs:comment "Not available." ;
                                    rdfs:label "unavailable" .


:GenericNonLinearLoadModelKind.exponentialRecovery 
                                                   rdfs:comment "Exponential recovery model." ;
                                                   rdfs:label "exponentialRecovery" .


:GenericNonLinearLoadModelKind.loadAdaptive 
                                            rdfs:comment "Load adaptive model." ;
                                            rdfs:label "loadAdaptive" .


:GeosphericAnalogKind.lightningDensity 
                                       rdfs:comment "Flash rate in strikes/hour/km<sup>2</sup>." ;
                                       rdfs:label "lightningDensity" .


:GeosphericAnalogKind.seismicEastWest 
                                      rdfs:label "seismicEastWest" .


:GeosphericAnalogKind.seismicNorthSouth 
                                        rdfs:label "seismicNorthSouth" .


:GeosphericAnalogKind.seismicVertical 
                                      rdfs:label "seismicVertical" .


:GeosphericAnalogKind.snowPackDepth 
                                    rdfs:label "snowPackDepth" .


:GeosphericAnalogKind.temperature 
                                  rdfs:label "temperature" .


:GovHydro4ModelKind.francisPelton 
                                  rdfs:comment "Francis or Pelton model." ;
                                  rdfs:label "francisPelton" .


:GovHydro4ModelKind.kaplan 
                           rdfs:comment "Kaplan model." ;
                           rdfs:label "kaplan" .


:GovHydro4ModelKind.simple 
                           rdfs:comment "Simple model." ;
                           rdfs:label "simple" .


:HydroEnergyConversionKind.generator 
                                     rdfs:comment "Able to generate power, but not able to pump water for energy storage." ;
                                     rdfs:label "generator" .


:HydroEnergyConversionKind.pumpAndGenerator 
                                            rdfs:comment "Able to both generate power and pump water for energy storage." ;
                                            rdfs:label "pumpAndGenerator" .


:HydroPlantStorageKind.pumpedStorage 
                                     rdfs:comment "Pumped storage." ;
                                     rdfs:label "pumpedStorage" .


:HydroPlantStorageKind.runOfRiver 
                                  rdfs:comment "Run of river." ;
                                  rdfs:label "runOfRiver" .


:HydroPlantStorageKind.storage 
                               rdfs:comment "Storage." ;
                               rdfs:label "storage" .


:HydroTurbineKind.francis 
                          rdfs:comment "Francis." ;
                          rdfs:label "francis" .


:HydroTurbineKind.kaplan 
                         rdfs:comment "Kaplan." ;
                         rdfs:label "kaplan" .


:HydroTurbineKind.pelton 
                         rdfs:comment "Pelton." ;
                         rdfs:label "pelton" .


:HydrosphericAnalogKind.floodLevel 
                                   rdfs:label "floodLevel" .


:HydrosphericAnalogKind.stormSurgeHeight 
                                         rdfs:label "stormSurgeHeight" .


:HydrosphericAnalogKind.surfaceTemperature 
                                           rdfs:label "surfaceTemperature" .


:HydrosphericAnalogKind.waterTemperature 
                                         rdfs:label "waterTemperature" .


:HydrosphericAnalogKind.waveHeight 
                                   rdfs:label "waveHeight" .


:ICCPAccessPrivilegeKind.readOnly 
                                  rdfs:comment "Indicates that the remote is not allowed to change the value of the ICCPPoint." ;
                                  rdfs:label "readOnly" .


:ICCPAccessPrivilegeKind.readWrite 
                                   rdfs:comment "Indicates that the remote can not only get the value, but may also change the value of the ICCP Point." ;
                                   rdfs:label "readWrite" .


:ICCPPointKind.discrete 
                        rdfs:comment "Indicates that an ICCP discrete type is to be conveyed." ;
                        rdfs:label "discrete" .


:ICCPPointKind.packedProtectionEvent 
                                     rdfs:comment "Indicates that an ICCP packed Protection Event is to be conveyed." ;
                                     rdfs:label "packedProtectionEvent" .


:ICCPPointKind.real 
                    rdfs:comment "Indicates that an ICCP real type is to be conveyed." ;
                    rdfs:label "real" .


:ICCPPointKind.singleProtectionEvent 
                                     rdfs:comment "Indicates that an ICCP single Protection Event  type is to be conveyed." ;
                                     rdfs:label "singleProtectionEvent" .


:ICCPPointKind.state 
                     rdfs:comment "Indicates that an ICCP state type is to be conveyed." ;
                     rdfs:label "state" .


:ICCPPointKind.stateSupplemental 
                                 rdfs:comment "Indicates that an ICCP state supplemental type is to be conveyed." ;
                                 rdfs:label "stateSupplemental" .


:ICCPQualityKind.extended 
                          rdfs:comment "Indicates that only extended information is to be provided." ;
                          rdfs:label "extended" .


:ICCPQualityKind.extendedwithQualityTime 
                                         rdfs:comment "Provides quality, timestamp, and extended information." ;
                                         rdfs:label "extendedwithQualityTime" .


:ICCPQualityKind.none 
                      rdfs:comment "Indicates that no quality is conveyed with the ICCP point." ;
                      rdfs:label "none" .


:ICCPQualityKind.qualityAndTime 
                                rdfs:comment "Indicates that quality and a timestamp are to be provided." ;
                                rdfs:label "qualityAndTime" .


:ICCPQualityKind.qualityOnly 
                             rdfs:comment "Indicates that only quality is to be provided." ;
                             rdfs:label "qualityOnly" .


:ICCPScopeKind.iCC 
                   rdfs:comment "Inter-Control Centre scope – available for exchange between the control centres in the bilateral table." ;
                   rdfs:label "iCC" .


:ICCPScopeKind.vCC 
                   rdfs:comment "Virtual Control Centre Scope – globally available." ;
                   rdfs:label "vCC" .


:IECStandardEditionKind._1963 
                              rdfs:comment "1963 edition." ;
                              rdfs:label "1963" .


:IECStandardEditionKind._1967 
                              rdfs:comment "1967 edition." ;
                              rdfs:label "1967" .


:IECStandardEditionKind._1973 
                              rdfs:comment "1973 edition." ;
                              rdfs:label "1973" .


:IECStandardEditionKind._1974 
                              rdfs:comment "1974 edition." ;
                              rdfs:label "1974" .


:IECStandardEditionKind._1977 
                              rdfs:comment "1977 edition." ;
                              rdfs:label "1977" .


:IECStandardEditionKind._1978 
                              rdfs:comment "1978 edition." ;
                              rdfs:label "1978" .


:IECStandardEditionKind._1979 
                              rdfs:comment "1979 edition." ;
                              rdfs:label "1979" .


:IECStandardEditionKind._1985 
                              rdfs:comment "1985 edition." ;
                              rdfs:label "1985" .


:IECStandardEditionKind._1989 
                              rdfs:comment "1989 edition." ;
                              rdfs:label "1989" .


:IECStandardEditionKind._1992 
                              rdfs:comment "1992 edition." ;
                              rdfs:label "1992" .


:IECStandardEditionKind._1992_AMD1_2004 
                                        rdfs:comment "1992/AMD1:2004 edition." ;
                                        rdfs:label "1992/AMD1:2004" .


:IECStandardEditionKind._1992_COR1_1992 
                                        rdfs:comment "1992/COR1:1992 edition." ;
                                        rdfs:label "1992/COR1:1992" .


:IECStandardEditionKind._1993 
                              rdfs:comment "1993 edition." ;
                              rdfs:label "1993" .


:IECStandardEditionKind._1995 
                              rdfs:comment "1995 edition." ;
                              rdfs:label "1995" .


:IECStandardEditionKind._1997 
                              rdfs:comment "1997 edition." ;
                              rdfs:label "1997" .


:IECStandardEditionKind._1998 
                              rdfs:comment "1998 edition." ;
                              rdfs:label "1998" .


:IECStandardEditionKind._2004 
                              rdfs:comment "2004 edition." ;
                              rdfs:label "2004" .


:IECStandardEditionKind._2004_AMD1_2007 
                                        rdfs:comment "2004/AMD1:2007 edition." ;
                                        rdfs:label "2004/AMD1:2007" .


:IECStandardEditionKind._2004_AMD1_2007CSV 
                                           rdfs:comment "2004/AMD1:2007CSV edition." ;
                                           rdfs:label "2004/AMD1:2007CSV" .


:IECStandardEditionKind._2005 
                              rdfs:comment "2005 edition." ;
                              rdfs:label "2005" .


:IECStandardEditionKind._2007 
                              rdfs:comment "2007 edition." ;
                              rdfs:label "2007" .


:IECStandardEditionKind._2008 
                              rdfs:comment "2008 edition." ;
                              rdfs:label "2008" .


:IECStandardEditionKind._2010 
                              rdfs:comment "2010 edition." ;
                              rdfs:label "2010" .


:IECStandardEditionKind._2011 
                              rdfs:comment "2011 edition." ;
                              rdfs:label "2011" .


:IECStandardEditionKind._2012 
                              rdfs:comment "2012 edition." ;
                              rdfs:label "2012" .


:IECStandardEditionKind._2013 
                              rdfs:comment "2013 edition." ;
                              rdfs:label "2013" .


:IECStandardEditionKind._2013_COR_2013 
                                       rdfs:comment "2013/COR:2013 edition." ;
                                       rdfs:label "2013/COR:2013" .


:IECStandardEditionKind.none 
                             rdfs:comment "No edition." ;
                             rdfs:label "none" .


:IECStandardEditionKind.unknown 
                                rdfs:comment "Unknown edition." ;
                                rdfs:label "unknown" .


:IECStandardKind._60156 
                        rdfs:comment "Insulating liquids - Determination of the breakdown voltage at power frequency - Test method." ;
                        rdfs:label "60156" .


:IECStandardKind._60243-1 
                          rdfs:comment "Electric strength of insulating materials - Test methods - Part 1: Tests at power frequencies." ;
                          rdfs:label "60243-1" .


:IECStandardKind._60243-2 
                          rdfs:comment "Electric strength of insulating materials - Test methods - Part 2: Additional requirements for tests using direct voltage." ;
                          rdfs:label "60243-2" .


:IECStandardKind._60243-3 
                          rdfs:comment "Electric strength of insulating materials - Test methods - Part 3: Additional requirements for 1,2/50 µs impulse tests." ;
                          rdfs:label "60243-3" .


:IECStandardKind._60247 
                        rdfs:comment """Insulating liquids - Measurement of relative permittivity, dielectric dissipation factor (tan d) and d.c. resistivity  -or-
Measurement of relative permittivity, dielectric dissipation factor and d.c. resistivity of insulating liquids  -or-
Recommended test cells for measuring the resistivity of insulating liquids and methods of cleaning the cells.""" ;
                        rdfs:label "60247" .


:IECStandardKind._60422 
                        rdfs:comment "Mineral insulating oils in electrical equipment - Supervision and maintenance guidance." ;
                        rdfs:label "60422" .


:IECStandardKind._60450 
                        rdfs:comment "Measurement of the average viscometric degree of polymerization of new and aged cellulosic electrically insulating materials." ;
                        rdfs:label "60450" .


:IECStandardKind._60567 
                        rdfs:comment """Oil-filled electrical equipment - Sampling of gases and analysis of free and dissolved gasses - Guidance  -or-
Oil-filled electrical equipment - Sampling of gases and of oil for analysis of free and dissolved gases - Guidance  -or-
Guide for the sampling of gases and of oil form oil-filled electrical equipment and for the analysis of free and dissolved gases.""" ;
                        rdfs:label "60567" .


:IECStandardKind._60666 
                        rdfs:comment """Detection and determination of specified additives in mineral insulating oils  -or-
Detection and determination of specified anti-oxidant additives in insulating oils.""" ;
                        rdfs:label "60666" .


:IECStandardKind._60814 
                        rdfs:comment "Insulating liquids - Oil-impregnated paper and pressboard - Determination of water by automatic coulometric Karl Fischer titration." ;
                        rdfs:label "60814" .


:IECStandardKind._60970 
                        rdfs:comment """Insulating liquids - Methods for counting and sizing particles  -or-
Methods for counting and sizing particles in insulating liquids.""" ;
                        rdfs:label "60970" .


:IECStandardKind._60997 
                        rdfs:comment """Determination of polychlorinated biphenyls (PCBs) in mineral insulating oils by packed column gas chromatography (GC).
Withdrawn.""" ;
                        rdfs:label "60997" .


:IECStandardKind._61125 
                        rdfs:comment "Unused hydrocarbon based insulating liquids - Test methods for evaluating the oxidation stability." ;
                        rdfs:label "61125" .


:IECStandardKind._61198 
                        rdfs:comment "Mineral insulating oils - Methods for the determination of 2-furfural and related compounds." ;
                        rdfs:label "61198" .


:IECStandardKind._61619 
                        rdfs:comment "Insulating liquids - Contamination by polychlorinated biphenyls (PCBs) - Method of determination by capillary column gas chromatography." ;
                        rdfs:label "61619" .


:IECStandardKind._61868 
                        rdfs:comment "Mineral insulating oils – Determination of kinematic viscosity at very low temperatures." ;
                        rdfs:label "61868" .


:IECStandardKind._62535 
                        rdfs:comment "Insulating liquids – Test method for detection of potentially corrosive sulphur in used and unused insulating oil." ;
                        rdfs:label "62535" .


:IECStandardKind._62697-1 
                          rdfs:comment "Test methods for quantitative determination of corrosive sulfur compounds in unused and used insulating liquids - Part 1: Test method for quantitative determination of dibenzyldisulfide (DBDS)." ;
                          rdfs:label "62697-1" .


:IECStandardKind._62770 
                        rdfs:comment "Fluids for electrotechnical applications – Unused natural esters for transformers and similar electrical equipment." ;
                        rdfs:label "62770" .


:IEEEStandardEditionKind._1978 
                               rdfs:comment "1978 standard edition." ;
                               rdfs:label "1978" .


:IEEEStandardEditionKind._1995 
                               rdfs:comment "1995 standard edition." ;
                               rdfs:label "1995" .


:IEEEStandardEditionKind.none 
                              rdfs:comment "No standard edition." ;
                              rdfs:label "none" .


:IEEEStandardEditionKind.unknown 
                                 rdfs:comment "Unknown standard edition." ;
                                 rdfs:label "unknown" .


:IEEEStandardKind._62 
                      rdfs:comment """IEEE Guide for Diagnostic Field Testing of Electric Power Apparatus - Part 1: Oil Filled Power Transformers, Regulators, and Reactors -or-
IEEE Guide for Field Testing Power Apparatus Insulation.""" ;
                      rdfs:label "62" .


:IPAddressKind.iPv4 
                    rdfs:comment "Indicates that IPv4 dotted decimal notation is in use." ;
                    rdfs:label "iPv4" .


:IPAddressKind.iPv6 
                    rdfs:comment "Indicates that an IPv6 dotted decimal is in use." ;
                    rdfs:label "iPv6" .


:ISOStandardEditionKind._1973 
                              rdfs:comment "1973 standard edition." ;
                              rdfs:label "1973" .


:ISOStandardEditionKind._1974 
                              rdfs:comment "1974 standard edition." ;
                              rdfs:label "1974" .


:ISOStandardEditionKind._1976 
                              rdfs:comment "1976 standard edition." ;
                              rdfs:label "1976" .


:ISOStandardEditionKind._1983 
                              rdfs:comment "1983 standard edition." ;
                              rdfs:label "1983" .


:ISOStandardEditionKind._1985 
                              rdfs:comment "1985 standard edition." ;
                              rdfs:label "1985" .


:ISOStandardEditionKind._1988 
                              rdfs:comment "1988 standard edition." ;
                              rdfs:label "1988" .


:ISOStandardEditionKind._1992 
                              rdfs:comment "1992 standard edition." ;
                              rdfs:label "1992" .


:ISOStandardEditionKind._1993 
                              rdfs:comment "1993 standard edition." ;
                              rdfs:label "1993" .


:ISOStandardEditionKind._1994 
                              rdfs:comment "1994 standard edition." ;
                              rdfs:label "1994" .


:ISOStandardEditionKind._1994_Cor1_1997 
                                        rdfs:comment "1994/Cor1:1997 standard edition." ;
                                        rdfs:label "1994/Cor1:1997" .


:ISOStandardEditionKind._1998 
                              rdfs:comment "1998 standard edition." ;
                              rdfs:label "1998" .


:ISOStandardEditionKind._2000 
                              rdfs:comment "2000 standard edition." ;
                              rdfs:label "2000" .


:ISOStandardEditionKind._2002 
                              rdfs:comment "2002 standard edition." ;
                              rdfs:label "2002" .


:ISOStandardEditionKind._2005 
                              rdfs:comment "2005 standard edition." ;
                              rdfs:label "2005" .


:ISOStandardEditionKind._2008 
                              rdfs:comment "2008 standard edition." ;
                              rdfs:label "2008" .


:ISOStandardEditionKind.none 
                             rdfs:comment "No standard edition." ;
                             rdfs:label "none" .


:ISOStandardEditionKind.unknown 
                                rdfs:comment "Unknown standard edition." ;
                                rdfs:label "unknown" .


:ISOStandardKind._1924 
                       rdfs:comment "Paper and board -- Determination of tensile strength." ;
                       rdfs:label "1924" .


:ISOStandardKind._1924-1 
                         rdfs:comment "Paper and board -- Determination of tensile properties -- Part 1: Constant rate of loading method." ;
                         rdfs:label "1924-1" .


:ISOStandardKind._1924-2 
                         rdfs:comment """Paper and board -- Determination of tensile properties -- Part 2: Constant rate of elongation method (20 mm/min)  -or-
Paper and board -- Determination of tensile properties -- Part 2: Constant rate of elongation method.""" ;
                         rdfs:label "1924-2" .


:ISOStandardKind._1924-3 
                         rdfs:comment "Paper and board -- Determination of tensile properties -- Part 3: Constant rate of elongation method (100 mm/min)." ;
                         rdfs:label "1924-3" .


:ISOStandardKind._2592 
                       rdfs:comment "Determination of flash and fire points -- Cleveland open cup method (copied directly from ASTM D92)." ;
                       rdfs:label "2592" .


:ISOStandardKind._2719 
                       rdfs:comment """Determination of flash point -- Pensky-Martens closed cup method (copied directly from ASTM D93)  -or-
Petroleum products and lubricants -- Determination of flash point -- Pensky-Martens closed cup method (copied directly from ASTM D93)  -or-
Petroleum products -- Determination of flash point -- Pensky-Martens closed cup method (copied directly from ASTM D93).""" ;
                       rdfs:label "2719" .


:ISOStandardKind._3016 
                       rdfs:comment """Petroleum products -- Determination of pour point  -or-
Petroleum oils -- Determination of pour point.""" ;
                       rdfs:label "3016" .


:ISOStandardKind._3104 
                       rdfs:comment "Petroleum products -- Transparent and opaque liquids -- Determination of kinematic viscosity and calculation of dynamic viscosity." ;
                       rdfs:label "3104" .


:ISOStandardKind._3675 
                       rdfs:comment """Crude petroleum and liquid petroleum products -- Laboratory determination of density -- Hydrometer method  -or-
Crude petroleum and liquid petroleum products -- Laboratory determination of density or relative density -- Hydrometer method.""" ;
                       rdfs:label "3675" .


:IfdBaseKind.ifag 
                  rdfs:comment "Air gap line mode." ;
                  rdfs:label "ifag" .


:IfdBaseKind.iffl 
                  rdfs:comment "Full load system mode." ;
                  rdfs:label "iffl" .


:IfdBaseKind.ifnl 
                  rdfs:comment "No load system with saturation mode." ;
                  rdfs:label "ifnl" .


:InUseStateKind.inUse 
                      rdfs:comment "Asset is deployed (in use) or is being put into use." ;
                      rdfs:label "inUse" .


:InUseStateKind.notReadyForUse 
                               rdfs:comment "Asset is not ready to be put into use." ;
                               rdfs:label "notReadyForUse" .


:InUseStateKind.readyForUse 
                            rdfs:comment "Asset is ready to be put into use." ;
                            rdfs:label "readyForUse" .


:InputSignalKind.branchCurrent 
                               rdfs:comment "Input signal is amplitude of remote branch current." ;
                               rdfs:label "branchCurrent" .


:InputSignalKind.busFrequency 
                              rdfs:comment "Input signal is bus voltage fr<font color=\"#0f0f0f\">equency.  This could be a terminal frequency or remote frequency.</font>" ;
                              rdfs:label "busFrequency" .


:InputSignalKind.busFrequencyDeviation 
                                       rdfs:comment "Input signal is deviation of bus voltage frequ<font color=\"#0f0f0f\">ency.  This could be a terminal frequency deviation or remote frequency deviation.</font>" ;
                                       rdfs:label "busFrequencyDeviation" .


:InputSignalKind.busVoltage 
                            rdfs:comment "Input signal <font color=\"#0f0f0f\">is bus voltage.  This could be a terminal voltage or remote voltage.</font>" ;
                            rdfs:label "busVoltage" .


:InputSignalKind.busVoltageDerivative 
                                      rdfs:comment "Input signal is derivative of bus voltag<font color=\"#0f0f0f\">e.  This could be a terminal voltage derivative or remote voltage derivative.</font>" ;
                                      rdfs:label "busVoltageDerivative" .


:InputSignalKind.fieldCurrent 
                              rdfs:comment "Input signal is generator field current." ;
                              rdfs:label "fieldCurrent" .


:InputSignalKind.generatorAcceleratingPower 
                                            rdfs:comment "Input signal is generator accelerating power." ;
                                            rdfs:label "generatorAcceleratingPower" .


:InputSignalKind.generatorElectricalPower 
                                          rdfs:comment "Input signal is generator electrical power on rated <i>S</i>." ;
                                          rdfs:label "generatorElectricalPower" .


:InputSignalKind.generatorMechanicalPower 
                                          rdfs:comment "Input signal is generator mechanical power." ;
                                          rdfs:label "generatorMechanicalPower" .


:InputSignalKind.rotorAngularFrequencyDeviation 
                                                rdfs:comment "Input signal is rotor or shaft angular frequency deviation." ;
                                                rdfs:label "rotorAngularFrequencyDeviation" .


:InputSignalKind.rotorSpeed 
                            rdfs:comment "Input signal is rotor or shaft speed (angular frequency)." ;
                            rdfs:label "rotorSpeed" .


:InspectionAnalogKind.airPressureHPSystemReading 
                                                 rdfs:comment "Analog value represents High Pressure system air pressure." ;
                                                 rdfs:label "airPressureHPSystemReading" .


:InspectionAnalogKind.airPressureLPSystemReading 
                                                 rdfs:comment "Analog value represents Low Pressure system air pressure." ;
                                                 rdfs:label "airPressureLPSystemReading" .


:InspectionAnalogKind.airPressureReading 
                                         rdfs:comment "Analog value represents air pressure." ;
                                         rdfs:label "airPressureReading" .


:InspectionAnalogKind.compressorHourMeterReading 
                                                 rdfs:comment "Analog value represents reading from compressor hour meter." ;
                                                 rdfs:label "compressorHourMeterReading" .


:InspectionAnalogKind.sF6PressureReading 
                                         rdfs:comment "Analog value represents SF6 gas pressure." ;
                                         rdfs:label "sF6PressureReading" .


:InspectionDiscreteKind.bushingOilLevelsOK 
                                           rdfs:comment "Are bushing oil levels OK?" ;
                                           rdfs:label "bushingOilLevelsOK" .


:InspectionDiscreteKind.checkOilLevelOK 
                                        rdfs:comment "Check oil level OK?" ;
                                        rdfs:label "checkOilLevelOK" .


:InspectionDiscreteKind.controlCabinetHeaterOn 
                                               rdfs:comment "Is the control cabinet heater on?" ;
                                               rdfs:label "controlCabinetHeaterOn" .


:InspectionDiscreteKind.gasIndicatorNormal 
                                           rdfs:comment "Is the circuit switcher gas indicator normal?" ;
                                           rdfs:label "gasIndicatorNormal" .


:InspectionDiscreteKind.hydraulicFluidLevelOK 
                                              rdfs:comment "Hydraulic fluid level OK?" ;
                                              rdfs:label "hydraulicFluidLevelOK" .


:InspectionDiscreteKind.hydraulicOilLevelOK 
                                            rdfs:comment "Is the hydraulic oil level OK? Can apply to any individual pole." ;
                                            rdfs:label "hydraulicOilLevelOK" .


:InspectionDiscreteKind.lowToHighPressureCount 
                                               rdfs:comment "Count of ??." ;
                                               rdfs:label "lowToHighPressureCount" .


:InspectionDiscreteKind.motorOperationsCount 
                                             rdfs:comment "Count of motor operations." ;
                                             rdfs:label "motorOperationsCount" .


:InspectionDiscreteKind.oilTankLevelsOK 
                                        rdfs:comment "Are the oil tank levels OK?" ;
                                        rdfs:label "oilTankLevelsOK" .


:InspectionDiscreteKind.operationCount 
                                       rdfs:comment "Count of operations." ;
                                       rdfs:label "operationCount" .


:InspectionDiscreteKind.pumpMotorOperationCount 
                                                rdfs:comment "Count of pump motor operations." ;
                                                rdfs:label "pumpMotorOperationCount" .


:InspectionDiscreteKind.springPressureReadingOK 
                                                rdfs:comment "Is the spring pressure reading OK? Can apply to whole breaker or any individual pole." ;
                                                rdfs:label "springPressureReadingOK" .


:InspectionDiscreteKind.visibleDamageOrLeaks 
                                             rdfs:comment "Any visible damage and/or oil/air/SF6 leaks?." ;
                                             rdfs:label "visibleDamageOrLeaks" .


:IntensityCodeKind.heavy 
                         rdfs:label "heavy" .


:IntensityCodeKind.light 
                         rdfs:label "light" .


:IntensityCodeKind.veryHeavy 
                             rdfs:label "veryHeavy" .


:IntensityCodeKind.veryLight 
                             rdfs:label "veryLight" .


:InterTieDirection.E 
                     rdfs:comment "Export." ;
                     rdfs:label "E" .


:InterTieDirection.I 
                     rdfs:comment "Import." ;
                     rdfs:label "I" .


:InterruptingMediumKind.airBlast 
                                 rdfs:comment "Air blast." ;
                                 rdfs:label "airBlast" .


:InterruptingMediumKind.airMagnetic 
                                    rdfs:comment "Air magnetic." ;
                                    rdfs:label "airMagnetic" .


:InterruptingMediumKind.bulkOil 
                                rdfs:comment "Bulk oil." ;
                                rdfs:label "bulkOil" .


:InterruptingMediumKind.gasSinglePressure 
                                          rdfs:comment "Gas single pressure." ;
                                          rdfs:label "gasSinglePressure" .


:InterruptingMediumKind.gasTwoPressure 
                                       rdfs:comment "Gas two pressure." ;
                                       rdfs:label "gasTwoPressure" .


:InterruptingMediumKind.minimumOil 
                                   rdfs:comment "Minimum oil." ;
                                   rdfs:label "minimumOil" .


:InterruptingMediumKind.vacuum 
                               rdfs:comment "Vacuum." ;
                               rdfs:label "vacuum" .


:JobFlagType.CREATED 
                     rdfs:label "CREATED" .


:JobFlagType.DELETED 
                     rdfs:label "DELETED" .


:JobFlagType.MODIFIED 
                      rdfs:label "MODIFIED" .


:JobScheduleType.CRITICAL 
                          rdfs:label "CRITICAL" .


:JobScheduleType.NONCRITICAL 
                             rdfs:label "NONCRITICAL" .


:JobStartEndType.END 
                     rdfs:label "END" .


:JobStartEndType.NA 
                    rdfs:label "NA" .


:JobStartEndType.START 
                       rdfs:label "START" .


:JointConfigurationKind.other 
                              rdfs:label "other" .


:JointConfigurationKind.wires1to1 
                                  rdfs:label "wires1to1" .


:JointConfigurationKind.wires2to1 
                                  rdfs:label "wires2to1" .


:JointConfigurationKind.wires3to1 
                                  rdfs:label "wires3to1" .


:JointFillKind.airNoFilling 
                            rdfs:label "airNoFilling" .


:JointFillKind.asphaltic 
                         rdfs:label "asphaltic" .


:JointFillKind.bluefill254 
                           rdfs:label "bluefill254" .


:JointFillKind.epoxy 
                     rdfs:label "epoxy" .


:JointFillKind.insoluseal 
                          rdfs:label "insoluseal" .


:JointFillKind.noFillPrefab 
                            rdfs:label "noFillPrefab" .


:JointFillKind.noVoid 
                      rdfs:label "noVoid" .


:JointFillKind.oil 
                   rdfs:label "oil" .


:JointFillKind.other 
                     rdfs:label "other" .


:JointFillKind.petrolatum 
                          rdfs:label "petrolatum" .


:LFCResourceType.GEN 
                     rdfs:label "GEN" .


:LFCResourceType.PUMP 
                      rdfs:label "PUMP" .


:LaborelecStandardEditionKind.none 
                                   rdfs:comment "No standard edition." ;
                                   rdfs:label "none" .


:LaborelecStandardEditionKind.unknown 
                                      rdfs:comment "Unknown standard edition." ;
                                      rdfs:label "unknown" .


:LaborelecStandardKind.methanol 
                                rdfs:comment "Laborelec test for methanol." ;
                                rdfs:label "methanol" .


:LandPropertyKind.building 
                           rdfs:comment "Site enclosed within a building." ;
                           rdfs:label "building" .


:LandPropertyKind.customerPremise 
                                  rdfs:comment "Site with a customer." ;
                                  rdfs:label "customerPremise" .


:LandPropertyKind.depot 
                        rdfs:comment "Storehouse for supplies that also serves as a station for supporting crews." ;
                        rdfs:label "depot" .


:LandPropertyKind.external 
                           rdfs:comment "Property owned or used by an external party that is not a customer." ;
                           rdfs:label "external" .


:LandPropertyKind.gridSupplyPoint 
                                  rdfs:comment "Substation where the distribution and transmission networks meet and hence have mixed ownership and mixed operational control." ;
                                  rdfs:label "gridSupplyPoint" .


:LandPropertyKind.store 
                        rdfs:comment "Place of storage (e.g., a warehouse) to put aside, or accumulate, material and equipment for use when needed." ;
                        rdfs:label "store" .


:LandPropertyKind.substation 
                             rdfs:comment "Transmission network switchyard." ;
                             rdfs:label "substation" .


:LoadFollowingCapacityType.DOWN 
                                rdfs:label "DOWN" .


:LoadFollowingCapacityType.UP 
                              rdfs:label "UP" .


:LoadForecastType.LFZ 
                      rdfs:comment "Load forecast zone." ;
                      rdfs:label "LFZ" .


:LoadForecastType.LZMS 
                       rdfs:comment "Metered sub system zone." ;
                       rdfs:label "LZMS" .


:LocationKind.center 
                     rdfs:comment "The center of a phenomenon. Will typically be used with a Location with a single PositionPoint instance." ;
                     rdfs:label "center" .


:LocationKind.extent 
                     rdfs:comment "The area or line of a phenomenon, not the center. Will typically be used with a Location with multiple PositionPoint instances." ;
                     rdfs:label "extent" .


:LocationKind.primary 
                      rdfs:comment "Primary area to which an environmental alert applies." ;
                      rdfs:label "primary" .


:LocationKind.secondary 
                        rdfs:comment "Secondary area to which an environmental alert applies." ;
                        rdfs:label "secondary" .


:LookUpTableFunctionKind.additionalQcurrent 
                                            rdfs:label "additionalQcurrent" .


:LookUpTableFunctionKind.vdcol 
                               rdfs:label "vdcol" .


:MPMTestIdentifierType._1 
                          rdfs:comment "1 - Global Price Test." ;
                          rdfs:label "1" .


:MPMTestIdentifierType._2 
                          rdfs:comment "2 - Global Conduct Test." ;
                          rdfs:label "2" .


:MPMTestIdentifierType._3 
                          rdfs:comment "3 - Global Impact Test." ;
                          rdfs:label "3" .


:MPMTestIdentifierType._4 
                          rdfs:comment "4 - Local Price Test." ;
                          rdfs:label "4" .


:MPMTestIdentifierType._5 
                          rdfs:comment "5 - Local Conduct Test." ;
                          rdfs:label "5" .


:MPMTestIdentifierType._6 
                          rdfs:comment "6 - Local Impact Test." ;
                          rdfs:label "6" .


:MPMTestMethodType.ALTERNATE 
                             rdfs:comment "Alternate." ;
                             rdfs:label "ALTERNATE" .


:MPMTestMethodType.NORMAL 
                          rdfs:comment "Normal." ;
                          rdfs:label "NORMAL" .


:MPMTestOutcome.D 
                  rdfs:comment "Disabled" ;
                  rdfs:label "D" .


:MPMTestOutcome.F 
                  rdfs:comment "Failed" ;
                  rdfs:label "F" .


:MPMTestOutcome.P 
                  rdfs:comment "Passed" ;
                  rdfs:label "P" .


:MPMTestOutcome.S 
                  rdfs:comment "Skipped" ;
                  rdfs:label "S" .


:MQSCHGType.ADD 
                rdfs:label "ADD" .


:MQSCHGType.CHG 
                rdfs:label "CHG" .


:MQSDELType.ADD 
                rdfs:label "ADD" .


:MQSDELType.CHG 
                rdfs:label "CHG" .


:MQSDELType.DEL 
                rdfs:label "DEL" .


:MQSInstructionSource.ACT 
                          rdfs:label "ACT" .


:MQSInstructionSource.INS 
                          rdfs:label "INS" .


:MacroPeriodKind.billingPeriod uml:hasInitialValue "8" ;
                               
                               rdfs:comment "Captured during the billing period starting at midnight of the first day of the billing period (as defined by the billing cycle day). If during the current billing period, it specifies a period from the start of the current billing period until \"now\"." ;
                               rdfs:label "billingPeriod" .


:MacroPeriodKind.daily uml:hasInitialValue "11" ;
                       
                       rdfs:comment "Daily period starting at midnight. If for the current day, this specifies the time from midnight to \"now\"." ;
                       rdfs:label "daily" .


:MacroPeriodKind.monthly uml:hasInitialValue "13" ;
                         
                         rdfs:comment "Monthly period starting at midnight on the first day of the month. If within the current month, this specifies the period from the start of the month until \"now.\"" ;
                         rdfs:label "monthly" .


:MacroPeriodKind.none uml:hasInitialValue "0" ;
                      
                      rdfs:comment "Not applicable." ;
                      rdfs:label "none" .


:MacroPeriodKind.seasonal uml:hasInitialValue "22" ;
                          
                          rdfs:comment "A season of time spanning multiple months. E.g. \"Summer,\" \"Spring,\" \"Fall,\" and \"Winter\" based cycle. If within the current season, it specifies the period from the start of the current season until \"now.\"" ;
                          rdfs:label "seasonal" .


:MacroPeriodKind.specifiedPeriod uml:hasInitialValue "32" ;
                                 
                                 rdfs:comment "For the period defined by the start and end of the TimePeriod element in the message." ;
                                 rdfs:label "specifiedPeriod" .


:MacroPeriodKind.weekly uml:hasInitialValue "24" ;
                        
                        rdfs:comment "Weekly period starting at midnight on the first day of the week and ending the instant before midnight the last day of the week. If within the current week, it specifies the period from the start of the week until \"now.\"" ;
                        rdfs:label "weekly" .


:MarketEventStatusKind.active 
                              rdfs:comment """The status of the event is currently in a active state.
Active (when sysdate is equal or greater than to planned start time)""" ;
                              rdfs:label "active" .


:MarketEventStatusKind.cancelled 
                                 rdfs:comment """The status of the event is currently in a cancelled state.
Cancelled (stopped before planned start time or planned end time)""" ;
                                 rdfs:label "cancelled" .


:MarketEventStatusKind.completed 
                                 rdfs:comment """The status of the event is currently in a completed state.
Complete (when sysdate is equal to the release time)""" ;
                                 rdfs:label "completed" .


:MarketEventStatusKind.planned 
                               rdfs:comment """The status of the event is currently in a planned state.
Planned (sysdate is less than planned start time)""" ;
                               rdfs:label "planned" .


:MarketProductSelfSchedType.ETC 
                                rdfs:comment "Existing Transmission Contract." ;
                                rdfs:label "ETC" .


:MarketProductSelfSchedType.LPT 
                                rdfs:comment "Low price taker." ;
                                rdfs:label "LPT" .


:MarketProductSelfSchedType.PT 
                               rdfs:comment "Price taker." ;
                               rdfs:label "PT" .


:MarketProductSelfSchedType.RA 
                               rdfs:comment "Resource adequacy." ;
                               rdfs:label "RA" .


:MarketProductSelfSchedType.RGMR 
                                 rdfs:comment "Regulatory must run." ;
                                 rdfs:label "RGMR" .


:MarketProductSelfSchedType.RMR 
                                rdfs:comment "Reliability Must Run." ;
                                rdfs:label "RMR" .


:MarketProductSelfSchedType.RMT 
                                rdfs:comment "Reliability must take." ;
                                rdfs:label "RMT" .


:MarketProductSelfSchedType.SP 
                               rdfs:comment "Self provision." ;
                               rdfs:label "SP" .


:MarketProductSelfSchedType.TOR 
                                rdfs:comment "Transmission Ownership Right." ;
                                rdfs:label "TOR" .


:MarketProductType.EN 
                      rdfs:comment "energy type" ;
                      rdfs:label "EN" .


:MarketProductType.LFD 
                       rdfs:comment "Load following down" ;
                       rdfs:label "LFD" .


:MarketProductType.LFU 
                       rdfs:comment "Load following up" ;
                       rdfs:label "LFU" .


:MarketProductType.NR 
                      rdfs:comment "non spinning reserve" ;
                      rdfs:label "NR" .


:MarketProductType.RC 
                      rdfs:comment "Residual Unit Commitment" ;
                      rdfs:label "RC" .


:MarketProductType.RD 
                      rdfs:comment "regulation down" ;
                      rdfs:label "RD" .


:MarketProductType.REG 
                       rdfs:comment "Regulation" ;
                       rdfs:label "REG" .


:MarketProductType.RU 
                      rdfs:comment "regulation up" ;
                      rdfs:label "RU" .


:MarketProductType.SR 
                      rdfs:comment "spinning reserve" ;
                      rdfs:label "SR" .


:MarketProductTypeAsReq.AS 
                           rdfs:label "AS" .


:MarketProductTypeAsReq.NR 
                           rdfs:comment "non spinning reserve" ;
                           rdfs:label "NR" .


:MarketProductTypeAsReq.RD 
                           rdfs:comment "regulation down" ;
                           rdfs:label "RD" .


:MarketProductTypeAsReq.RU 
                           rdfs:comment "regulation up" ;
                           rdfs:label "RU" .


:MarketProductTypeAsReq.SR 
                           rdfs:comment "spinning reserve" ;
                           rdfs:label "SR" .


:MarketRoleKind.BalanceResponsibleParty 
                                        rdfs:comment """A party that has a contract proving financial security and identifying balance responsibility with the Imbalance Settlement Responsible of the Market Balance Area entitling the party to operate in the market. This is the only role allowing a party to nominate energy on a wholesale level.
<b><i>Additional information:</i></b>
The meaning of the word \"balance\" in this context signifies that the quantity contracted to provide or to consume shall be equal to the quantity really provided or consumed. Equivalent to \"Program responsible party\" in the Netherlands. Equivalent to \"Balance group manager\" in Germany. Equivalent to \"market agent\" in Spain.""" ;
                                        rdfs:label "BalanceResponsibleParty" .


:MarketRoleKind.BalanceSupplier 
                                rdfs:comment """A party that markets the difference between actual metered energy consumption and the energy bought with firm energy contracts by the Party Connected to the Grid. In addition the Balance Supplier markets any difference with the firm energy contract (of the Party Connected to the Grid) and the metered production.
<b><i>Additional information:</i></b>
There is only one Balance Supplier for each Accounting Point.""" ;
                                rdfs:label "BalanceSupplier" .


:MarketRoleKind.BillingAgent 
                             rdfs:comment "The party responsible for invoicing a concerned party." ;
                             rdfs:label "BillingAgent" .


:MarketRoleKind.BlockEnergyTrader 
                                  rdfs:comment "A party that is selling or buying energy on a firm basis (a fixed volume per market time period)." ;
                                  rdfs:label "BlockEnergyTrader" .


:MarketRoleKind.CapacityCoordinator 
                                    rdfs:comment "A party, acting on behalf of the System Operators involved, responsible for establishing a coordinated Offered Capacity and/or Net Transfer Capacity (NTC) and/or Available Transfer Capacity (ATC) between several Market Balance Areas." ;
                                    rdfs:label "CapacityCoordinator" .


:MarketRoleKind.CapacityTrader 
                               rdfs:comment """A party that has a contract to participate in the Capacity Market to acquire capacity through a Transmission Capacity Allocator.

The capacity may be acquired on behalf of an Interconnection Trade Responsible or for sale on secondary capacity markets.""" ;
                               rdfs:label "CapacityTrader" .


:MarketRoleKind.Consumer 
                         rdfs:comment """A party that consumes electricity.
<b><i>Additional information:</i></b>
This is a Type of Party Connected to the Grid.""" ;
                         rdfs:label "Consumer" .


:MarketRoleKind.ConsumptionResponsibleParty 
                                            rdfs:comment """A party who can be brought to rights, legally and financially, for any imbalance between enegry nominated and consumed for all associated Accounting Points.
<b><i>Additional information:</i></b>
This is a type of Balance Responsible Party.""" ;
                                            rdfs:label "ConsumptionResponsibleParty" .


:MarketRoleKind.ControlAreaOperator 
                                    rdfs:comment """Responsible for :
1. The coordination of exchange programs between its related Market Balance Areas and for the exchanges between its associated Control Areas.
2. The load frequency control for its own area.
3. The coordination of the correction of time deviations.""" ;
                                    rdfs:label "ControlAreaOperator" .


:MarketRoleKind.ControlBlockOperator 
                                     rdfs:comment """Responsible for :
1. The coordination of exchanges between its associated Control Blocks and the organisation of the coordination of exchange programs between its related Control Areas.
2. The load frequency control within its own block and ensuring that its Control Areas respect their obligations in respect to load frequency control and time deviation.
3. The organisation of the settlement and/or compensation between its Control Areas.""" ;
                                     rdfs:label "ControlBlockOperator" .


:MarketRoleKind.CoordinationCenterOperator 
                                           rdfs:comment """Responsible for :
1. The coordination of exchange programs between its related Control Blocks and for the exchanges between its associated Coordination Center Zones.
2. Ensuring that its Control Blocks respect their obligations in respect to load frequency control.
3. Calculating the time deviation in cooperation with the associated coordination centers.
4. Carrying out the settlement and/or compensation between its Control Blocks and against the other Coordination Center Zones.""" ;
                                           rdfs:label "CoordinationCenterOperator" .


:MarketRoleKind.GridAccessProvider 
                                   rdfs:comment "A party responsible for providing access to the grid through an Accounting Point and its use for energy consumption or production to the Party Connected to the Grid." ;
                                   rdfs:label "GridAccessProvider" .


:MarketRoleKind.GridOperator 
                             rdfs:comment "A party that operates one or more grids." ;
                             rdfs:label "GridOperator" .


:MarketRoleKind.ImbalanceSettlementResponsible 
                                               rdfs:comment """A party that is responsible for settlement of the difference between the contracted quantities and the realised quantities of energy products for the Balance Responsible Parties in a Market Balance Area.
Note:
The Imbalance Settlement Responsible has not the responsibility to invoice. The Imbalance Settlement Responsible may delegate the invoicing responsibility to a more generic role such as a Billing Agent.""" ;
                                               rdfs:label "ImbalanceSettlementResponsible" .


:MarketRoleKind.InterconnectionTradeResponsible 
                                                rdfs:comment """Is a Balance Responsible Party or depends on one. They are recognized by the Nomination Validator for the nomination of already allocated capacity.
<b><i>Additional information:</i></b>
This is a type of Balance Responsible Party.""" ;
                                                rdfs:label "InterconnectionTradeResponsible" .


:MarketRoleKind.MOLResponsible 
                               rdfs:comment "Responsible for the management of the available tenders for all Acquiring System Operators to establish the order of the reserve capacity that can be activated." ;
                               rdfs:label "MOLResponsible" .


:MarketRoleKind.MarketInformationAggregator 
                                            rdfs:comment """Market Information Aggregator, A party that provides market related information that has been compiled from the figures supplied by different actors in the market. This information may also be published or distributed for general use.
<b><i>Note:</i></b>
The Market Information Aggregator may receive information from any market participant that is relevant for publication or distribution.""" ;
                                            rdfs:label "MarketInformationAggregator" .


:MarketRoleKind.MarketOperator 
                               rdfs:comment "The unique power exchange of trades for the actual delivery of energy that receives the bids from the Balance Responsible Parties that have a contract to bid. The Market Operator determines the market energy price for the Market Balance Area after applying technical constraints from the System Operator. It may also establish the price for the reconciliation within a Metering Grid Area." ;
                               rdfs:label "MarketOperator" .


:MarketRoleKind.MeterAdministrator 
                                   rdfs:comment "A party responsible for keeping a database of meters." ;
                                   rdfs:label "MeterAdministrator" .


:MarketRoleKind.MeterOperator 
                              rdfs:comment "A party responsible for installing, maintaining, testing, certifying and decommissioning physical meters." ;
                              rdfs:label "MeterOperator" .


:MarketRoleKind.MeteredDataAggregator 
                                      rdfs:comment "A party responsible for the establishment and qualification of metered data from the Metered Data Responsible. This data is aggregated according to a defined set of market rules." ;
                                      rdfs:label "MeteredDataAggregator" .


:MarketRoleKind.MeteredDataCollector 
                                     rdfs:comment "A party responsible for meter reading and quality control of the reading." ;
                                     rdfs:label "MeteredDataCollector" .


:MarketRoleKind.MeteredDataResponsible 
                                       rdfs:comment "A party responsible for the establishment and validation of metered data based on the collected data received from the Metered Data Collector. The party is responsible for the history of metered data for a Metering Point." ;
                                       rdfs:label "MeteredDataResponsible" .


:MarketRoleKind.MeteringPointAdministrator 
                                           rdfs:comment "A party responsible for registering the parties linked to the metering points in a Metering Grid Area. They are also responsible for maintaining the Metering Point technical specifications. They are responsible for creating and terminating metering points." ;
                                           rdfs:label "MeteringPointAdministrator" .


:MarketRoleKind.NominationValidator 
                                    rdfs:comment "Has the responsibility of ensuring that all capacity nominated is within the allowed limits and confirming all valid nominations to all involved parties. They inform the Interconnection Trade Responsible of the maximum nominated capacity allowed. Depending on market rules for a given interconnection the corresponding System Operators may appoint one Nomination Validator." ;
                                    rdfs:label "NominationValidator" .


:MarketRoleKind.PartyConnectedToTheGrid 
                                        rdfs:comment "A party that contracts for the right to consume or produce electricity at an Accounting Point." ;
                                        rdfs:label "PartyConnectedToTheGrid" .


:MarketRoleKind.Producer 
                         rdfs:comment """A party that produces electricity.
<b><i>Additional information:</i></b>
This is a type of Party Connected to the Grid.""" ;
                         rdfs:label "Producer" .


:MarketRoleKind.ProductionResponsibleParty 
                                           rdfs:comment """A party who can be brought to rights, legally and financially, for any imbalance between energy nominated and produced for all associated Accounting Points.
<b><i>Additional information:</i></b>
This is a type of Balance Responsible Party.""" ;
                                           rdfs:label "ProductionResponsibleParty" .


:MarketRoleKind.ReconciliationAccountable 
                                          rdfs:comment "A party that is financially accountable for the reconciled volume of energy products for a profiled Accounting Point." ;
                                          rdfs:label "ReconciliationAccountable" .


:MarketRoleKind.ReconciliationResponsible 
                                          rdfs:comment """A party that is responsible for reconciling, within a Metering Grid Area, the volumes used in the imbalance settlement process for profiled Accounting Points and the actual metered quantities.
Note:
The Reconciliation Responsible may delegate the invoicing responsibility to a more generic role such as a Billing Agent.""" ;
                                          rdfs:label "ReconciliationResponsible" .


:MarketRoleKind.ReserveAllocator 
                                 rdfs:comment "Informs the market of reserve requirements, receives tenders against the requirements and in compliance with the prequalification criteria, determines what tenders meet requirements and assigns tenders." ;
                                 rdfs:label "ReserveAllocator" .


:MarketRoleKind.ResourceProvider 
                                 rdfs:comment "A role that manages a resource object and provides the schedules for it" ;
                                 rdfs:label "ResourceProvider" .


:MarketRoleKind.SchedulingCoordinator 
                                      rdfs:comment "A party that is responsible for the schedule information and its exchange on behalf of a Balance Responsible Party. For example in the Polish market a Scheduling Coordinator is responsible for information interchange for scheduling and settlement." ;
                                      rdfs:label "SchedulingCoordinator" .


:MarketRoleKind.SystemOperator 
                               rdfs:comment """A party that is responsible for a stable power system operation
(including the organisation of physical balance) through a transmission grid in a geographical area. The System Operator will also determine and be responsible for cross border capacity and exchanges. If necessary they may reduce allocated capacity to ensure operational stability. Transmission as mentioned above means \"the transport of electricity on the extra high or high voltage network with a view to its delivery to final customers or to distributors. Operation of transmission includes as well the tasks of system operation concerning its management of energy flows, reliability of the system and availability of all necessary system services.\" (definition taken from the ENTSO-E RGCE Operation handbook Glossary).
<b><i>Note: </i></b>additional obligations may be imposed through local market rules.""" ;
                               rdfs:label "SystemOperator" .


:MarketRoleKind.TradeResponsibleParty 
                                      rdfs:comment """A party who can be brought to rights, legally and financially, for any imbalance between energy nominated and consumed for all associated Accounting Points.
<b><i>Note:</i></b>
A power exchange without any privileged responsibilities acts as a Trade Responsible Party.
<b><i>Additional information:</i></b>
This is a type of Balance Responsible Party.""" ;
                                      rdfs:label "TradeResponsibleParty" .


:MarketRoleKind.TransmissionCapacityAllocator 
                                              rdfs:comment """Manages the allocation of transmission capacity for an Allocated Capacity Area.
<b><i>For explicit auctions:</i></b>
The Transmission Capacity Allocator manages, on behalf of the System Operators, the allocation of available transmission capacity for an Allocated capacity Area. They offer the available transmission capacity to the market, allocates the available transmission capacity to individual Capacity Traders and calculates the billing amount of already allocated capacities to the Capacity Traders.""" ;
                                              rdfs:label "TransmissionCapacityAllocator" .


:MarketRoleKind.balancingAuthority 
                                   rdfs:comment "Balancing authority." ;
                                   rdfs:label "balancingAuthority" .


:MarketRoleKind.competitiveRetailer 
                                    rdfs:comment "Competitive retailer." ;
                                    rdfs:label "competitiveRetailer" .


:MarketRoleKind.complianceMonitor 
                                  rdfs:comment "Compliance monitor." ;
                                  rdfs:label "complianceMonitor" .


:MarketRoleKind.distributionProvider 
                                     rdfs:comment "Distribution provider." ;
                                     rdfs:label "distributionProvider" .


:MarketRoleKind.energyServiceConsumer 
                                      rdfs:comment "Energy service consumer." ;
                                      rdfs:label "energyServiceConsumer" .


:MarketRoleKind.generatorOperator 
                                  rdfs:comment "Generator merchant operator." ;
                                  rdfs:label "generatorOperator" .


:MarketRoleKind.generatorOwner 
                               rdfs:comment "Generator merchant owner." ;
                               rdfs:label "generatorOwner" .


:MarketRoleKind.interchangeAuthority 
                                     rdfs:comment "Interchange authority." ;
                                     rdfs:label "interchangeAuthority" .


:MarketRoleKind.loadServingEntity 
                                  rdfs:comment "Load serving entity." ;
                                  rdfs:label "loadServingEntity" .


:MarketRoleKind.planningAuthority 
                                  rdfs:comment "Planning authority." ;
                                  rdfs:label "planningAuthority" .


:MarketRoleKind.purchasingSellingEntity 
                                        rdfs:comment "Purchasing selling entity." ;
                                        rdfs:label "purchasingSellingEntity" .


:MarketRoleKind.reliabilityAuthority 
                                     rdfs:comment "Reliability authority." ;
                                     rdfs:label "reliabilityAuthority" .


:MarketRoleKind.resourcePlanner 
                                rdfs:comment "Resource planner." ;
                                rdfs:label "resourcePlanner" .


:MarketRoleKind.standardsDeveloper 
                                   rdfs:comment "Standards developer." ;
                                   rdfs:label "standardsDeveloper" .


:MarketRoleKind.transmissionOperator 
                                     rdfs:comment "Transmission operator." ;
                                     rdfs:label "transmissionOperator" .


:MarketRoleKind.transmissionOwner 
                                  rdfs:comment "Transmission owner." ;
                                  rdfs:label "transmissionOwner" .


:MarketRoleKind.transmissionPlanner 
                                    rdfs:comment "Transmission planner." ;
                                    rdfs:label "transmissionPlanner" .


:MarketRoleKind.transmissionServiceProvider 
                                            rdfs:comment "Transmission service provider." ;
                                            rdfs:label "transmissionServiceProvider" .


:MarketScheduleServices.retrieveDefaultBidCurves 
                                                 rdfs:label "retrieveDefaultBidCurves" .


:MarketScheduleServices.retrieveMPMResults 
                                           rdfs:label "retrieveMPMResults" .


:MarketScheduleServices.retrieveMarketAwards 
                                             rdfs:label "retrieveMarketAwards" .


:MarketScheduleServices.retrieveSchedulePrices 
                                               rdfs:label "retrieveSchedulePrices" .


:MarketScheduleServices.retrieveStartUpShutDownInstructions 
                                                            rdfs:label "retrieveStartUpShutDownInstructions" .


:MarketStatementDescription.DAILY_INITIAL_CREDIT 
                                                 rdfs:label "DAILY_INITIAL_CREDIT" .


:MarketStatementDescription.DAILY_INITIAL_MARKET 
                                                 rdfs:label "DAILY_INITIAL_MARKET" .


:MarketStatementDescription.DAILY_RECALC_MARKET 
                                                rdfs:label "DAILY_RECALC_MARKET" .


:MarketStatementDescription.MONTHLY_INITIAL_MARKET 
                                                   rdfs:label "MONTHLY_INITIAL_MARKET" .


:MarketStatementDescription.MONTHLY_RECALC_MARKET 
                                                  rdfs:label "MONTHLY_RECALC_MARKET" .


:MarketStatementDocStatus.APPROVED 
                                   rdfs:label "APPROVED" .


:MarketStatementDocStatus.CANCELLED 
                                    rdfs:label "CANCELLED" .


:MarketStatementDocType.CREDIT 
                               rdfs:label "CREDIT" .


:MarketStatementDocType.MARKET_INITIAL 
                                       rdfs:label "MARKET_INITIAL" .


:MarketStatementDocType.MARKET_RECALC 
                                      rdfs:label "MARKET_RECALC" .


:MarketStatementLineItemAliasName.CHARGE_CODE_INTERVAL_DETAIL 
                                                              rdfs:label "CHARGE_CODE_INTERVAL_DETAIL" .


:MarketStatementLineItemAliasName.CHARGE_CODE_INTERVAL_TOTAL 
                                                             rdfs:label "CHARGE_CODE_INTERVAL_TOTAL" .


:MarketStatementLineItemAliasName.CHARGE_CODE_SUMMARY 
                                                      rdfs:label "CHARGE_CODE_SUMMARY" .


:MarketStatementLineItemAliasName.CHARGE_GROUP 
                                               rdfs:label "CHARGE_GROUP" .


:MarketStatementLineItemAliasName.PARENT_CHARGE_GROUP 
                                                      rdfs:label "PARENT_CHARGE_GROUP" .


:MarketStatementLineItemAliasName.TRADE_DATE 
                                             rdfs:label "TRADE_DATE" .


:MarketType.DAM 
                rdfs:comment "Day ahead market." ;
                rdfs:label "DAM" .


:MarketType.HAM 
                rdfs:comment "Hour Ahead Market." ;
                rdfs:label "HAM" .


:MarketType.RTM 
                rdfs:comment "Real time market." ;
                rdfs:label "RTM" .


:MarketType.RUC 
                rdfs:comment "Residual Unit Commitment." ;
                rdfs:label "RUC" .


:MeasurementKind-Old.alarm uml:hasInitialValue "118" ;
                           
                           rdfs:comment "A measurement related to an alarm" ;
                           rdfs:label "alarm" .


:MeasurementKind-Old.apTitle uml:hasInitialValue "91" ;
                             
                             rdfs:comment "An application name which is making or has made a request" ;
                             rdfs:label "apTitle" .


:MeasurementKind-Old.apparentPowerFactor uml:hasInitialValue "2" ;
                                         
                                         rdfs:comment "The ratio of real energy (usually net Wh) to apparent energy (kVAh)" ;
                                         rdfs:label "apparentPowerFactor" .


:MeasurementKind-Old.applicationContext uml:hasInitialValue "90" ;
                                        
                                        rdfs:comment "Information that describes the logical context in which a request, measurement, or command is made." ;
                                        rdfs:label "applicationContext" .


:MeasurementKind-Old.assetNumber uml:hasInitialValue "92" ;
                                 
                                 rdfs:comment "An asset identifier" ;
                                 rdfs:label "assetNumber" .


:MeasurementKind-Old.audibleVolume uml:hasInitialValue "154" ;
                                   
                                   rdfs:comment "Sound" ;
                                   rdfs:label "audibleVolume" .


:MeasurementKind-Old.bandwidth uml:hasInitialValue "93" ;
                               
                               rdfs:comment "A measurement of dataflow" ;
                               rdfs:label "bandwidth" .


:MeasurementKind-Old.batteryCarryover uml:hasInitialValue "119" ;
                                      
                                      rdfs:comment "An estimate of the battery ride through capacity" ;
                                      rdfs:label "batteryCarryover" .


:MeasurementKind-Old.batteryVoltage uml:hasInitialValue "94" ;
                                    
                                    rdfs:comment "Battery voltage" ;
                                    rdfs:label "batteryVoltage" .


:MeasurementKind-Old.billCarryover uml:hasInitialValue "152" ;
                                   
                                   rdfs:comment "Customer’s bill for the (Currency)" ;
                                   rdfs:label "billCarryover" .


:MeasurementKind-Old.billLastPeriod uml:hasInitialValue "150" ;
                                    
                                    rdfs:comment "Customer’s bill for the previous billing period (Currency)" ;
                                    rdfs:label "billLastPeriod" .


:MeasurementKind-Old.billToDate uml:hasInitialValue "151" ;
                                
                                rdfs:comment "Customer’s bill, as known thus far within the present billing period (Currency)" ;
                                rdfs:label "billToDate" .


:MeasurementKind-Old.broadcastAddress uml:hasInitialValue "95" ;
                                      
                                      rdfs:comment "A message target address implying all endpoint units within range of a particular sender" ;
                                      rdfs:label "broadcastAddress" .


:MeasurementKind-Old.connectionFee uml:hasInitialValue "153" ;
                                   
                                   rdfs:comment "Monthly fee for connection to commodity." ;
                                   rdfs:label "connectionFee" .


:MeasurementKind-Old.currency uml:hasInitialValue "3" ;
                              
                              rdfs:comment "funds" ;
                              rdfs:label "currency" .


:MeasurementKind-Old.current uml:hasInitialValue "4" ;
                             
                             rdfs:comment "The flow of electrons" ;
                             rdfs:label "current" .


:MeasurementKind-Old.currentAngle uml:hasInitialValue "5" ;
                                  
                                  rdfs:comment "A phase current zerocross timing measurement releative to a reference voltage zerocross" ;
                                  rdfs:label "currentAngle" .


:MeasurementKind-Old.currentImbalance uml:hasInitialValue "6" ;
                                      
                                      rdfs:comment "A measurement of the departure of a phase current relative to the average current of all phases" ;
                                      rdfs:label "currentImbalance" .


:MeasurementKind-Old.dataOverflowAlarm uml:hasInitialValue "120" ;
                                       
                                       rdfs:comment "An indication of or measurement of a loss of data" ;
                                       rdfs:label "dataOverflowAlarm" .


:MeasurementKind-Old.date uml:hasInitialValue "7" ;
                          
                          rdfs:comment "A measurement of the date and/or time in a clock, or a time stamp indicating when data was captured, when a maximum or minimum occurred, or to commemorate some other important aspect of a measurement" ;
                          rdfs:label "date" .


:MeasurementKind-Old.demand uml:hasInitialValue "8" ;
                            
                            rdfs:comment "The measurement of maximum power flow which is computed as energy usage over time, the dimensions of which are defined by a tariff" ;
                            rdfs:label "demand" .


:MeasurementKind-Old.demandLimit uml:hasInitialValue "121" ;
                                 
                                 rdfs:comment "A threshold setting that determines the trip point that if exceeded would trigger a demand limiting action or alarm" ;
                                 rdfs:label "demandLimit" .


:MeasurementKind-Old.demandReset uml:hasInitialValue "122" ;
                                 
                                 rdfs:comment "A count of the number of times demand has been reset (remotely, locally, and/or automatically.)" ;
                                 rdfs:label "demandReset" .


:MeasurementKind-Old.deviceAddressType1 uml:hasInitialValue "96" ;
                                        
                                        rdfs:comment "Endpoint target address Type1" ;
                                        rdfs:label "deviceAddressType1" .


:MeasurementKind-Old.deviceAddressType2 uml:hasInitialValue "97" ;
                                        
                                        rdfs:comment "Endpoint target address Type2" ;
                                        rdfs:label "deviceAddressType2" .


:MeasurementKind-Old.deviceAddressType3 uml:hasInitialValue "98" ;
                                        
                                        rdfs:comment "Endpoint target address Type3" ;
                                        rdfs:label "deviceAddressType3" .


:MeasurementKind-Old.deviceAddressType4 uml:hasInitialValue "99" ;
                                        
                                        rdfs:comment "Endpoint target address Type4" ;
                                        rdfs:label "deviceAddressType4" .


:MeasurementKind-Old.deviceClass uml:hasInitialValue "100" ;
                                 
                                 rdfs:comment "A unique identifier for the Endpoint’s configuration" ;
                                 rdfs:label "deviceClass" .


:MeasurementKind-Old.diagnostic uml:hasInitialValue "123" ;
                                
                                rdfs:comment "A measurement related to equipment diagnostics" ;
                                rdfs:label "diagnostic" .


:MeasurementKind-Old.distance uml:hasInitialValue "9" ;
                              
                              rdfs:comment "A linear distance or range radius" ;
                              rdfs:label "distance" .


:MeasurementKind-Old.distortionPowerFactor uml:hasInitialValue "64" ;
                                           
                                           rdfs:comment "The ratio of the distortion VAh to the apparent VAh" ;
                                           rdfs:label "distortionPowerFactor" .


:MeasurementKind-Old.distortionVoltAmp uml:hasInitialValue "10" ;
                                       
                                       rdfs:comment "A measurement in which a V<sup>2</sup> I<sup>2</sup> term has both real and reactive components removed leaving only distortion. For example, distortion VAh = Sqrt( (V<sup>2</sup>h)(I<sup>2</sup>h) – (Wh)<sup>2</sup> – (VArh)<sup>2</sup>)" ;
                                       rdfs:label "distortionVoltAmp" .


:MeasurementKind-Old.electronicSerialNumber uml:hasInitialValue "101" ;
                                            
                                            rdfs:comment "A device serial number" ;
                                            rdfs:label "electronicSerialNumber" .


:MeasurementKind-Old.emergencyLimit uml:hasInitialValue "124" ;
                                    
                                    rdfs:comment "A setting that indicates an emergency limit" ;
                                    rdfs:label "emergencyLimit" .


:MeasurementKind-Old.encoderTamper uml:hasInitialValue "125" ;
                                   
                                   rdfs:comment "An indication of tampering with a meter encoder" ;
                                   rdfs:label "encoderTamper" .


:MeasurementKind-Old.endDeviceID uml:hasInitialValue "102" ;
                                 
                                 rdfs:comment "A unique identifier of the endDevice – the device providing measurements or under control of the network" ;
                                 rdfs:label "endDeviceID" .


:MeasurementKind-Old.energization uml:hasInitialValue "11" ;
                                  
                                  rdfs:comment "Pertaining to the presence of voltage" ;
                                  rdfs:label "energization" .


:MeasurementKind-Old.energizationLoadSide uml:hasInitialValue "13" ;
                                          
                                          rdfs:comment "Measuring the presence or absence of voltage on the load side of an electricity meter" ;
                                          rdfs:label "energizationLoadSide" .


:MeasurementKind-Old.energy uml:hasInitialValue "12" ;
                            
                            rdfs:comment "Scalar quantity which may be increased or decreased in a system when it receives or produces work, respectively" ;
                            rdfs:label "energy" .


:MeasurementKind-Old.fan uml:hasInitialValue "14" ;
                         
                         rdfs:comment "A forced air moving device" ;
                         rdfs:label "fan" .


:MeasurementKind-Old.frequency uml:hasInitialValue "15" ;
                               
                               rdfs:comment "Reciprocal of the period" ;
                               rdfs:label "frequency" .


:MeasurementKind-Old.frequencyExcursion uml:hasInitialValue "81" ;
                                        
                                        rdfs:comment "A measurement of the departure of the frequency from the nominal frequency" ;
                                        rdfs:label "frequencyExcursion" .


:MeasurementKind-Old.fund uml:hasInitialValue "16" ;
                          
                          rdfs:comment "Duplicate with “currency”" ;
                          rdfs:label "fund" .


:MeasurementKind-Old.groupAddressType1 uml:hasInitialValue "103" ;
                                       
                                       rdfs:comment "Group target address Type1" ;
                                       rdfs:label "groupAddressType1" .


:MeasurementKind-Old.groupAddressType2 uml:hasInitialValue "104" ;
                                       
                                       rdfs:comment "Group target address Type2" ;
                                       rdfs:label "groupAddressType2" .


:MeasurementKind-Old.groupAddressType3 uml:hasInitialValue "105" ;
                                       
                                       rdfs:comment "Group target address Type3" ;
                                       rdfs:label "groupAddressType3" .


:MeasurementKind-Old.groupAddressType4 uml:hasInitialValue "106" ;
                                       
                                       rdfs:comment "Group target address Type4" ;
                                       rdfs:label "groupAddressType4" .


:MeasurementKind-Old.ieee1366ASAI uml:hasInitialValue "17" ;
                                  
                                  rdfs:comment "A measurement of IEEE-1366 Average Service Availability Index" ;
                                  rdfs:label "ieee1366ASAI" .


:MeasurementKind-Old.ieee1366ASIDI uml:hasInitialValue "18" ;
                                   
                                   rdfs:comment "A measurement of the IEEE-1366 Average Service Interruption Duration Index" ;
                                   rdfs:label "ieee1366ASIDI" .


:MeasurementKind-Old.ieee1366ASIFI uml:hasInitialValue "19" ;
                                   
                                   rdfs:comment "A measurement of the IEEE-1366 Average Service Interruption Frequency Index" ;
                                   rdfs:label "ieee1366ASIFI" .


:MeasurementKind-Old.ieee1366CAIDI uml:hasInitialValue "20" ;
                                   
                                   rdfs:comment "A measurement of the IEEE-1366 Customer average interruption duration index" ;
                                   rdfs:label "ieee1366CAIDI" .


:MeasurementKind-Old.ieee1366CAIFI uml:hasInitialValue "21" ;
                                   
                                   rdfs:comment "A measurement of the IEEE-1366 Customer average interruption frequency index" ;
                                   rdfs:label "ieee1366CAIFI" .


:MeasurementKind-Old.ieee1366CEMIn uml:hasInitialValue "22" ;
                                   
                                   rdfs:comment "A measurement of the IEEE-1366 Customers Experiencing Multiple Interruptions" ;
                                   rdfs:label "ieee1366CEMIn" .


:MeasurementKind-Old.ieee1366CEMSMIn uml:hasInitialValue "23" ;
                                     
                                     rdfs:comment "A measurement of the IEEE-1366 Customers Experiencing Multiple Sustained and Momentary Interruptions" ;
                                     rdfs:label "ieee1366CEMSMIn" .


:MeasurementKind-Old.ieee1366CTAIDI uml:hasInitialValue "24" ;
                                    
                                    rdfs:comment "A measurement of the IEEE-1366 Customer Total Average Interruption Duration Index" ;
                                    rdfs:label "ieee1366CTAIDI" .


:MeasurementKind-Old.ieee1366MAIFI uml:hasInitialValue "25" ;
                                   
                                   rdfs:comment "A measurement of the IEEE-1366 Momentary Average Interruption Frequency Index" ;
                                   rdfs:label "ieee1366MAIFI" .


:MeasurementKind-Old.ieee1366MAIFIe uml:hasInitialValue "26" ;
                                    
                                    rdfs:comment "A measurement of the IEEE-1366 Momentary Average event Interruption Frequency Index" ;
                                    rdfs:label "ieee1366MAIFIe" .


:MeasurementKind-Old.ieee1366MomentaryInterruption uml:hasInitialValue "126" ;
                                                   
                                                   rdfs:comment "IEEE-1366 Momentary Interruption count" ;
                                                   rdfs:label "ieee1366MomentaryInterruption" .


:MeasurementKind-Old.ieee1366MomentaryInterruptionEvent uml:hasInitialValue "127" ;
                                                        
                                                        rdfs:comment "IEEE-1366 Momentary Interruption event count" ;
                                                        rdfs:label "ieee1366MomentaryInterruptionEvent" .


:MeasurementKind-Old.ieee1366SAIDI uml:hasInitialValue "27" ;
                                   
                                   rdfs:comment "IEEE-1366 System Average Interruption Duration Index" ;
                                   rdfs:label "ieee1366SAIDI" .


:MeasurementKind-Old.ieee1366SAIFI uml:hasInitialValue "28" ;
                                   
                                   rdfs:comment "IEEE-1366 System Average Interruption Frequency Index" ;
                                   rdfs:label "ieee1366SAIFI" .


:MeasurementKind-Old.ieee1366SustainedInterruption uml:hasInitialValue "128" ;
                                                   
                                                   rdfs:comment "IEEE-1366 Sustained Interruption duration" ;
                                                   rdfs:label "ieee1366SustainedInterruption" .


:MeasurementKind-Old.interruptionBehaviour uml:hasInitialValue "129" ;
                                           
                                           rdfs:comment "A measurement related to power interruptions (Note: often an interruption count or duration.)" ;
                                           rdfs:label "interruptionBehaviour" .


:MeasurementKind-Old.inversionTamper uml:hasInitialValue "130" ;
                                     
                                     rdfs:comment "A measurement related to inversion tamper (Note: typically a count of inversions)" ;
                                     rdfs:label "inversionTamper" .


:MeasurementKind-Old.ipAddress uml:hasInitialValue "107" ;
                               
                               rdfs:comment "An IP address for the endpoint" ;
                               rdfs:label "ipAddress" .


:MeasurementKind-Old.lineLoss uml:hasInitialValue "31" ;
                              
                              rdfs:comment "An energy, power, voltage, or current loss attributed to transmission or distribution line impedance" ;
                              rdfs:label "lineLoss" .


:MeasurementKind-Old.loadInterrupt uml:hasInitialValue "131" ;
                                   
                                   rdfs:comment "A measurement related to load interruption (Note: typically a load interruption count or measurement of duration)" ;
                                   rdfs:label "loadInterrupt" .


:MeasurementKind-Old.loadShed uml:hasInitialValue "132" ;
                              
                              rdfs:comment "A measurement related to load shed (Note: typically a load shed count or load shed duration)" ;
                              rdfs:label "loadShed" .


:MeasurementKind-Old.loss uml:hasInitialValue "32" ;
                          
                          rdfs:comment "A quantity lost due to “technical” reasons (such as line loss) or “non-technical” reasons (such as theft.)" ;
                          rdfs:label "loss" .


:MeasurementKind-Old.macAddress uml:hasInitialValue "108" ;
                                
                                rdfs:comment "A MAC address for the endpoint" ;
                                rdfs:label "macAddress" .


:MeasurementKind-Old.maintenance uml:hasInitialValue "133" ;
                                 
                                 rdfs:comment "A measurement related to the pending maintenance of equipment" ;
                                 rdfs:label "maintenance" .


:MeasurementKind-Old.mfgAssignedConfigurationID uml:hasInitialValue "109" ;
                                                
                                                rdfs:comment "The configuration given to a device at time of manufacture" ;
                                                rdfs:label "mfgAssignedConfigurationID" .


:MeasurementKind-Old.mfgAssignedPhysicalSerialNumber uml:hasInitialValue "110" ;
                                                     
                                                     rdfs:comment "The serial number assigned to a device at time of manufacture" ;
                                                     rdfs:label "mfgAssignedPhysicalSerialNumber" .


:MeasurementKind-Old.mfgAssignedProductNumber uml:hasInitialValue "111" ;
                                              
                                              rdfs:comment "The product number assigned to a device at time of manufacture" ;
                                              rdfs:label "mfgAssignedProductNumber" .


:MeasurementKind-Old.mfgAssignedUniqueCommunicationAddress uml:hasInitialValue "112" ;
                                                           
                                                           rdfs:comment "A communication address assigned to a device at time of manufacture" ;
                                                           rdfs:label "mfgAssignedUniqueCommunicationAddress" .


:MeasurementKind-Old.multiCastAddress uml:hasInitialValue "113" ;
                                      
                                      rdfs:comment "A message target address implying a large group of endpoint units within range of a particular sender" ;
                                      rdfs:label "multiCastAddress" .


:MeasurementKind-Old.negativeSequence uml:hasInitialValue "33" ;
                                      
                                      rdfs:comment "A quantity that has a rotation sequence which is opposite to that of the power system" ;
                                      rdfs:label "negativeSequence" .


:MeasurementKind-Old.none uml:hasInitialValue "0" ;
                          
                          rdfs:comment "Not Applicable" ;
                          rdfs:label "none" .


:MeasurementKind-Old.oneWayAddress uml:hasInitialValue "114" ;
                                   
                                   rdfs:comment "A communication address of a network endpoint used in one-way communication" ;
                                   rdfs:label "oneWayAddress" .


:MeasurementKind-Old.phasorPowerFactor uml:hasInitialValue "34" ;
                                       
                                       rdfs:comment "The ratio of real energy (usually net Wh) to phasor apparent energy (kVAh)" ;
                                       rdfs:label "phasorPowerFactor" .


:MeasurementKind-Old.phasorReactivePower uml:hasInitialValue "35" ;
                                         
                                         rdfs:comment "The ratio of real energy (usually net Wh) to phasor reactive energy (kVAh)" ;
                                         rdfs:label "phasorReactivePower" .


:MeasurementKind-Old.physicalTamper uml:hasInitialValue "134" ;
                                    
                                    rdfs:comment "A measurement related to physical tampering (Note: typically a tamper count)" ;
                                    rdfs:label "physicalTamper" .


:MeasurementKind-Old.positiveSequence uml:hasInitialValue "36" ;
                                      
                                      rdfs:comment "A quantity that has a rotation sequence in agreement with that of the power system" ;
                                      rdfs:label "positiveSequence" .


:MeasurementKind-Old.power uml:hasInitialValue "37" ;
                           
                           rdfs:comment "The derivative of energy with respect to time, where the energy is being transferred or transformed." ;
                           rdfs:label "power" .


:MeasurementKind-Old.powerFactor uml:hasInitialValue "38" ;
                                 
                                 rdfs:comment "The ratio of real energy (usually net Wh) to apparent energy (kVAh)" ;
                                 rdfs:label "powerFactor" .


:MeasurementKind-Old.powerLossTamper uml:hasInitialValue "135" ;
                                     
                                     rdfs:comment "Tamper indicated while power was out" ;
                                     rdfs:label "powerLossTamper" .


:MeasurementKind-Old.powerOutage uml:hasInitialValue "136" ;
                                 
                                 rdfs:comment "A measurement related to power outages (Note: typically a status)" ;
                                 rdfs:label "powerOutage" .


:MeasurementKind-Old.powerQuality uml:hasInitialValue "137" ;
                                  
                                  rdfs:comment "A measurement related to power quality" ;
                                  rdfs:label "powerQuality" .


:MeasurementKind-Old.powerRestoration uml:hasInitialValue "138" ;
                                      
                                      rdfs:comment "A measurement related to power restoration (Note: typically a status)" ;
                                      rdfs:label "powerRestoration" .


:MeasurementKind-Old.programmed uml:hasInitialValue "139" ;
                                
                                rdfs:comment "A measurement related to device programming (Note: typically a status measurement)" ;
                                rdfs:label "programmed" .


:MeasurementKind-Old.pushbutton uml:hasInitialValue "140" ;
                                
                                rdfs:comment "A measurement related to pushbutton (Note: typically a status or count)" ;
                                rdfs:label "pushbutton" .


:MeasurementKind-Old.quantityPower uml:hasInitialValue "40" ;
                                   
                                   rdfs:comment "A power measurement of Qh, where Qh is defined to be half of the sum of the Wh measurements on each phase plus the squareroot of 3 over two times the sum of the VArh measurements on each phase." ;
                                   rdfs:label "quantityPower" .


:MeasurementKind-Old.relayActivation uml:hasInitialValue "141" ;
                                     
                                     rdfs:comment "A measurement related to relay activations" ;
                                     rdfs:label "relayActivation" .


:MeasurementKind-Old.relayCycle uml:hasInitialValue "142" ;
                                
                                rdfs:comment "A measurement related to relay cycling (Note1: one open and one closure together is one cycle, Note2: Usually expressed as a count)" ;
                                rdfs:label "relayCycle" .


:MeasurementKind-Old.removalTamper uml:hasInitialValue "143" ;
                                   
                                   rdfs:comment "An indication of equipment tampering that shows equipment was moved or opened" ;
                                   rdfs:label "removalTamper" .


:MeasurementKind-Old.reprogrammingTamper uml:hasInitialValue "144" ;
                                         
                                         rdfs:comment "An indication of equipment tampering that shows equipment has been reprogrammed" ;
                                         rdfs:label "reprogrammingTamper" .


:MeasurementKind-Old.reverseRotationTamper uml:hasInitialValue "145" ;
                                           
                                           rdfs:comment "An indication of tampering as evidenced by reverse power flow" ;
                                           rdfs:label "reverseRotationTamper" .


:MeasurementKind-Old.sag uml:hasInitialValue "41" ;
                         
                         rdfs:comment "A temporary dip in the supply voltage below the nominal value" ;
                         rdfs:label "sag" .


:MeasurementKind-Old.signalStrength uml:hasInitialValue "115" ;
                                    
                                    rdfs:comment "A measurement of RF signal strength" ;
                                    rdfs:label "signalStrength" .


:MeasurementKind-Old.signaltoNoiseRatio uml:hasInitialValue "117" ;
                                        
                                        rdfs:comment "A measurement of received (RF) signal strength divided by the (RF) noise floor" ;
                                        rdfs:label "signaltoNoiseRatio" .


:MeasurementKind-Old.swell uml:hasInitialValue "42" ;
                           
                           rdfs:comment "A temporary rise of the supply voltage over the nominal value" ;
                           rdfs:label "swell" .


:MeasurementKind-Old.switchArmed uml:hasInitialValue "146" ;
                                 
                                 rdfs:comment "A measurement of the switch arm condition" ;
                                 rdfs:label "switchArmed" .


:MeasurementKind-Old.switchDisabled uml:hasInitialValue "147" ;
                                    
                                    rdfs:comment "A measurement of the switch enablement status" ;
                                    rdfs:label "switchDisabled" .


:MeasurementKind-Old.switchPosition uml:hasInitialValue "43" ;
                                    
                                    rdfs:comment "A physical or logical switch position status which includes “opened” and “closed”, but for some products may also include “armed,” or other states that indicate a temporary state due to some condition." ;
                                    rdfs:label "switchPosition" .


:MeasurementKind-Old.tamper uml:hasInitialValue "148" ;
                            
                            rdfs:comment "An indication of equipment tampering" ;
                            rdfs:label "tamper" .


:MeasurementKind-Old.tapPosition uml:hasInitialValue "44" ;
                                 
                                 rdfs:comment "Tap changer position" ;
                                 rdfs:label "tapPosition" .


:MeasurementKind-Old.tariffRate uml:hasInitialValue "45" ;
                                
                                rdfs:comment "An energy price defined in a contract. The rate might be a price for energy, for power (usually expressed as a demand value), or some other measurement. The rate might be currency based, or as a code, or as a component of a larger tariff description." ;
                                rdfs:label "tariffRate" .


:MeasurementKind-Old.temperature uml:hasInitialValue "46" ;
                                 
                                 rdfs:comment "A quantity proportional to the energy of a system" ;
                                 rdfs:label "temperature" .


:MeasurementKind-Old.totalHarmonicDistortion uml:hasInitialValue "47" ;
                                             
                                             rdfs:comment "The ratio of the sum of the harmonics to the fundamental. (THD may measure either voltage or current, and may isolated to a given phase)" ;
                                             rdfs:label "totalHarmonicDistortion" .


:MeasurementKind-Old.transformerLoss uml:hasInitialValue "48" ;
                                     
                                     rdfs:comment "A measurement of the energy or power loss in a transformer due to inefficiency" ;
                                     rdfs:label "transformerLoss" .


:MeasurementKind-Old.twoWayAddress uml:hasInitialValue "116" ;
                                   
                                   rdfs:comment "A communication address used for bidirectional communication" ;
                                   rdfs:label "twoWayAddress" .


:MeasurementKind-Old.unipedeVoltageDip10to15 uml:hasInitialValue "49" ;
                                             
                                             rdfs:comment "A voltage dip classification per EN50160 or a similar national standard measuring the number of dips in the 10-15% range" ;
                                             rdfs:label "unipedeVoltageDip10to15" .


:MeasurementKind-Old.unipedeVoltageDip15to30 uml:hasInitialValue "50" ;
                                             
                                             rdfs:comment "A voltage dip classification per EN50160 or a similar national standard measuring the number of dips in the 15-30% range" ;
                                             rdfs:label "unipedeVoltageDip15to30" .


:MeasurementKind-Old.unipedeVoltageDip30to60 uml:hasInitialValue "51" ;
                                             
                                             rdfs:comment "A voltage dip classification per EN50160 or a similar national standard measuring the number of dips in the 30-60% range" ;
                                             rdfs:label "unipedeVoltageDip30to60" .


:MeasurementKind-Old.unipedeVoltageDip60to90 uml:hasInitialValue "52" ;
                                             
                                             rdfs:comment "A voltage dip classification per EN50160 or a similar national standard measuring the number of dips in the 60-90% rangeA voltage dip classification per EN50160 or a similar national standard measuring the number of dips in the 60-90% range" ;
                                             rdfs:label "unipedeVoltageDip60to90" .


:MeasurementKind-Old.unipedeVoltageDip90to100 uml:hasInitialValue "53" ;
                                              
                                              rdfs:comment "A voltage dip classification per EN50160 or a similar national standard measuring the number of dips in the 90-100% range" ;
                                              rdfs:label "unipedeVoltageDip90to100" .


:MeasurementKind-Old.voltage uml:hasInitialValue "54" ;
                             
                             rdfs:comment "The difference in electric potential between two points" ;
                             rdfs:label "voltage" .


:MeasurementKind-Old.voltageAngle uml:hasInitialValue "55" ;
                                  
                                  rdfs:comment "A phase voltage zerocross timing measurement relative to a reference voltage zerocross" ;
                                  rdfs:label "voltageAngle" .


:MeasurementKind-Old.voltageExcursion uml:hasInitialValue "56" ;
                                      
                                      rdfs:comment "A measurement of the departure of the voltage from the nominal voltage" ;
                                      rdfs:label "voltageExcursion" .


:MeasurementKind-Old.voltageImbalance uml:hasInitialValue "57" ;
                                      
                                      rdfs:comment "A measurement of the departure of a phase voltage relative to the average voltage of all phases." ;
                                      rdfs:label "voltageImbalance" .


:MeasurementKind-Old.volume uml:hasInitialValue "58" ;
                            
                            rdfs:comment "fluid volume" ;
                            rdfs:label "volume" .


:MeasurementKind-Old.volumetricFlow uml:hasInitialValue "155" ;
                                    
                                    rdfs:comment "A fluid flow rate" ;
                                    rdfs:label "volumetricFlow" .


:MeasurementKind-Old.watchdogTimeout uml:hasInitialValue "149" ;
                                     
                                     rdfs:comment "A reset triggered by a hardware “watchdog” circuit" ;
                                     rdfs:label "watchdogTimeout" .


:MeasurementKind-Old.zeroFlowDuration uml:hasInitialValue "59" ;
                                      
                                      rdfs:comment "The amount of time that current flow drops to a zero level or level below the ability of the sensor to sense" ;
                                      rdfs:label "zeroFlowDuration" .


:MeasurementKind-Old.zeroSequence uml:hasInitialValue "60" ;
                                  
                                  rdfs:comment "The zero sequence current is the vector sum of the phase currents" ;
                                  rdfs:label "zeroSequence" .


:MeasurementKind.alarm uml:hasInitialValue "118" ;
                       
                       rdfs:comment "A measurement related to an alarm" ;
                       rdfs:label "alarm" .


:MeasurementKind.apTitle uml:hasInitialValue "91" ;
                         
                         rdfs:comment "An application name which is making or has made a request" ;
                         rdfs:label "apTitle" .


:MeasurementKind.apparentPowerFactor uml:hasInitialValue "2" ;
                                     
                                     rdfs:comment "The ratio of real energy (usually net Wh) to apparent energy (kVAh)" ;
                                     rdfs:label "apparentPowerFactor" .


:MeasurementKind.applicationContext uml:hasInitialValue "90" ;
                                    
                                    rdfs:comment "Information that describes the logical context in which a request, measurement, or command is made." ;
                                    rdfs:label "applicationContext" .


:MeasurementKind.assetNumber uml:hasInitialValue "92" ;
                             
                             rdfs:comment "An asset identifier" ;
                             rdfs:label "assetNumber" .


:MeasurementKind.audibleVolume uml:hasInitialValue "154" ;
                               
                               rdfs:comment "Sound" ;
                               rdfs:label "audibleVolume" .


:MeasurementKind.bandwidth uml:hasInitialValue "93" ;
                           
                           rdfs:comment "A measurement of dataflow" ;
                           rdfs:label "bandwidth" .


:MeasurementKind.batteryCarryover uml:hasInitialValue "119" ;
                                  
                                  rdfs:comment "An estimate of the battery ride through capacity" ;
                                  rdfs:label "batteryCarryover" .


:MeasurementKind.batteryVoltage uml:hasInitialValue "94" ;
                                
                                rdfs:comment "Battery voltage" ;
                                rdfs:label "batteryVoltage" .


:MeasurementKind.billCarryover uml:hasInitialValue "152" ;
                               
                               rdfs:comment "Customer’s bill for the (Currency)" ;
                               rdfs:label "billCarryover" .


:MeasurementKind.billLastPeriod uml:hasInitialValue "150" ;
                                
                                rdfs:comment "Customer’s bill for the previous billing period (Currency)" ;
                                rdfs:label "billLastPeriod" .


:MeasurementKind.billToDate uml:hasInitialValue "151" ;
                            
                            rdfs:comment "Customer’s bill, as known thus far within the present billing period (Currency)" ;
                            rdfs:label "billToDate" .


:MeasurementKind.broadcastAddress uml:hasInitialValue "95" ;
                                  
                                  rdfs:comment "A message target address implying all endpoint units within range of a particular sender" ;
                                  rdfs:label "broadcastAddress" .


:MeasurementKind.connectionFee uml:hasInitialValue "153" ;
                               
                               rdfs:comment "Monthly fee for connection to commodity." ;
                               rdfs:label "connectionFee" .


:MeasurementKind.currency uml:hasInitialValue "3" ;
                          
                          rdfs:comment "funds" ;
                          rdfs:label "currency" .


:MeasurementKind.current uml:hasInitialValue "4" ;
                         
                         rdfs:comment "The flow of electrons" ;
                         rdfs:label "current" .


:MeasurementKind.currentAngle uml:hasInitialValue "5" ;
                              
                              rdfs:comment "A phase current zerocross timing measurement releative to a reference voltage zerocross" ;
                              rdfs:label "currentAngle" .


:MeasurementKind.currentImbalance uml:hasInitialValue "6" ;
                                  
                                  rdfs:comment "A measurement of the departure of a phase current relative to the average current of all phases" ;
                                  rdfs:label "currentImbalance" .


:MeasurementKind.dataOverflowAlarm uml:hasInitialValue "120" ;
                                   
                                   rdfs:comment "An indication of or measurement of a loss of data" ;
                                   rdfs:label "dataOverflowAlarm" .


:MeasurementKind.date uml:hasInitialValue "7" ;
                      
                      rdfs:comment "A measurement of the date and/or time in a clock, or a time stamp indicating when data was captured, when a maximum or minimum occurred, or to commemorate some other important aspect of a measurement" ;
                      rdfs:label "date" .


:MeasurementKind.demand uml:hasInitialValue "8" ;
                        
                        rdfs:comment "The measurement of maximum power flow which is computed as energy usage over time, the dimensions of which are defined by a tariff" ;
                        rdfs:label "demand" .


:MeasurementKind.demandLimit uml:hasInitialValue "121" ;
                             
                             rdfs:comment "A threshold setting that determines the trip point that if exceeded would trigger a demand limiting action or alarm" ;
                             rdfs:label "demandLimit" .


:MeasurementKind.demandReset uml:hasInitialValue "122" ;
                             
                             rdfs:comment "A count of the number of times demand has been reset (remotely, locally, and/or automatically.)" ;
                             rdfs:label "demandReset" .


:MeasurementKind.deviceAddressType1 uml:hasInitialValue "96" ;
                                    
                                    rdfs:comment "Endpoint target address Type1" ;
                                    rdfs:label "deviceAddressType1" .


:MeasurementKind.deviceAddressType2 uml:hasInitialValue "97" ;
                                    
                                    rdfs:comment "Endpoint target address Type2" ;
                                    rdfs:label "deviceAddressType2" .


:MeasurementKind.deviceAddressType3 uml:hasInitialValue "98" ;
                                    
                                    rdfs:comment "Endpoint target address Type3" ;
                                    rdfs:label "deviceAddressType3" .


:MeasurementKind.deviceAddressType4 uml:hasInitialValue "99" ;
                                    
                                    rdfs:comment "Endpoint target address Type4" ;
                                    rdfs:label "deviceAddressType4" .


:MeasurementKind.deviceClass uml:hasInitialValue "100" ;
                             
                             rdfs:comment "A unique identifier for the Endpoint’s configuration" ;
                             rdfs:label "deviceClass" .


:MeasurementKind.diagnostic uml:hasInitialValue "123" ;
                            
                            rdfs:comment "A measurement related to equipment diagnostics" ;
                            rdfs:label "diagnostic" .


:MeasurementKind.distance uml:hasInitialValue "9" ;
                          
                          rdfs:comment "A linear distance or range radius" ;
                          rdfs:label "distance" .


:MeasurementKind.distortionPowerFactor uml:hasInitialValue "64" ;
                                       
                                       rdfs:comment "The ratio of the distortion VAh to the apparent VAh" ;
                                       rdfs:label "distortionPowerFactor" .


:MeasurementKind.distortionVoltAmp uml:hasInitialValue "10" ;
                                   
                                   rdfs:comment "A measurement in which a V<sup>2</sup> I<sup>2</sup> term has both real and reactive components removed leaving only distortion. For example, distortion VAh = Sqrt( (V<sup>2</sup>h)(I<sup>2</sup>h) – (Wh)<sup>2</sup> – (VArh)<sup>2</sup>)" ;
                                   rdfs:label "distortionVoltAmp" .


:MeasurementKind.electronicSerialNumber uml:hasInitialValue "101" ;
                                        
                                        rdfs:comment "A device serial number" ;
                                        rdfs:label "electronicSerialNumber" .


:MeasurementKind.emergencyLimit uml:hasInitialValue "124" ;
                                
                                rdfs:comment "A setting that indicates an emergency limit" ;
                                rdfs:label "emergencyLimit" .


:MeasurementKind.encoderTamper uml:hasInitialValue "125" ;
                               
                               rdfs:comment "An indication of tampering with a meter encoder" ;
                               rdfs:label "encoderTamper" .


:MeasurementKind.endDeviceID uml:hasInitialValue "102" ;
                             
                             rdfs:comment "A unique identifier of the endDevice – the device providing measurements or under control of the network" ;
                             rdfs:label "endDeviceID" .


:MeasurementKind.energization uml:hasInitialValue "11" ;
                              
                              rdfs:comment "Pertaining to the presence of voltage" ;
                              rdfs:label "energization" .


:MeasurementKind.energizationLoadSide uml:hasInitialValue "13" ;
                                      
                                      rdfs:comment "Measuring the presence or absence of voltage on the load side of an electricity meter" ;
                                      rdfs:label "energizationLoadSide" .


:MeasurementKind.energy uml:hasInitialValue "12" ;
                        
                        rdfs:comment "Scalar quantity which may be increased or decreased in a system when it receives or produces work, respectively" ;
                        rdfs:label "energy" .


:MeasurementKind.fan uml:hasInitialValue "14" ;
                     
                     rdfs:comment "A forced air moving device" ;
                     rdfs:label "fan" .


:MeasurementKind.frequency uml:hasInitialValue "15" ;
                           
                           rdfs:comment "Reciprocal of the period" ;
                           rdfs:label "frequency" .


:MeasurementKind.frequencyExcursion uml:hasInitialValue "81" ;
                                    
                                    rdfs:comment "A measurement of the departure of the frequency from the nominal frequency" ;
                                    rdfs:label "frequencyExcursion" .


:MeasurementKind.fund uml:hasInitialValue "16" ;
                      
                      rdfs:comment "Duplicate with “currency”" ;
                      rdfs:label "fund" .


:MeasurementKind.groupAddressType1 uml:hasInitialValue "103" ;
                                   
                                   rdfs:comment "Group target address Type1" ;
                                   rdfs:label "groupAddressType1" .


:MeasurementKind.groupAddressType2 uml:hasInitialValue "104" ;
                                   
                                   rdfs:comment "Group target address Type2" ;
                                   rdfs:label "groupAddressType2" .


:MeasurementKind.groupAddressType3 uml:hasInitialValue "105" ;
                                   
                                   rdfs:comment "Group target address Type3" ;
                                   rdfs:label "groupAddressType3" .


:MeasurementKind.groupAddressType4 uml:hasInitialValue "106" ;
                                   
                                   rdfs:comment "Group target address Type4" ;
                                   rdfs:label "groupAddressType4" .


:MeasurementKind.ieee1366ASAI uml:hasInitialValue "17" ;
                              
                              rdfs:comment "A measurement of IEEE-1366 Average Service Availability Index" ;
                              rdfs:label "ieee1366ASAI" .


:MeasurementKind.ieee1366ASIDI uml:hasInitialValue "18" ;
                               
                               rdfs:comment "A measurement of the IEEE-1366 Average Service Interruption Duration Index" ;
                               rdfs:label "ieee1366ASIDI" .


:MeasurementKind.ieee1366ASIFI uml:hasInitialValue "19" ;
                               
                               rdfs:comment "A measurement of the IEEE-1366 Average Service Interruption Frequency Index" ;
                               rdfs:label "ieee1366ASIFI" .


:MeasurementKind.ieee1366CAIDI uml:hasInitialValue "20" ;
                               
                               rdfs:comment "A measurement of the IEEE-1366 Customer average interruption duration index" ;
                               rdfs:label "ieee1366CAIDI" .


:MeasurementKind.ieee1366CAIFI uml:hasInitialValue "21" ;
                               
                               rdfs:comment "A measurement of the IEEE-1366 Customer average interruption frequency index" ;
                               rdfs:label "ieee1366CAIFI" .


:MeasurementKind.ieee1366CEMIn uml:hasInitialValue "22" ;
                               
                               rdfs:comment "A measurement of the IEEE-1366 Customers Experiencing Multiple Interruptions" ;
                               rdfs:label "ieee1366CEMIn" .


:MeasurementKind.ieee1366CEMSMIn uml:hasInitialValue "23" ;
                                 
                                 rdfs:comment "A measurement of the IEEE-1366 Customers Experiencing Multiple Sustained and Momentary Interruptions" ;
                                 rdfs:label "ieee1366CEMSMIn" .


:MeasurementKind.ieee1366CTAIDI uml:hasInitialValue "24" ;
                                
                                rdfs:comment "A measurement of the IEEE-1366 Customer Total Average Interruption Duration Index" ;
                                rdfs:label "ieee1366CTAIDI" .


:MeasurementKind.ieee1366MAIFI uml:hasInitialValue "25" ;
                               
                               rdfs:comment "A measurement of the IEEE-1366 Momentary Average Interruption Frequency Index" ;
                               rdfs:label "ieee1366MAIFI" .


:MeasurementKind.ieee1366MAIFIe uml:hasInitialValue "26" ;
                                
                                rdfs:comment "A measurement of the IEEE-1366 Momentary Average event Interruption Frequency Index" ;
                                rdfs:label "ieee1366MAIFIe" .


:MeasurementKind.ieee1366MomentaryInterruption uml:hasInitialValue "126" ;
                                               
                                               rdfs:comment "IEEE-1366 Momentary Interruption count" ;
                                               rdfs:label "ieee1366MomentaryInterruption" .


:MeasurementKind.ieee1366MomentaryInterruptionEvent uml:hasInitialValue "127" ;
                                                    
                                                    rdfs:comment "IEEE-1366 Momentary Interruption event count" ;
                                                    rdfs:label "ieee1366MomentaryInterruptionEvent" .


:MeasurementKind.ieee1366SAIDI uml:hasInitialValue "27" ;
                               
                               rdfs:comment "IEEE-1366 System Average Interruption Duration Index" ;
                               rdfs:label "ieee1366SAIDI" .


:MeasurementKind.ieee1366SAIFI uml:hasInitialValue "28" ;
                               
                               rdfs:comment "IEEE-1366 System Average Interruption Frequency Index" ;
                               rdfs:label "ieee1366SAIFI" .


:MeasurementKind.ieee1366SustainedInterruption uml:hasInitialValue "128" ;
                                               
                                               rdfs:comment "IEEE-1366 Sustained Interruption duration" ;
                                               rdfs:label "ieee1366SustainedInterruption" .


:MeasurementKind.interruptionBehaviour uml:hasInitialValue "129" ;
                                       
                                       rdfs:comment "A measurement related to power interruptions (Note: often an interruption count or duration.)" ;
                                       rdfs:label "interruptionBehaviour" .


:MeasurementKind.inversionTamper uml:hasInitialValue "130" ;
                                 
                                 rdfs:comment "A measurement related to inversion tamper (Note: typically a count of inversions)" ;
                                 rdfs:label "inversionTamper" .


:MeasurementKind.ipAddress uml:hasInitialValue "107" ;
                           
                           rdfs:comment "An IP address for the endpoint" ;
                           rdfs:label "ipAddress" .


:MeasurementKind.lineLoss uml:hasInitialValue "31" ;
                          
                          rdfs:comment "An energy, power, voltage, or current loss attributed to transmission or distribution line impedance" ;
                          rdfs:label "lineLoss" .


:MeasurementKind.loadInterrupt uml:hasInitialValue "131" ;
                               
                               rdfs:comment "A measurement related to load interruption (Note: typically a load interruption count or measurement of duration)" ;
                               rdfs:label "loadInterrupt" .


:MeasurementKind.loadShed uml:hasInitialValue "132" ;
                          
                          rdfs:comment "A measurement related to load shed (Note: typically a load shed count or load shed duration)" ;
                          rdfs:label "loadShed" .


:MeasurementKind.loss uml:hasInitialValue "32" ;
                      
                      rdfs:comment "A quantity lost due to “technical” reasons (such as line loss) or “non-technical” reasons (such as theft.)" ;
                      rdfs:label "loss" .


:MeasurementKind.macAddress uml:hasInitialValue "108" ;
                            
                            rdfs:comment "A MAC address for the endpoint" ;
                            rdfs:label "macAddress" .


:MeasurementKind.maintenance uml:hasInitialValue "133" ;
                             
                             rdfs:comment "A measurement related to the pending maintenance of equipment" ;
                             rdfs:label "maintenance" .


:MeasurementKind.mfgAssignedConfigurationID uml:hasInitialValue "109" ;
                                            
                                            rdfs:comment "The configuration given to a device at time of manufacture" ;
                                            rdfs:label "mfgAssignedConfigurationID" .


:MeasurementKind.mfgAssignedPhysicalSerialNumber uml:hasInitialValue "110" ;
                                                 
                                                 rdfs:comment "The serial number assigned to a device at time of manufacture" ;
                                                 rdfs:label "mfgAssignedPhysicalSerialNumber" .


:MeasurementKind.mfgAssignedProductNumber uml:hasInitialValue "111" ;
                                          
                                          rdfs:comment "The product number assigned to a device at time of manufacture" ;
                                          rdfs:label "mfgAssignedProductNumber" .


:MeasurementKind.mfgAssignedUniqueCommunicationAddress uml:hasInitialValue "112" ;
                                                       
                                                       rdfs:comment "A communication address assigned to a device at time of manufacture" ;
                                                       rdfs:label "mfgAssignedUniqueCommunicationAddress" .


:MeasurementKind.multiCastAddress uml:hasInitialValue "113" ;
                                  
                                  rdfs:comment "A message target address implying a large group of endpoint units within range of a particular sender" ;
                                  rdfs:label "multiCastAddress" .


:MeasurementKind.negativeSequence uml:hasInitialValue "33" ;
                                  
                                  rdfs:comment "A quantity that has a rotation sequence which is opposite to that of the power system" ;
                                  rdfs:label "negativeSequence" .


:MeasurementKind.none uml:hasInitialValue "0" ;
                      
                      rdfs:comment "Not Applicable" ;
                      rdfs:label "none" .


:MeasurementKind.oneWayAddress uml:hasInitialValue "114" ;
                               
                               rdfs:comment "A communication address of a network endpoint used in one-way communication" ;
                               rdfs:label "oneWayAddress" .


:MeasurementKind.phasorPowerFactor uml:hasInitialValue "34" ;
                                   
                                   rdfs:comment "The ratio of real energy (usually net Wh) to phasor apparent energy (kVAh)" ;
                                   rdfs:label "phasorPowerFactor" .


:MeasurementKind.phasorReactivePower uml:hasInitialValue "35" ;
                                     
                                     rdfs:comment "The ratio of real energy (usually net Wh) to phasor reactive energy (kVAh)" ;
                                     rdfs:label "phasorReactivePower" .


:MeasurementKind.physicalTamper uml:hasInitialValue "134" ;
                                
                                rdfs:comment "A measurement related to physical tampering (Note: typically a tamper count)" ;
                                rdfs:label "physicalTamper" .


:MeasurementKind.positiveSequence uml:hasInitialValue "36" ;
                                  
                                  rdfs:comment "A quantity that has a rotation sequence in agreement with that of the power system" ;
                                  rdfs:label "positiveSequence" .


:MeasurementKind.power uml:hasInitialValue "37" ;
                       
                       rdfs:comment "The derivative of energy with respect to time, where the energy is being transferred or transformed." ;
                       rdfs:label "power" .


:MeasurementKind.powerFactor uml:hasInitialValue "38" ;
                             
                             rdfs:comment "The ratio of real energy (usually net Wh) to apparent energy (kVAh)" ;
                             rdfs:label "powerFactor" .


:MeasurementKind.powerLossTamper uml:hasInitialValue "135" ;
                                 
                                 rdfs:comment "Tamper indicated while power was out" ;
                                 rdfs:label "powerLossTamper" .


:MeasurementKind.powerOutage uml:hasInitialValue "136" ;
                             
                             rdfs:comment "A measurement related to power outages (Note: typically a status)" ;
                             rdfs:label "powerOutage" .


:MeasurementKind.powerQuality uml:hasInitialValue "137" ;
                              
                              rdfs:comment "A measurement related to power quality" ;
                              rdfs:label "powerQuality" .


:MeasurementKind.powerRestoration uml:hasInitialValue "138" ;
                                  
                                  rdfs:comment "A measurement related to power restoration (Note: typically a status)" ;
                                  rdfs:label "powerRestoration" .


:MeasurementKind.programmed uml:hasInitialValue "139" ;
                            
                            rdfs:comment "A measurement related to device programming (Note: typically a status measurement)" ;
                            rdfs:label "programmed" .


:MeasurementKind.pushbutton uml:hasInitialValue "140" ;
                            
                            rdfs:comment "A measurement related to pushbutton (Note: typically a status or count)" ;
                            rdfs:label "pushbutton" .


:MeasurementKind.quantityPower uml:hasInitialValue "40" ;
                               
                               rdfs:comment "A power measurement of Qh, where Qh is defined to be half of the sum of the Wh measurements on each phase plus the squareroot of 3 over two times the sum of the VArh measurements on each phase." ;
                               rdfs:label "quantityPower" .


:MeasurementKind.relayActivation uml:hasInitialValue "141" ;
                                 
                                 rdfs:comment "A measurement related to relay activations" ;
                                 rdfs:label "relayActivation" .


:MeasurementKind.relayCycle uml:hasInitialValue "142" ;
                            
                            rdfs:comment "A measurement related to relay cycling (Note1: one open and one closure together is one cycle, Note2: Usually expressed as a count)" ;
                            rdfs:label "relayCycle" .


:MeasurementKind.removalTamper uml:hasInitialValue "143" ;
                               
                               rdfs:comment "An indication of equipment tampering that shows equipment was moved or opened" ;
                               rdfs:label "removalTamper" .


:MeasurementKind.reprogrammingTamper uml:hasInitialValue "144" ;
                                     
                                     rdfs:comment "An indication of equipment tampering that shows equipment has been reprogrammed" ;
                                     rdfs:label "reprogrammingTamper" .


:MeasurementKind.reverseRotationTamper uml:hasInitialValue "145" ;
                                       
                                       rdfs:comment "An indication of tampering as evidenced by reverse power flow" ;
                                       rdfs:label "reverseRotationTamper" .


:MeasurementKind.sag uml:hasInitialValue "41" ;
                     
                     rdfs:comment "A temporary dip in the supply voltage below the nominal value" ;
                     rdfs:label "sag" .


:MeasurementKind.signalStrength uml:hasInitialValue "115" ;
                                
                                rdfs:comment "A measurement of RF signal strength" ;
                                rdfs:label "signalStrength" .


:MeasurementKind.signaltoNoiseRatio uml:hasInitialValue "117" ;
                                    
                                    rdfs:comment "A measurement of received (RF) signal strength divided by the (RF) noise floor" ;
                                    rdfs:label "signaltoNoiseRatio" .


:MeasurementKind.swell uml:hasInitialValue "42" ;
                       
                       rdfs:comment "A temporary rise of the supply voltage over the nominal value" ;
                       rdfs:label "swell" .


:MeasurementKind.switchArmed uml:hasInitialValue "146" ;
                             
                             rdfs:comment "A measurement of the switch arm condition" ;
                             rdfs:label "switchArmed" .


:MeasurementKind.switchDisabled uml:hasInitialValue "147" ;
                                
                                rdfs:comment "A measurement of the switch enablement status" ;
                                rdfs:label "switchDisabled" .


:MeasurementKind.switchPosition uml:hasInitialValue "43" ;
                                
                                rdfs:comment "A physical or logical switch position status which includes “opened” and “closed”, but for some products may also include “armed,” or other states that indicate a temporary state due to some condition." ;
                                rdfs:label "switchPosition" .


:MeasurementKind.tamper uml:hasInitialValue "148" ;
                        
                        rdfs:comment "An indication of equipment tampering" ;
                        rdfs:label "tamper" .


:MeasurementKind.tapPosition uml:hasInitialValue "44" ;
                             
                             rdfs:comment "Tap changer position" ;
                             rdfs:label "tapPosition" .


:MeasurementKind.tariffRate uml:hasInitialValue "45" ;
                            
                            rdfs:comment "An energy price defined in a contract. The rate might be a price for energy, for power (usually expressed as a demand value), or some other measurement. The rate might be currency based, or as a code, or as a component of a larger tariff description." ;
                            rdfs:label "tariffRate" .


:MeasurementKind.temperature uml:hasInitialValue "46" ;
                             
                             rdfs:comment "A quantity proportional to the energy of a system" ;
                             rdfs:label "temperature" .


:MeasurementKind.totalHarmonicDistortion uml:hasInitialValue "47" ;
                                         
                                         rdfs:comment "The ratio of the sum of the harmonics to the fundamental. (THD may measure either voltage or current, and may isolated to a given phase)" ;
                                         rdfs:label "totalHarmonicDistortion" .


:MeasurementKind.transformerLoss uml:hasInitialValue "48" ;
                                 
                                 rdfs:comment "A measurement of the energy or power loss in a transformer due to inefficiency" ;
                                 rdfs:label "transformerLoss" .


:MeasurementKind.twoWayAddress uml:hasInitialValue "116" ;
                               
                               rdfs:comment "A communication address used for bidirectional communication" ;
                               rdfs:label "twoWayAddress" .


:MeasurementKind.unipedeVoltageDip10to15 uml:hasInitialValue "49" ;
                                         
                                         rdfs:comment "A voltage dip classification per EN50160 or a similar national standard measuring the number of dips in the 10-15% range" ;
                                         rdfs:label "unipedeVoltageDip10to15" .


:MeasurementKind.unipedeVoltageDip15to30 uml:hasInitialValue "50" ;
                                         
                                         rdfs:comment "A voltage dip classification per EN50160 or a similar national standard measuring the number of dips in the 15-30% range" ;
                                         rdfs:label "unipedeVoltageDip15to30" .


:MeasurementKind.unipedeVoltageDip30to60 uml:hasInitialValue "51" ;
                                         
                                         rdfs:comment "A voltage dip classification per EN50160 or a similar national standard measuring the number of dips in the 30-60% range" ;
                                         rdfs:label "unipedeVoltageDip30to60" .


:MeasurementKind.unipedeVoltageDip60to90 uml:hasInitialValue "52" ;
                                         
                                         rdfs:comment "A voltage dip classification per EN50160 or a similar national standard measuring the number of dips in the 60-90% rangeA voltage dip classification per EN50160 or a similar national standard measuring the number of dips in the 60-90% range" ;
                                         rdfs:label "unipedeVoltageDip60to90" .


:MeasurementKind.unipedeVoltageDip90to100 uml:hasInitialValue "53" ;
                                          
                                          rdfs:comment "A voltage dip classification per EN50160 or a similar national standard measuring the number of dips in the 90-100% range" ;
                                          rdfs:label "unipedeVoltageDip90to100" .


:MeasurementKind.voltage uml:hasInitialValue "54" ;
                         
                         rdfs:comment "The difference in electric potential between two points" ;
                         rdfs:label "voltage" .


:MeasurementKind.voltageAngle uml:hasInitialValue "55" ;
                              
                              rdfs:comment "A phase voltage zerocross timing measurement relative to a reference voltage zerocross" ;
                              rdfs:label "voltageAngle" .


:MeasurementKind.voltageExcursion uml:hasInitialValue "56" ;
                                  
                                  rdfs:comment "A measurement of the departure of the voltage from the nominal voltage" ;
                                  rdfs:label "voltageExcursion" .


:MeasurementKind.voltageImbalance uml:hasInitialValue "57" ;
                                  
                                  rdfs:comment "A measurement of the departure of a phase voltage relative to the average voltage of all phases." ;
                                  rdfs:label "voltageImbalance" .


:MeasurementKind.volume uml:hasInitialValue "58" ;
                        
                        rdfs:comment "fluid volume" ;
                        rdfs:label "volume" .


:MeasurementKind.volumetricFlow uml:hasInitialValue "155" ;
                                
                                rdfs:comment "A fluid flow rate" ;
                                rdfs:label "volumetricFlow" .


:MeasurementKind.watchdogTimeout uml:hasInitialValue "149" ;
                                 
                                 rdfs:comment "A reset triggered by a hardware “watchdog” circuit" ;
                                 rdfs:label "watchdogTimeout" .


:MeasurementKind.zeroFlowDuration uml:hasInitialValue "59" ;
                                  
                                  rdfs:comment "The amount of time that current flow drops to a zero level or level below the ability of the sensor to sense" ;
                                  rdfs:label "zeroFlowDuration" .


:MeasurementKind.zeroSequence uml:hasInitialValue "60" ;
                              
                              rdfs:comment "The zero sequence current is the vector sum of the phase currents" ;
                              rdfs:label "zeroSequence" .


:MeasurementTypeEMS.ACE 
                        rdfs:label "ACE" .


:MeasurementTypeEMS.GMOL 
                         rdfs:label "GMOL" .


:MeasurementTypeEMS.GNOL 
                         rdfs:label "GNOL" .


:MeasurementTypeEMS.GO 
                       rdfs:label "GO" .


:MeasurementTypeEMS.GR 
                       rdfs:label "GR" .


:MeasurementTypeEMS.GS 
                       rdfs:label "GS" .


:MeasurementTypeEMS.INADV 
                          rdfs:label "INADV" .


:MeasurementTypeEMS.OARL 
                         rdfs:label "OARL" .


:MeasurementTypeEMS.PF 
                       rdfs:label "PF" .


:MeasurementTypeEMS.PIAL 
                         rdfs:label "PIAL" .


:MeasurementTypeEMS.PIL 
                        rdfs:label "PIL" .


:MeasurementTypeEMS.PIML 
                         rdfs:label "PIML" .


:MeasurementTypeEMS.POAL 
                         rdfs:label "POAL" .


:MeasurementTypeEMS.POL 
                        rdfs:label "POL" .


:MeasurementTypeEMS.PP 
                       rdfs:label "PP" .


:MeasurementTypeEMS.SL 
                       rdfs:label "SL" .


:MeasuringPeriodKind.fifteenMinute uml:hasInitialValue "2" ;
                                   
                                   rdfs:comment "15-minute" ;
                                   rdfs:label "fifteenMinute" .


:MeasuringPeriodKind.fiveMinute uml:hasInitialValue "6" ;
                                
                                rdfs:comment "5-minute" ;
                                rdfs:label "fiveMinute" .


:MeasuringPeriodKind.fixedBlock10Min uml:hasInitialValue "54" ;
                                     
                                     rdfs:comment "10-minute Fixed Block" ;
                                     rdfs:label "fixedBlock10Min" .


:MeasuringPeriodKind.fixedBlock15Min uml:hasInitialValue "53" ;
                                     
                                     rdfs:comment "15-minute Fixed Block" ;
                                     rdfs:label "fixedBlock15Min" .


:MeasuringPeriodKind.fixedBlock1Min uml:hasInitialValue "56" ;
                                    
                                    rdfs:comment "1-minute Fixed Block" ;
                                    rdfs:label "fixedBlock1Min" .


:MeasuringPeriodKind.fixedBlock20Min uml:hasInitialValue "52" ;
                                     
                                     rdfs:comment "20-minute Fixed Block" ;
                                     rdfs:label "fixedBlock20Min" .


:MeasuringPeriodKind.fixedBlock30Min uml:hasInitialValue "51" ;
                                     
                                     rdfs:comment "30-minute Fixed Block" ;
                                     rdfs:label "fixedBlock30Min" .


:MeasuringPeriodKind.fixedBlock5Min uml:hasInitialValue "55" ;
                                    
                                    rdfs:comment "5-minute Fixed Block" ;
                                    rdfs:label "fixedBlock5Min" .


:MeasuringPeriodKind.fixedBlock60Min uml:hasInitialValue "50" ;
                                     
                                     rdfs:comment "60-minute Fixed Block" ;
                                     rdfs:label "fixedBlock60Min" .


:MeasuringPeriodKind.none uml:hasInitialValue "0" ;
                          
                          rdfs:comment "Not applicable." ;
                          rdfs:label "none" .


:MeasuringPeriodKind.oneMinute uml:hasInitialValue "3" ;
                               
                               rdfs:comment "1-minute" ;
                               rdfs:label "oneMinute" .


:MeasuringPeriodKind.present uml:hasInitialValue "15" ;
                             
                             rdfs:comment "Within the present period of time" ;
                             rdfs:label "present" .


:MeasuringPeriodKind.previous uml:hasInitialValue "16" ;
                              
                              rdfs:comment "Shifted within the previous monthly cycle and data set" ;
                              rdfs:label "previous" .


:MeasuringPeriodKind.rollingBlock10MinIntvl1MinSubIntvl uml:hasInitialValue "76" ;
                                                        
                                                        rdfs:comment "10-minute Rolling Block with 1-minute sub-intervals" ;
                                                        rdfs:label "rollingBlock10MinIntvl1MinSubIntvl" .


:MeasuringPeriodKind.rollingBlock10MinIntvl2MinSubIntvl uml:hasInitialValue "75" ;
                                                        
                                                        rdfs:comment "10-minute Rolling Block with 2-minute sub-intervals" ;
                                                        rdfs:label "rollingBlock10MinIntvl2MinSubIntvl" .


:MeasuringPeriodKind.rollingBlock10MinIntvl5MinSubIntvl uml:hasInitialValue "74" ;
                                                        
                                                        rdfs:comment "10-minute Rolling Block with 5-minute sub-intervals" ;
                                                        rdfs:label "rollingBlock10MinIntvl5MinSubIntvl" .


:MeasuringPeriodKind.rollingBlock15MinIntvl1MinSubIntvl uml:hasInitialValue "73" ;
                                                        
                                                        rdfs:comment "15-minute Rolling Block with 1-minute sub-intervals" ;
                                                        rdfs:label "rollingBlock15MinIntvl1MinSubIntvl" .


:MeasuringPeriodKind.rollingBlock15MinIntvl3MinSubIntvl uml:hasInitialValue "72" ;
                                                        
                                                        rdfs:comment "15-minute Rolling Block with 3-minute sub-intervals" ;
                                                        rdfs:label "rollingBlock15MinIntvl3MinSubIntvl" .


:MeasuringPeriodKind.rollingBlock15MinIntvl5MinSubIntvl uml:hasInitialValue "71" ;
                                                        
                                                        rdfs:comment "15-minute Rolling Block with 5-minute sub-intervals" ;
                                                        rdfs:label "rollingBlock15MinIntvl5MinSubIntvl" .


:MeasuringPeriodKind.rollingBlock30MinIntvl10MinSubIntvl uml:hasInitialValue "66" ;
                                                         
                                                         rdfs:comment "30-minute Rolling Block with 10-minute sub-intervals" ;
                                                         rdfs:label "rollingBlock30MinIntvl10MinSubIntvl" .


:MeasuringPeriodKind.rollingBlock30MinIntvl15MinSubIntvl uml:hasInitialValue "65" ;
                                                         
                                                         rdfs:comment "30-minute Rolling Block with 15-minute sub-intervals" ;
                                                         rdfs:label "rollingBlock30MinIntvl15MinSubIntvl" .


:MeasuringPeriodKind.rollingBlock30MinIntvl2MinSubIntvl uml:hasInitialValue "70" ;
                                                        
                                                        rdfs:comment "30-minute Rolling Block with 2-minute sub-intervals" ;
                                                        rdfs:label "rollingBlock30MinIntvl2MinSubIntvl" .


:MeasuringPeriodKind.rollingBlock30MinIntvl3MinSubIntvl uml:hasInitialValue "69" ;
                                                        
                                                        rdfs:comment "30-minute Rolling Block with 3-minute sub-intervals" ;
                                                        rdfs:label "rollingBlock30MinIntvl3MinSubIntvl" .


:MeasuringPeriodKind.rollingBlock30MinIntvl5MinSubIntvl uml:hasInitialValue "68" ;
                                                        
                                                        rdfs:comment "30-minute Rolling Block with 5-minute sub-intervals." ;
                                                        rdfs:label "rollingBlock30MinIntvl5MinSubIntvl" .


:MeasuringPeriodKind.rollingBlock30MinIntvl6MinSubIntvl uml:hasInitialValue "67" ;
                                                        
                                                        rdfs:comment "30-minute Rolling Block with 6-minute sub-intervals" ;
                                                        rdfs:label "rollingBlock30MinIntvl6MinSubIntvl" .


:MeasuringPeriodKind.rollingBlock5MinIntvl1MinSubIntvl uml:hasInitialValue "77" ;
                                                       
                                                       rdfs:comment "5-minute Rolling Block with 1-minute sub-intervals" ;
                                                       rdfs:label "rollingBlock5MinIntvl1MinSubIntvl" .


:MeasuringPeriodKind.rollingBlock60MinIntvl10MinSubIntvl uml:hasInitialValue "61" ;
                                                         
                                                         rdfs:comment "60-minute Rolling Block with 10-minute sub-intervals" ;
                                                         rdfs:label "rollingBlock60MinIntvl10MinSubIntvl" .


:MeasuringPeriodKind.rollingBlock60MinIntvl12MinSubIntvl uml:hasInitialValue "60" ;
                                                         
                                                         rdfs:comment "60-minute Rolling Block with 12-minute sub-intervals" ;
                                                         rdfs:label "rollingBlock60MinIntvl12MinSubIntvl" .


:MeasuringPeriodKind.rollingBlock60MinIntvl15MinSubIntvl uml:hasInitialValue "59" ;
                                                         
                                                         rdfs:comment "60-minute Rolling Block with 15-minute sub-intervals" ;
                                                         rdfs:label "rollingBlock60MinIntvl15MinSubIntvl" .


:MeasuringPeriodKind.rollingBlock60MinIntvl20MinSubIntvl uml:hasInitialValue "58" ;
                                                         
                                                         rdfs:comment "60-minute Rolling Block with 20-minute sub-intervals" ;
                                                         rdfs:label "rollingBlock60MinIntvl20MinSubIntvl" .


:MeasuringPeriodKind.rollingBlock60MinIntvl30MinSubIntvl uml:hasInitialValue "57" ;
                                                         
                                                         rdfs:comment "60-minute Rolling Block with 30-minute sub-intervals" ;
                                                         rdfs:label "rollingBlock60MinIntvl30MinSubIntvl" .


:MeasuringPeriodKind.rollingBlock60MinIntvl4MinSubIntvl uml:hasInitialValue "64" ;
                                                        
                                                        rdfs:comment "60-minute Rolling Block with 4-minute sub-intervals" ;
                                                        rdfs:label "rollingBlock60MinIntvl4MinSubIntvl" .


:MeasuringPeriodKind.rollingBlock60MinIntvl5MinSubIntvl uml:hasInitialValue "63" ;
                                                        
                                                        rdfs:comment "60-minute Rolling Block with 5-minute sub-intervals" ;
                                                        rdfs:label "rollingBlock60MinIntvl5MinSubIntvl" .


:MeasuringPeriodKind.rollingBlock60MinIntvl6MinSubIntvl uml:hasInitialValue "62" ;
                                                        
                                                        rdfs:comment "60-minute Rolling Block with 6-minute sub-intervals" ;
                                                        rdfs:label "rollingBlock60MinIntvl6MinSubIntvl" .


:MeasuringPeriodKind.sixtyMinute uml:hasInitialValue "7" ;
                                 
                                 rdfs:comment "60-minute" ;
                                 rdfs:label "sixtyMinute" .


:MeasuringPeriodKind.tenMinute uml:hasInitialValue "1" ;
                               
                               rdfs:comment "10-minute" ;
                               rdfs:label "tenMinute" .


:MeasuringPeriodKind.thirtyMinute uml:hasInitialValue "5" ;
                                  
                                  rdfs:comment "30-minute" ;
                                  rdfs:label "thirtyMinute" .


:MeasuringPeriodKind.threeMinute uml:hasInitialValue "14" ;
                                 
                                 rdfs:comment "3-minute" ;
                                 rdfs:label "threeMinute" .


:MeasuringPeriodKind.twentyMinute uml:hasInitialValue "31" ;
                                  
                                  rdfs:comment "20-minute interval" ;
                                  rdfs:label "twentyMinute" .


:MeasuringPeriodKind.twentyfourHour uml:hasInitialValue "4" ;
                                    
                                    rdfs:comment "24-hour" ;
                                    rdfs:label "twentyfourHour" .


:MeasuringPeriodKind.twoMinute uml:hasInitialValue "10" ;
                               
                               rdfs:comment "2-minute" ;
                               rdfs:label "twoMinute" .


:MediumKind.SF6 
                rdfs:comment "Medium is SF6." ;
                rdfs:label "SF6" .


:MediumKind.SF6CF4 
                   rdfs:comment "Medium is SF6CF4." ;
                   rdfs:label "SF6CF4" .


:MediumKind.SF6N2 
                  rdfs:comment "Medium is SF6N2." ;
                  rdfs:label "SF6N2" .


:MediumKind.air 
                rdfs:comment "Medium is air." ;
                rdfs:label "air" .


:MediumKind.gas 
                rdfs:comment "Medium is gas." ;
                rdfs:label "gas" .


:MediumKind.liquid 
                   rdfs:comment "Medium is liquid." ;
                   rdfs:label "liquid" .


:MediumKind.mineralOil 
                       rdfs:comment "Medium is mineral oil." ;
                       rdfs:label "mineralOil" .


:MediumKind.solid 
                  rdfs:comment "Medium is solid." ;
                  rdfs:label "solid" .


:MeterMultiplierKind.ctRatio 
                             rdfs:comment "Current transformer ratio used to convert associated quantities to real measurements." ;
                             rdfs:label "ctRatio" .


:MeterMultiplierKind.kE 
                        rdfs:comment "Test constant." ;
                        rdfs:label "kE" .


:MeterMultiplierKind.kH 
                        rdfs:comment "Meter kh (watthour) constant. The number of watthours that must be applied to the meter to cause one disk revolution for an electromechanical meter or the number of watthours represented by one increment pulse for an electronic meter." ;
                        rdfs:label "kH" .


:MeterMultiplierKind.kR 
                        rdfs:comment "Register multiplier. The number to multiply the register reading by in order to get kWh." ;
                        rdfs:label "kR" .


:MeterMultiplierKind.ptRatio 
                             rdfs:comment "Potential transformer ratio used to convert associated quantities to real measurements." ;
                             rdfs:label "ptRatio" .


:MeterMultiplierKind.transformerRatio 
                                      rdfs:comment "Product of the CT ratio and PT ratio." ;
                                      rdfs:label "transformerRatio" .


:MktAccountKind.estimate 
                         rdfs:label "estimate" .


:MktAccountKind.normal 
                       rdfs:label "normal" .


:MktAccountKind.reversal 
                         rdfs:label "reversal" .


:MktAccountKind.statistical 
                            rdfs:label "statistical" .


:MktBillMediaKind.electronic 
                             rdfs:label "electronic" .


:MktBillMediaKind.other 
                        rdfs:label "other" .


:MktBillMediaKind.paper 
                        rdfs:label "paper" .


:MktInvoiceLineItemKind.initial 
                                rdfs:label "initial" .


:MktInvoiceLineItemKind.other 
                              rdfs:label "other" .


:MktInvoiceLineItemKind.recalculation 
                                      rdfs:label "recalculation" .


:MktSubClassType.Branch_Group_Derates 
                                      rdfs:label "Branch_Group_Derates" .


:MktSubClassType.Day_Ahead_Final_Market_Info 
                                             rdfs:label "Day_Ahead_Final_Market_Info" .


:MktSubClassType.Day_Ahead_Forecast_Information 
                                                rdfs:label "Day_Ahead_Forecast_Information" .


:MktSubClassType.Day_Ahead_Interim_Market_Info 
                                               rdfs:label "Day_Ahead_Interim_Market_Info" .


:MktSubClassType.Day_Ahead_RMR 
                               rdfs:label "Day_Ahead_RMR" .


:MktSubClassType.Forecasted_UDC_Direct_Access_Load 
                                                   rdfs:label "Forecasted_UDC_Direct_Access_Load" .


:MktSubClassType.Hour_Ahead_Market_Info 
                                        rdfs:label "Hour_Ahead_Market_Info" .


:MktSubClassType.Hourly_Expost_Market_Info 
                                           rdfs:label "Hourly_Expost_Market_Info" .


:MktSubClassType.Public_Bid_Data 
                                 rdfs:label "Public_Bid_Data" .


:MktSubClassType.TTC_ATC_Forecast_Information 
                                              rdfs:label "TTC/ATC_Forecast_Information" .


:MktSubClassType.TTC_ATC_Hourly_Forecast 
                                         rdfs:label "TTC/ATC_Hourly_Forecast" .


:MktSubClassType.Ten_Min_Expost_Market_Info 
                                            rdfs:label "Ten_Min_Expost_Market_Info" .


:NotificationTriggerKind.etrChange 
                                   rdfs:comment "Notify customer if estimated restoration time changes." ;
                                   rdfs:label "etrChange" .


:NotificationTriggerKind.informDispatched 
                                          rdfs:comment "Notify customer that a crew has been dispatched to investigate the problem." ;
                                          rdfs:label "informDispatched" .


:NotificationTriggerKind.initialEtr 
                                    rdfs:comment "Notify customer for the first time that estimated restoration time is available." ;
                                    rdfs:label "initialEtr" .


:NotificationTriggerKind.powerOut 
                                  rdfs:comment "Notify customer of planned outage." ;
                                  rdfs:label "powerOut" .


:NotificationTriggerKind.powerRestored 
                                       rdfs:comment "Notify customer when power has been restored." ;
                                       rdfs:label "powerRestored" .


:OASISBidReportType.BIDS_PUBLIC 
                                rdfs:label "BIDS_PUBLIC" .


:OASISDataItems.AS_CLEAR_ASMP_IFM 
                                  rdfs:label "AS_CLEAR_ASMP_IFM" .


:OASISDataItems.AS_CLEAR_ASMP_RTM 
                                  rdfs:label "AS_CLEAR_ASMP_RTM" .


:OASISDataItems.AS_CLEAR_COST_IFM 
                                  rdfs:label "AS_CLEAR_COST_IFM" .


:OASISDataItems.AS_CLEAR_COST_RTM 
                                  rdfs:label "AS_CLEAR_COST_RTM" .


:OASISDataItems.AS_CLEAR_MW_IFM 
                                rdfs:label "AS_CLEAR_MW_IFM" .


:OASISDataItems.AS_CLEAR_MW_RTM 
                                rdfs:label "AS_CLEAR_MW_RTM" .


:OASISDataItems.AS_GEN_TOTAL_MW_IFM 
                                    rdfs:label "AS_GEN_TOTAL_MW_IFM" .


:OASISDataItems.AS_GEN_TOTAL_MW_RTM 
                                    rdfs:label "AS_GEN_TOTAL_MW_RTM" .


:OASISDataItems.AS_IMP_TOTAL_MW_IFM 
                                    rdfs:label "AS_IMP_TOTAL_MW_IFM" .


:OASISDataItems.AS_IMP_TOTAL_MW_RTM 
                                    rdfs:label "AS_IMP_TOTAL_MW_RTM" .


:OASISDataItems.AS_LOAD_TOTAL_MW_IFM 
                                     rdfs:label "AS_LOAD_TOTAL_MW_IFM" .


:OASISDataItems.AS_LOAD_TOTAL_MW_RTM 
                                     rdfs:label "AS_LOAD_TOTAL_MW_RTM" .


:OASISDataItems.AS_REGION_REQ_MAX 
                                  rdfs:label "AS_REGION_REQ_MAX" .


:OASISDataItems.AS_REGION_REQ_MIN 
                                  rdfs:label "AS_REGION_REQ_MIN" .


:OASISDataItems.AS_REGION_value 
                                rdfs:label "AS_REGION_value" .


:OASISDataItems.AS_SELF_MW_IFM 
                               rdfs:label "AS_SELF_MW_IFM" .


:OASISDataItems.AS_SELF_MW_RTM 
                               rdfs:label "AS_SELF_MW_RTM" .


:OASISDataItems.AS_TOTAL_MW 
                            rdfs:label "AS_TOTAL_MW" .


:OASISDataItems.AS_TOTAL_MW_IFM 
                                rdfs:label "AS_TOTAL_MW_IFM" .


:OASISDataItems.AS_TOTAL_MW_RTM 
                                rdfs:label "AS_TOTAL_MW_RTM" .


:OASISDataItems.AS_TYPE 
                        rdfs:label "AS_TYPE" .


:OASISDataItems.AS_USER_RATE 
                             rdfs:label "AS_USER_RATE" .


:OASISDataItems.CA_value 
                         rdfs:label "CA_value" .


:OASISDataItems.CMMT_MINLOAD_MLC 
                                 rdfs:label "CMMT_MINLOAD_MLC" .


:OASISDataItems.CMMT_MINLOAD_MW 
                                rdfs:label "CMMT_MINLOAD_MW" .


:OASISDataItems.CMMT_RA_MLC 
                            rdfs:label "CMMT_RA_MLC" .


:OASISDataItems.CMMT_RA_MW 
                           rdfs:label "CMMT_RA_MW" .


:OASISDataItems.CMMT_RA_START_COST 
                                   rdfs:label "CMMT_RA_START_COST" .


:OASISDataItems.CMMT_RA_UNITS 
                              rdfs:label "CMMT_RA_UNITS" .


:OASISDataItems.CMMT_TOTAL_MW 
                              rdfs:label "CMMT_TOTAL_MW" .


:OASISDataItems.CMMT_TOTAL_START_COST 
                                      rdfs:label "CMMT_TOTAL_START_COST" .


:OASISDataItems.CMMT_TOTAL_UNITS 
                                 rdfs:label "CMMT_TOTAL_UNITS" .


:OASISDataItems.CRR_CAT 
                        rdfs:label "CRR_CAT" .


:OASISDataItems.CRR_MARKET_value 
                                 rdfs:label "CRR_MARKET_value" .


:OASISDataItems.CRR_MW 
                       rdfs:label "CRR_MW" .


:OASISDataItems.CRR_NSR 
                        rdfs:label "CRR_NSR" .


:OASISDataItems.CRR_OPTION 
                           rdfs:label "CRR_OPTION" .


:OASISDataItems.CRR_OWNER 
                          rdfs:label "CRR_OWNER" .


:OASISDataItems.CRR_SEGMENT 
                            rdfs:label "CRR_SEGMENT" .


:OASISDataItems.CRR_TERM 
                         rdfs:label "CRR_TERM" .


:OASISDataItems.CRR_TOU 
                        rdfs:label "CRR_TOU" .


:OASISDataItems.CRR_TYPE 
                         rdfs:label "CRR_TYPE" .


:OASISDataItems.ENE_EA_DA 
                          rdfs:label "ENE_EA_DA" .


:OASISDataItems.ENE_EA_EXCEPT 
                              rdfs:label "ENE_EA_EXCEPT" .


:OASISDataItems.ENE_EA_HASP 
                            rdfs:label "ENE_EA_HASP" .


:OASISDataItems.ENE_EA_MLE 
                           rdfs:label "ENE_EA_MLE" .


:OASISDataItems.ENE_EA_MSSLF 
                             rdfs:label "ENE_EA_MSSLF" .


:OASISDataItems.ENE_EA_OPTIMAL 
                               rdfs:label "ENE_EA_OPTIMAL" .


:OASISDataItems.ENE_EA_RAMP_DEV 
                                rdfs:label "ENE_EA_RAMP_DEV" .


:OASISDataItems.ENE_EA_RAMP_STD 
                                rdfs:label "ENE_EA_RAMP_STD" .


:OASISDataItems.ENE_EA_RESIDUAL 
                                rdfs:label "ENE_EA_RESIDUAL" .


:OASISDataItems.ENE_EA_RMR 
                           rdfs:label "ENE_EA_RMR" .


:OASISDataItems.ENE_EA_SELF 
                            rdfs:label "ENE_EA_SELF" .


:OASISDataItems.ENE_EA_SLIC 
                            rdfs:label "ENE_EA_SLIC" .


:OASISDataItems.ENE_EXP_CLEAR_HASP 
                                   rdfs:label "ENE_EXP_CLEAR_HASP" .


:OASISDataItems.ENE_EXP_CLEAR_IFM 
                                  rdfs:label "ENE_EXP_CLEAR_IFM" .


:OASISDataItems.ENE_EXP_CLEAR_RTM 
                                  rdfs:label "ENE_EXP_CLEAR_RTM" .


:OASISDataItems.ENE_GEN_CLEAR_HASP 
                                   rdfs:label "ENE_GEN_CLEAR_HASP" .


:OASISDataItems.ENE_GEN_CLEAR_IFM 
                                  rdfs:label "ENE_GEN_CLEAR_IFM" .


:OASISDataItems.ENE_GEN_CLEAR_RTM 
                                  rdfs:label "ENE_GEN_CLEAR_RTM" .


:OASISDataItems.ENE_IMP_CLEAR_HASP 
                                   rdfs:label "ENE_IMP_CLEAR_HASP" .


:OASISDataItems.ENE_IMP_CLEAR_IFM 
                                  rdfs:label "ENE_IMP_CLEAR_IFM" .


:OASISDataItems.ENE_IMP_CLEAR_RTM 
                                  rdfs:label "ENE_IMP_CLEAR_RTM" .


:OASISDataItems.ENE_LOAD_ACTUAL 
                                rdfs:label "ENE_LOAD_ACTUAL" .


:OASISDataItems.ENE_LOAD_CLEAR_HASP 
                                    rdfs:label "ENE_LOAD_CLEAR_HASP" .


:OASISDataItems.ENE_LOAD_CLEAR_IFM 
                                   rdfs:label "ENE_LOAD_CLEAR_IFM" .


:OASISDataItems.ENE_LOAD_CLEAR_RTM 
                                   rdfs:label "ENE_LOAD_CLEAR_RTM" .


:OASISDataItems.ENE_LOAD_FCST 
                              rdfs:label "ENE_LOAD_FCST" .


:OASISDataItems.ENE_PEAK_HOUR 
                              rdfs:label "ENE_PEAK_HOUR" .


:OASISDataItems.ENE_PEAK_LOAD 
                              rdfs:label "ENE_PEAK_LOAD" .


:OASISDataItems.FUEL_REGION_value 
                                  rdfs:label "FUEL_REGION_value" .


:OASISDataItems.INVT_DATETIME 
                              rdfs:label "INVT_DATETIME" .


:OASISDataItems.LOAD_ACTUAL 
                            rdfs:label "LOAD_ACTUAL" .


:OASISDataItems.LOAD_CLEAR_RTM 
                               rdfs:label "LOAD_CLEAR_RTM" .


:OASISDataItems.LOSS_TOTAL_COST_HASP 
                                     rdfs:label "LOSS_TOTAL_COST_HASP" .


:OASISDataItems.LOSS_TOTAL_COST_RTM 
                                    rdfs:label "LOSS_TOTAL_COST_RTM" .


:OASISDataItems.LOSS_TOTAL_MW_HASP 
                                   rdfs:label "LOSS_TOTAL_MW_HASP" .


:OASISDataItems.LOSS_TOTAL_MW_RTM 
                                  rdfs:label "LOSS_TOTAL_MW_RTM" .


:OASISDataItems.MPM_FLAG 
                         rdfs:label "MPM_FLAG" .


:OASISDataItems.OP_RSRV_TOTAL 
                              rdfs:label "OP_RSRV_TOTAL" .


:OASISDataItems.PRC_NG 
                       rdfs:label "PRC_NG" .


:OASISDataItems.PRC_SHADOW 
                           rdfs:label "PRC_SHADOW" .


:OASISDataItems.RATING_ATC 
                           rdfs:label "RATING_ATC" .


:OASISDataItems.RMR_DETER_DAM 
                              rdfs:label "RMR_DETER_DAM" .


:OASISDataItems.RMR_DETER_HASP 
                               rdfs:label "RMR_DETER_HASP" .


:OASISDataItems.RMR_DISPATCH_DAM 
                                 rdfs:label "RMR_DISPATCH_DAM" .


:OASISDataItems.RMR_DISPATCH_HASP 
                                  rdfs:label "RMR_DISPATCH_HASP" .


:OASISDataItems.RMR_TOTAL 
                          rdfs:label "RMR_TOTAL" .


:OASISDataItems.RMR_TOTAL_AVAIL 
                                rdfs:label "RMR_TOTAL_AVAIL" .


:OASISDataItems.RUC_GEN_CLEAR_RUC 
                                  rdfs:label "RUC_GEN_CLEAR_RUC" .


:OASISDataItems.RUC_IMP_CLEAR_RUC 
                                  rdfs:label "RUC_IMP_CLEAR_RUC" .


:OASISDataItems.RUC_LOAD_CLEAR_RUC 
                                   rdfs:label "RUC_LOAD_CLEAR_RUC" .


:OASISDataItems.RUC_ZONE_value 
                               rdfs:label "RUC_ZONE_value" .


:OASISDataItems.TAC_AREA_value 
                               rdfs:label "TAC_AREA_value" .


:OASISDataItems.TINTRFCE_value 
                               rdfs:label "TINTRFCE_value" .


:OASISDataItems.TRNS_AS_IMPORT 
                               rdfs:label "TRNS_AS_IMPORT" .


:OASISDataItems.TRNS_ENE_IMPORT 
                                rdfs:label "TRNS_ENE_IMPORT" .


:OASISDataItems.TRNS_EQUIP_value 
                                 rdfs:label "TRNS_EQUIP_value" .


:OASISDataItems.TRNS_RATING_CBM 
                                rdfs:label "TRNS_RATING_CBM" .


:OASISDataItems.TRNS_RATING_DIRECTION 
                                      rdfs:label "TRNS_RATING_DIRECTION" .


:OASISDataItems.TRNS_RATING_OTC 
                                rdfs:label "TRNS_RATING_OTC" .


:OASISDataItems.TRNS_RATING_OTC_DERATE 
                                       rdfs:label "TRNS_RATING_OTC_DERATE" .


:OASISDataItems.TRNS_RATING_TTC 
                                rdfs:label "TRNS_RATING_TTC" .


:OASISDataItems.TRNS_TI_value 
                              rdfs:label "TRNS_TI_value" .


:OASISDataItems.TRNS_TR_ENTMTS 
                               rdfs:label "TRNS_TR_ENTMTS" .


:OASISDataItems.TRNS_TR_USEAGE 
                               rdfs:label "TRNS_TR_USEAGE" .


:OASISErrCode._1000 
                    rdfs:label "1000" .


:OASISErrCode._1001 
                    rdfs:label "1001" .


:OASISErrCode._1002 
                    rdfs:label "1002" .


:OASISErrCode._1003 
                    rdfs:label "1003" .


:OASISErrCode._1004 
                    rdfs:label "1004" .


:OASISErrCode._1005 
                    rdfs:label "1005" .


:OASISErrCode._1006 
                    rdfs:label "1006" .


:OASISErrCode._1007 
                    rdfs:label "1007" .


:OASISErrCode._1008 
                    rdfs:label "1008" .


:OASISErrCode._1009 
                    rdfs:label "1009" .


:OASISErrCode._1010 
                    rdfs:label "1010" .


:OASISErrDescription.Data_can_be_requested_for_period_of_31_days_only 
                                                                      rdfs:label "Data can be requested for period of 31 days only" .


:OASISErrDescription.Exceptions_in_reading_and_writing_of_XML_files 
                                                                    rdfs:label "Exceptions in reading and writing of XML files" .


:OASISErrDescription.Invalid_date_format__please_use_valid_date_format 
                                                                       rdfs:label "Invalid date format, please use valid date format" .


:OASISErrDescription.No_data_returned_for_the_specified_selection 
                                                                  rdfs:label "No data returned for the specified selection" .


:OASISErrDescription.Out_of_memory_exception 
                                             rdfs:label "Out of memory exception" .


:OASISErrDescription.Report_name_does_not_exit__please_use_valid_report_name 
                                                                             rdfs:label "Report name does not exit, please use valid report name" .


:OASISErrDescription.Required_file_does_not_exist 
                                                  rdfs:label "Required file does not exist" .


:OASISErrDescription.System_Error 
                                  rdfs:label "System Error" .


:OASISErrDescription.Timed_out_waiting_for_query_response 
                                                          rdfs:label "Timed out waiting for query response" .


:OASISErrDescription.Validation_exception_during_transformation_of_XML 
                                                                       rdfs:label "Validation exception during transformation of XML" .


:OASISIntervalType.BEGINNING 
                             rdfs:label "BEGINNING" .


:OASISIntervalType.ENDING 
                          rdfs:label "ENDING" .


:OASISMarketType.All 
                     rdfs:label "All" .


:OASISMarketType.HASP 
                      rdfs:label "HASP" .


:OASISMarketType.IFM 
                     rdfs:label "IFM" .


:OASISMarketType.N_A 
                     rdfs:label "N/A" .


:OASISMarketType.RTM 
                     rdfs:label "RTM" .


:OASISMarketType.RUC 
                     rdfs:label "RUC" .


:OASISMasterType.ATL_APNODE 
                            rdfs:label "ATL_APNODE" .


:OASISMasterType.ATL_AS_REGION 
                               rdfs:label "ATL_AS_REGION" .


:OASISMasterType.ATL_AS_REGION_MAP 
                                   rdfs:label "ATL_AS_REGION_MAP" .


:OASISMasterType.ATL_HUB 
                         rdfs:label "ATL_HUB" .


:OASISMasterType.ATL_LAP 
                         rdfs:label "ATL_LAP" .


:OASISMasterType.ATL_LDF 
                         rdfs:label "ATL_LDF" .


:OASISMasterType.ATL_PNODE 
                           rdfs:label "ATL_PNODE" .


:OASISMasterType.ATL_PNODE_MAP 
                               rdfs:label "ATL_PNODE_MAP" .


:OASISMasterType.ATL_PUB 
                         rdfs:label "ATL_PUB" .


:OASISMasterType.ATL_PUB_SCHED 
                               rdfs:label "ATL_PUB_SCHED" .


:OASISMasterType.ATL_RESOURCE 
                              rdfs:label "ATL_RESOURCE" .


:OASISMasterType.ATL_RUC_ZONE 
                              rdfs:label "ATL_RUC_ZONE" .


:OASISMasterType.ATL_RUC_ZONE_MAP 
                                  rdfs:label "ATL_RUC_ZONE_MAP" .


:OASISMasterType.ATL_STAT 
                          rdfs:label "ATL_STAT" .


:OASISMasterType.ATL_TAC_AREA 
                              rdfs:label "ATL_TAC_AREA" .


:OASISMasterType.ATL_TAC_AREA_MAP 
                                  rdfs:label "ATL_TAC_AREA_MAP" .


:OASISMasterType.ATL_TI 
                        rdfs:label "ATL_TI" .


:OASISMasterType.ATL_TIEPOINT 
                              rdfs:label "ATL_TIEPOINT" .


:OASISMasterType.ATL_XREF 
                          rdfs:label "ATL_XREF" .


:OASISMeasType.FACTOR 
                      rdfs:label "FACTOR" .


:OASISMeasType.FLAG 
                    rdfs:label "FLAG" .


:OASISMeasType.INTEGER 
                       rdfs:label "INTEGER" .


:OASISMeasType.MW 
                  rdfs:label "MW" .


:OASISMeasType.MWh 
                   rdfs:label "MWh" .


:OASISMeasType.US_ 
                   rdfs:label "US$" .


:OASISMeasType.US__MW 
                      rdfs:label "US$/MW" .


:OASISMeasType.US__MWh 
                       rdfs:label "US$/MWh" .


:OASISMeasType._ 
                 rdfs:label "%" .


:OASISReportType.AS_DA_RESULT 
                              rdfs:label "AS_DA_RESULT" .


:OASISReportType.AS_OP_RSRV 
                            rdfs:label "AS_OP_RSRV" .


:OASISReportType.AS_REQ 
                        rdfs:label "AS_REQ" .


:OASISReportType.AS_RTM_RESULT 
                               rdfs:label "AS_RTM_RESULT" .


:OASISReportType.BIDS_PUBLIC 
                             rdfs:label "BIDS_PUBLIC" .


:OASISReportType.CMMT_RA_MLC 
                             rdfs:label "CMMT_RA_MLC" .


:OASISReportType.CMMT_RMR 
                          rdfs:label "CMMT_RMR" .


:OASISReportType.CRR_CLEARING 
                              rdfs:label "CRR_CLEARING" .


:OASISReportType.CRR_INVENTORY 
                               rdfs:label "CRR_INVENTORY" .


:OASISReportType.ENE_EA 
                        rdfs:label "ENE_EA" .


:OASISReportType.ENE_HASP 
                          rdfs:label "ENE_HASP" .


:OASISReportType.ENE_IFM 
                         rdfs:label "ENE_IFM" .


:OASISReportType.ENE_MPM 
                         rdfs:label "ENE_MPM" .


:OASISReportType.ENE_RTM 
                         rdfs:label "ENE_RTM" .


:OASISReportType.ENE_RUC 
                         rdfs:label "ENE_RUC" .


:OASISReportType.LOSS_DA_HASP 
                              rdfs:label "LOSS_DA_HASP" .


:OASISReportType.LOSS_RTM 
                          rdfs:label "LOSS_RTM" .


:OASISReportType.PRC_AS 
                        rdfs:label "PRC_AS" .


:OASISReportType.PRC_CNSTR 
                           rdfs:label "PRC_CNSTR" .


:OASISReportType.PRC_FUEL 
                          rdfs:label "PRC_FUEL" .


:OASISReportType.PRC_HRLY_LMP 
                              rdfs:label "PRC_HRLY_LMP" .


:OASISReportType.PRC_INTVL_LMP 
                               rdfs:label "PRC_INTVL_LMP" .


:OASISReportType.SLD_FCST 
                          rdfs:label "SLD_FCST" .


:OASISReportType.SLD_FCST_PEAK 
                               rdfs:label "SLD_FCST_PEAK" .


:OASISReportType.SLD_MKTS 
                          rdfs:label "SLD_MKTS" .


:OASISReportType.TRNS_ATC 
                          rdfs:label "TRNS_ATC" .


:OASISReportType.TRNS_OUTAGE 
                             rdfs:label "TRNS_OUTAGE" .


:OASISReportType.TRNS_USAGE 
                            rdfs:label "TRNS_USAGE" .


:OASISStatusType.Data_Transfer_Procedure_Initiated 
                                                   rdfs:label "Data_Transfer_Procedure_Initiated" .


:OASISStatusType.Data_Transfer_Succesful 
                                         rdfs:label "Data_Transfer_Succesful" .


:OASISStatusType.Forced_Termination 
                                    rdfs:label "Forced_Termination" .


:OASISStatusType.Obsolete 
                          rdfs:label "Obsolete" .


:OASISStatusType.Push_Failed 
                             rdfs:label "Push_Failed" .


:OASISStatusType.Valid 
                       rdfs:label "Valid" .


:OilAnalysisFluidAnalogKind.acidNumber 
                                       rdfs:comment "Acid neutralization number (in milligram of KOH/gram)." ;
                                       rdfs:label "acidNumber" .


:OilAnalysisFluidAnalogKind.additiveDBDS 
                                         rdfs:comment "Dibenzyl disulfide (DBDS) concentration (in ppm, specificially in milligram/kilogram)." ;
                                         rdfs:label "additiveDBDS" .


:OilAnalysisFluidAnalogKind.aromatics 
                                      rdfs:comment "Concentration of aromatic compounds determined using infrared spectroscopy (in percent)." ;
                                      rdfs:label "aromatics" .


:OilAnalysisFluidAnalogKind.carbonyl 
                                     rdfs:comment "Concentration of carbonyl compounds (aldehydes and ketones) determined using infrared spectroscopy (in percent)." ;
                                     rdfs:label "carbonyl" .


:OilAnalysisFluidAnalogKind.density 
                                    rdfs:comment "Density (in gram/millilitre)." ;
                                    rdfs:label "density" .


:OilAnalysisFluidAnalogKind.dielectricBreakdown 
                                                rdfs:comment "Dielectric breakdown, for electrode gap size and temperature specified by selected standard  (in kV)." ;
                                                rdfs:label "dielectricBreakdown" .


:OilAnalysisFluidAnalogKind.dissipationFactor 
                                              rdfs:comment "Fluid dissipation factor in absolute value, not a percentage. (Multiplying this value by 100 would result in dissipation factor percent)." ;
                                              rdfs:label "dissipationFactor" .


:OilAnalysisFluidAnalogKind.dissipationFactorPercent 
                                                     rdfs:comment "Fluid dissipation factor (in percent). Commonly used in Asia. Dissipation factor is also known as loss factor or tan delta." ;
                                                     rdfs:label "dissipationFactorPercent" .


:OilAnalysisFluidAnalogKind.duration61125MethodC 
                                                 rdfs:comment "Duration of oxidation stablity test performed according to IEC 61125, method C. This value should accompany values resulting from testing according to IEC 61125, method C to allow interpretation. Standard specified values are: 164, 332, and 500, but others can be used if agreed upon." ;
                                                 rdfs:label "duration61125MethodC" .


:OilAnalysisFluidAnalogKind.firePoint 
                                      rdfs:comment "Fire point (in °C). Fire point is when fire is sustained (oil catches fire). Can only be done by means of open cup test, which is commonly used in US." ;
                                      rdfs:label "firePoint" .


:OilAnalysisFluidAnalogKind.flashPointClosedCup 
                                                rdfs:comment "Flash point (in °C) determined via closed cup test. Flash point occurs when enough vapors have accumulated to sustain a flash. Closed cup is used in Europe." ;
                                                rdfs:label "flashPointClosedCup" .


:OilAnalysisFluidAnalogKind.flashPointOpenCup 
                                              rdfs:comment "Flash point (in °C) determined via open cup test. Flash point occurs when enough vapors have accumulated to sustain a flash. Open cup is used in US." ;
                                              rdfs:label "flashPointOpenCup" .


:OilAnalysisFluidAnalogKind.inductionTime 
                                          rdfs:comment "Oxidation induction time (in hours). Typically performed on new oil,but can be done on used oil." ;
                                          rdfs:label "inductionTime" .


:OilAnalysisFluidAnalogKind.inhibitor61125MethodC 
                                                  rdfs:comment "Amount of inhibitor used in oxidation stablity test performed according to IEC 61125, method C. This value should accompany values resulting from testing according to IEC 61125, method  C to allow interpretation." ;
                                                  rdfs:label "inhibitor61125MethodC" .


:OilAnalysisFluidAnalogKind.interfacialTension 
                                               rdfs:comment "Interfacial tension (in dyne/centimetre or milliNewton/metre, which are the same)." ;
                                               rdfs:label "interfacialTension" .


:OilAnalysisFluidAnalogKind.kinematicViscosity 
                                               rdfs:comment "Kinematic viscosity (in millimetre2/second). Kinematic viscosity is the ratio of - absolute (or dynamic) viscosity to density." ;
                                               rdfs:label "kinematicViscosity" .


:OilAnalysisFluidAnalogKind.oxidation 
                                      rdfs:comment "Measure of oxidation stability (in hours)." ;
                                      rdfs:label "oxidation" .


:OilAnalysisFluidAnalogKind.oxidationInhibitorD2668 
                                                    rdfs:comment "2,6-ditertiary-butyl para-cresol and 2,6-ditertiary-butyl phenol concentration (in percent by weight)." ;
                                                    rdfs:label "oxidationInhibitorD2668" .


:OilAnalysisFluidAnalogKind.oxidationInhibitorDBP 
                                                  rdfs:comment "2,6-ditertiary-butyl phenol (DBP) oxidation inhibitor concentration (in percent by weight)." ;
                                                  rdfs:label "oxidationInhibitorDBP" .


:OilAnalysisFluidAnalogKind.oxidationInhibitorDBPC 
                                                   rdfs:comment "2,6-ditertiarybutyl para-cresol (DBPC) oxidation inhibitor concentration (in percent by weight)." ;
                                                   rdfs:label "oxidationInhibitorDBPC" .


:OilAnalysisFluidAnalogKind.passivatorBTA 
                                          rdfs:comment "Metal passivator BTA content (in milligram/kilogram)." ;
                                          rdfs:label "passivatorBTA" .


:OilAnalysisFluidAnalogKind.passivatorContent 
                                              rdfs:comment "Total passivator content (in milligram/kilogram)." ;
                                              rdfs:label "passivatorContent" .


:OilAnalysisFluidAnalogKind.passivatorIrgamet39 
                                                rdfs:comment "Irgamet 39 metal passivator content (in ppm, specifically milligram/kilogram)." ;
                                                rdfs:label "passivatorIrgamet39" .


:OilAnalysisFluidAnalogKind.passivatorTTA 
                                          rdfs:comment "Metal passivator TTA (Irgamet39 in solid form) content (in milligram/kilogram)." ;
                                          rdfs:label "passivatorTTA" .


:OilAnalysisFluidAnalogKind.petroleumOrigin 
                                            rdfs:comment "Characterization of the carbon-type composition of insulating oils by petroleum origin." ;
                                            rdfs:label "petroleumOrigin" .


:OilAnalysisFluidAnalogKind.pourPoint 
                                      rdfs:comment "Pour point (in °C). The pour point of a liquid is the temperature at which it becomes semi solid and loses its flow characteristics." ;
                                      rdfs:label "pourPoint" .


:OilAnalysisFluidAnalogKind.pourPointAutomatic 
                                               rdfs:comment "Pour point (in °C) determined by automatic method. The pour point of a liquid is the temperature at which it becomes semi solid and loses its flow characteristics." ;
                                               rdfs:label "pourPointAutomatic" .


:OilAnalysisFluidAnalogKind.powerFactorPercent 
                                               rdfs:comment "Fluid power factor at specified temperature (in percent). Commonly used in US. (Note: Fluid power factor is very similar to fluid dissapation factor, but fluid power factor is cosine of the phase angle between an AC voltage applied to oil and the resulting current (where dissipation factor is the tangent). For values up to 0.005, fluid power factor and dissapation factor are very close. There is a conversion equation between the two)." ;
                                               rdfs:label "powerFactorPercent" .


:OilAnalysisFluidAnalogKind.resistivity 
                                        rdfs:comment "Resistivity at 90°C (in gigohm-metre)." ;
                                        rdfs:label "resistivity" .


:OilAnalysisFluidAnalogKind.sedimentAndSludgePercent 
                                                     rdfs:comment "Sediment and sludge (in percent)." ;
                                                     rdfs:label "sedimentAndSludgePercent" .


:OilAnalysisFluidAnalogKind.sludge 
                                   rdfs:comment "Sludge (in percent by mass). Typically performed on new oil,but can be done on used oil." ;
                                   rdfs:label "sludge" .


:OilAnalysisFluidAnalogKind.solubleAcids 
                                         rdfs:comment "Soluble acids  (in milligram of KOH/gram). Typically performed on new oil,but can be done on used oil." ;
                                         rdfs:label "solubleAcids" .


:OilAnalysisFluidAnalogKind.specificGravity 
                                            rdfs:comment "Specific gravity corrected to 15°C. Also known as relative density. It is a ratio of density of tested oil to density of water at a specific temperature." ;
                                            rdfs:label "specificGravity" .


:OilAnalysisFluidAnalogKind.staticElectrification 
                                                  rdfs:comment "Static electrification tendency (in microcoulombs per metre3). Also called static charging tendency and electrostatic charging tendency (ECT)." ;
                                                  rdfs:label "staticElectrification" .


:OilAnalysisFluidAnalogKind.totalAcids 
                                       rdfs:comment "Total acids (soluble plus volatile) (in milligram of KOH/gram). Typically performed on new oil,but can be done on used oil." ;
                                       rdfs:label "totalAcids" .


:OilAnalysisFluidAnalogKind.volatileAcids 
                                          rdfs:comment "Volatile acids (in milligram of KOH/gram). Typically performed on new oil,but can be done on used oil." ;
                                          rdfs:label "volatileAcids" .


:OilAnalysisFluidDiscreteKind.colorNumber 
                                          rdfs:comment """Fluid color index number.  Color numbers are expressed in 0.5 intervals and value specified is  \"less-than\". For example, a value of '2.5' means the color index number is between 2.0 and 2.5.
Possible values: 0.5, 1.0, 1.5, 2.0, 2.5, 3.0, 3.5, 4.0, 4.5, 5.0, 5.5, 6.0, 6.5, 7.0, 7.5, 8.0.""" ;
                                          rdfs:label "colorNumber" .


:OilAnalysisFluidDiscreteKind.colorNumberPlatinumCobaltScale 
                                                             rdfs:comment """Fluid color index on the platinum cobalt scale. 
Possible values: 5, 10, 15, 20, 25, 30, 35, 40, 50, 60, 70, 100, 150, 200, 250, 300, 350, 400, 450.""" ;
                                                             rdfs:label "colorNumberPlatinumCobaltScale" .


:OilAnalysisFluidDiscreteKind.corrosiveSulphurBy51353 
                                                      rdfs:comment """Corrosive sulphur test result using silver strip test.
Possible values: absent, present.""" ;
                                                      rdfs:label "corrosiveSulphurBy51353" .


:OilAnalysisFluidDiscreteKind.corrosiveSulphurBy62535 
                                                      rdfs:comment """Corrosive sulphur test result using covered (copper) conductor deposition test.
Possible values: potentiallyCorrosive, nonCorrosive.""" ;
                                                      rdfs:label "corrosiveSulphurBy62535" .


:OilAnalysisFluidDiscreteKind.corrosiveSulphurByD1275 
                                                      rdfs:comment """Corrosive sulphur test result using bare copper strip test.
Possible values: corrosive, nonCorrosive.""" ;
                                                      rdfs:label "corrosiveSulphurByD1275" .


:OilAnalysisFluidDiscreteKind.sludgePrecipitation 
                                                  rdfs:comment """Sludge precipitation test results.
Possible values: present, notPresent.""" ;
                                                  rdfs:label "sludgePrecipitation" .


:OilAnalysisFluidDiscreteKind.tarnishLevel 
                                           rdfs:comment """Tarnish level indicated by corrosive sulphur test.
Possible values: 1A, 1B, 2A, 2B, 2C, 2D, 2E, 3A, 3B, 4A, 4B, 4C.""" ;
                                           rdfs:label "tarnishLevel" .


:OilAnalysisGasAnalogKind.acetylene 
                                    rdfs:comment "C2H2 concentration (in ppm, specifically in microlitre/litre)." ;
                                    rdfs:label "acetylene" .


:OilAnalysisGasAnalogKind.butane 
                                 rdfs:comment "C4H10 concentration (in ppm, specifically in microlitre/litre)." ;
                                 rdfs:label "butane" .


:OilAnalysisGasAnalogKind.carbon 
                                 rdfs:comment "C? concentration (in ppm, specifically in microlitre/litre)." ;
                                 rdfs:label "carbon" .


:OilAnalysisGasAnalogKind.carbon3 
                                  rdfs:comment "C3 concentration (in ppm, specifically in microlitre/litre)." ;
                                  rdfs:label "carbon3" .


:OilAnalysisGasAnalogKind.carbon4 
                                  rdfs:comment "C4 concentration (in ppm, specifically in microlitre/litre)." ;
                                  rdfs:label "carbon4" .


:OilAnalysisGasAnalogKind.carbonDioxide 
                                        rdfs:comment "CO2 concentration (in ppm, specifically in microlitre/litre)." ;
                                        rdfs:label "carbonDioxide" .


:OilAnalysisGasAnalogKind.carbonMonoxide 
                                         rdfs:comment "CO concentration (in ppm, specifically in microlitre/litre)." ;
                                         rdfs:label "carbonMonoxide" .


:OilAnalysisGasAnalogKind.equivalentTCGPercent 
                                               rdfs:comment """Equivalent Total Combustible Gas (ETCG) percent.
An estimate, calculated from the dissolved-gas concentrations and the oil sample temperature, of what the TCG would be in a gas space in equilibrium with the oil. ETCG reflects what the TCG would be in air spaces near the oil.""" ;
                                               rdfs:label "equivalentTCGPercent" .


:OilAnalysisGasAnalogKind.estimatedSafeHandlingLimit 
                                                     rdfs:comment """Estimated Safe Handling Limit (ESHL) (in percent). Estimated safe handling limit is an estimate of the lower flammability limit (LFL) of the combustible gas mixture which the dissolved gas in the oil would give off by the oil if exposed to air. 
Expressed in percent like the equivalent total combustible gas percent, it is calculated from the dissolved-gas concentrations, the oil sample temperature, and the lower flammability limits of the individual combustible gases.""" ;
                                                     rdfs:label "estimatedSafeHandlingLimit" .


:OilAnalysisGasAnalogKind.ethane 
                                 rdfs:comment "C2H6 concentration (in ppm, specifically in microlitre/litre)." ;
                                 rdfs:label "ethane" .


:OilAnalysisGasAnalogKind.ethylene 
                                   rdfs:comment "C2H4 concentration (in ppm, specifically in microlitre/litre)." ;
                                   rdfs:label "ethylene" .


:OilAnalysisGasAnalogKind.hydran 
                                 rdfs:comment """Measured composite of dissolved fault gas concentrations (in ppm, specifically in microlitre/litre). Relative sensitivity
- H2: 100 % of concentration
- CO: 15 ± 4 % of concentration
- C2H2: 8 ± 2 % of concentration
- C2H4: 1.5 ± 0.5 % of concentration.""" ;
                                 rdfs:label "hydran" .


:OilAnalysisGasAnalogKind.hydranPredicted 
                                          rdfs:comment """Predicted hydran value (in ppm, specifically in microlitre/litre), calculated based on individual measured dissolved gas concentrations.
- H2: 100 % of concentration
- CO: 15 ± 4 % of concentration
- C2H2: 8 ± 2 % of concentration
- C2H4: 1.5 ± 0.5 % of concentration""" ;
                                          rdfs:label "hydranPredicted" .


:OilAnalysisGasAnalogKind.hydrogen 
                                   rdfs:comment "H2 concentration (in ppm, specifically in microlitre/litre)." ;
                                   rdfs:label "hydrogen" .


:OilAnalysisGasAnalogKind.isobutane 
                                    rdfs:comment "isoC4 (C4H10) concentration (in ppm, specifically in microlitre/litre). Isobutane is also known as methylpropane." ;
                                    rdfs:label "isobutane" .


:OilAnalysisGasAnalogKind.methane 
                                  rdfs:comment "CH4 concentration (in ppm, specifically in microlitre/litre)." ;
                                  rdfs:label "methane" .


:OilAnalysisGasAnalogKind.nitrogen 
                                   rdfs:comment "N2 concentration (in ppm, specifically in microlitre/litre)." ;
                                   rdfs:label "nitrogen" .


:OilAnalysisGasAnalogKind.oxygen 
                                 rdfs:comment "O2 concentration (in ppm, specifically in microlitre/litre)." ;
                                 rdfs:label "oxygen" .


:OilAnalysisGasAnalogKind.propane 
                                  rdfs:comment "C3H8 concentration (in ppm, specifically in microlitre/litre)." ;
                                  rdfs:label "propane" .


:OilAnalysisGasAnalogKind.propene 
                                  rdfs:comment "C3H6 concentration (in ppm, specifically in microlitre/litre)." ;
                                  rdfs:label "propene" .


:OilAnalysisGasAnalogKind.totalCombustibleGasPercent 
                                                     rdfs:comment "Total Combustible Gas (TCG) measured in headspace (in percent by volume)." ;
                                                     rdfs:label "totalCombustibleGasPercent" .


:OilAnalysisGasAnalogKind.totalDissolvedCombustibleGas 
                                                       rdfs:comment "Total dissolved combustible gas concentration (in ppm, specifically in microlitre/litre). Calculated by adding the ppm of combustible gasses: hydrogen (H2), methane (CH4), ethane (C2H6), ethylene (C2H4), acetylene (C2H2), and carbon monoxide (CO)." ;
                                                       rdfs:label "totalDissolvedCombustibleGas" .


:OilAnalysisGasAnalogKind.totalDissolvedGasPercent 
                                                   rdfs:comment "Total dissolved gas in oil (in percent by volume). Derived from the total area of all the gas peaks in the chromatogram." ;
                                                   rdfs:label "totalDissolvedGasPercent" .


:OilAnalysisGasAnalogKind.totalHeatGas 
                                       rdfs:comment "Sum of concentrations of methane, ethane, and ethylene (in ppm, specifically in microlitre/litre). Used in some diagnostic gas ratios, especially THG/acetylene, which compares “heat gas” to “arcing gas.”" ;
                                       rdfs:label "totalHeatGas" .


:OilAnalysisGasAnalogKind.totalPartialPressure 
                                               rdfs:comment """Total partial pressure (in Pa).
Calculated value reflecting total of partial pressures of all combustible gasses.""" ;
                                               rdfs:label "totalPartialPressure" .


:OilAnalysisMetalsAnalogKind.aluminum 
                                      rdfs:comment "Aluminum concentration (in ppb, specifically in microgram/litre)." ;
                                      rdfs:label "aluminum" .


:OilAnalysisMetalsAnalogKind.aluminumParticulate 
                                                 rdfs:comment "Aluminum concentration of particles larger than 0.45 microns  (in ppb,specifically in microgram/litre)." ;
                                                 rdfs:label "aluminumParticulate" .


:OilAnalysisMetalsAnalogKind.barium 
                                    rdfs:comment "Barium concentration (in ppb, specifically in microgram/litre)." ;
                                    rdfs:label "barium" .


:OilAnalysisMetalsAnalogKind.boron 
                                   rdfs:comment "Boron concentration (in ppb, specifically in microgram/litre)." ;
                                   rdfs:label "boron" .


:OilAnalysisMetalsAnalogKind.cadmium 
                                     rdfs:comment "Cadmium concentration (in ppb, specifically in microgram/litre)." ;
                                     rdfs:label "cadmium" .


:OilAnalysisMetalsAnalogKind.calcium 
                                     rdfs:comment "Calcium concentration (in ppb, specifically in microgram/litre)." ;
                                     rdfs:label "calcium" .


:OilAnalysisMetalsAnalogKind.chromium 
                                      rdfs:comment "Chromium concentration (in ppb, specifically in microgram/litre)." ;
                                      rdfs:label "chromium" .


:OilAnalysisMetalsAnalogKind.copper 
                                    rdfs:comment "Copper concentration (in ppb, specifically in microgram/litre)." ;
                                    rdfs:label "copper" .


:OilAnalysisMetalsAnalogKind.copperParticulate 
                                               rdfs:comment "Copper concentration of particles larger than 0.45 microns  (in ppb,specifically in microgram/litre)." ;
                                               rdfs:label "copperParticulate" .


:OilAnalysisMetalsAnalogKind.iron 
                                  rdfs:comment "Iron concentration (in ppb, specifically in microgram/litre)." ;
                                  rdfs:label "iron" .


:OilAnalysisMetalsAnalogKind.ironParticulate 
                                             rdfs:comment "Iron concentration of particles larger than 0.45 microns (in ppb, specifically in microgram/litre)." ;
                                             rdfs:label "ironParticulate" .


:OilAnalysisMetalsAnalogKind.lead 
                                  rdfs:comment "Lead concentration (in ppb, specifically in microgram/litre)." ;
                                  rdfs:label "lead" .


:OilAnalysisMetalsAnalogKind.leadParticulate 
                                             rdfs:comment "Lead concentration of particles larger than 0.45 microns (in ppb, specifically in microgram/litre)." ;
                                             rdfs:label "leadParticulate" .


:OilAnalysisMetalsAnalogKind.lithium 
                                     rdfs:comment "Lithium concentration (in ppb, specifically in microgram/litre)." ;
                                     rdfs:label "lithium" .


:OilAnalysisMetalsAnalogKind.magnesium 
                                       rdfs:comment "Magnesium concentration (in ppb, specifically in microgram/litre)." ;
                                       rdfs:label "magnesium" .


:OilAnalysisMetalsAnalogKind.molybdenum 
                                        rdfs:comment "Molybdenum concentration (in ppb, specifically in microgram/litre)." ;
                                        rdfs:label "molybdenum" .


:OilAnalysisMetalsAnalogKind.nickel 
                                    rdfs:comment "Nickel concentration (in ppb, specifically in microgram/litre)." ;
                                    rdfs:label "nickel" .


:OilAnalysisMetalsAnalogKind.phosphorus 
                                        rdfs:comment "Phosphorus concentration (in ppb, specifically in microgram/litre)." ;
                                        rdfs:label "phosphorus" .


:OilAnalysisMetalsAnalogKind.silicon 
                                     rdfs:comment "Silicon concentration (in ppb, specifically in microgram/litre)." ;
                                     rdfs:label "silicon" .


:OilAnalysisMetalsAnalogKind.silver 
                                    rdfs:comment "Silver concentration (in ppb, specifically in microgram/litre)." ;
                                    rdfs:label "silver" .


:OilAnalysisMetalsAnalogKind.silverParticulate 
                                               rdfs:comment "Silver concentration of particles larger than 0.45 microns (in ppb, specifically in microgram/litre)." ;
                                               rdfs:label "silverParticulate" .


:OilAnalysisMetalsAnalogKind.sodium 
                                    rdfs:comment "Sodium concentration (in ppb, specifically in microgram/litre)." ;
                                    rdfs:label "sodium" .


:OilAnalysisMetalsAnalogKind.tin 
                                 rdfs:comment "Tin concentration (in ppb, specifically in microgram/litre)." ;
                                 rdfs:label "tin" .


:OilAnalysisMetalsAnalogKind.titanium 
                                      rdfs:comment "Titanium concentration (in ppb, specifically in microgram/litre)." ;
                                      rdfs:label "titanium" .


:OilAnalysisMetalsAnalogKind.tungsten 
                                      rdfs:comment "Tungsten concentration (in ppb, specifically in microgram/litre)." ;
                                      rdfs:label "tungsten" .


:OilAnalysisMetalsAnalogKind.vanadium 
                                      rdfs:comment "Vanadium concentration (in ppb, specifically in microgram/litre)." ;
                                      rdfs:label "vanadium" .


:OilAnalysisMetalsAnalogKind.zinc 
                                  rdfs:comment "Zinc concentration (in ppb, specifically in microgram/litre)." ;
                                  rdfs:label "zinc" .


:OilAnalysisMetalsAnalogKind.zincParticulate 
                                             rdfs:comment "Zinc concentration of particles larger than 0.45 microns (in ppb, specifically in microgram/litre)." ;
                                             rdfs:label "zincParticulate" .


:OilAnalysisMoistureAnalogKind.dewPoint 
                                        rdfs:comment "Dew point (in °C). Is usually a negative value." ;
                                        rdfs:label "dewPoint" .


:OilAnalysisMoistureAnalogKind.relativeSaturation 
                                                  rdfs:comment "Relative saturation of water in fluid (in percent)." ;
                                                  rdfs:label "relativeSaturation" .


:OilAnalysisMoistureAnalogKind.relativeSaturationCalculated 
                                                            rdfs:comment "Calculated relative saturation of water in fluid (in percent)." ;
                                                            rdfs:label "relativeSaturationCalculated" .


:OilAnalysisMoistureAnalogKind.waterContent 
                                            rdfs:comment "Moisture measured via coulometric Karl Fischer titration (in ppm, specifically milligram/kilogram)." ;
                                            rdfs:label "waterContent" .


:OilAnalysisMoistureAnalogKind.waterContentMonitoredViaAluminumOxide 
                                                                     rdfs:comment "Water content by aluminum oxide sensor (in ppm, specifically milligram/kilogram)." ;
                                                                     rdfs:label "waterContentMonitoredViaAluminumOxide" .


:OilAnalysisMoistureAnalogKind.waterContentMonitoredViaCapacitance 
                                                                   rdfs:comment "Water content by capacitance sensor (in ppm, specifically milligram/kilogram)." ;
                                                                   rdfs:label "waterContentMonitoredViaCapacitance" .


:OilAnalysisMoistureAnalogKind.waterContentMonitoredViaInfrared 
                                                                rdfs:comment "Water content by infrared sensor (in ppm, specifically milligram/kilogram)." ;
                                                                rdfs:label "waterContentMonitoredViaInfrared" .


:OilAnalysisMoistureAnalogKind.waterContentMonitoredViaOther 
                                                             rdfs:comment "Water content by other sensor (in ppm, specifically milligram/kilogram)." ;
                                                             rdfs:label "waterContentMonitoredViaOther" .


:OilAnalysisPCBAnalogKind.aroclor1016 
                                      rdfs:comment "Concentration of Aroclor 1016 (in ppm, specifically in mg/kg)." ;
                                      rdfs:label "aroclor1016" .


:OilAnalysisPCBAnalogKind.aroclor1221 
                                      rdfs:comment "Concentration of Aroclor 1221 (in ppm, specifically in mg/kg)." ;
                                      rdfs:label "aroclor1221" .


:OilAnalysisPCBAnalogKind.aroclor1242 
                                      rdfs:comment "Concentration of Aroclor 1242 (in ppm, specifically in mg/kg)." ;
                                      rdfs:label "aroclor1242" .


:OilAnalysisPCBAnalogKind.aroclor1254 
                                      rdfs:comment "Concentration of Aroclor 1254 (in ppm, specifically in mg/kg)." ;
                                      rdfs:label "aroclor1254" .


:OilAnalysisPCBAnalogKind.aroclor1260 
                                      rdfs:comment "Concentration of Aroclor 1260 (in ppm, specifically in mg/kg)." ;
                                      rdfs:label "aroclor1260" .


:OilAnalysisPCBAnalogKind.totalPCB 
                                   rdfs:comment "Total arochlor (PCB) content (in ppm, specifically in mg/kg). Is the sum of Aroclor 1221, Aroclor 1242, Aroclor 1254, Aroclor 1260, Aroclor 1016." ;
                                   rdfs:label "totalPCB" .


:OilAnalysisPCBDiscreteKind.testKitPCB 
                                       rdfs:comment "Possible values:  <blank>, <50, >50." ;
                                       rdfs:label "testKitPCB" .


:OilAnalysisPaperAnalogKind.acetylfuran 
                                        rdfs:comment "2-acetylfuran (2ACF) (in ppb). Also known as: 2-acetylfuran, furyl methyl ketone, 2-furyl methyl ketone, methyl 2-furyl ketone, and 1-(2-furanyl)ethanone." ;
                                        rdfs:label "acetylfuran" .


:OilAnalysisPaperAnalogKind.degreeOfPolymerization 
                                                   rdfs:comment "Direct measurement of degree of polymerization (DP) (unitless)." ;
                                                   rdfs:label "degreeOfPolymerization" .


:OilAnalysisPaperAnalogKind.degreeOfPolymerizationCalculated 
                                                             rdfs:comment "Calculated degree of polymerization (DP) calculated using the Chendong equation (unitless)." ;
                                                             rdfs:label "degreeOfPolymerizationCalculated" .


:OilAnalysisPaperAnalogKind.ethanol 
                                    rdfs:comment "Concentration of ethanol (in ppb, specifically microgram/kilogram)." ;
                                    rdfs:label "ethanol" .


:OilAnalysisPaperAnalogKind.furfural 
                                     rdfs:comment "2-furaldehyde (2FAL) (in ppb). Also known as: 2-furfural, 2-furaldehyde, 2-furanaldehyde, fural, furfuraldehyde, furaldehyde, and 2-furancarboxaldehyde." ;
                                     rdfs:label "furfural" .


:OilAnalysisPaperAnalogKind.furfurylAlcohol 
                                            rdfs:comment "Furfuryl alcohol (2FOL) (in ppb). Also known as: 2-furyl alcohol, 2-furfurol, 2-furylmethanol, 2-hydroxymethylfuran, 2-furancarbinol, furancarbinol, 2-furanmethanol, furanmethanol, furfural alcohol, and alpha-furylcarbinol." ;
                                            rdfs:label "furfurylAlcohol" .


:OilAnalysisPaperAnalogKind.hydroxymethylfurfural 
                                                  rdfs:comment "5-hydroxymethyl-2-furaldehyde (5H2F) (in ppb). Also known as: 5-hydroxymethyl-2-furfural, 5-hydroxymethyl-2-furaldehyde, 5-hydroxymethylfurfuraldehyde, and 5-hydroxymethylfurfural." ;
                                                  rdfs:label "hydroxymethylfurfural" .


:OilAnalysisPaperAnalogKind.methanol 
                                     rdfs:comment "Concentration of methanol (in ppb, specifically microgram/kilogram)." ;
                                     rdfs:label "methanol" .


:OilAnalysisPaperAnalogKind.methylfurfural 
                                           rdfs:comment "5-methyl-2-furaldehyde (5M2F) (in ppb). Also known as: 5-methyl-2-furfural, 5-methyl-2-furaldehyde, 5-methyl-2-furfuraldehyde, and 5-methylfurfural." ;
                                           rdfs:label "methylfurfural" .


:OilAnalysisPaperAnalogKind.solidInsulationDielectricStrength 
                                                              rdfs:comment "Dielectric breakdown of solid electrical insulating materials (in kV)." ;
                                                              rdfs:label "solidInsulationDielectricStrength" .


:OilAnalysisPaperAnalogKind.tensileStrength 
                                            rdfs:comment "Tensile strength (in kilonewtons/metre)." ;
                                            rdfs:label "tensileStrength" .


:OilAnalysisPaperAnalogKind.totalFuran 
                                       rdfs:comment "Total furan (in ppb). Is the total of the concentrations of 5-hydroxymethyl-2-furaldehyde (5H2F), furfuryl alcohol (2FOL), 2-furaldehyde (2FAL), 2-acetylfuran (2ACF), 5-methyl-2-furaldehyde (5M2F)." ;
                                       rdfs:label "totalFuran" .


:OilAnalysisParticleAnalogKind.carbonPercent 
                                             rdfs:comment "Percent of particles which are carbon." ;
                                             rdfs:label "carbonPercent" .


:OilAnalysisParticleAnalogKind.count100Plus 
                                            rdfs:comment "Count of particles 100 microns and larger in a 1 millilitre sample." ;
                                            rdfs:label "count100Plus" .


:OilAnalysisParticleAnalogKind.count10Plus 
                                           rdfs:comment "Count of particles 10 microns and larger in a 1 millilitre sample." ;
                                           rdfs:label "count10Plus" .


:OilAnalysisParticleAnalogKind.count14Plus 
                                           rdfs:comment "Count of particles 14 microns and larger in a 1 millilitre sample." ;
                                           rdfs:label "count14Plus" .


:OilAnalysisParticleAnalogKind.count15Plus 
                                           rdfs:comment "Count of particles 15 microns and larger in a 1 millilitre sample." ;
                                           rdfs:label "count15Plus" .


:OilAnalysisParticleAnalogKind.count21Plus 
                                           rdfs:comment "Count of particles 21 microns and larger in a 1 millilitre sample." ;
                                           rdfs:label "count21Plus" .


:OilAnalysisParticleAnalogKind.count25Plus 
                                           rdfs:comment "Count of particles 25 microns and larger in a 1 millilitre sample." ;
                                           rdfs:label "count25Plus" .


:OilAnalysisParticleAnalogKind.count2Plus 
                                          rdfs:comment "Count of particles 2 microns and larger in a 1 millilitre sample." ;
                                          rdfs:label "count2Plus" .


:OilAnalysisParticleAnalogKind.count38Plus 
                                           rdfs:comment "Count of particles 38 microns and larger in a 1 millilitre sample." ;
                                           rdfs:label "count38Plus" .


:OilAnalysisParticleAnalogKind.count4Plus 
                                          rdfs:comment "Count of particles 4 microns and larger in a 1 millilitre sample." ;
                                          rdfs:label "count4Plus" .


:OilAnalysisParticleAnalogKind.count50Plus 
                                           rdfs:comment "Count of particles 50 microns and larger in a 1 millilitre sample." ;
                                           rdfs:label "count50Plus" .


:OilAnalysisParticleAnalogKind.count5Plus 
                                          rdfs:comment "Count of particles 5 microns and larger in a 1 millilitre sample." ;
                                          rdfs:label "count5Plus" .


:OilAnalysisParticleAnalogKind.count6Plus 
                                          rdfs:comment "Count of particles 6 microns and larger in a 1 millilitre sample." ;
                                          rdfs:label "count6Plus" .


:OilAnalysisParticleAnalogKind.count70Plus 
                                           rdfs:comment "Count of particles 70 microns and larger in a 1 millilitre sample." ;
                                           rdfs:label "count70Plus" .


:OilAnalysisParticleAnalogKind.fibrePercent 
                                            rdfs:comment "Percent of particles which are fibres." ;
                                            rdfs:label "fibrePercent" .


:OilAnalysisParticleAnalogKind.metalPercent 
                                            rdfs:comment "Percent of particles which are metal." ;
                                            rdfs:label "metalPercent" .


:OilAnalysisParticleAnalogKind.otherPercent 
                                            rdfs:comment "Percent of particles which are 'other'." ;
                                            rdfs:label "otherPercent" .


:OilAnalysisParticleDiscreteKind.opacity 
                                         rdfs:comment """Opacity of oil.
Possible values: any integer.""" ;
                                         rdfs:label "opacity" .


:OilPreservationKind.conservator 
                                 rdfs:label "conservator" .


:OilPreservationKind.freeBreathing 
                                   rdfs:label "freeBreathing" .


:OilPreservationKind.nitrogenBlanket 
                                     rdfs:label "nitrogenBlanket" .


:OilPreservationKind.other 
                           rdfs:label "other" .


:OilSampleLocation.oilDrainageDevice 
                                     rdfs:comment "Sample from oil drainage device." ;
                                     rdfs:label "oilDrainageDevice" .


:OilSampleLocation.oilSampleValve 
                                  rdfs:comment "Sample from oil sample valve." ;
                                  rdfs:label "oilSampleValve" .


:OilSampleLocation.other 
                         rdfs:comment "Sample from other location." ;
                         rdfs:label "other" .


:OilTemperatureSource.infraredGun 
                                  rdfs:comment "Oil temperature from infrared gun." ;
                                  rdfs:label "infraredGun" .


:OilTemperatureSource.other 
                            rdfs:comment "Oil temperature from other souce." ;
                            rdfs:label "other" .


:OilTemperatureSource.topOilTemperatureGauge 
                                             rdfs:comment "Oil temperature from top oil temperature gauge." ;
                                             rdfs:label "topOilTemperatureGauge" .


:OnOff.OFF 
           rdfs:label "OFF" .


:OnOff.ON 
          rdfs:label "ON" .


:OperatingMechanismKind.capacitorTrip 
                                      rdfs:comment "Capacitor trip mechanism." ;
                                      rdfs:label "capacitorTrip" .


:OperatingMechanismKind.hydraulic 
                                  rdfs:comment "Hydraulic mechanism." ;
                                  rdfs:label "hydraulic" .


:OperatingMechanismKind.pneudraulic 
                                    rdfs:comment "Pneudraulic mechanism." ;
                                    rdfs:label "pneudraulic" .


:OperatingMechanismKind.pneumatic 
                                  rdfs:comment "Pneumatic mechanism." ;
                                  rdfs:label "pneumatic" .


:OperatingMechanismKind.solenoid 
                                 rdfs:comment "Solenoid mechanism." ;
                                 rdfs:label "solenoid" .


:OperatingMechanismKind.spring 
                               rdfs:comment "Spring mechanism." ;
                               rdfs:label "spring" .


:OperatingMechanismKind.springHandCrank 
                                        rdfs:comment "Spring hand-crank mechanism." ;
                                        rdfs:label "springHandCrank" .


:OperatingMechanismKind.springHydraulic 
                                        rdfs:comment "Spring hydraulic mechanism." ;
                                        rdfs:label "springHydraulic" .


:OperatingMechanismKind.springMotor 
                                    rdfs:comment "Spring motor mechanism." ;
                                    rdfs:label "springMotor" .


:OperationalLimitDirectionKind.absoluteValue 
                                             rdfs:comment "An absoluteValue limit means that a monitored absolute value above the limit value is a violation." ;
                                             rdfs:label "absoluteValue" .


:OperationalLimitDirectionKind.high 
                                    rdfs:comment "High means that a monitored value above the limit value is a violation.   If applied to a terminal flow, the positive direction is into the terminal." ;
                                    rdfs:label "high" .


:OperationalLimitDirectionKind.low 
                                   rdfs:comment "Low means a monitored value below the limit is a violation.  If applied to a terminal flow, the positive direction is into the terminal." ;
                                   rdfs:label "low" .


:OrganisationCode.BILL_TO 
                          rdfs:label "BILL_TO" .


:OrganisationCode.PAY_TO 
                         rdfs:label "PAY_TO" .


:OrganisationCode.PROVIDED_BY 
                              rdfs:label "PROVIDED_BY" .


:OrganisationCode.SOLD_TO 
                          rdfs:label "SOLD_TO" .


:OrganisationType.CUSTOMER 
                           rdfs:label "CUSTOMER" .


:OrganisationType.RTO 
                      rdfs:label "RTO" .


:OrientationKind.negative 
                          rdfs:comment "For 2D diagrams, a negative orientation gives the left-hand orientation (favoured by computer graphics displays) with X values increasing from left to right and Y values increasing from top to bottom.   This is also known as a left hand orientation." ;
                          rdfs:label "negative" .


:OrientationKind.positive 
                          rdfs:comment "For 2D diagrams, a positive orientation will result in X values increasing from left to right and Y values increasing from bottom to top.  This is also known as a right hand orientation." ;
                          rdfs:label "positive" .


:OutageCauseKind.animal 
                        rdfs:comment "This outage was caused by an animal is was unplanned.  As such it is treated as a forced outage and is probably classified as \"trouble\" with a Trouble Ticket as well as a work/service order.  The primary difference between this and an unplanned outage is the reason for the outage.  If an animal caused this and perished as a result, the utility may have other actions that are required to be taken by the EPA or other groups with whom the utility has an agreement." ;
                        rdfs:label "animal" .


:OutageCauseKind.lightingStrike 
                                rdfs:comment "Outage is caused by a lighting strike" ;
                                rdfs:label "lightingStrike" .


:OutageCauseKind.lineDown 
                          rdfs:comment "The outage is caused by a line down" ;
                          rdfs:label "lineDown" .


:OutageCauseKind.poleDown 
                          rdfs:comment "The outage is caused by a pole down" ;
                          rdfs:label "poleDown" .


:OutageCauseKind.treeDown 
                          rdfs:comment "The outage is caused by a tree down" ;
                          rdfs:label "treeDown" .


:OutageStatusKind.closed 
                         rdfs:comment "The outage has been fully restored, the crews have been released and the outage is shown as closed" ;
                         rdfs:label "closed" .


:OutageStatusKind.confirmed 
                            rdfs:comment "the outage has been verified" ;
                            rdfs:label "confirmed" .


:OutageStatusKind.partiallyRestored 
                                    rdfs:comment "Some of the usage points affected by the outage have been restored but other usage points are still out of power." ;
                                    rdfs:label "partiallyRestored" .


:OutageStatusKind.predicted 
                            rdfs:comment "the outage may not be real since it has not been verified - it is only thought to be an outage." ;
                            rdfs:label "predicted" .


:OutageStatusKind.restored 
                           rdfs:comment "All usage points associated with the outage have been restored" ;
                           rdfs:label "restored" .


:PSREventKind.inService 
                        rdfs:comment "Power system resource state change to in service." ;
                        rdfs:label "inService" .


:PSREventKind.other 
                    rdfs:comment "Other power system resource state change." ;
                    rdfs:label "other" .


:PSREventKind.outOfService 
                           rdfs:comment "Power system resource state change to out of service." ;
                           rdfs:label "outOfService" .


:PSREventKind.pendingAdd 
                         rdfs:comment "Power system resource state change to pending add." ;
                         rdfs:label "pendingAdd" .


:PSREventKind.pendingRemove 
                            rdfs:comment "Power system resource state change to pending remove." ;
                            rdfs:label "pendingRemove" .


:PSREventKind.pendingReplace 
                             rdfs:comment "Power system resource state change to pending replace." ;
                             rdfs:label "pendingReplace" .


:PSREventKind.unknown 
                      rdfs:comment "Unknown power system resource state change." ;
                      rdfs:label "unknown" .


:ParticipationCategoryMPM.L 
                            rdfs:label "L" .


:ParticipationCategoryMPM.N 
                            rdfs:label "N" .


:ParticipationCategoryMPM.S 
                            rdfs:label "S" .


:ParticipationCategoryMPM.Y 
                            rdfs:label "Y" .


:PassIndicatorType.DA 
                      rdfs:comment "Day Ahead" ;
                      rdfs:label "DA" .


:PassIndicatorType.HA-SCUC 
                           rdfs:comment "Hour Ahead Security Constrained Unit Commitment" ;
                           rdfs:label "HA-SCUC" .


:PassIndicatorType.MPM-1 
                         rdfs:comment "Market Power Mitigation Pass 1" ;
                         rdfs:label "MPM-1" .


:PassIndicatorType.MPM-2 
                         rdfs:comment "Market Power Mitigation Pass 2" ;
                         rdfs:label "MPM-2" .


:PassIndicatorType.MPM-3 
                         rdfs:comment "Market Power Mitigation Pass 3" ;
                         rdfs:label "MPM-3" .


:PassIndicatorType.MPM-4 
                         rdfs:comment "Market Power Mitigation Pass 4" ;
                         rdfs:label "MPM-4" .


:PassIndicatorType.RTED 
                        rdfs:comment "Real Time Economic Dispatch" ;
                        rdfs:label "RTED" .


:PassIndicatorType.RTPD 
                        rdfs:comment "Real Time Pre Dispatch" ;
                        rdfs:label "RTPD" .


:PassIndicatorType.RUC 
                       rdfs:comment "Residual Unit Commitment" ;
                       rdfs:label "RUC" .


:PetersenCoilModeKind.automaticPositioning 
                                           rdfs:comment "Automatic positioning." ;
                                           rdfs:label "automaticPositioning" .


:PetersenCoilModeKind.fixed 
                            rdfs:comment "Fixed position." ;
                            rdfs:label "fixed" .


:PetersenCoilModeKind.manual 
                             rdfs:comment "Manual positioning." ;
                             rdfs:label "manual" .


:PhaseConnectedFaultKind.lineOpen 
                                  rdfs:comment "The fault is when the conductor path is broken between two terminals. Additional coexisting faults may be required if the broken conductor also causes connections to grounds or other lines or phases." ;
                                  rdfs:label "lineOpen" .


:PhaseConnectedFaultKind.lineToGround 
                                      rdfs:comment "The fault connects the indicated phases to ground. The line to line fault impedance is not used and assumed infinite. The full ground impedance is connected between each phase specified in the fault and ground, but not between the phases." ;
                                      rdfs:label "lineToGround" .


:PhaseConnectedFaultKind.lineToLine 
                                    rdfs:comment "The fault connects the specified phases together without a connection to ground. The ground impedance of this fault is ignored. The line to line impedance is connected between each of the phases specified in the fault. For example three times for a three phase fault, one time for a two phase fault.  A single phase fault should not be specified." ;
                                    rdfs:label "lineToLine" .


:PhaseConnectedFaultKind.lineToLineToGround 
                                            rdfs:comment "The fault connects the indicated phases to ground and to each other. The line to line impedance is connected between each of the phases specified in the fault in a full mesh. For example three times for a three phase fault, one time for a two phase fault. A single phase fault should not be specified. The full ground impedance is connected between each phase specified in the fault and ground." ;
                                            rdfs:label "lineToLineToGround" .


:PhaseShuntConnectionKind.D uml:hasInitialValue "1" ;
                            
                            rdfs:comment "Delta connection." ;
                            rdfs:label "D" .


:PhaseShuntConnectionKind.G uml:hasInitialValue "5" ;
                            
                            rdfs:comment "Ground connection; use when explicit connection to ground needs to be expressed in combination with the phase code, such as for electrical wire/cable or for meters." ;
                            rdfs:label "G" .


:PhaseShuntConnectionKind.I uml:hasInitialValue "4" ;
                            
                            rdfs:comment "Independent winding, for single-phase connections." ;
                            rdfs:label "I" .


:PhaseShuntConnectionKind.Y uml:hasInitialValue "2" ;
                            
                            rdfs:comment "Wye connection." ;
                            rdfs:label "Y" .


:PhaseShuntConnectionKind.Yn uml:hasInitialValue "3" ;
                             
                             rdfs:comment "Wye, with neutral brought out for grounding." ;
                             rdfs:label "Yn" .


:PinBranchGroupKind.activePower 
                                rdfs:comment "Active power in the branch group." ;
                                rdfs:label "activePower" .


:PinBranchGroupKind.reactivePower 
                                  rdfs:comment "Reactive power in the branch group." ;
                                  rdfs:label "reactivePower" .


:PinEquipmentKind.activePowerLimit 
                                   rdfs:comment "Compare load flow result against the active limit for active power for the given equipment." ;
                                   rdfs:label "activePowerLimit" .


:PinEquipmentKind.apparentPowerLimit 
                                     rdfs:comment "Compare load flow result against the active limit for apparent power for the given equipment." ;
                                     rdfs:label "apparentPowerLimit" .


:PinEquipmentKind.connected 
                            rdfs:comment "Check if all terminal on the equipment is connected." ;
                            rdfs:label "connected" .


:PinEquipmentKind.currentLimit 
                               rdfs:comment "Compare load flow result against the active current limit for the equipment." ;
                               rdfs:label "currentLimit" .


:PinEquipmentKind.inService 
                            rdfs:comment "Check if equipment is in service, True if in service otherwise false." ;
                            rdfs:label "inService" .


:PinEquipmentKind.ratedCurrent 
                               rdfs:comment "Compare load flow result against rated current on the equipment (switch)." ;
                               rdfs:label "ratedCurrent" .


:PinEquipmentKind.voltageLimit 
                               rdfs:comment "Compare load flow result against the active voltage limit for the equipment." ;
                               rdfs:label "voltageLimit" .


:PinTerminalKind.activePower 
                             rdfs:comment "Active Power on the Terminal." ;
                             rdfs:label "activePower" .


:PinTerminalKind.apparentPower 
                               rdfs:comment "Apparent Power on the Terminal." ;
                               rdfs:label "apparentPower" .


:PinTerminalKind.reactivePower 
                               rdfs:comment "Reactive Power on the Terminal." ;
                               rdfs:label "reactivePower" .


:PinTerminalKind.voltage 
                         rdfs:comment "Voltage on the Terminal." ;
                         rdfs:label "voltage" .


:PoleBaseKind.asphalt 
                      rdfs:label "asphalt" .


:PoleBaseKind.cement 
                     rdfs:label "cement" .


:PoleBaseKind.dirt 
                   rdfs:label "dirt" .


:PoleBaseKind.other 
                    rdfs:label "other" .


:PoleBaseKind.unknown 
                      rdfs:label "unknown" .


:PolePreservativeKind.cellon 
                             rdfs:label "cellon" .


:PolePreservativeKind.chemonite 
                                rdfs:label "chemonite" .


:PolePreservativeKind.creosote 
                               rdfs:label "creosote" .


:PolePreservativeKind.naphthena 
                                rdfs:label "naphthena" .


:PolePreservativeKind.other 
                            rdfs:label "other" .


:PolePreservativeKind.penta 
                            rdfs:label "penta" .


:PolePreservativeKind.unknown 
                              rdfs:label "unknown" .


:PoleTreatmentKind.butt 
                        rdfs:label "butt" .


:PoleTreatmentKind.full 
                        rdfs:label "full" .


:PoleTreatmentKind.grayStain 
                             rdfs:label "grayStain" .


:PoleTreatmentKind.greenStain 
                              rdfs:label "greenStain" .


:PoleTreatmentKind.natural 
                           rdfs:label "natural" .


:PoleTreatmentKind.other 
                         rdfs:label "other" .


:PoleTreatmentKind.penta 
                         rdfs:label "penta" .


:PoleTreatmentKind.unknown 
                           rdfs:label "unknown" .


:PotentialTransformerKind.capacitiveCoupling 
                                             rdfs:comment "The potential transformer is using capacitive coupling to create secondary voltage." ;
                                             rdfs:label "capacitiveCoupling" .


:PotentialTransformerKind.inductive 
                                    rdfs:comment "The potential transformer is using induction coils to create secondary voltage." ;
                                    rdfs:label "inductive" .


:PriceSetFlag.N 
                rdfs:label "N" .


:PriceSetFlag.S 
                rdfs:label "S" .


:PriceSetFlag.Y 
                rdfs:label "Y" .


:PriceTypeKind.capacity 
                        rdfs:label "capacity" .


:PriceTypeKind.congestion 
                          rdfs:label "congestion" .


:PriceTypeKind.delivery 
                        rdfs:label "delivery" .


:PriceTypeKind.loss 
                    rdfs:label "loss" .


:PriceTypeKind.mileage 
                       rdfs:label "mileage" .


:PriceTypeKind.system 
                      rdfs:label "system" .


:PriceTypeKind.total 
                     rdfs:label "total" .


:ProcedureKind.diagnosis 
                         rdfs:comment "Diagnosis procedure." ;
                         rdfs:label "diagnosis" .


:ProcedureKind.inspection 
                          rdfs:comment "Inspection procedure." ;
                          rdfs:label "inspection" .


:ProcedureKind.maintenance 
                           rdfs:comment "Maintenance procedure." ;
                           rdfs:label "maintenance" .


:ProcedureKind.other 
                     rdfs:comment "Other procedure." ;
                     rdfs:label "other" .


:ProcedureKind.test 
                    rdfs:comment "Test procedure." ;
                    rdfs:label "test" .


:ProjectStatusKind.cancelled 
                             rdfs:label "cancelled" .


:ProjectStatusKind.closed 
                          rdfs:label "closed" .


:ProjectStatusKind.draft 
                         rdfs:label "draft" .


:ProjectStatusKind.frozen 
                          rdfs:label "frozen" .


:ProtectiveActionAdjustmentKind.byPercentage 
                                             rdfs:comment "The adjustment is in percentage of the active value." ;
                                             rdfs:label "byPercentage" .


:ProtectiveActionAdjustmentKind.byValue 
                                        rdfs:comment "The adjustment is in given by a value that defined the changes that will be done to the active value." ;
                                        rdfs:label "byValue" .


:ProtectiveActionAdjustmentKind.measurement 
                                            rdfs:comment "The equipment will operating on a value given by a measurement." ;
                                            rdfs:label "measurement" .


:ProtectiveActionAdjustmentKind.setValue 
                                         rdfs:comment "The equipment will operate on the new value." ;
                                         rdfs:label "setValue" .


:PurposeFlagType.M 
                   rdfs:label "M" .


:PurposeFlagType.R 
                   rdfs:label "R" .


:RampCurveType._0 
                  rdfs:comment "Fixed ramp rate independent of rate function unit MW output" ;
                  rdfs:label "0" .


:RampCurveType._1 
                  rdfs:comment "Static ramp rates as a function of unit MW output only" ;
                  rdfs:label "1" .


:RampCurveType._2 
                  rdfs:comment "Dynamic ramp rates as a function of unit MW output and ramping time" ;
                  rdfs:label "2" .


:RampRateCondition.BEST 
                        rdfs:label "BEST" .


:RampRateCondition.NA 
                      rdfs:comment "not applicable" ;
                      rdfs:label "NA" .


:RampRateCondition.NORMAL 
                          rdfs:label "NORMAL" .


:RampRateCondition.WORST 
                         rdfs:label "WORST" .


:RampRateType.INTERTIE 
                       rdfs:comment "Intertie ramp rate." ;
                       rdfs:label "INTERTIE" .


:RampRateType.LD_DROP 
                      rdfs:comment "Load drop ramp rate." ;
                      rdfs:label "LD_DROP" .


:RampRateType.LD_PICKUP 
                        rdfs:comment "Load pick up rate." ;
                        rdfs:label "LD_PICKUP" .


:RampRateType.OP 
                 rdfs:comment "Operational ramp rate." ;
                 rdfs:label "OP" .


:RampRateType.OP_RES 
                     rdfs:comment "Operating reserve ramp rate." ;
                     rdfs:label "OP_RES" .


:RampRateType.REG 
                  rdfs:comment "Regulating ramp rate." ;
                  rdfs:label "REG" .


:RandomisationKind.default 
                           rdfs:comment "Randomisation of start and/or end times involving the operation of one or more devices is controlled by default settings for the device(s)." ;
                           rdfs:label "default" .


:RandomisationKind.end 
                       rdfs:comment "End time of an event or control action affecting one or more devices is randomised to prevent simultaneous operation." ;
                       rdfs:label "end" .


:RandomisationKind.none 
                        rdfs:comment "Neither the start time nor the end time of an event or control action affecting one or more devices is randomised." ;
                        rdfs:label "none" .


:RandomisationKind.start 
                         rdfs:comment "Start time of an event or control action affecting one or more multiple devices is randomised." ;
                         rdfs:label "start" .


:RandomisationKind.startAndEnd 
                               rdfs:comment "Both the start time and the end time of an event or control action affecting one or more devices are randomised to prevent simultaneous operation." ;
                               rdfs:label "startAndEnd" .


:ReadingReasonKind.billing 
                           rdfs:comment "Reading(s) taken or to be taken in response to a billing-related inquiry by a customer or other party. A variant of 'inquiry'." ;
                           rdfs:label "billing" .


:ReadingReasonKind.demandReset 
                               rdfs:comment "Reading(s) taken or to be taken in conjunction with the resetting of one or more demand registers in a meter." ;
                               rdfs:label "demandReset" .


:ReadingReasonKind.inquiry 
                           rdfs:comment "Reading(s) taken or to be taken in response to an inquiry by a customer or other party." ;
                           rdfs:label "inquiry" .


:ReadingReasonKind.installation 
                                rdfs:comment "Reading(s) taken or to be taken in conjunction with installation of a meter." ;
                                rdfs:label "installation" .


:ReadingReasonKind.loadManagement 
                                  rdfs:comment "Reading(s) taken or to be taken to support management of loads on distribution networks or devices." ;
                                  rdfs:label "loadManagement" .


:ReadingReasonKind.loadResearch 
                                rdfs:comment "Reading(s) taken or to be taken to support research and analysis of loads on distribution networks or devices." ;
                                rdfs:label "loadResearch" .


:ReadingReasonKind.moveIn 
                          rdfs:comment "Reading(s) taken or to be taken in conjunction with a customer move-in event." ;
                          rdfs:label "moveIn" .


:ReadingReasonKind.moveOut 
                           rdfs:comment "Reading(s) taken or to be taken in conjunction with a customer move-out event." ;
                           rdfs:label "moveOut" .


:ReadingReasonKind.other 
                         rdfs:comment "Reading(s) taken or to be taken for some other reason or purpose." ;
                         rdfs:label "other" .


:ReadingReasonKind.removal 
                           rdfs:comment "Reading(s) taken or to be taken in conjunction with removal of a meter." ;
                           rdfs:label "removal" .


:ReadingReasonKind.serviceConnect 
                                  rdfs:comment "Reading(s) taken or to be taken in conjunction with a connection or re-connection of service." ;
                                  rdfs:label "serviceConnect" .


:ReadingReasonKind.serviceDisconnect 
                                     rdfs:comment "Reading(s) taken or to be taken in conjunction with a disconnection of service." ;
                                     rdfs:label "serviceDisconnect" .


:RegulatingControlModeKind.activePower 
                                       rdfs:comment "Active power is specified." ;
                                       rdfs:label "activePower" .


:RegulatingControlModeKind.admittance 
                                      rdfs:comment "Admittance is specified." ;
                                      rdfs:label "admittance" .


:RegulatingControlModeKind.currentFlow 
                                       rdfs:comment "Current flow is specified." ;
                                       rdfs:label "currentFlow" .


:RegulatingControlModeKind.powerFactor 
                                       rdfs:comment "Power factor is specified." ;
                                       rdfs:label "powerFactor" .


:RegulatingControlModeKind.reactivePower 
                                         rdfs:comment "Reactive power is specified." ;
                                         rdfs:label "reactivePower" .


:RegulatingControlModeKind.temperature 
                                       rdfs:comment "Control switches on/off based on the local temperature (i.e., a thermostat)." ;
                                       rdfs:label "temperature" .


:RegulatingControlModeKind.timeScheduled 
                                         rdfs:comment "Control switches on/off by time of day. The times may change on the weekend, or in different seasons." ;
                                         rdfs:label "timeScheduled" .


:RegulatingControlModeKind.voltage 
                                   rdfs:comment "Voltage is specified." ;
                                   rdfs:label "voltage" .


:RegulationBranchKind.breaker 
                              rdfs:label "breaker" .


:RegulationBranchKind.fuse 
                           rdfs:label "fuse" .


:RegulationBranchKind.line 
                           rdfs:label "line" .


:RegulationBranchKind.other 
                            rdfs:label "other" .


:RegulationBranchKind.recloser 
                               rdfs:label "recloser" .


:RegulationBranchKind.sectionner 
                                 rdfs:label "sectionner" .


:RegulationBranchKind.switch 
                             rdfs:label "switch" .


:RegulationBranchKind.transformer 
                                  rdfs:label "transformer" .


:RelativeDisplacementKind.centreEarth 
                                      rdfs:label "centreEarth" .


:RelativeDisplacementKind.ground 
                                 rdfs:label "ground" .


:RelativeDisplacementKind.seaLevel 
                                   rdfs:label "seaLevel" .


:RemedialActionSchemeKind.rAP 
                              rdfs:comment "Remedial Action Plan (RAP)." ;
                              rdfs:label "rAP" .


:RemedialActionSchemeKind.rAS 
                              rdfs:comment "Remedial Action Scheme (RAS)." ;
                              rdfs:label "rAS" .


:RemoteSignalKind.remoteBranchCurrentAmplitude 
                                               rdfs:comment "Input is branch current amplitude from remote terminal bus." ;
                                               rdfs:label "remoteBranchCurrentAmplitude" .


:RemoteSignalKind.remoteBusFrequency 
                                     rdfs:comment "Input is frequency from remote terminal bus." ;
                                     rdfs:label "remoteBusFrequency" .


:RemoteSignalKind.remoteBusFrequencyDeviation 
                                              rdfs:comment "Input is frequency deviation from remote terminal bus." ;
                                              rdfs:label "remoteBusFrequencyDeviation" .


:RemoteSignalKind.remoteBusVoltage 
                                   rdfs:comment "Input is voltage from remote terminal bus." ;
                                   rdfs:label "remoteBusVoltage" .


:RemoteSignalKind.remoteBusVoltageAmplitude 
                                            rdfs:comment "Input is voltage amplitude from remote terminal bus." ;
                                            rdfs:label "remoteBusVoltageAmplitude" .


:RemoteSignalKind.remoteBusVoltageAmplitudeDerivative 
                                                      rdfs:comment "Input is branch current amplitude derivative from remote terminal bus." ;
                                                      rdfs:label "remoteBusVoltageAmplitudeDerivative" .


:RemoteSignalKind.remoteBusVoltageFrequency 
                                            rdfs:comment "Input is voltage frequency from remote terminal bus." ;
                                            rdfs:label "remoteBusVoltageFrequency" .


:RemoteSignalKind.remoteBusVoltageFrequencyDeviation 
                                                     rdfs:comment "Input is voltage frequency deviation from remote terminal bus." ;
                                                     rdfs:label "remoteBusVoltageFrequencyDeviation" .


:RemoteSignalKind.remotePuBusVoltageDerivative 
                                               rdfs:comment "Input is PU voltage derivative from remote terminal bus." ;
                                               rdfs:label "remotePuBusVoltageDerivative" .


:RemoteUnitType.ControlCenter 
                              rdfs:comment "Control centre." ;
                              rdfs:label "ControlCenter" .


:RemoteUnitType.IED 
                    rdfs:comment "Intelligent electronic device (IED)." ;
                    rdfs:label "IED" .


:RemoteUnitType.RTU 
                    rdfs:comment "Remote terminal unit." ;
                    rdfs:label "RTU" .


:RemoteUnitType.SubstationControlSystem 
                                        rdfs:comment "Substation control system." ;
                                        rdfs:label "SubstationControlSystem" .


:ReportingMethodKind.automated 
                               rdfs:comment "Station automatically reports." ;
                               rdfs:label "automated" .


:ReportingMethodKind.manual 
                            rdfs:comment "Station must be physically visited to gather observations." ;
                            rdfs:label "manual" .


:ReportingMethodKind.queried 
                             rdfs:comment "Station must be queried to obtain observations." ;
                             rdfs:label "queried" .


:RequestorRmrTest.ISO 
                      rdfs:label "ISO" .


:RequestorRmrTest.MP 
                     rdfs:label "MP" .


:ReserveRequirementType.CONT 
                             rdfs:comment "Contingency" ;
                             rdfs:label "CONT" .


:ReserveRequirementType.OPRSV 
                              rdfs:comment "Operating Reserve" ;
                              rdfs:label "OPRSV" .


:ReserveRequirementType.REG 
                            rdfs:comment "Regulation" ;
                            rdfs:label "REG" .


:ResourceAssnType.CSNK 
                       rdfs:label "CSNK" .


:ResourceAssnType.CSRC 
                       rdfs:label "CSRC" .


:ResourceAssnType.LSE 
                      rdfs:label "LSE" .


:ResourceAssnType.RMR 
                      rdfs:label "RMR" .


:ResourceAssnType.SC 
                     rdfs:label "SC" .


:ResourceCapacityType.FO 
                         rdfs:comment "Flexible Offer." ;
                         rdfs:label "FO" .


:ResourceCapacityType.MO 
                         rdfs:comment "Must Offer." ;
                         rdfs:label "MO" .


:ResourceCapacityType.NR 
                         rdfs:comment "Non spinning reserve." ;
                         rdfs:label "NR" .


:ResourceCapacityType.RA 
                         rdfs:comment "Resource Adequacy." ;
                         rdfs:label "RA" .


:ResourceCapacityType.RD 
                         rdfs:comment "Regulation Down." ;
                         rdfs:label "RD" .


:ResourceCapacityType.RMR 
                          rdfs:comment "Reliability Must Run." ;
                          rdfs:label "RMR" .


:ResourceCapacityType.RU 
                         rdfs:comment "Regulation Up." ;
                         rdfs:label "RU" .


:ResourceCapacityType.SR 
                         rdfs:comment "Spinning reserve." ;
                         rdfs:label "SR" .


:ResourceCertificationCategory.DAM 
                                   rdfs:label "DAM" .


:ResourceCertificationCategory.GT 
                                  rdfs:comment "Generic" ;
                                  rdfs:label "GT" .


:ResourceCertificationCategory.RC 
                                  rdfs:label "RC" .


:ResourceCertificationCategory.RTM 
                                   rdfs:label "RTM" .


:ResourceCertificationKind.BLACKSTART 
                                      rdfs:comment "Black start" ;
                                      rdfs:label "BLACKSTART" .


:ResourceCertificationKind.Capacity 
                                    rdfs:label "Capacity" .


:ResourceCertificationKind.DemandSideResponse 
                                              rdfs:comment "Demand Side Reponse (DSR)" ;
                                              rdfs:label "DemandSideResponse" .


:ResourceCertificationKind.Energy 
                                  rdfs:label "Energy" .


:ResourceCertificationKind.IntermittentResource 
                                                rdfs:comment "Intermittent resource" ;
                                                rdfs:label "IntermittentResource" .


:ResourceCertificationKind.NonSpinningReserve 
                                              rdfs:comment "Non Spinning Reserve (NR, NONSPIN)" ;
                                              rdfs:label "NonSpinningReserve" .


:ResourceCertificationKind.RegulationDown 
                                          rdfs:comment "Regulation Down (RD, REGDN)" ;
                                          rdfs:label "RegulationDown" .


:ResourceCertificationKind.RegulationUp 
                                        rdfs:comment "Regulation Up (RU, REGUP)" ;
                                        rdfs:label "RegulationUp" .


:ResourceCertificationKind.ReliabilityMustRun 
                                              rdfs:comment "Reliability Must Run (RMR)" ;
                                              rdfs:label "ReliabilityMustRun" .


:ResourceCertificationKind.ReliabilityUnitCommitment 
                                                     rdfs:comment "Reliability unit commitment (RUC)" ;
                                                     rdfs:label "ReliabilityUnitCommitment" .


:ResourceCertificationKind.SpinningReserve 
                                           rdfs:comment "Spinning Reserve (SR, RRSPIN)" ;
                                           rdfs:label "SpinningReserve" .


:ResourceCertificationKind.SynchronousCondenser 
                                                rdfs:comment "Synchronous Condenser (SYNCCOND)" ;
                                                rdfs:label "SynchronousCondenser" .


:ResourceCertificationType.GT 
                              rdfs:comment "Generic Type" ;
                              rdfs:label "GT" .


:ResourceCertificationType.IR 
                              rdfs:comment "Intermittent Resource" ;
                              rdfs:label "IR" .


:ResourceCertificationType.NR 
                              rdfs:comment """Generic
Regulation
Spinning
Non-spinning
Intermittent Resource""" ;
                              rdfs:label "NR" .


:ResourceCertificationType.RG 
                              rdfs:comment "Regulating" ;
                              rdfs:label "RG" .


:ResourceCertificationType.SR 
                              rdfs:comment "Spinning Reserve" ;
                              rdfs:label "SR" .


:ResourceLimitIndicator.LOWER 
                              rdfs:label "LOWER" .


:ResourceLimitIndicator.UPPER 
                              rdfs:label "UPPER" .


:ResourceRegistrationStatus.Active 
                                   rdfs:comment "Resource registration is active" ;
                                   rdfs:label "Active" .


:ResourceRegistrationStatus.Decommissioned 
                                           rdfs:comment "Resource registration status is decommissioned" ;
                                           rdfs:label "Decommissioned" .


:ResourceRegistrationStatus.Mothballed 
                                       rdfs:comment "Resource registration has been suspended" ;
                                       rdfs:label "Mothballed" .


:ResourceRegistrationStatus.Planned 
                                    rdfs:comment "Registration status is in the planning stage" ;
                                    rdfs:label "Planned" .


:ResultsConstraintType.Actual 
                              rdfs:comment "Actual." ;
                              rdfs:label "Actual" .


:ResultsConstraintType.Contingency 
                                   rdfs:comment "Contingency." ;
                                   rdfs:label "Contingency" .


:ResultsConstraintType.FG_act 
                              rdfs:comment "Flowgate actual base case" ;
                              rdfs:label "FG_act" .


:ResultsConstraintType.Interface 
                                 rdfs:comment "Interface." ;
                                 rdfs:label "Interface" .


:RetiredReasonKind.environmental 
                                 rdfs:comment "Retired due to environmental reasons." ;
                                 rdfs:label "environmental" .


:RetiredReasonKind.excessiveMaintenance 
                                        rdfs:comment "Retired due to excessive maintainance issues." ;
                                        rdfs:label "excessiveMaintenance" .


:RetiredReasonKind.facilitiesUpgrade 
                                     rdfs:comment "Retired due to facility upgrade." ;
                                     rdfs:label "facilitiesUpgrade" .


:RetiredReasonKind.failed 
                          rdfs:comment "Retired because of failure." ;
                          rdfs:label "failed" .


:RetiredReasonKind.obsolescence 
                                rdfs:comment "Retired due to obsolescence." ;
                                rdfs:label "obsolescence" .


:RetiredReasonKind.other 
                         rdfs:comment "Retired due to other reasons." ;
                         rdfs:label "other" .


:RetiredReasonKind.sold 
                        rdfs:comment "Retired and sold." ;
                        rdfs:label "sold" .


:RevenueKind.commercial 
                        rdfs:comment "Commercial revenue." ;
                        rdfs:label "commercial" .


:RevenueKind.industrial 
                        rdfs:comment "Industrial revenue." ;
                        rdfs:label "industrial" .


:RevenueKind.irrigation 
                        rdfs:comment "Irrigation revenue." ;
                        rdfs:label "irrigation" .


:RevenueKind.nonResidential 
                            rdfs:comment "Non-residential revenue." ;
                            rdfs:label "nonResidential" .


:RevenueKind.other 
                   rdfs:comment "Other revenue kind." ;
                   rdfs:label "other" .


:RevenueKind.residential 
                         rdfs:comment "Residential revenue." ;
                         rdfs:label "residential" .


:RevenueKind.streetLight 
                         rdfs:comment "Streetlight revenue." ;
                         rdfs:label "streetLight" .


:RevisionKind.added 
                    rdfs:label "added" .


:RevisionKind.void 
                   rdfs:label "void" .


:RiskScoreKind.customerRisk 
                            rdfs:comment "Customer risk score." ;
                            rdfs:label "customerRisk" .


:RiskScoreKind.financialRisk 
                             rdfs:comment "Financial risk score." ;
                             rdfs:label "financialRisk" .


:RiskScoreKind.safetyRisk 
                          rdfs:comment "Safety risk score." ;
                          rdfs:label "safetyRisk" .


:RotorKind.roundRotor 
                      rdfs:comment "Round rotor type of synchronous machine." ;
                      rdfs:label "roundRotor" .


:RotorKind.salientPole 
                       rdfs:comment "Salient pole type of synchronous machine." ;
                       rdfs:label "salientPole" .


:SVCControlMode.reactivePower 
                              rdfs:comment "Reactive power control." ;
                              rdfs:label "reactivePower" .


:SVCControlMode.voltage 
                        rdfs:comment "Voltage control." ;
                        rdfs:label "voltage" .


:SampleContainerType.glassCan 
                              rdfs:comment "Glass can container." ;
                              rdfs:label "glassCan" .


:SampleContainerType.metalCan 
                              rdfs:comment "Metal can container." ;
                              rdfs:label "metalCan" .


:SampleContainerType.syringe 
                             rdfs:comment "Syringe." ;
                             rdfs:label "syringe" .


:ScaleKind.exponential 
                       rdfs:comment "Exponential scale." ;
                       rdfs:label "exponential" .


:ScaleKind.linear 
                  rdfs:comment "Linear scale." ;
                  rdfs:label "linear" .


:SchedClassType.F 
                  rdfs:label "F" .


:SchedClassType.P 
                  rdfs:label "P" .


:SchedClassType.R 
                  rdfs:label "R" .


:SealConditionKind.broken 
                          rdfs:comment "Seal is broken." ;
                          rdfs:label "broken" .


:SealConditionKind.locked 
                          rdfs:comment "Seal is locked." ;
                          rdfs:label "locked" .


:SealConditionKind.missing 
                           rdfs:comment "Seal is missing." ;
                           rdfs:label "missing" .


:SealConditionKind.open 
                        rdfs:comment "Seal is open." ;
                        rdfs:label "open" .


:SealConditionKind.other 
                         rdfs:comment "Other kind of seal condition." ;
                         rdfs:label "other" .


:SealKind.lead 
               rdfs:comment "Lead seal." ;
               rdfs:label "lead" .


:SealKind.lock 
               rdfs:comment "Lock seal." ;
               rdfs:label "lock" .


:SealKind.other 
                rdfs:comment "Other kind of seal." ;
                rdfs:label "other" .


:SealKind.steel 
                rdfs:comment "Steel seal." ;
                rdfs:label "steel" .


:SegmentCurveType.CONSULTATIVE 
                               rdfs:label "CONSULTATIVE" .


:SegmentCurveType.COST 
                       rdfs:label "COST" .


:SelfSchedReferenceType.ETC 
                            rdfs:comment "Existing transmission contract." ;
                            rdfs:label "ETC" .


:SelfSchedReferenceType.TOR 
                            rdfs:comment "Transmission ownership right." ;
                            rdfs:label "TOR" .


:SelfSchedTypeCleanBid.BAS 
                           rdfs:label "BAS" .


:SelfSchedTypeCleanBid.ETC 
                           rdfs:label "ETC" .


:SelfSchedTypeCleanBid.IFM 
                           rdfs:label "IFM" .


:SelfSchedTypeCleanBid.LOF 
                           rdfs:label "LOF" .


:SelfSchedTypeCleanBid.LPT 
                           rdfs:label "LPT" .


:SelfSchedTypeCleanBid.PT 
                          rdfs:label "PT" .


:SelfSchedTypeCleanBid.RA 
                          rdfs:comment "RA Obligations" ;
                          rdfs:label "RA" .


:SelfSchedTypeCleanBid.RMT 
                           rdfs:label "RMT" .


:SelfSchedTypeCleanBid.SP 
                          rdfs:comment "Self-Provision" ;
                          rdfs:label "SP" .


:SelfSchedTypeCleanBid.TOR 
                           rdfs:label "TOR" .


:SelfSchedTypeCleanBid.WHL 
                           rdfs:label "WHL" .


:SelfSchedTypeRawBid.BAS 
                         rdfs:label "BAS" .


:SelfSchedTypeRawBid.ETC 
                         rdfs:label "ETC" .


:SelfSchedTypeRawBid.LOF 
                         rdfs:label "LOF" .


:SelfSchedTypeRawBid.LPT 
                         rdfs:label "LPT" .


:SelfSchedTypeRawBid.PT 
                        rdfs:label "PT" .


:SelfSchedTypeRawBid.RA 
                        rdfs:comment "RA Obligations" ;
                        rdfs:label "RA" .


:SelfSchedTypeRawBid.RMT 
                         rdfs:label "RMT" .


:SelfSchedTypeRawBid.SP 
                        rdfs:comment "Self-Provision" ;
                        rdfs:label "SP" .


:SelfSchedTypeRawBid.TOR 
                         rdfs:label "TOR" .


:SelfSchedTypeRawBid.WHL 
                         rdfs:label "WHL" .


:SelfScheduleBreakdownType.ETC 
                               rdfs:comment "Existing transmission contract." ;
                               rdfs:label "ETC" .


:SelfScheduleBreakdownType.LPT 
                               rdfs:comment "Low price taker." ;
                               rdfs:label "LPT" .


:SelfScheduleBreakdownType.TOR 
                               rdfs:comment "Transmission ownership right." ;
                               rdfs:label "TOR" .


:SelfScheduleType.BAS 
                      rdfs:comment "Base Schedule" ;
                      rdfs:label "BAS" .


:SelfScheduleType.ETC 
                      rdfs:label "ETC" .


:SelfScheduleType.IFM 
                      rdfs:label "IFM" .


:SelfScheduleType.LOF 
                      rdfs:comment "Lay-off schedule" ;
                      rdfs:label "LOF" .


:SelfScheduleType.ORFC 
                       rdfs:label "ORFC" .


:SelfScheduleType.PT 
                     rdfs:label "PT" .


:SelfScheduleType.PUMP_ETC 
                           rdfs:label "PUMP_ETC" .


:SelfScheduleType.PUMP_TOR 
                           rdfs:label "PUMP_TOR" .


:SelfScheduleType.RA 
                     rdfs:comment "RA Obligations" ;
                     rdfs:label "RA" .


:SelfScheduleType.RGMR 
                       rdfs:label "RGMR" .


:SelfScheduleType.RMR 
                      rdfs:label "RMR" .


:SelfScheduleType.RMT 
                      rdfs:label "RMT" .


:SelfScheduleType.RUC 
                      rdfs:label "RUC" .


:SelfScheduleType.SP 
                     rdfs:comment "Self-Provision" ;
                     rdfs:label "SP" .


:SelfScheduleType.TOR 
                      rdfs:label "TOR" .


:SelfScheduleType.WHL 
                      rdfs:label "WHL" .


:SelfScheduleTypeMB.RMR 
                        rdfs:label "RMR" .


:ServiceKind.air 
                 rdfs:comment "Air service." ;
                 rdfs:label "air" .


:ServiceKind.electricity 
                         rdfs:comment "Electricity service." ;
                         rdfs:label "electricity" .


:ServiceKind.gas 
                 rdfs:comment "Gas service." ;
                 rdfs:label "gas" .


:ServiceKind.heat 
                  rdfs:comment "Heat service." ;
                  rdfs:label "heat" .


:ServiceKind.heatingFluid 
                          rdfs:comment "Heating fluid service." ;
                          rdfs:label "heatingFluid" .


:ServiceKind.internet 
                      rdfs:comment "Internet service." ;
                      rdfs:label "internet" .


:ServiceKind.naturalGas 
                        rdfs:comment "Natural gas service." ;
                        rdfs:label "naturalGas" .


:ServiceKind.other 
                   rdfs:comment "Other kind of service." ;
                   rdfs:label "other" .


:ServiceKind.propane 
                     rdfs:comment "Propane service." ;
                     rdfs:label "propane" .


:ServiceKind.rates 
                   rdfs:comment "Rates (e.g. tax, charge, toll, duty, tariff, etc.) service." ;
                   rdfs:label "rates" .


:ServiceKind.refuse 
                    rdfs:comment "Refuse (waster) service." ;
                    rdfs:label "refuse" .


:ServiceKind.sewerage 
                      rdfs:comment "Sewerage service." ;
                      rdfs:label "sewerage" .


:ServiceKind.steam 
                   rdfs:comment "Steam service." ;
                   rdfs:label "steam" .


:ServiceKind.time 
                  rdfs:comment "Time service." ;
                  rdfs:label "time" .


:ServiceKind.tvLicence 
                       rdfs:comment "TV license service." ;
                       rdfs:label "tvLicence" .


:ServiceKind.water 
                   rdfs:comment "Water service." ;
                   rdfs:label "water" .


:ServiceMultiplierKind.ctRatio 
                               rdfs:comment "Current transformer ratio used to convert associated quantities to real measurements." ;
                               rdfs:label "ctRatio" .


:ServiceMultiplierKind.ptRatio 
                               rdfs:comment "Voltage transformer ratio used to convert associated quantities to real measurements." ;
                               rdfs:label "ptRatio" .


:ServiceMultiplierKind.transformerRatio 
                                        rdfs:comment "Product of the CT ratio and PT ratio." ;
                                        rdfs:label "transformerRatio" .


:ServiceRequestKind.connect 
                            rdfs:comment "Physically connect the service." ;
                            rdfs:label "connect" .


:ServiceRequestKind.construction 
                                 rdfs:comment "The construction work requested." ;
                                 rdfs:label "construction" .


:ServiceRequestKind.disconnect 
                               rdfs:comment "Physically disconnect the service." ;
                               rdfs:label "disconnect" .


:ServiceRequestKind.inspection 
                               rdfs:comment "Inspection work." ;
                               rdfs:label "inspection" .


:ServiceRequestKind.newservice 
                               rdfs:comment "A new service is requested by the customer" ;
                               rdfs:label "newservice" .


:ServiceRequestKind.other 
                          rdfs:comment "Other kind of work." ;
                          rdfs:label "other" .


:ServiceRequestKind.reconnect 
                              rdfs:comment "Physically reconnect the service." ;
                              rdfs:label "reconnect" .


:ServiceRequestKind.repair 
                           rdfs:comment "Repair work." ;
                           rdfs:label "repair" .


:ServiceRequestKind.replace 
                            rdfs:comment "replace an asset" ;
                            rdfs:label "replace" .


:ServiceRequestKind.test 
                         rdfs:comment "Test work." ;
                         rdfs:label "test" .


:ServiceRequestKind.turn-off 
                             rdfs:comment "Temporarily turn off the service but leave the connection in place." ;
                             rdfs:label "turn-off" .


:ServiceRequestKind.turn-on 
                            rdfs:comment "Turn on the service." ;
                            rdfs:label "turn-on" .


:ShortCircuitRotorKind.salientPole1 
                                    rdfs:comment "Salient pole 1 in IEC 60909." ;
                                    rdfs:label "salientPole1" .


:ShortCircuitRotorKind.salientPole2 
                                    rdfs:comment "Salient pole 2 in IEC 60909." ;
                                    rdfs:label "salientPole2" .


:ShortCircuitRotorKind.turboSeries1 
                                    rdfs:comment "Turbo Series 1 in IEC 60909." ;
                                    rdfs:label "turboSeries1" .


:ShortCircuitRotorKind.turboSeries2 
                                    rdfs:comment "Turbo series 2 in IEC 60909." ;
                                    rdfs:label "turboSeries2" .


:ShuntImpedanceControlKind.fixed 
                                 rdfs:label "fixed" .


:ShuntImpedanceControlKind.localOnly 
                                     rdfs:label "localOnly" .


:ShuntImpedanceControlKind.remoteOnly 
                                      rdfs:label "remoteOnly" .


:ShuntImpedanceControlKind.remoteWithLocalOverride 
                                                   rdfs:label "remoteWithLocalOverride" .


:ShuntImpedanceLocalControlKind.current 
                                        rdfs:label "current" .


:ShuntImpedanceLocalControlKind.none 
                                     rdfs:label "none" .


:ShuntImpedanceLocalControlKind.powerFactor 
                                            rdfs:label "powerFactor" .


:ShuntImpedanceLocalControlKind.reactivePower 
                                              rdfs:label "reactivePower" .


:ShuntImpedanceLocalControlKind.temperature 
                                            rdfs:label "temperature" .


:ShuntImpedanceLocalControlKind.time 
                                     rdfs:label "time" .


:ShuntImpedanceLocalControlKind.voltage 
                                        rdfs:label "voltage" .


:SinglePhaseKind.A 
                   rdfs:comment "Phase A." ;
                   rdfs:label "A" .


:SinglePhaseKind.B 
                   rdfs:comment "Phase B." ;
                   rdfs:label "B" .


:SinglePhaseKind.C 
                   rdfs:comment "Phase C." ;
                   rdfs:label "C" .


:SinglePhaseKind.N 
                   rdfs:comment "Neutral." ;
                   rdfs:label "N" .


:SinglePhaseKind.s1 
                    rdfs:comment "Secondary phase 1." ;
                    rdfs:label "s1" .


:SinglePhaseKind.s2 
                    rdfs:comment "Secondary phase 2." ;
                    rdfs:label "s2" .


:SkillLevelKind.apprentice 
                           rdfs:label "apprentice" .


:SkillLevelKind.master 
                       rdfs:label "master" .


:SkillLevelKind.other 
                      rdfs:label "other" .


:SkillLevelKind.standard 
                         rdfs:label "standard" .


:Source.DEFAULTED 
                  rdfs:comment "The value contains a default value." ;
                  rdfs:label "DEFAULTED" .


:Source.PROCESS 
                rdfs:comment "The value is provided by input from the process I/O or being calculated from some function." ;
                rdfs:label "PROCESS" .


:Source.SUBSTITUTED 
                    rdfs:comment "The value is provided by input of an operator or by an automatic source." ;
                    rdfs:label "SUBSTITUTED" .


:SourceSinkFlag.CSNK 
                     rdfs:label "CSNK" .


:SourceSinkFlag.CSRC 
                     rdfs:label "CSRC" .


:SourceSinkType.Neither 
                        rdfs:label "Neither" .


:SourceSinkType.Sink 
                     rdfs:label "Sink" .


:SourceSinkType.Source 
                       rdfs:label "Source" .


:SpaceAnalogKind.magneticFieldDirection 
                                        rdfs:label "magneticFieldDirection" .


:SpaceAnalogKind.magneticFieldStrength 
                                       rdfs:label "magneticFieldStrength" .


:SpinningEventNameType.EASTERN 
                               rdfs:label "EASTERN" .


:SpinningEventNameType.PJM 
                           rdfs:label "PJM" .


:SpinningEventNameType.RFC-SR 
                              rdfs:label "RFC-SR" .


:SpinningEventNameType.SOUTH-S 
                               rdfs:label "SOUTH-S" .


:SpinningEventType.AA 
                      rdfs:label "AA" .


:SpinningEventType.CA 
                      rdfs:label "CA" .


:SpinningEventType.RZ 
                      rdfs:label "RZ" .


:StaticLoadModelKind.constantZ 
                               rdfs:comment "The load is represented as a constant impedance.  ConstantZ equations are used  for active and reactive power and no attributes are required." ;
                               rdfs:label "constantZ" .


:StaticLoadModelKind.exponential 
                                 rdfs:comment """This model is an exponential representation of the load. Exponential equations for active and reactive power are used and the following attributes are required:
kp1, kp2, kp3, kpf, ep1, ep2, ep3
kq1, kq2, kq3, kqf, eq1, eq2, eq3.""" ;
                                 rdfs:label "exponential" .


:StaticLoadModelKind.zIP1 
                          rdfs:comment """This model integrates the frequency-dependent load (primarily motors).  ZIP1 equations for active and reactive power are used and the following attributes are required:
kp1, kp2, kp3, kpf
kq1, kq2, kq3, kqf.""" ;
                          rdfs:label "zIP1" .


:StaticLoadModelKind.zIP2 
                          rdfs:comment """This model separates the frequency-dependent load (primarily motors) from other load.  ZIP2 equations for active and reactive power are used and the following attributes are required:
kp1, kp2, kp3, kq4, kpf
kq1, kq2, kq3, kq4, kqf.""" ;
                          rdfs:label "zIP2" .


:StreetlightLampKind.highPressureSodium 
                                        rdfs:label "highPressureSodium" .


:StreetlightLampKind.mercuryVapor 
                                  rdfs:label "mercuryVapor" .


:StreetlightLampKind.metalHalide 
                                 rdfs:label "metalHalide" .


:StreetlightLampKind.other 
                           rdfs:label "other" .


:StructureMaterialKind.concrete 
                                rdfs:label "concrete" .


:StructureMaterialKind.other 
                             rdfs:label "other" .


:StructureMaterialKind.steel 
                             rdfs:label "steel" .


:StructureMaterialKind.wood 
                            rdfs:label "wood" .


:StructureSupportKind.anchor 
                             rdfs:label "anchor" .


:StructureSupportKind.guy 
                          rdfs:label "guy" .


:SupplierKind.lse 
                  rdfs:comment "Load Serving Entity" ;
                  rdfs:label "lse" .


:SupplierKind.mdma 
                   rdfs:comment "Meter Data Management Agent (MDMA) reads meters, validates meter data, and estimates missing data to be used in various applications" ;
                   rdfs:label "mdma" .


:SupplierKind.msp 
                  rdfs:comment "Managed service provider (MSP) delivers services, such as network, application, infrastructure and security, via ongoing and regular support and active administration" ;
                  rdfs:label "msp" .


:SupplierKind.other 
                    rdfs:comment "Other kind of supplier." ;
                    rdfs:label "other" .


:SupplierKind.retailer 
                       rdfs:comment "Entity that sells the service, but does not deliver to the customer; applies to the deregulated markets." ;
                       rdfs:label "retailer" .


:SupplierKind.utility 
                      rdfs:comment "Entity that delivers the service to the customer." ;
                      rdfs:label "utility" .


:SwitchActionKind.close 
                        rdfs:comment "Close the switch." ;
                        rdfs:label "close" .


:SwitchActionKind.disableReclosing 
                                   rdfs:comment "Disable (automatic) switch reclosing." ;
                                   rdfs:label "disableReclosing" .


:SwitchActionKind.enableReclosing 
                                  rdfs:comment "Enable (automatic) switch reclosing." ;
                                  rdfs:label "enableReclosing" .


:SwitchActionKind.open 
                       rdfs:comment "Open the switch." ;
                       rdfs:label "open" .


:SwitchStatusType.Closed 
                         rdfs:comment "Closed status." ;
                         rdfs:label "Closed" .


:SwitchStatusType.Open 
                       rdfs:comment "Open status." ;
                       rdfs:label "Open" .


:SynchronousMachineKind.condenser 
                                  rdfs:comment "Indicates the synchronous machine can operate as a condenser." ;
                                  rdfs:label "condenser" .


:SynchronousMachineKind.generator 
                                  rdfs:comment "Indicates the synchronous machine can operate as a generator." ;
                                  rdfs:label "generator" .


:SynchronousMachineKind.generatorOrCondenser 
                                             rdfs:comment "Indicates the synchronous machine can operate as a generator or as a condenser." ;
                                             rdfs:label "generatorOrCondenser" .


:SynchronousMachineKind.generatorOrCondenserOrMotor 
                                                    rdfs:comment "Indicates the synchronous machine can operate as a generator or as a condenser or as a motor." ;
                                                    rdfs:label "generatorOrCondenserOrMotor" .


:SynchronousMachineKind.generatorOrMotor 
                                         rdfs:comment "Indicates the synchronous machine can operate as a generator or as a motor." ;
                                         rdfs:label "generatorOrMotor" .


:SynchronousMachineKind.motor 
                              rdfs:comment "Indicates the synchronous machine can operate as a motor." ;
                              rdfs:label "motor" .


:SynchronousMachineKind.motorOrCondenser 
                                         rdfs:comment "Indicates the synchronous machine can operate as a motor or as a condenser." ;
                                         rdfs:label "motorOrCondenser" .


:SynchronousMachineModelKind.subtransient 
                                          rdfs:comment "Subtransient synchronous machine model." ;
                                          rdfs:label "subtransient" .


:SynchronousMachineModelKind.subtransientSimplified 
                                                    rdfs:comment "Simplified version of subtransient synchronous machine model where magnetic coupling between the direct- and quadrature- axes is ignored." ;
                                                    rdfs:label "subtransientSimplified" .


:SynchronousMachineModelKind.subtransientSimplifiedDirectAxis 
                                                              rdfs:comment "Simplified version of a subtransient synchronous machine model with no damper circuit on the direct-axis." ;
                                                              rdfs:label "subtransientSimplifiedDirectAxis" .


:SynchronousMachineModelKind.subtransientTypeF 
                                               rdfs:comment "WECC type F variant of subtransient synchronous machine model." ;
                                               rdfs:label "subtransientTypeF" .


:SynchronousMachineModelKind.subtransientTypeJ 
                                               rdfs:comment "WECC type J variant of subtransient synchronous machine model." ;
                                               rdfs:label "subtransientTypeJ" .


:SynchronousMachineOperatingMode.condenser 
                                           rdfs:comment "Operating as condenser." ;
                                           rdfs:label "condenser" .


:SynchronousMachineOperatingMode.generator 
                                           rdfs:comment "Operating as generator." ;
                                           rdfs:label "generator" .


:SynchronousMachineOperatingMode.motor 
                                       rdfs:comment "Operating as motor." ;
                                       rdfs:label "motor" .


:SystemType.OASIS 
                  rdfs:label "OASIS" .


:TAPPIStandardEditionKind._2009 
                                rdfs:comment "2009 standard edition." ;
                                rdfs:label "2009" .


:TAPPIStandardEditionKind.none 
                               rdfs:comment "No standard edition." ;
                               rdfs:label "none" .


:TAPPIStandardEditionKind.unknown 
                                  rdfs:comment "Unknown standard edition." ;
                                  rdfs:label "unknown" .


:TAPPIStandardKind.T494 
                        rdfs:comment "Tensile properties of paper and paperboard(using constant rate of elongation apparatus), Test Method TAPPI/ANSI T 494 om-13." ;
                        rdfs:label "T494" .


:TRType.CHAIN 
              rdfs:comment "TR chain" ;
              rdfs:label "CHAIN" .


:TRType.INDIVIDUAL 
                   rdfs:comment "Individual TR" ;
                   rdfs:label "INDIVIDUAL" .


:TagActionKind.place 
                     rdfs:comment "Place the tag." ;
                     rdfs:label "place" .


:TagActionKind.remove 
                      rdfs:comment "Remove the tag." ;
                      rdfs:label "remove" .


:TagActionKind.verify 
                      rdfs:comment "Verify the tag." ;
                      rdfs:label "verify" .


:TempEquipActionKind.connect 
                             rdfs:comment "Connect the temp equipment to its terminal" ;
                             rdfs:label "connect" .


:TempEquipActionKind.disconnect 
                                rdfs:comment "Disconnect the temp equipment from its terminal" ;
                                rdfs:label "disconnect" .


:TempEquipActionKind.place 
                           rdfs:comment "Place the jumper (close) or the cut (open)." ;
                           rdfs:label "place" .


:TempEquipActionKind.remove 
                            rdfs:comment "Remove the jumper (open) or the cut (close)." ;
                            rdfs:label "remove" .


:TenderKind.card 
                 rdfs:comment "Payment method by means of a credit or debit card." ;
                 rdfs:label "card" .


:TenderKind.cash 
                 rdfs:comment "Payment method by means of cash." ;
                 rdfs:label "cash" .


:TenderKind.cheque 
                   rdfs:comment "Payment method by means of a cheque." ;
                   rdfs:label "cheque" .


:TenderKind.other 
                  rdfs:comment "Other payment method such as electronic finds transfer." ;
                  rdfs:label "other" .


:TenderKind.unspecified 
                        rdfs:comment "Payment method is not known." ;
                        rdfs:label "unspecified" .


:TestKind.equalTo 
                  rdfs:label "equalTo" .


:TestKind.greaterThan 
                      rdfs:label "greaterThan" .


:TestKind.greaterThanOrEqualTo 
                               rdfs:label "greaterThanOrEqualTo" .


:TestKind.lessThan 
                   rdfs:label "lessThan" .


:TestKind.lessThanOrEqualTo 
                            rdfs:label "lessThanOrEqualTo" .


:TestMethod.D1275A 
                   rdfs:comment "D1275A method." ;
                   rdfs:label "D1275A" .


:TestMethod.D1275B 
                   rdfs:comment "D1275B method." ;
                   rdfs:label "D1275B" .


:TestMethod.D3612A 
                   rdfs:comment "D3612A method." ;
                   rdfs:label "D3612A" .


:TestMethod.D3612B 
                   rdfs:comment "D3612B method." ;
                   rdfs:label "D3612B" .


:TestMethod.D3612C 
                   rdfs:comment "D3612C method." ;
                   rdfs:label "D3612C" .


:TestMethod._60567ByDisplacement 
                                 rdfs:comment "60567 by displacement method." ;
                                 rdfs:label "60567ByDisplacement" .


:TestMethod._60567ByPartition 
                              rdfs:comment "60567 by partition method." ;
                              rdfs:label "60567ByPartition" .


:TestMethod._60567ByVacuum 
                           rdfs:comment "60567 by vacuum method." ;
                           rdfs:label "60567ByVacuum" .


:TestMethod._60970Automatic 
                            rdfs:comment "Automatic method." ;
                            rdfs:label "60970Automatic" .


:TestMethod._60970Manual1 
                          rdfs:comment "Manual method 1." ;
                          rdfs:label "60970Manual1" .


:TestMethod._60970Manual2 
                          rdfs:comment "Manual method 2." ;
                          rdfs:label "60970Manual2" .


:TestMethod._61125A 
                    rdfs:comment "61125A method." ;
                    rdfs:label "61125A" .


:TestMethod._61125B 
                    rdfs:comment "61125B method." ;
                    rdfs:label "61125B" .


:TestMethod._61125C 
                    rdfs:comment "61125C method." ;
                    rdfs:label "61125C" .


:TestMethod._62270AnnexA 
                         rdfs:comment "62270 Annex A method." ;
                         rdfs:label "62270AnnexA" .


:TestMethod._62535AnnexA 
                         rdfs:comment "62535 Annex A method." ;
                         rdfs:label "62535AnnexA" .


:TestMethod._62535Main 
                       rdfs:comment "62535 main method." ;
                       rdfs:label "62535Main" .


:TestReason.postOilTreatment 
                             rdfs:comment "Test after oil treatment." ;
                             rdfs:label "postOilTreatment" .


:TestReason.postOperationFault 
                               rdfs:comment "Test after operation fault." ;
                               rdfs:label "postOperationFault" .


:TestReason.postRepair 
                       rdfs:comment "Test after repair." ;
                       rdfs:label "postRepair" .


:TestReason.routine 
                    rdfs:comment "Routine test." ;
                    rdfs:label "routine" .


:TestVariantKind._0C 
                     rdfs:comment "Testing done at temperature of 0°C." ;
                     rdfs:label "0C" .


:TestVariantKind._100C 
                       rdfs:comment "Testing done at temperature of  100°C." ;
                       rdfs:label "100C" .


:TestVariantKind._164hours 
                           rdfs:comment "Measurements taken at 164 hours." ;
                           rdfs:label "164hours" .


:TestVariantKind._1mm 
                      rdfs:comment "Specimen of 1 mm thickness used in testing." ;
                      rdfs:label "1mm" .


:TestVariantKind._25C 
                      rdfs:comment "Testing done at temperature of  25°C." ;
                      rdfs:label "25C" .


:TestVariantKind._2mm 
                      rdfs:comment "Specimen of 2 mm thickness used in testing." ;
                      rdfs:label "2mm" .


:TestVariantKind._30C 
                      rdfs:comment "Testing done at temperature of 30°C." ;
                      rdfs:label "30C" .


:TestVariantKind._40C 
                      rdfs:comment "Testing done at temperature of 40°C." ;
                      rdfs:label "40C" .


:TestVariantKind._72hours 
                          rdfs:comment "Measurements taken at 72 hours." ;
                          rdfs:label "72hours" .


:TestVariantKind.minus30C 
                          rdfs:comment "Testing done at temperature of -30°C." ;
                          rdfs:label "minus30C" .


:TestVariantKind.minus40C 
                          rdfs:comment "Testing done at temperature of -40°C." ;
                          rdfs:label "minus40C" .


:TimeIntervalKind.D uml:hasInitialValue "3" ;
                    
                    rdfs:comment "Day" ;
                    rdfs:label "D" .


:TimeIntervalKind.M uml:hasInitialValue "2" ;
                    
                    rdfs:comment "Month" ;
                    rdfs:label "M" .


:TimeIntervalKind.Y uml:hasInitialValue "1" ;
                    
                    rdfs:comment "Year" ;
                    rdfs:label "Y" .


:TimeIntervalKind.h uml:hasInitialValue "4" ;
                    
                    rdfs:comment "Hour" ;
                    rdfs:label "h" .


:TimeIntervalKind.m uml:hasInitialValue "5" ;
                    
                    rdfs:comment "Minute" ;
                    rdfs:label "m" .


:TimeIntervalKind.s uml:hasInitialValue "6" ;
                    
                    rdfs:comment "Second" ;
                    rdfs:label "s" .


:TimeOfUse.OFF 
               rdfs:comment "Time of use spans only the off peak hours of the day." ;
               rdfs:label "OFF" .


:TimeOfUse.ON 
              rdfs:comment "Time of use spans only the on peak hours of the day." ;
              rdfs:label "ON" .


:TimeOfUse._24HR 
                 rdfs:comment "Time of use spans the entire day, 24 hours." ;
                 rdfs:label "24HR" .


:TimePeriodUnit.days 
                     rdfs:label "days" .


:TimePeriodUnit.hours 
                      rdfs:label "hours" .


:TimePeriodUnit.minutes 
                        rdfs:label "minutes" .


:TimePeriodUnit.months 
                       rdfs:label "months" .


:TimePeriodUnit.seconds 
                        rdfs:label "seconds" .


:TimePeriodUnit.weeks 
                      rdfs:label "weeks" .


:TimeZoneType.PPT 
                  rdfs:label "PPT" .


:TowerConstructionKind.suspension 
                                  rdfs:label "suspension" .


:TowerConstructionKind.tension 
                               rdfs:label "tension" .


:TradeProductType.APN 
                      rdfs:comment "Energy Trades at Aggregated Pricing Nodes" ;
                      rdfs:label "APN" .


:TradeProductType.CAP 
                      rdfs:comment "Capacity type trade" ;
                      rdfs:label "CAP" .


:TradeProductType.NRT 
                      rdfs:comment "Non-Spinning Reserve Trade" ;
                      rdfs:label "NRT" .


:TradeProductType.PHY 
                      rdfs:comment "Physical Energy Tra" ;
                      rdfs:label "PHY" .


:TradeProductType.RDT 
                      rdfs:comment "Regulation Down Trade" ;
                      rdfs:label "RDT" .


:TradeProductType.RUT 
                      rdfs:comment "Regulation Up Trade" ;
                      rdfs:label "RUT" .


:TradeProductType.SRT 
                      rdfs:comment "Spinning Reserve Trade" ;
                      rdfs:label "SRT" .


:TradeStatusType.CI 
                    rdfs:label "CI" .


:TradeStatusType.CM 
                    rdfs:label "CM" .


:TradeStatusType.CV 
                    rdfs:label "CV" .


:TradeStatusType.CX 
                    rdfs:label "CX" .


:TradeStatusType.I 
                   rdfs:label "I" .


:TradeStatusType.M 
                   rdfs:label "M" .


:TradeStatusType.MT 
                    rdfs:label "MT" .


:TradeStatusType.O 
                   rdfs:label "O" .


:TradeStatusType.RJ 
                    rdfs:label "RJ" .


:TradeStatusType.U 
                   rdfs:label "U" .


:TradeStatusType.V 
                   rdfs:label "V" .


:TradeType.AST 
               rdfs:comment "Ancillary Services Trade." ;
               rdfs:label "AST" .


:TradeType.IST 
               rdfs:comment "InterSC Trade." ;
               rdfs:label "IST" .


:TradeType.UCT 
               rdfs:comment "Unit Commitment Trade." ;
               rdfs:label "UCT" .


:TransactionKind.accountPayment 
                                rdfs:comment "Payment against a specified account." ;
                                rdfs:label "accountPayment" .


:TransactionKind.auxiliaryChargePayment 
                                        rdfs:comment "Payment against a specified auxiliary account." ;
                                        rdfs:label "auxiliaryChargePayment" .


:TransactionKind.diversePayment 
                                rdfs:comment "Payment against an item other than an account." ;
                                rdfs:label "diversePayment" .


:TransactionKind.meterConfigurationToken 
                                         rdfs:comment "Issue of token that will alter the meter configuration." ;
                                         rdfs:label "meterConfigurationToken" .


:TransactionKind.other 
                       rdfs:comment "Other kind of transaction." ;
                       rdfs:label "other" .


:TransactionKind.serviceChargePayment 
                                      rdfs:comment "Payment for a service." ;
                                      rdfs:label "serviceChargePayment" .


:TransactionKind.taxChargePayment 
                                  rdfs:comment "Payment for a tax." ;
                                  rdfs:label "taxChargePayment" .


:TransactionKind.tokenCancellation 
                                   rdfs:comment "Cancellation of a previously issued token." ;
                                   rdfs:label "tokenCancellation" .


:TransactionKind.tokenExchange 
                               rdfs:comment "Exchange of a previously issued token for a new token." ;
                               rdfs:label "tokenExchange" .


:TransactionKind.tokenFreeIssue 
                                rdfs:comment "Issue of a free credit token where the donor is the supplier." ;
                                rdfs:label "tokenFreeIssue" .


:TransactionKind.tokenGrant 
                            rdfs:comment "Issue of a free credit token where the donor is a 3rd party." ;
                            rdfs:label "tokenGrant" .


:TransactionKind.tokenSalePayment 
                                  rdfs:comment "Payment for a credit token sale to a customer." ;
                                  rdfs:label "tokenSalePayment" .


:TransactionKind.transactionReversal 
                                     rdfs:comment "Reversal of a previous transaction." ;
                                     rdfs:label "transactionReversal" .


:TransformerApplicationKind.distribution 
                                         rdfs:comment "Transformer between one distribution voltage level and another distribution voltage level." ;
                                         rdfs:label "distribution" .


:TransformerApplicationKind.generatorStepUp 
                                            rdfs:comment "Transformer is generator step-up transformer." ;
                                            rdfs:label "generatorStepUp" .


:TransformerApplicationKind.transmissionBusToBus 
                                                 rdfs:comment "Transformer between bus at one transmission voltage level and a bus at another transmission voltage level." ;
                                                 rdfs:label "transmissionBusToBus" .


:TransformerApplicationKind.transmissionBusToDistribution 
                                                          rdfs:comment "Transformer between bus at transmission voltage level and bus at distribution voltage level." ;
                                                          rdfs:label "transmissionBusToDistribution" .


:TransformerConstructionKind.aerial 
                                    rdfs:label "aerial" .


:TransformerConstructionKind.dryType 
                                     rdfs:label "dryType" .


:TransformerConstructionKind.network 
                                     rdfs:label "network" .


:TransformerConstructionKind.onePhase 
                                      rdfs:label "onePhase" .


:TransformerConstructionKind.overhead 
                                      rdfs:label "overhead" .


:TransformerConstructionKind.padmountDeadFront 
                                               rdfs:label "padmountDeadFront" .


:TransformerConstructionKind.padmountFeedThrough 
                                                 rdfs:label "padmountFeedThrough" .


:TransformerConstructionKind.padmountLiveFront 
                                               rdfs:label "padmountLiveFront" .


:TransformerConstructionKind.padmountLoopThrough 
                                                 rdfs:label "padmountLoopThrough" .


:TransformerConstructionKind.padmounted 
                                        rdfs:label "padmounted" .


:TransformerConstructionKind.subway 
                                    rdfs:label "subway" .


:TransformerConstructionKind.threePhase 
                                        rdfs:label "threePhase" .


:TransformerConstructionKind.underground 
                                         rdfs:label "underground" .


:TransformerConstructionKind.unknown 
                                     rdfs:label "unknown" .


:TransformerConstructionKind.vault 
                                   rdfs:label "vault" .


:TransformerConstructionKind.vaultThreePhase 
                                             rdfs:label "vaultThreePhase" .


:TransformerControlMode.reactive 
                                 rdfs:comment "Reactive power flow control." ;
                                 rdfs:label "reactive" .


:TransformerControlMode.volt 
                             rdfs:comment "Voltage control." ;
                             rdfs:label "volt" .


:TransformerCoreKind.core 
                          rdfs:label "core" .


:TransformerCoreKind.shell 
                           rdfs:label "shell" .


:TransformerFailureReasonKind.bushingFailure 
                                             rdfs:comment "Bushing-caused failure." ;
                                             rdfs:label "bushingFailure" .


:TransformerFailureReasonKind.lossOfOil 
                                        rdfs:comment "Loss-of-oil-caused faliure." ;
                                        rdfs:label "lossOfOil" .


:TransformerFailureReasonKind.oilRelatedFailure 
                                                rdfs:comment "Oil-related failure." ;
                                                rdfs:label "oilRelatedFailure" .


:TransformerFailureReasonKind.poorOilQuality 
                                             rdfs:comment "Oil quality-related failure." ;
                                             rdfs:label "poorOilQuality" .


:TransformerFunctionKind.autotransformer 
                                         rdfs:label "autotransformer" .


:TransformerFunctionKind.other 
                               rdfs:label "other" .


:TransformerFunctionKind.powerTransformer 
                                          rdfs:label "powerTransformer" .


:TransformerFunctionKind.secondaryTransformer 
                                              rdfs:label "secondaryTransformer" .


:TransformerFunctionKind.voltageRegulator 
                                          rdfs:label "voltageRegulator" .


:TransmissionModeKind.anonymous 
                                rdfs:comment "Message transmission mode whereby messages or commands are broadcast to unspecified devices listening for such communications." ;
                                rdfs:label "anonymous" .


:TransmissionModeKind.both 
                           rdfs:comment "Message transmission mode whereby messages or commands are sent by both 'normal' and 'anonymous' methods." ;
                           rdfs:label "both" .


:TransmissionModeKind.normal 
                             rdfs:comment "Message transmission mode whereby messages or commands are sent to specific devices." ;
                             rdfs:label "normal" .


:TroubleCallKind.lineDown 
                          rdfs:comment "The customer is reporting a line down" ;
                          rdfs:label "lineDown" .


:TroubleCallKind.powerOut 
                          rdfs:comment "The customer is reporting an outage." ;
                          rdfs:label "powerOut" .


:TroubleReportingKind.app 
                          rdfs:label "app" .


:TroubleReportingKind.call uml:id "_082F4DA0-389D-4879-8BE5-F7103D5DB45A" ,
                                  "_E3DBCDD0-C040-4bb7-983D-CF2171EE375B" ;
                           rdfs:comment "Trouble call received by customer service representative." ;
                           rdfs:label "call" .


:TroubleReportingKind.email uml:id "_6A4F782D-C145-4228-AD70-333E39C40D08" ,
                                   "_C447B6E0-5BA5-49ca-A32B-A836324D5D47" ;
                            rdfs:comment "Trouble reported by email." ;
                            rdfs:label "email" .


:TroubleReportingKind.ivr uml:id "_37E8A66F-9052-4249-AE73-F0EDBD9C666B" ,
                                 "_F6A3821F-1FCE-498b-87B0-E3AF4A38ADDC" ;
                          rdfs:comment "Trouble reported through interactive voice response system." ;
                          rdfs:label "ivr" .


:TroubleReportingKind.letter uml:id "_5A807F00-9C57-4678-A748-FEE2CF766BF5" ,
                                    "_9B7EFA04-525A-4c2b-BBC8-807696DD7EE8" ;
                             rdfs:comment "Trouble reported by letter." ;
                             rdfs:label "letter" .


:TroubleReportingKind.other uml:id "_0FF97738-C280-4c67-B858-256038633AFE" ,
                                   "_53E43CD9-13AE-455f-A787-ED4B7B81A9E0" ;
                            rdfs:comment "Trouble reported by other means." ;
                            rdfs:label "other" .


:TroubleReportingKind.sms 
                          rdfs:label "sms" .


:TroubleReportingKind.web 
                          rdfs:label "web" .


:TroubleSymptomsExtentKind.entireNeighbourhood 
                                               rdfs:label "entireNeighbourhood" .


:TroubleSymptomsExtentKind.neighbour 
                                     rdfs:label "neighbour" .


:TroubleSymptomsExtentKind.ok 
                              rdfs:label "ok" .


:TroubleSymptomsExtentKind.other 
                                 rdfs:label "other" .


:TroubleSymptomsExtentKind.singleCustomer 
                                          rdfs:label "singleCustomer" .


:TroubleSymptomsLightKind.allOut 
                                 rdfs:label "allOut" .


:TroubleSymptomsLightKind.dim 
                              rdfs:label "dim" .


:TroubleSymptomsLightKind.flickering 
                                     rdfs:label "flickering" .


:TroubleSymptomsLightKind.ok 
                             rdfs:label "ok" .


:TroubleSymptomsLightKind.other 
                                rdfs:label "other" .


:TroubleSymptomsLightKind.partOut 
                                  rdfs:label "partOut" .


:TroubleSymptomsPoleKind.down 
                              rdfs:label "down" .


:TroubleSymptomsPoleKind.hit 
                             rdfs:label "hit" .


:TroubleSymptomsPoleKind.leaning 
                                 rdfs:label "leaning" .


:TroubleSymptomsPoleKind.ok 
                            rdfs:label "ok" .


:TroubleSymptomsPoleKind.other 
                               rdfs:label "other" .


:TroubleSymptomsTransformerKind.burning 
                                        rdfs:label "burning" .


:TroubleSymptomsTransformerKind.ok 
                                   rdfs:label "ok" .


:TroubleSymptomsTransformerKind.other 
                                      rdfs:label "other" .


:TroubleSymptomsTree_Kind.limbOnService 
                                        rdfs:label "limbOnService" .


:TroubleSymptomsTree_Kind.limbOnWire 
                                     rdfs:label "limbOnWire" .


:TroubleSymptomsTree_Kind.ok 
                             rdfs:label "ok" .


:TroubleSymptomsTree_Kind.other 
                                rdfs:label "other" .


:TroubleSymptomsWireKind.digIn 
                               rdfs:label "digIn" .


:TroubleSymptomsWireKind.ok 
                            rdfs:label "ok" .


:TroubleSymptomsWireKind.other 
                               rdfs:label "other" .


:TroubleSymptomsWireKind.serviceDown 
                                     rdfs:label "serviceDown" .


:TroubleSymptomsWireKind.wireDown 
                                  rdfs:label "wireDown" .


:TroubleSymptomsWireKind.wireburning 
                                     rdfs:label "wireburning" .


:UKMinistryOfDefenceStandardEditionKind.Issue_1 
                                                rdfs:comment "Issue 1 standard edition." ;
                                                rdfs:label "Issue 1" .


:UKMinistryOfDefenceStandardEditionKind.none 
                                             rdfs:comment "No standard edition." ;
                                             rdfs:label "none" .


:UKMinistryOfDefenceStandardEditionKind.unknown 
                                                rdfs:comment "Unknown standard edition." ;
                                                rdfs:label "unknown" .


:UKMinistryofDefenceStandardKind._05-50__Part_65_ 
                                                  rdfs:comment "Ministry of Defence, Defence Standard 05-50 (Part 65)/Issue 1 METHODS FOR TESTING FUELS, LUBRICANTS AND ASSOCIATED PRODUCTS." ;
                                                  rdfs:label "05-50 (Part 65)" .


:UOMType.FACTOR 
                rdfs:label "FACTOR" .


:UOMType.FLAG 
              rdfs:label "FLAG" .


:UOMType.INTEGER 
                 rdfs:label "INTEGER" .


:UOMType.MW 
            rdfs:label "MW" .


:UOMType.MWh 
             rdfs:label "MWh" .


:UOMType.US_ 
             rdfs:label "US$" .


:UOMType.US__MW 
                rdfs:label "US$/MW" .


:UOMType.US__MWh 
                 rdfs:label "US$/MWh" .


:UOMType._ 
           rdfs:label "%" .


:UOMType.__lb 
              rdfs:label "$/lb" .


:UOMType.__mmBTU 
                 rdfs:label "$/mmBTU" .


:UncertaintyKind.estimated 
                           rdfs:comment "The value is estimated." ;
                           rdfs:label "estimated" .


:UncertaintyKind.interpolated 
                              rdfs:comment "The value is interpolated." ;
                              rdfs:label "interpolated" .


:UncertaintyKind.standard 
                          rdfs:comment "The value has standard uncertainty consistent with National Weather Service practises given the instrument and manner of observation." ;
                          rdfs:label "standard" .


:UncertaintyKind.unknown 
                         rdfs:comment "The process of value calculation or measurement is unknown." ;
                         rdfs:label "unknown" .


:UndergroundStructureKind.burd 
                               rdfs:label "burd" .


:UndergroundStructureKind.enclosure 
                                    rdfs:label "enclosure" .


:UndergroundStructureKind.handhole 
                                   rdfs:label "handhole" .


:UndergroundStructureKind.manhole 
                                  rdfs:label "manhole" .


:UndergroundStructureKind.pad 
                              rdfs:label "pad" .


:UndergroundStructureKind.pullbox 
                                  rdfs:label "pullbox" .


:UndergroundStructureKind.subsurfaceEnclosure 
                                              rdfs:label "subsurfaceEnclosure" .


:UndergroundStructureKind.trench 
                                 rdfs:label "trench" .


:UndergroundStructureKind.tunnel 
                                 rdfs:label "tunnel" .


:UndergroundStructureKind.vault 
                                rdfs:label "vault" .


:UnitMultiplier.E uml:hasInitialValue "18" ;
                  
                  rdfs:comment "Exa 10**18." ;
                  rdfs:label "E" .


:UnitMultiplier.G uml:hasInitialValue "9" ;
                  
                  rdfs:comment "Giga 10**9." ;
                  rdfs:label "G" .


:UnitMultiplier.M uml:hasInitialValue "6" ;
                  
                  rdfs:comment "Mega 10**6." ;
                  rdfs:label "M" .


:UnitMultiplier.P uml:hasInitialValue "15" ;
                  
                  rdfs:comment "Peta 10**15." ;
                  rdfs:label "P" .


:UnitMultiplier.T uml:hasInitialValue "12" ;
                  
                  rdfs:comment "Tera 10**12." ;
                  rdfs:label "T" .


:UnitMultiplier.Y uml:hasInitialValue "24" ;
                  
                  rdfs:comment "Yotta 10**24." ;
                  rdfs:label "Y" .


:UnitMultiplier.Z uml:hasInitialValue "21" ;
                  
                  rdfs:comment "Zetta 10**21." ;
                  rdfs:label "Z" .


:UnitMultiplier.a uml:hasInitialValue "-18" ;
                  
                  rdfs:comment "Atto 10**-18." ;
                  rdfs:label "a" .


:UnitMultiplier.c uml:hasInitialValue "-2" ;
                  
                  rdfs:comment "Centi 10**-2." ;
                  rdfs:label "c" .


:UnitMultiplier.d uml:hasInitialValue "-1" ;
                  
                  rdfs:comment "Deci 10**-1." ;
                  rdfs:label "d" .


:UnitMultiplier.da uml:hasInitialValue "1" ;
                   
                   rdfs:comment "Deca 10**1." ;
                   rdfs:label "da" .


:UnitMultiplier.f uml:hasInitialValue "-15" ;
                  
                  rdfs:comment "Femto 10**-15." ;
                  rdfs:label "f" .


:UnitMultiplier.h uml:hasInitialValue "2" ;
                  
                  rdfs:comment "Hecto 10**2." ;
                  rdfs:label "h" .


:UnitMultiplier.k uml:hasInitialValue "3" ;
                  
                  rdfs:comment "Kilo 10**3." ;
                  rdfs:label "k" .


:UnitMultiplier.m uml:hasInitialValue "-3" ;
                  
                  rdfs:comment "Milli 10**-3." ;
                  rdfs:label "m" .


:UnitMultiplier.micro uml:hasInitialValue "-6" ;
                      
                      rdfs:comment "Micro 10**-6." ;
                      rdfs:label "micro" .


:UnitMultiplier.n uml:hasInitialValue "-9" ;
                  
                  rdfs:comment "Nano 10**-9." ;
                  rdfs:label "n" .


:UnitMultiplier.none uml:hasInitialValue "0" ;
                     
                     rdfs:comment "No multiplier or equivalently multiply by 1." ;
                     rdfs:label "none" .


:UnitMultiplier.p uml:hasInitialValue "-12" ;
                  
                  rdfs:comment "Pico 10**-12." ;
                  rdfs:label "p" .


:UnitMultiplier.y uml:hasInitialValue "-24" ;
                  
                  rdfs:comment "Yocto 10**-24." ;
                  rdfs:label "y" .


:UnitMultiplier.z uml:hasInitialValue "-21" ;
                  
                  rdfs:comment "Zepto 10**-21." ;
                  rdfs:label "z" .


:UnitRegulationKind._0 
                       rdfs:comment "Unit is not on regulation." ;
                       rdfs:label "0" .


:UnitRegulationKind._1 
                       rdfs:comment "Unit is on AGC and regulating." ;
                       rdfs:label "1" .


:UnitRegulationKind._2 
                       rdfs:comment "Unit is suppose to be on regulation but it is not under regulation now." ;
                       rdfs:label "2" .


:UnitSymbol.A uml:hasInitialValue "5" ;
              
              rdfs:comment "Current in amperes." ;
              rdfs:label "A" .


:UnitSymbol.A2 uml:hasInitialValue "69" ;
               
               rdfs:comment "Amperes squared (A²)." ;
               rdfs:label "A2" .


:UnitSymbol.A2h uml:hasInitialValue "105" ;
                
                rdfs:comment "Ampere-squared hour, ampere-squared hour." ;
                rdfs:label "A2h" .


:UnitSymbol.A2s uml:hasInitialValue "70" ;
                
                rdfs:comment "Ampere squared time in square amperes (A²s)." ;
                rdfs:label "A2s" .


:UnitSymbol.APerA uml:hasInitialValue "152" ;
                  
                  rdfs:comment "Current, ratio of amperages.   Note: Users may need to supply a prefix such as ‘m’ to show rates such as ‘mA/A’." ;
                  rdfs:label "APerA" .


:UnitSymbol.APerm uml:hasInitialValue "103" ;
                  
                  rdfs:comment "A/m, magnetic field strength, amperes per metre." ;
                  rdfs:label "APerm" .


:UnitSymbol.Ah uml:hasInitialValue "106" ;
               
               rdfs:comment "Ampere-hours, ampere-hours." ;
               rdfs:label "Ah" .


:UnitSymbol.As uml:hasInitialValue "68" ;
               
               rdfs:comment "Ampere seconds (A·s)." ;
               rdfs:label "As" .


:UnitSymbol.Bq uml:hasInitialValue "22" ;
               
               rdfs:comment "Radioactivity in becquerels (1/s)." ;
               rdfs:label "Bq" .


:UnitSymbol.Btu uml:hasInitialValue "132" ;
                
                rdfs:comment "Energy, British Thermal Units." ;
                rdfs:label "Btu" .


:UnitSymbol.C uml:hasInitialValue "26" ;
              
              rdfs:comment "Electric charge in coulombs (A·s)." ;
              rdfs:label "C" .


:UnitSymbol.CPerkg uml:hasInitialValue "189" ;
                   
                   rdfs:comment "Exposure (x rays), coulombs per kilogram." ;
                   rdfs:label "CPerkg" .


:UnitSymbol.CPerm2 uml:hasInitialValue "184" ;
                   
                   rdfs:comment "Surface charge density, coulombs per square metre." ;
                   rdfs:label "CPerm2" .


:UnitSymbol.CPerm3 uml:hasInitialValue "183" ;
                   
                   rdfs:comment "Electric charge density, coulombs per cubic metre." ;
                   rdfs:label "CPerm3" .


:UnitSymbol.F uml:hasInitialValue "25" ;
              
              rdfs:comment "Electric capacitance in farads (C/V)." ;
              rdfs:label "F" .


:UnitSymbol.FPerm uml:hasInitialValue "185" ;
                  
                  rdfs:comment "Permittivity, farads per metre." ;
                  rdfs:label "FPerm" .


:UnitSymbol.G uml:hasInitialValue "277" ;
              
              rdfs:comment "Magnetic flux density, gausses (1 G = 10-4 T)." ;
              rdfs:label "G" .


:UnitSymbol.Gy uml:hasInitialValue "21" ;
               
               rdfs:comment "Absorbed dose in grays (J/kg)." ;
               rdfs:label "Gy" .


:UnitSymbol.GyPers uml:hasInitialValue "190" ;
                   
                   rdfs:comment "Absorbed dose rate, grays per second." ;
                   rdfs:label "GyPers" .


:UnitSymbol.H uml:hasInitialValue "28" ;
              
              rdfs:comment "Electric inductance in henrys (Wb/A)." ;
              rdfs:label "H" .


:UnitSymbol.HPerm uml:hasInitialValue "186" ;
                  
                  rdfs:comment "Permeability, henrys per metre." ;
                  rdfs:label "HPerm" .


:UnitSymbol.Hz uml:hasInitialValue "33" ;
               
               rdfs:comment "Frequency in hertz (1/s)." ;
               rdfs:label "Hz" .


:UnitSymbol.HzPerHz uml:hasInitialValue "150" ;
                    
                    rdfs:comment "Frequency, rate of frequency change.   Note: Users may need to supply a prefix such as ‘m’ to show rates such as ‘mHz/Hz’." ;
                    rdfs:label "HzPerHz" .


:UnitSymbol.HzPers uml:hasInitialValue "75" ;
                   
                   rdfs:comment "Rate of change of frequency in hertz per second." ;
                   rdfs:label "HzPers" .


:UnitSymbol.J uml:hasInitialValue "31" ;
              
              rdfs:comment "Energy in joules (N·m = C·V = W·s)." ;
              rdfs:label "J" .


:UnitSymbol.JPerK uml:hasInitialValue "51" ;
                  
                  rdfs:comment "Heat capacity in joules/kelvin." ;
                  rdfs:label "JPerK" .


:UnitSymbol.JPerkg uml:hasInitialValue "165" ;
                   
                   rdfs:comment "Specific energy, Joules / kg." ;
                   rdfs:label "JPerkg" .


:UnitSymbol.JPerkgK uml:hasInitialValue "60" ;
                    
                    rdfs:comment "Specific heat capacity, specific entropy, joules per kilogram Kelvin." ;
                    rdfs:label "JPerkgK" .


:UnitSymbol.JPerm2 uml:hasInitialValue "56" ;
                   
                   rdfs:comment "Insulation energy density, joules per square metre or watt second per square metre." ;
                   rdfs:label "JPerm2" .


:UnitSymbol.JPerm3 uml:hasInitialValue "181" ;
                   
                   rdfs:comment "Energy density, joules per cubic metre." ;
                   rdfs:label "JPerm3" .


:UnitSymbol.JPermol uml:hasInitialValue "187" ;
                    
                    rdfs:comment "Molar energy, joules per mole." ;
                    rdfs:label "JPermol" .


:UnitSymbol.JPermolK uml:hasInitialValue "188" ;
                     
                     rdfs:comment "Molar entropy, molar heat capacity, joules per mole kelvin." ;
                     rdfs:label "JPermolK" .


:UnitSymbol.JPers 
                  rdfs:comment "Energy rate in joules per second (J/s)." ;
                  rdfs:label "JPers" .


:UnitSymbol.K uml:hasInitialValue "6" ;
              
              rdfs:comment "Temperature in kelvins." ;
              rdfs:label "K" .


:UnitSymbol.KPers uml:hasInitialValue "58" ;
                  
                  rdfs:comment "Temperature change rate in kelvins per second." ;
                  rdfs:label "KPers" .


:UnitSymbol.M uml:hasInitialValue "217" ;
              
              rdfs:comment "Length, nautical miles (1 M = 1852 m)." ;
              rdfs:label "M" .


:UnitSymbol.Mx uml:hasInitialValue "276" ;
               
               rdfs:comment "Magnetic flux, maxwells (1 Mx = 10-8 Wb)." ;
               rdfs:label "Mx" .


:UnitSymbol.N uml:hasInitialValue "32" ;
              
              rdfs:comment "Force in newtons (kg·m/s²)." ;
              rdfs:label "N" .


:UnitSymbol.NPerm uml:hasInitialValue "177" ;
                  
                  rdfs:comment "Surface tension, newton per metre." ;
                  rdfs:label "NPerm" .


:UnitSymbol.Nm uml:hasInitialValue "176" ;
               
               rdfs:comment "Moment of force, newton metres." ;
               rdfs:label "Nm" .


:UnitSymbol.Oe uml:hasInitialValue "278" ;
               
               rdfs:comment "Magnetic field in oersteds, (1 Oe = (103/4p) A/m)." ;
               rdfs:label "Oe" .


:UnitSymbol.Pa uml:hasInitialValue "39" ;
               
               rdfs:comment "Pressure in pascals (N/m²). Note: the absolute or relative measurement of pressure is implied with this entry. See below for more explicit forms." ;
               rdfs:label "Pa" .


:UnitSymbol.PaPers uml:hasInitialValue "59" ;
                   
                   rdfs:comment "Pressure change rate in pascals per second." ;
                   rdfs:label "PaPers" .


:UnitSymbol.Pas uml:hasInitialValue "175" ;
                
                rdfs:comment "Dynamic viscosity, pascal seconds." ;
                rdfs:label "Pas" .


:UnitSymbol.Q uml:hasInitialValue "100" ;
              
              rdfs:comment "Quantity power, Q." ;
              rdfs:label "Q" .


:UnitSymbol.Qh uml:hasInitialValue "101" ;
               
               rdfs:comment "Quantity energy, Qh." ;
               rdfs:label "Qh" .


:UnitSymbol.S uml:hasInitialValue "27" ;
              
              rdfs:comment "Conductance in siemens." ;
              rdfs:label "S" .


:UnitSymbol.SPerm uml:hasInitialValue "57" ;
                  
                  rdfs:comment "Conductance per length (F/m)." ;
                  rdfs:label "SPerm" .


:UnitSymbol.Sv uml:hasInitialValue "24" ;
               
               rdfs:comment "Dose equivalent in sieverts (J/kg)." ;
               rdfs:label "Sv" .


:UnitSymbol.T uml:hasInitialValue "37" ;
              
              rdfs:comment "Magnetic flux density in teslas (Wb/m2)." ;
              rdfs:label "T" .


:UnitSymbol.V uml:hasInitialValue "29" ;
              
              rdfs:comment "Electric potential in volts (W/A)." ;
              rdfs:label "V" .


:UnitSymbol.V2 uml:hasInitialValue "67" ;
               
               rdfs:comment "Volt squared (W²/A²)." ;
               rdfs:label "V2" .


:UnitSymbol.V2h uml:hasInitialValue "104" ;
                
                rdfs:comment "Volt-squared hour, volt-squared-hours." ;
                rdfs:label "V2h" .


:UnitSymbol.VA uml:hasInitialValue "61" ;
               
               rdfs:comment "Apparent power in volt amperes. See also real power and reactive power." ;
               rdfs:label "VA" .


:UnitSymbol.VAh uml:hasInitialValue "71" ;
                
                rdfs:comment "Apparent energy in volt ampere hours." ;
                rdfs:label "VAh" .


:UnitSymbol.VAr uml:hasInitialValue "63" ;
                
                rdfs:comment """Reactive power in volt amperes reactive. The “reactive” or “imaginary” component of electrical power (VIsin(phi)). (See also real power and apparent power).
Note: Different meter designs use different methods to arrive at their results. Some meters may compute reactive power as an arithmetic value, while others compute the value vectorially. The data consumer should determine the method in use and the suitability of the measurement for the intended purpose.""" ;
                rdfs:label "VAr" .


:UnitSymbol.VArh uml:hasInitialValue "73" ;
                 
                 rdfs:comment "Reactive energy in volt ampere reactive hours." ;
                 rdfs:label "VArh" .


:UnitSymbol.VPerHz uml:hasInitialValue "74" ;
                   
                   rdfs:comment "Magnetic flux in volt per hertz." ;
                   rdfs:label "VPerHz" .


:UnitSymbol.VPerV uml:hasInitialValue "151" ;
                  
                  rdfs:comment "Voltage, ratio of voltages.  Note: Users may need to supply a prefix such as ‘m’ to show rates such as ‘mV/V’." ;
                  rdfs:label "VPerV" .


:UnitSymbol.VPerVA uml:hasInitialValue "153" ;
                   
                   rdfs:comment "Power factor, PF, the ratio of the active power to the apparent power.  Note: The sign convention used for power factor will differ between IEC meters and EEI (ANSI) meters. It is assumed that the data consumers understand the type of meter being used and agree on the sign convention in use at any given utility." ;
                   rdfs:label "VPerVA" .


:UnitSymbol.VPerVAr 
                    rdfs:comment "Power factor, PF, the ratio of the active power to the apparent power. Note: The sign convention used for power factor will differ between IEC meters and EEI (ANSI) meters. It is assumed that the data consumers understand the type of meter being used and agree on the sign convention in use at any given utility." ;
                    rdfs:label "VPerVAr" .


:UnitSymbol.VPerm uml:hasInitialValue "182" ;
                  
                  rdfs:comment "Electric field strength, volts per metre." ;
                  rdfs:label "VPerm" .


:UnitSymbol.Vh uml:hasInitialValue "280" ;
               
               rdfs:comment "Volt-hour, Volt hours." ;
               rdfs:label "Vh" .


:UnitSymbol.Vs uml:hasInitialValue "66" ;
               
               rdfs:comment "Volt seconds (Ws/A)." ;
               rdfs:label "Vs" .


:UnitSymbol.W uml:hasInitialValue "38" ;
              
              rdfs:comment "Real power in watts (J/s). Electrical power may have real and reactive components. The real portion of electrical power (I&#178;R or VIcos(phi)), is expressed in Watts. See also apparent power and reactive power." ;
              rdfs:label "W" .


:UnitSymbol.WPerA 
                  rdfs:comment "Active power per current flow, watts per Ampere." ;
                  rdfs:label "WPerA" .


:UnitSymbol.WPerW uml:hasInitialValue "168" ;
                  
                  rdfs:comment "Signal Strength, ratio of power.   Note: Users may need to supply a prefix such as ‘m’ to show rates such as ‘mW/W’." ;
                  rdfs:label "WPerW" .


:UnitSymbol.WPerm2 uml:hasInitialValue "55" ;
                   
                   rdfs:comment "Heat flux density, irradiance, watts per square metre." ;
                   rdfs:label "WPerm2" .


:UnitSymbol.WPerm2sr uml:hasInitialValue "192" ;
                     
                     rdfs:comment "Radiance, watts per square metre steradian." ;
                     rdfs:label "WPerm2sr" .


:UnitSymbol.WPermK uml:hasInitialValue "50" ;
                   
                   rdfs:comment "Thermal conductivity in watt/metres kelvin." ;
                   rdfs:label "WPermK" .


:UnitSymbol.WPers uml:hasInitialValue "81" ;
                  
                  rdfs:comment "Ramp rate in watts per second." ;
                  rdfs:label "WPers" .


:UnitSymbol.WPersr uml:hasInitialValue "191" ;
                   
                   rdfs:comment "Radiant intensity, watts per steradian." ;
                   rdfs:label "WPersr" .


:UnitSymbol.Wb uml:hasInitialValue "36" ;
               
               rdfs:comment "Magnetic flux in webers (V·s)." ;
               rdfs:label "Wb" .


:UnitSymbol.Wh uml:hasInitialValue "72" ;
               
               rdfs:comment "Real energy in watt hours." ;
               rdfs:label "Wh" .


:UnitSymbol.anglemin uml:hasInitialValue "196" ;
                     
                     rdfs:comment "Plane angle, minutes." ;
                     rdfs:label "anglemin" .


:UnitSymbol.anglesec uml:hasInitialValue "197" ;
                     
                     rdfs:comment "Plane angle, seconds." ;
                     rdfs:label "anglesec" .


:UnitSymbol.bar uml:hasInitialValue "214" ;
                
                rdfs:comment "Pressure in bars, (1 bar = 100 kPa)." ;
                rdfs:label "bar" .


:UnitSymbol.cd uml:hasInitialValue "8" ;
               
               rdfs:comment "Luminous intensity in candelas." ;
               rdfs:label "cd" .


:UnitSymbol.charPers uml:hasInitialValue "77" ;
                     
                     rdfs:comment "Data rate (baud) in characters per second." ;
                     rdfs:label "charPers" .


:UnitSymbol.character uml:hasInitialValue "76" ;
                      
                      rdfs:comment "Number of characters." ;
                      rdfs:label "character" .


:UnitSymbol.cosPhi uml:hasInitialValue "65" ;
                   
                   rdfs:comment """Power factor, dimensionless.
Note 1: This definition of power factor only holds for balanced systems. See the alternative definition under code 153.
Note 2 : Beware of differing sign conventions in use between the IEC and EEI. It is assumed that the data consumer understands the type of meter in use and the sign convention in use by the utility.""" ;
                   rdfs:label "cosPhi" .


:UnitSymbol.count uml:hasInitialValue "111" ;
                  
                  rdfs:comment "Amount of substance, Counter value." ;
                  rdfs:label "count" .


:UnitSymbol.d uml:hasInitialValue "195" ;
              
              rdfs:comment "Time in days, day = 24 h = 86400 s." ;
              rdfs:label "d" .


:UnitSymbol.dB uml:hasInitialValue "79" ;
               
               rdfs:comment "Sound pressure level in decibels. Note:  multiplier “d” is included in this unit symbol for compatibility with IEC 61850-7-3." ;
               rdfs:label "dB" .


:UnitSymbol.dBm uml:hasInitialValue "83" ;
                
                rdfs:comment "Power level (logarithmic ratio of signal strength , Bel-mW), normalized to 1mW. Note:  multiplier “d” is included in this unit symbol for compatibility with IEC 61850-7-3." ;
                rdfs:label "dBm" .


:UnitSymbol.deg uml:hasInitialValue "9" ;
                
                rdfs:comment "Plane angle in degrees." ;
                rdfs:label "deg" .


:UnitSymbol.degC uml:hasInitialValue "23" ;
                 
                 rdfs:comment """Relative temperature in degrees Celsius.
In the SI unit system the symbol is °C. Electric charge is measured in coulomb that has the unit symbol C. To distinguish degree Celsius from coulomb the symbol used in the UML is degC. The reason for not using °C is that the special character ° is difficult to manage in software.""" ;
                 rdfs:label "degC" .


:UnitSymbol.ft3 uml:hasInitialValue "119" ;
                
                rdfs:comment "Volume, cubic feet." ;
                rdfs:label "ft3" .


:UnitSymbol.gPerg uml:hasInitialValue "144" ;
                  
                  rdfs:comment "Concentration, The ratio of the mass of a solute divided by the mass of  the solution. Note: Users may need use a prefix such a ‘µ’ to express a quantity such as ‘µg/g’." ;
                  rdfs:label "gPerg" .


:UnitSymbol.gal uml:hasInitialValue "128" ;
                
                rdfs:comment "Volume in gallons, US gallon (1 gal = 231 in3 = 128 fl ounce)." ;
                rdfs:label "gal" .


:UnitSymbol.h uml:hasInitialValue "84" ;
              
              rdfs:comment "Time in hours, hour = 60 min = 3600 s." ;
              rdfs:label "h" .


:UnitSymbol.ha uml:hasInitialValue "198" ;
               
               rdfs:comment "Area, hectares." ;
               rdfs:label "ha" .


:UnitSymbol.kat uml:hasInitialValue "158" ;
                
                rdfs:comment "Catalytic activity, katal = mol / s." ;
                rdfs:label "kat" .


:UnitSymbol.katPerm3 uml:hasInitialValue "193" ;
                     
                     rdfs:comment "Catalytic activity concentration, katals per cubic metre." ;
                     rdfs:label "katPerm3" .


:UnitSymbol.kg uml:hasInitialValue "3" ;
               
               rdfs:comment "Mass in kilograms.  Note: multiplier “k” is included in this unit symbol for compatibility with IEC 61850-7-3." ;
               rdfs:label "kg" .


:UnitSymbol.kgPerJ 
                   rdfs:comment "Weight per energy in kilograms per joule (kg/J). Note: multiplier “k” is included in this unit symbol for compatibility with IEC 61850-7-3." ;
                   rdfs:label "kgPerJ" .


:UnitSymbol.kgPerm3 uml:hasInitialValue "48" ;
                    
                    rdfs:comment "Density in kilogram/cubic metres (kg/m³). Note: multiplier “k” is included in this unit symbol for compatibility with IEC 61850-7-3." ;
                    rdfs:label "kgPerm3" .


:UnitSymbol.kgm uml:hasInitialValue "47" ;
                
                rdfs:comment "Moment of mass in kilogram metres (kg·m) (first moment of mass). Note: multiplier “k” is included in this unit symbol for compatibility with IEC 61850-7-3." ;
                rdfs:label "kgm" .


:UnitSymbol.kgm2 uml:hasInitialValue "78" ;
                 
                 rdfs:comment "Moment of mass in kilogram square metres (kg·m²) (Second moment of mass, commonly called the moment of inertia). Note: multiplier “k” is included in this unit symbol for compatibility with IEC 61850-7-3." ;
                 rdfs:label "kgm2" .


:UnitSymbol.kn uml:hasInitialValue "219" ;
               
               rdfs:comment "Speed, knots (1 kn = 1852/3600) m/s." ;
               rdfs:label "kn" .


:UnitSymbol.l uml:hasInitialValue "134" ;
              
              rdfs:comment "Volume in litres, litre = dm3 = m3/1000." ;
              rdfs:label "l" .


:UnitSymbol.lPerh uml:hasInitialValue "137" ;
                  
                  rdfs:comment "Volumetric flow rate, litres per hour." ;
                  rdfs:label "lPerh" .


:UnitSymbol.lPerl uml:hasInitialValue "143" ;
                  
                  rdfs:comment "Concentration, The ratio of the volume of a solute divided by the volume of  the solution. Note: Users may need use a prefix such a ‘µ’ to express a quantity such as ‘µL/L’." ;
                  rdfs:label "lPerl" .


:UnitSymbol.lPers uml:hasInitialValue "82" ;
                  
                  rdfs:comment "Volumetric flow rate in litres per second." ;
                  rdfs:label "lPers" .


:UnitSymbol.lm uml:hasInitialValue "35" ;
               
               rdfs:comment "Luminous flux in lumens (cd·sr)." ;
               rdfs:label "lm" .


:UnitSymbol.lx uml:hasInitialValue "34" ;
               
               rdfs:comment "Illuminance in lux (lm/m²)." ;
               rdfs:label "lx" .


:UnitSymbol.m uml:hasInitialValue "2" ;
              
              rdfs:comment "Length in metres." ;
              rdfs:label "m" .


:UnitSymbol.m2 uml:hasInitialValue "41" ;
               
               rdfs:comment "Area in square metres (m²)." ;
               rdfs:label "m2" .


:UnitSymbol.m2Pers uml:hasInitialValue "49" ;
                   
                   rdfs:comment "Viscosity in square metres / second (m²/s)." ;
                   rdfs:label "m2Pers" .


:UnitSymbol.m3 uml:hasInitialValue "42" ;
               
               rdfs:comment "Volume in cubic metres (m³)." ;
               rdfs:label "m3" .


:UnitSymbol.m3Compensated uml:hasInitialValue "167" ;
                          
                          rdfs:comment "Volume, cubic metres, with the value compensated for weather effects." ;
                          rdfs:label "m3Compensated" .


:UnitSymbol.m3Perh uml:hasInitialValue "125" ;
                   
                   rdfs:comment "Volumetric flow rate, cubic metres per hour." ;
                   rdfs:label "m3Perh" .


:UnitSymbol.m3Perkg uml:hasInitialValue "174" ;
                    
                    rdfs:comment "Specific volume, cubic metres per kilogram, v." ;
                    rdfs:label "m3Perkg" .


:UnitSymbol.m3Pers uml:hasInitialValue "45" ;
                   
                   rdfs:comment "Volumetric flow rate in cubic metres per second (m³/s)." ;
                   rdfs:label "m3Pers" .


:UnitSymbol.m3Uncompensated uml:hasInitialValue "166" ;
                            
                            rdfs:comment "Volume, cubic metres, with the value uncompensated for weather effects." ;
                            rdfs:label "m3Uncompensated" .


:UnitSymbol.mPerm3 uml:hasInitialValue "46" ;
                   
                   rdfs:comment "Fuel efficiency in metres per cubic metres (m/m³)." ;
                   rdfs:label "mPerm3" .


:UnitSymbol.mPers uml:hasInitialValue "43" ;
                  
                  rdfs:comment "Velocity in metres per second (m/s)." ;
                  rdfs:label "mPers" .


:UnitSymbol.mPers2 uml:hasInitialValue "44" ;
                   
                   rdfs:comment "Acceleration in metres per second squared (m/s²)." ;
                   rdfs:label "mPers2" .


:UnitSymbol.min uml:hasInitialValue "85" ;
                
                rdfs:comment "Time in minutes, minute  = 60 s." ;
                rdfs:label "min" .


:UnitSymbol.mmHg uml:hasInitialValue "215" ;
                 
                 rdfs:comment "Pressure, millimetres of mercury (1 mmHg is approximately 133.3 Pa)." ;
                 rdfs:label "mmHg" .


:UnitSymbol.mol uml:hasInitialValue "7" ;
                
                rdfs:comment "Amount of substance in moles." ;
                rdfs:label "mol" .


:UnitSymbol.molPerkg uml:hasInitialValue "147" ;
                     
                     rdfs:comment "Concentration, Molality, the amount of solute in moles and the amount of solvent in kilograms." ;
                     rdfs:label "molPerkg" .


:UnitSymbol.molPerm3 uml:hasInitialValue "145" ;
                     
                     rdfs:comment "Concentration, The amount of substance concentration, (c), the amount of solvent in moles divided by the volume of solution in m³." ;
                     rdfs:label "molPerm3" .


:UnitSymbol.molPermol uml:hasInitialValue "146" ;
                      
                      rdfs:comment "Concentration, Molar fraction, the ratio of the molar amount of a solute divided by the molar amount of the solution." ;
                      rdfs:label "molPermol" .


:UnitSymbol.none uml:hasInitialValue "0" ;
                 
                 rdfs:comment "Dimension less quantity, e.g. count, per unit, etc." ;
                 rdfs:label "none" .


:UnitSymbol.ohm uml:hasInitialValue "30" ;
                
                rdfs:comment "Electric resistance in ohms (V/A)." ;
                rdfs:label "ohm" .


:UnitSymbol.ohmPerm uml:hasInitialValue "86" ;
                    
                    rdfs:comment "Electric resistance per length in ohms per metre ((V/A)/m)." ;
                    rdfs:label "ohmPerm" .


:UnitSymbol.ohmm uml:hasInitialValue "102" ;
                 
                 rdfs:comment "Resistivity, ohm metres, (rho)." ;
                 rdfs:label "ohmm" .


:UnitSymbol.onePerHz 
                     rdfs:comment "Reciprocal of frequency (1/Hz)." ;
                     rdfs:label "onePerHz" .


:UnitSymbol.onePerm uml:hasInitialValue "173" ;
                    
                    rdfs:comment "Wavenumber, reciprocal metres,  (1/m)." ;
                    rdfs:label "onePerm" .


:UnitSymbol.ppm uml:hasInitialValue "52" ;
                
                rdfs:comment "Concentration in parts per million." ;
                rdfs:label "ppm" .


:UnitSymbol.rad uml:hasInitialValue "10" ;
                
                rdfs:comment "Plane angle in radians (m/m)." ;
                rdfs:label "rad" .


:UnitSymbol.radPers uml:hasInitialValue "54" ;
                    
                    rdfs:comment "Angular velocity in radians per second (rad/s)." ;
                    rdfs:label "radPers" .


:UnitSymbol.radPers2 uml:hasInitialValue "178" ;
                     
                     rdfs:comment "Angular acceleration, radians per second squared." ;
                     rdfs:label "radPers2" .


:UnitSymbol.rev uml:hasInitialValue "154" ;
                
                rdfs:comment "Amount of rotation, revolutions." ;
                rdfs:label "rev" .


:UnitSymbol.rotPers uml:hasInitialValue "53" ;
                    
                    rdfs:comment "Rotations per second (1/s). See also Hz (1/s)." ;
                    rdfs:label "rotPers" .


:UnitSymbol.s uml:hasInitialValue "4" ;
              
              rdfs:comment "Time in seconds." ;
              rdfs:label "s" .


:UnitSymbol.sPers uml:hasInitialValue "149" ;
                  
                  rdfs:comment "Time, Ratio of time.  Note: Users may need to supply a prefix such as ‘&#181;’ to show rates such as ‘&#181;s/s’." ;
                  rdfs:label "sPers" .


:UnitSymbol.sr uml:hasInitialValue "11" ;
               
               rdfs:comment "Solid angle in steradians (m2/m2)." ;
               rdfs:label "sr" .


:UnitSymbol.therm uml:hasInitialValue "169" ;
                  
                  rdfs:comment "Energy, therms." ;
                  rdfs:label "therm" .


:UnitSymbol.tonne uml:hasInitialValue "199" ;
                  
                  rdfs:comment "Mass in tons, “tonne” or “metric  ton” (1000 kg = 1 Mg)." ;
                  rdfs:label "tonne" .


:UnitType.CCYC 
               rdfs:comment "Combined Cycle" ;
               rdfs:label "CCYC" .


:UnitType.GTUR 
               rdfs:comment "Gas Turbine" ;
               rdfs:label "GTUR" .


:UnitType.HYDR 
               rdfs:comment "Hydro Turbine" ;
               rdfs:label "HYDR" .


:UnitType.OTHR 
               rdfs:comment "Other" ;
               rdfs:label "OTHR" .


:UnitType.PHOT 
               rdfs:comment "Photovoltaic" ;
               rdfs:label "PHOT" .


:UnitType.PTUR 
               rdfs:comment "Hydro Pump-Turbine" ;
               rdfs:label "PTUR" .


:UnitType.RECP 
               rdfs:comment "Reciprocating Engine" ;
               rdfs:label "RECP" .


:UnitType.STUR 
               rdfs:comment "Steam Turbine" ;
               rdfs:label "STUR" .


:UnitType.SYNC 
               rdfs:comment "Synchronous Condenser" ;
               rdfs:label "SYNC" .


:UnitType.WIND 
               rdfs:comment "Wind Turbine" ;
               rdfs:label "WIND" .


:UnitTypeEMS.FLAG 
                  rdfs:label "FLAG" .


:UnitTypeEMS.MW 
                rdfs:label "MW" .


:UsagePointConnectedKind.connected 
                                   rdfs:comment "The usage point is connected to the network and able to receive or send the applicable commodity (electricity, gas, water, etc.)." ;
                                   rdfs:label "connected" .


:UsagePointConnectedKind.logicallyDisconnected 
                                               rdfs:comment "The usage point has been disconnected through operation of a disconnect function within the meter present at the usage point.  The usage point is unable to receive or send the applicable commodity (electricity, gas, water, etc.)  A logical disconnect can often be achieved without utilising a field crew." ;
                                               rdfs:label "logicallyDisconnected" .


:UsagePointConnectedKind.physicallyDisconnected 
                                                rdfs:comment "The usage point has been disconnected from the network at a point upstream of the meter. The usage point is unable to receive or send the applicable commodity (electricity, gas, water, etc.). A physical disconnect is often achieved by utilising a field crew." ;
                                                rdfs:label "physicallyDisconnected" .


:Validity.GOOD 
               rdfs:comment "The value is marked good if no abnormal condition of the acquisition function or the information source is detected." ;
               rdfs:label "GOOD" .


:Validity.INVALID 
                  rdfs:comment "The value is marked invalid when a supervision function recognises abnormal conditions of the acquisition function or the information source (missing or non-operating updating devices). The value is not defined under this condition. The mark invalid is used to indicate to the client that the value may be incorrect and shall not be used." ;
                  rdfs:label "INVALID" .


:Validity.QUESTIONABLE 
                       rdfs:comment "The value is marked questionable if a supervision function detects an abnormal behaviour, however the value could still be valid. The client is responsible for determining whether or not values marked \"questionable\" should be used." ;
                       rdfs:label "QUESTIONABLE" .


:VehicleUsageKind.contractor 
                             rdfs:comment "Contractor vehicle." ;
                             rdfs:label "contractor" .


:VehicleUsageKind.crew 
                       rdfs:comment "Crew vehicle." ;
                       rdfs:label "crew" .


:VehicleUsageKind.other 
                        rdfs:comment "Other vehicle." ;
                        rdfs:label "other" .


:VehicleUsageKind.user 
                       rdfs:comment "User vehicle." ;
                       rdfs:label "user" .


:VsPpccControlKind.pPcc 
                        rdfs:comment "Control is real power at point of common coupling. The target value is provided by ACDCConverter.targetPpcc." ;
                        rdfs:label "pPcc" .


:VsPpccControlKind.pPccAndUdcDroop 
                                   rdfs:comment "Control is active power at point of common coupling and local DC voltage, with the droop. Target values are provided by ACDCConverter.targetPpcc, ACDCConverter.targetUdc and VsConverter.droop." ;
                                   rdfs:label "pPccAndUdcDroop" .


:VsPpccControlKind.pPccAndUdcDroopPilot 
                                        rdfs:comment "Control is active power at point of common coupling and the pilot DC voltage, with the droop. The mode is used for Multi Terminal High Voltage DC (MTDC) systems where multiple HVDC Substations are connected to the HVDC transmission lines. The pilot voltage is then used to coordinate the control the DC voltage across the HVDC substations. Targets are provided by ACDCConverter.targetPpcc, ACDCConverter.targetUdc and  VsConverter.droop." ;
                                        rdfs:label "pPccAndUdcDroopPilot" .


:VsPpccControlKind.pPccAndUdcDroopWithCompensation 
                                                   rdfs:comment "Control is active power at point of common coupling and compensated DC voltage, with the droop. Compensation factor is the resistance, as an approximation of the DC voltage of a common (real or virtual) node in the DC network. Targets are provided by ACDCConverter.targetPpcc, ACDCConverter.targetUdc, VsConverter.droop and VsConverter.droopCompensation." ;
                                                   rdfs:label "pPccAndUdcDroopWithCompensation" .


:VsPpccControlKind.phasePcc 
                            rdfs:comment "Control is phase at point of common coupling. Target is provided by VsConverter.targetPhasePcc." ;
                            rdfs:label "phasePcc" .


:VsPpccControlKind.udc 
                       rdfs:comment "Control is DC voltage  with target value provided by ACDCConverter.targetUdc." ;
                       rdfs:label "udc" .


:VsQpccControlKind.powerFactorPcc 
                                  rdfs:comment "Control is power factor at point of common coupling. Target is provided by VsConverter.targetPowerFactorPcc." ;
                                  rdfs:label "powerFactorPcc" .


:VsQpccControlKind.pulseWidthModulation 
                                        rdfs:comment "No explicit control. Pulse-modulation factor is directly set in magnitude (VsConverter.targetPWMfactor) and phase (VsConverter.targetPhasePcc)." ;
                                        rdfs:label "pulseWidthModulation" .


:VsQpccControlKind.reactivePcc 
                               rdfs:comment "Control is reactive power at point of common coupling. Target is provided by VsConverter.targetQpcc." ;
                               rdfs:label "reactivePcc" .


:VsQpccControlKind.voltagePcc 
                              rdfs:comment "Control is voltage at point of common coupling. Target is provided by VsConverter.targetUpcc." ;
                              rdfs:label "voltagePcc" .


:WEPStandardEditionKind.none 
                             rdfs:comment "No edition." ;
                             rdfs:label "none" .


:WEPStandardEditionKind.unknown 
                                rdfs:comment "Unknown edition." ;
                                rdfs:label "unknown" .


:WEPStandardKind._12__1254E 
                            rdfs:comment "Westinghouse Engineering Procedure 12,1254E." ;
                            rdfs:label "12, 1254E" .


:WeatherCodeKind.blowingDust 
                             rdfs:comment "\"BD\" weather code (\"Blowing Dust\")." ;
                             rdfs:label "blowingDust" .


:WeatherCodeKind.blowingSand 
                             rdfs:comment "\"BN\" weather code (\"Blowing Sand\")." ;
                             rdfs:label "blowingSand" .


:WeatherCodeKind.blowingSnow 
                             rdfs:comment "\"BS\" weather code (\"Blowing Snow\")." ;
                             rdfs:label "blowingSnow" .


:WeatherCodeKind.cloudy 
                        rdfs:label "cloudy" .


:WeatherCodeKind.drizzle 
                         rdfs:comment "\"L\" weather code (\"Drizzle\")." ;
                         rdfs:label "drizzle" .


:WeatherCodeKind.fog 
                     rdfs:comment "\"F weather code (\"Fog" ;
                     rdfs:label "fog" .


:WeatherCodeKind.freezingDrizzle 
                                 rdfs:comment "\"ZL\" weather code (\"Freezing Drizzle\")." ;
                                 rdfs:label "freezingDrizzle" .


:WeatherCodeKind.freezingRain 
                              rdfs:comment "\"ZR\" weather code (\"Freezing Rain\")." ;
                              rdfs:label "freezingRain" .


:WeatherCodeKind.freezingSpray 
                               rdfs:comment "\"ZF\" weather code (\"Freezing Spray\")." ;
                               rdfs:label "freezingSpray" .


:WeatherCodeKind.frost 
                       rdfs:comment "\"FR\" weather code (\"Frost\")." ;
                       rdfs:label "frost" .


:WeatherCodeKind.hail 
                      rdfs:comment "\"A\" weather code (\"Hail\")." ;
                      rdfs:label "hail" .


:WeatherCodeKind.haze 
                      rdfs:comment "\"H\" weather code (\"Haze\")." ;
                      rdfs:label "haze" .


:WeatherCodeKind.iceCrystals 
                             rdfs:comment "\"IC\" weather code (\"Ice Crystals\")." ;
                             rdfs:label "iceCrystals" .


:WeatherCodeKind.iceFog 
                        rdfs:comment "\"IF\" weather code (\"Ice Fog\")." ;
                        rdfs:label "iceFog" .


:WeatherCodeKind.mist 
                      rdfs:comment "\"BR\" weather code (\"Mist\")," ;
                      rdfs:label "mist" .


:WeatherCodeKind.rain 
                      rdfs:comment "\"R\" weather code (\"Rain\")." ;
                      rdfs:label "rain" .


:WeatherCodeKind.rainShowers 
                             rdfs:comment "\"RW\" weather code (\"Rain Showers\")." ;
                             rdfs:label "rainShowers" .


:WeatherCodeKind.rainSnowMix 
                             rdfs:comment "\"RS\" weather code (\"Rain/Snow Mix\")." ;
                             rdfs:label "rainSnowMix" .


:WeatherCodeKind.sleet 
                       rdfs:comment "\"IP\" weather code (\"Ice Pellets/Sleet\")." ;
                       rdfs:label "sleet" .


:WeatherCodeKind.smoke 
                       rdfs:comment "\"K\" weather code (\"Smoke\")." ;
                       rdfs:label "smoke" .


:WeatherCodeKind.snow 
                      rdfs:comment "\"S\" weather code (\"Snow\")." ;
                      rdfs:label "snow" .


:WeatherCodeKind.snowShowers 
                             rdfs:comment "\"SW\" weather code (\"Snow Showers\")." ;
                             rdfs:label "snowShowers" .


:WeatherCodeKind.snowSleetMix 
                              rdfs:comment "\"SI\" weather code (\"Snow/Sleet Mix\")." ;
                              rdfs:label "snowSleetMix" .


:WeatherCodeKind.sunny 
                       rdfs:label "sunny" .


:WeatherCodeKind.thunderStorms 
                               rdfs:comment "\"T\" weather code (\"Thunder Storms\")." ;
                               rdfs:label "thunderStorms" .


:WeatherCodeKind.volcanicAsh 
                             rdfs:comment "\"VA\" weather code (\"Volcanic Ash\")." ;
                             rdfs:label "volcanicAsh" .


:WeatherCodeKind.waterSpouts 
                             rdfs:comment "\"WP\" weather code (\"Water Spouts\")" ;
                             rdfs:label "waterSpouts" .


:WeatherCodeKind.wintryMix 
                           rdfs:comment "\"WS\" weather code (\"Wintry Mix\")." ;
                           rdfs:label "wintryMix" .


:WindGenUnitKind.offshore 
                          rdfs:comment "The wind generating unit is located offshore." ;
                          rdfs:label "offshore" .


:WindGenUnitKind.onshore 
                         rdfs:comment "The wind generating unit is located onshore." ;
                         rdfs:label "onshore" .


:WindLookupTableFunctionKind.ipmax 
                                   rdfs:comment "Lookup table for voltage dependency of active current limits (i<sub>pmax</sub>(u<sub>WT</sub>)). It is used for the current limitation model, IEC 61400-27-1:2015, 5.6.5.8." ;
                                   rdfs:label "ipmax" .


:WindLookupTableFunctionKind.iqmax 
                                   rdfs:comment "Lookup table for voltage dependency of reactive current limits (i<sub>qmax</sub>(u<sub>WT</sub>)). It is used for the current limitation model, IEC 61400-27-1:2015, 5.6.5.8." ;
                                   rdfs:label "iqmax" .


:WindLookupTableFunctionKind.omegap 
                                    rdfs:comment "Power vs. speed lookup table (omega(p)). It is used for the P control model type 3, IEC 61400-27-1:2015, 5.6.5.4." ;
                                    rdfs:label "omegap" .


:WindLookupTableFunctionKind.prr 
                                 rdfs:comment "Power versus speed change (negative slip) lookup table (p<sub>rr</sub>(deltaomega)). It is used for the rotor resistance control model, IEC 61400-27-1:2015, 5.6.5.3." ;
                                 rdfs:label "prr" .


:WindLookupTableFunctionKind.pwp 
                                 rdfs:comment "Power vs. frequency lookup table (p<sub>WPbias</sub>(f)). It is used for the wind power plant frequency and active power control model, IEC 61400-27-1:2015, Annex D." ;
                                 rdfs:label "pwp" .


:WindLookupTableFunctionKind.qmaxp 
                                   rdfs:comment "Lookup table for active power dependency of reactive power maximum limit (q<sub>maxp</sub>(p)). It is used for the QP and QU limitation model, IEC 61400-27-1:2015, 5.6.5.10." ;
                                   rdfs:label "qmaxp" .


:WindLookupTableFunctionKind.qmaxu 
                                   rdfs:comment "Lookup table for voltage dependency of reactive power maximum limit (q<sub>maxu</sub>(p)). It is used for the QP and QU limitation model, IEC 61400-27-1:2015, 5.6.5.10." ;
                                   rdfs:label "qmaxu" .


:WindLookupTableFunctionKind.qminp 
                                   rdfs:comment "Lookup table for active power dependency of reactive power minimum limit (q<sub>minp</sub>(p)). It is used for the QP and QU limitation model, IEC 61400-27-1:2015, 5.6.5.10." ;
                                   rdfs:label "qminp" .


:WindLookupTableFunctionKind.qminu 
                                   rdfs:comment "Lookup table for voltage dependency of reactive power minimum limit (q<sub>minu</sub>(p)). It is used for the QP and QU limitation model, IEC 61400-27-1:2015, 5.6.5.10." ;
                                   rdfs:label "qminu" .


:WindLookupTableFunctionKind.qwp 
                                 rdfs:comment "Look up table for the UQ static mode (q<sub>WP</sub>(u<sub>err</sub>)). It is used for the voltage and reactive power control model, IEC 61400-27-1:2015, Annex D." ;
                                 rdfs:label "qwp" .


:WindLookupTableFunctionKind.tcwdu 
                                   rdfs:comment "Crowbar duration versus voltage variation look-up table (T<sub>CW</sub>(du)). It is a case-dependent parameter. It is used for the type 3B generator set model, IEC 61400-27-1:2015, 5.6.3.3." ;
                                   rdfs:label "tcwdu" .


:WindLookupTableFunctionKind.tduwt 
                                   rdfs:comment "Lookup table to determine the duration of the power reduction after a voltage dip, depending on the size of the voltage dip (T<sub>d</sub>(u<sub>WT</sub>)). It is a type-dependent parameter. It is used for the pitch control power model, IEC 61400-27-1:2015, 5.6.5.1." ;
                                   rdfs:label "tduwt" .


:WindLookupTableFunctionKind.tfover 
                                    rdfs:comment "Disconnection time versus over-frequency lookup table (T<sub>fover</sub>(f<sub>WT</sub>)). It is used for the grid protection model, IEC 61400-27-1:2015, 5.6.6." ;
                                    rdfs:label "tfover" .


:WindLookupTableFunctionKind.tfunder 
                                     rdfs:comment "Disconnection time versus under-frequency lookup table (T<sub>funder</sub>(f<sub>WT</sub>)). It is used for the grid protection model, IEC 61400-27-1:2015, 5.6.6." ;
                                     rdfs:label "tfunder" .


:WindLookupTableFunctionKind.tuover 
                                    rdfs:comment "Disconnection time versus over-voltage lookup table (T<sub>uover</sub>(u<sub>WT</sub>)). It is used for the grid protection model, IEC 61400-27-1:2015, 5.6.6." ;
                                    rdfs:label "tuover" .


:WindLookupTableFunctionKind.tuunder 
                                     rdfs:comment "Disconnection time versus under-voltage lookup table (T<sub>uunder</sub>(u<sub>WT</sub>)). It is used for the grid protection model, IEC 61400-27-1:2015, 5.6.6." ;
                                     rdfs:label "tuunder" .


:WindPlantQcontrolModeKind.powerFactor 
                                       rdfs:comment "Power factor reference." ;
                                       rdfs:label "powerFactor" .


:WindPlantQcontrolModeKind.reactivePower 
                                         rdfs:comment "Reactive power reference." ;
                                         rdfs:label "reactivePower" .


:WindPlantQcontrolModeKind.uqStatic 
                                    rdfs:comment "UQ static." ;
                                    rdfs:label "uqStatic" .


:WindPlantQcontrolModeKind.voltageControl 
                                          rdfs:comment "Voltage control." ;
                                          rdfs:label "voltageControl" .


:WindQcontrolModeKind.openLoopReactivePower 
                                            rdfs:comment "Open loop reactive power control (only used with closed loop at plant level) (<i>M</i><i><sub>qG</sub></i><sub> </sub>equals 2)." ;
                                            rdfs:label "openLoopReactivePower" .


:WindQcontrolModeKind.openLooppowerFactor 
                                          rdfs:comment "Open loop power factor control (<i>M</i><i><sub>qG</sub></i><sub> </sub>equals 4)." ;
                                          rdfs:label "openLooppowerFactor" .


:WindQcontrolModeKind.powerFactor 
                                  rdfs:comment "Power factor control (<i>M</i><i><sub>qG</sub></i><sub> </sub>equals 3)." ;
                                  rdfs:label "powerFactor" .


:WindQcontrolModeKind.reactivePower 
                                    rdfs:comment "Reactive power control (<i>M</i><i><sub>qG</sub></i> equals 1)." ;
                                    rdfs:label "reactivePower" .


:WindQcontrolModeKind.voltage 
                              rdfs:comment "Voltage control (<i>M</i><i><sub>qG</sub></i> equals 0)." ;
                              rdfs:label "voltage" .


:WindUVRTQcontrolModeKind.mode0 
                                rdfs:comment "Voltage-dependent reactive current injection (<i>M</i><i><sub>qUVRT</sub></i> <sub> </sub>equals 0)." ;
                                rdfs:label "mode0" .


:WindUVRTQcontrolModeKind.mode1 
                                rdfs:comment "Reactive current injection controlled as the pre-fault value plus an additional voltage dependent reactive current injection (<i>M</i><i><sub>qUVRT</sub></i> equals 1)." ;
                                rdfs:label "mode1" .


:WindUVRTQcontrolModeKind.mode2 
                                rdfs:comment "Reactive current injection controlled as the pre-fault value plus an additional voltage-dependent reactive current injection during fault, and as the pre-fault value plus an additional constant reactive current injection post fault (<i>M</i><i><sub>qUVRT</sub></i><sub>  </sub>equals 2)." ;
                                rdfs:label "mode2" .


:WindingConnection.A 
                     rdfs:comment "Autotransformer common winding." ;
                     rdfs:label "A" .


:WindingConnection.D 
                     rdfs:comment "Delta." ;
                     rdfs:label "D" .


:WindingConnection.I 
                     rdfs:comment "Independent winding, for single-phase connections." ;
                     rdfs:label "I" .


:WindingConnection.Y 
                     rdfs:comment "Wye." ;
                     rdfs:label "Y" .


:WindingConnection.Yn 
                      rdfs:comment "Wye, with neutral brought out for grounding." ;
                      rdfs:label "Yn" .


:WindingConnection.Z 
                     rdfs:comment "ZigZag." ;
                     rdfs:label "Z" .


:WindingConnection.Zn 
                      rdfs:comment "ZigZag, with neutral brought out for grounding." ;
                      rdfs:label "Zn" .


:WindingInsulationKind.nomex 
                             rdfs:label "nomex" .


:WindingInsulationKind.other 
                             rdfs:label "other" .


:WindingInsulationKind.paper 
                             rdfs:label "paper" .


:WindingInsulationKind.thermallyUpgradedPaper 
                                              rdfs:label "thermallyUpgradedPaper" .


:WireInsulationKind.asbestosAndVarnishedCambric 
                                                rdfs:comment "Asbestos and varnished cambric wire insulation." ;
                                                rdfs:label "asbestosAndVarnishedCambric" .


:WireInsulationKind.beltedPilc 
                               rdfs:comment "Belted pilc wire insulation." ;
                               rdfs:label "beltedPilc" .


:WireInsulationKind.butyl 
                          rdfs:comment "Butyl wire insulation." ;
                          rdfs:label "butyl" .


:WireInsulationKind.crosslinkedPolyethylene 
                                            rdfs:comment "Crosslinked polyethylene wire insulation." ;
                                            rdfs:label "crosslinkedPolyethylene" .


:WireInsulationKind.ethylenePropyleneRubber 
                                            rdfs:comment "Ethylene propylene rubber wire insulation." ;
                                            rdfs:label "ethylenePropyleneRubber" .


:WireInsulationKind.highMolecularWeightPolyethylene 
                                                    rdfs:comment "High nolecular weight polyethylene wire insulation." ;
                                                    rdfs:label "highMolecularWeightPolyethylene" .


:WireInsulationKind.highPressureFluidFilled 
                                            rdfs:comment "High pressure fluid filled wire insulation." ;
                                            rdfs:label "highPressureFluidFilled" .


:WireInsulationKind.lowCapacitanceRubber 
                                         rdfs:comment "Low capacitance rubber wire insulation." ;
                                         rdfs:label "lowCapacitanceRubber" .


:WireInsulationKind.oilPaper 
                             rdfs:comment "Oil paper wire insulation." ;
                             rdfs:label "oilPaper" .


:WireInsulationKind.other 
                          rdfs:comment "Other kind of wire insulation." ;
                          rdfs:label "other" .


:WireInsulationKind.ozoneResistantRubber 
                                         rdfs:comment "Ozone resistant rubber wire insulation." ;
                                         rdfs:label "ozoneResistantRubber" .


:WireInsulationKind.rubber 
                           rdfs:comment "Rubber wire insulation." ;
                           rdfs:label "rubber" .


:WireInsulationKind.siliconRubber 
                                  rdfs:comment "Silicon rubber wire insulation." ;
                                  rdfs:label "siliconRubber" .


:WireInsulationKind.treeResistantHighMolecularWeightPolyethylene 
                                                                 rdfs:comment "Tree resistant high molecular weight polyethylene wire insulation." ;
                                                                 rdfs:label "treeResistantHighMolecularWeightPolyethylene" .


:WireInsulationKind.treeRetardantCrosslinkedPolyethylene 
                                                         rdfs:comment "Tree retardant crosslinked polyethylene wire insulation." ;
                                                         rdfs:label "treeRetardantCrosslinkedPolyethylene" .


:WireInsulationKind.unbeltedPilc 
                                 rdfs:comment "Unbelted pilc wire insulation." ;
                                 rdfs:label "unbeltedPilc" .


:WireInsulationKind.varnishedCambricCloth 
                                          rdfs:comment "Varnished cambric cloth wire insulation." ;
                                          rdfs:label "varnishedCambricCloth" .


:WireInsulationKind.varnishedDacronGlass 
                                         rdfs:comment "Varnished dacron glass wire insulation." ;
                                         rdfs:label "varnishedDacronGlass" .


:WireMaterialKind.aaac 
                       rdfs:comment "Aluminum-alloy conductor steel reinforced." ;
                       rdfs:label "aaac" .


:WireMaterialKind.acsr 
                       rdfs:comment "Aluminum conductor steel reinforced." ;
                       rdfs:label "acsr" .


:WireMaterialKind.aluminum 
                           rdfs:comment "Aluminum wire." ;
                           rdfs:label "aluminum" .


:WireMaterialKind.aluminumAlloy 
                                rdfs:comment "Aluminum-alloy wire." ;
                                rdfs:label "aluminumAlloy" .


:WireMaterialKind.aluminumAlloySteel 
                                     rdfs:comment "Aluminum-alloy-steel wire." ;
                                     rdfs:label "aluminumAlloySteel" .


:WireMaterialKind.aluminumSteel 
                                rdfs:comment "Aluminum-steel wire." ;
                                rdfs:label "aluminumSteel" .


:WireMaterialKind.copper 
                         rdfs:comment "Copper wire." ;
                         rdfs:label "copper" .


:WireMaterialKind.other 
                        rdfs:comment "Other wire material." ;
                        rdfs:label "other" .


:WireMaterialKind.steel 
                        rdfs:comment "Steel wire." ;
                        rdfs:label "steel" .


:WireUsageKind.distribution 
                            rdfs:comment "Wire is used in medium voltage network." ;
                            rdfs:label "distribution" .


:WireUsageKind.other 
                     rdfs:comment "Other kind of wire usage." ;
                     rdfs:label "other" .


:WireUsageKind.secondary 
                         rdfs:comment "Wire is used in low voltage circuit." ;
                         rdfs:label "secondary" .


:WireUsageKind.transmission 
                            rdfs:comment "Wire is used in extra-high voltage or high voltage network." ;
                            rdfs:label "transmission" .


:WorkActionKind.abandon 
                        rdfs:comment "Leave it in place but not use it." ;
                        rdfs:label "abandon" .


:WorkActionKind.install 
                        rdfs:comment "Install." ;
                        rdfs:label "install" .


:WorkActionKind.remove 
                       rdfs:comment "Remove." ;
                       rdfs:label "remove" .


:WorkActionKind.transfer 
                         rdfs:comment "Remove from one and install at another loctation." ;
                         rdfs:label "transfer" .


:WorkStatusKind.approved 
                         rdfs:comment "Work has been approved." ;
                         rdfs:label "approved" .


:WorkStatusKind.cancelled 
                          rdfs:comment "Work has been canceled." ;
                          rdfs:label "cancelled" .


:WorkStatusKind.closed 
                       rdfs:comment "Work has been closed (typically by a person responsible for work management) and is ready for billing." ;
                       rdfs:label "closed" .


:WorkStatusKind.completed 
                          rdfs:comment "Work has been completed, i.e., crew can leave the work location and is available for another work." ;
                          rdfs:label "completed" .


:WorkStatusKind.dispatched 
                           rdfs:comment "Crew has been dispatched." ;
                           rdfs:label "dispatched" .


:WorkStatusKind.enroute 
                        rdfs:comment "Crew is 'en route'." ;
                        rdfs:label "enroute" .


:WorkStatusKind.inProgress 
                           rdfs:comment "Work is in progress." ;
                           rdfs:label "inProgress" .


:WorkStatusKind.onSite 
                       rdfs:comment "Crew is on the site." ;
                       rdfs:label "onSite" .


:WorkStatusKind.scheduled 
                          rdfs:comment "Work has been scheduled." ;
                          rdfs:label "scheduled" .


:WorkStatusKind.waitingOnApproval 
                                  rdfs:comment "Work approval is pending." ;
                                  rdfs:label "waitingOnApproval" .


:WorkStatusKind.waitingOnMaterial 
                                  rdfs:comment "Work has been waiting on material." ;
                                  rdfs:label "waitingOnMaterial" .


:WorkStatusKind.waitingToBeScheduled 
                                     rdfs:comment "Work needs to be scheduled." ;
                                     rdfs:label "waitingToBeScheduled" .


:WorkTaskKind.exchange 
                       rdfs:comment "Work task deals with exchange of assets." ;
                       rdfs:label "exchange" .


:WorkTaskKind.install 
                      rdfs:comment "Work task deals with installation of assets." ;
                      rdfs:label "install" .


:WorkTaskKind.investigate 
                          rdfs:comment "Work task deals with investigation about assets." ;
                          rdfs:label "investigate" .


:WorkTaskKind.remove 
                     rdfs:comment "Work task deals with removal of assets." ;
                     rdfs:label "remove" .


:WorkTimeScheduleKind.actual 
                             rdfs:comment "Actual work time schedule." ;
                             rdfs:label "actual" .


:WorkTimeScheduleKind.earliest 
                               rdfs:comment "Earliest work time schedule." ;
                               rdfs:label "earliest" .


:WorkTimeScheduleKind.estimate 
                               rdfs:comment "Estimate work time schedule." ;
                               rdfs:label "estimate" .


:WorkTimeScheduleKind.immediate 
                                rdfs:comment "??." ;
                                rdfs:label "immediate" .


:WorkTimeScheduleKind.latest 
                             rdfs:comment "Latest work time schedule." ;
                             rdfs:label "latest" .


:WorkTimeScheduleKind.request 
                              rdfs:comment "Request work time schedule." ;
                              rdfs:label "request" .


:YesNo.NO 
          rdfs:label "NO" .


:YesNo.YES 
           rdfs:label "YES" .


:ZoneKind.electricalNetwork 
                            rdfs:label "electricalNetwork" .


:ZoneKind.other 
                rdfs:label "other" .


:ZoneKind.specialRestrictionLand 
                                 rdfs:label "specialRestrictionLand" .


:ZoneKind.weatherZone 
                      rdfs:label "weatherZone" .


:ZoneType.ASREGION 
                   rdfs:comment "ancillary service region" ;
                   rdfs:label "ASREGION" .


:ZoneType.DCA 
              rdfs:comment "designated congestion area" ;
              rdfs:label "DCA" .


:ZoneType.LOADZONE 
                   rdfs:comment "load zone" ;
                   rdfs:label "LOADZONE" .


:ZoneType.RUCZONE 
                  rdfs:comment "RUC zone" ;
                  rdfs:label "RUCZONE" .


:ZoneType.TRADINGHUB 
                     rdfs:comment "trading hub" ;
                     rdfs:label "TRADINGHUB" .


:runTypeCAISO.P 
                rdfs:label "P" .


:runTypeCAISO.S 
                rdfs:label "S" .


###  Generated by the OWL API (version 4.5.26.2023-07-17T20:34:13Z) https://github.com/owlcs/owlapi
